@prefix CECW-11-2-220: <https://usace-data.com/civil-works/glossary/CECW-11-2-220#> .
@prefix dcterms: <http://purl.org/dc/terms/> .
@prefix owl: <http://www.w3.org/2002/07/owl#> .
@prefix pav: <http://purl.org/pav#> .
@prefix rdfs: <http://www.w3.org/2000/01/rdf-schema#> .
@prefix skos: <http://www.w3.org/2004/02/skos/core#> .
@prefix vann: <http://purl.org/vocab/vann/> .
@prefix voaf: <https://lov.linkeddata.es/vocommons/voaf/v2.0/voaf_v2.0.rdf#> .
@prefix wov: <http://www.knowledgesmarts.com/ontologies/wov#> .
@prefix xsd: <http://www.w3.org/2001/XMLSchema#> .

CECW-11-2-220:Activity a wov:GlossaryTerm,
        skos:Concept ;
    rdfs:label "Activity" ;
    dcterms:bibliographicCitation "Civil Works Direct Program Development Policy Guidance CECW-IP No. 11-2-220" ;
    pav:wasDerivedFrom "glossaries/CivilWorks/CECW-11-2-220.yaml#term[Activity]" ;
    skos:definition "A component of work performed during the course of a project. An activity could be a process (e.g. Collection of data) or lead to a deliverable (write a report). Activities are the building blocks of the CWIF-D system they have assigned durations, resources, and relationships." ;
    skos:inScheme CECW-11-2-220: ;
    skos:prefLabel "Activity" .

CECW-11-2-220:Benefit_Cost_Ratio a wov:GlossaryTerm,
        skos:Concept ;
    rdfs:label "Benefit Cost Ratio" ;
    dcterms:bibliographicCitation "Civil Works Direct Program Development Policy Guidance CECW-IP No. 11-2-220" ;
    pav:wasDerivedFrom "glossaries/CivilWorks/CECW-11-2-220.yaml#term[Benefit Cost Ratio]" ;
    skos:altLabel "BCR" ;
    skos:definition """A benefit-cost analysis which is performed to calculate and compare benefits and costs for a project to determine whether the project is a sound investment (justification/feasibility) and to see how it compares with other competing projects (ranking/priority assignment). BCR computations must be based on benefits in the latest approved economic analysis and must be no older than 3 years for New Start construction projects and no more than five years for continuing construction projects. Note distinctions of the different BCRs below:
- BCR AT APPLICABLE RATE: The BCR is the ratio of benefits to costs of all project purposes, from the last approved report or updated for budget purposes, evaluated at the applicable discount rate. If the BCR is not reported, put NA in the field and explain why in the REMARKS.
- BCR Current “The BCR with most current updated costs/benefits.
- BCR @ 7% - Using a discount rate allows for comparison of benefits and costs accruing at different points in time. The benefit-cost analysis uses discounting procedures to normalize financial outcomes over time.
- BCR National Economic Development Plan (BCR-NED) “ The objective in formulating the National Economic Development Plan is to maximize the difference between monetized benefits and costs. Benefits are increases in the net value of national outputs (goods and services) and vary by type of water resource project. The costs (opportunity costs) are the costs of the resources required or displaced to achieve the plan, such as concrete and steel for building a floodwall.
- BCR “ Locally Preferred Plan (BCR-LPP) “ A Sponsor may support formulation of an alternative plan with a scope that results in a decrease in the difference between monetized benefits and costs compared to the National Economic Development Plan""" ;
    skos:inScheme CECW-11-2-220: ;
    skos:prefLabel "Benefit Cost Ratio" .

CECW-11-2-220:Capability a wov:GlossaryTerm,
        skos:Concept ;
    rdfs:label "Capability" ;
    dcterms:bibliographicCitation "Civil Works Direct Program Development Policy Guidance CECW-IP No. 11-2-220" ;
    pav:wasDerivedFrom "glossaries/CivilWorks/CECW-11-2-220.yaml#term[Capability]" ;
    skos:definition """Capability is defined as the estimate for the amount of additional, new funding (over and above projected or actual unobligated carry-in) that, if provided in the applicable fiscal year, can either be obligated or committed for a contract solicitation effectively and efficiently in that fiscal year, consistent with law and policy, assuming that all projected or actual uncommitted carry-in to that fiscal year is obligated or committed first. (not to be confused with definition for Enterprise-Wide Capability)
- Capability on a contract work package proposed for funding in the BY does not include out- year costs of engineering and design (E&D), supervision and administration (S&A), or contingencies on the contract. The exception is that out-year E&D, S&A, and contingencies should be included if the BY is the last year that contracts are planned to be funded on the project or the study phase, since in this case including them would enable full funding of the project or phase. Furthermore, once the allocations in the President's Budget for a given FY (which becomes BY-1) have been finalized, the capability estimate for an unbudgeted, fully funded contract work package should be adjusted to include out-year E&D, S&A, and contingencies, among other adjustments, because future-FY funding is not certain if the unbudgeted work package is funded in a BY-1 work plan.
- Capability is stated in terms of obligations and commitments for contract solicitations, not expenditures. Capability and Amount That Could Be Used are identical, where used means obligated or committed for a contract solicitation. Project capability for a FY is the sum of its work package capabilities for that FY.""" ;
    skos:inScheme CECW-11-2-220: ;
    skos:prefLabel "Capability" .

CECW-11-2-220:Caretaker_Status a wov:GlossaryTerm,
        skos:Concept ;
    rdfs:label "Caretaker Status" ;
    dcterms:bibliographicCitation "https://www.publications.usace.army.mil/Portals/76/Users/182/86/2486/EC_11-2-220.pdf#page=272" ;
    pav:wasDerivedFrom "glossaries/CivilWorks/CECW-11-2-220.yaml#term[Caretaker Status]" ;
    skos:definition "Real or personal property at a project site, in part or in whole that is currently not utilized or occupied for current program authorized purposes. This status is applied to inactive assets (see Inactive Facility) for which there are no reactivation plans. Facility systems and collateral equipment may be considered for excess; corresponding to the Federal Real Property Indicator status excess and dispose. Caretaker status is distinct from standby or mothball status and is defined at the project or project site level, not the feature level." ;
    skos:inScheme CECW-11-2-220: ;
    skos:prefLabel "Caretaker Status" .

CECW-11-2-220:Civil_Works_Integrated_Funding_Database a wov:GlossaryTerm,
        skos:Concept ;
    rdfs:label "Civil Works Integrated Funding Database" ;
    dcterms:bibliographicCitation "https://www.publications.usace.army.mil/Portals/76/Users/182/86/2486/EC_11-2-220.pdf#page=273" ;
    pav:wasDerivedFrom "glossaries/CivilWorks/CECW-11-2-220.yaml#term[Civil Works Integrated Funding Database]" ;
    skos:altLabel "CW-IFD",
        "CWIFD" ;
    skos:definition """CW-IFD is defined as the integrated data set for supporting budget allocations and related funding decisions. CW-IFD includes data used to support the following processes:
- Budget development
- Work plan development/Allocation Strategy
- Documentation and decisions on funding emergency repairs
- Authoritative data on project authorization and cost, to facilitate life cycle cost management, deauthorization, and portfolio management
Data is organized into one of three general categories: - Program or Project data
- Facility or Feature data
- Work package data""" ;
    skos:inScheme CECW-11-2-220: ;
    skos:prefLabel "Civil Works Integrated Funding Database" .

CECW-11-2-220:Common_Operation_and_Maintenance a wov:GlossaryTerm,
        skos:Concept ;
    rdfs:label "Common Operation and Maintenance" ;
    dcterms:bibliographicCitation "https://www.publications.usace.army.mil/Portals/76/Users/182/86/2486/EC_11-2-220.pdf#page=272" ;
    pav:wasDerivedFrom "glossaries/CivilWorks/CECW-11-2-220.yaml#term[Common Operation and Maintenance]" ;
    skos:definition "Includes work that is commonly performed at similar projects such as operation at all performance levels, preventive maintenance, budget development, financial and execution management, environmental monitoring and mitigation, and other things necessary to support operation, recurring maintenance, and small scale corrective maintenance of the project. Budget requests for O&M in this category do not resource O&M work which is necessary to support facility performance in future budget years. Common O&M includes work in programmatic activities, administrative and technical support, and legal & environmental mandates. Common O&M is distinct from Specific Work Activities in budget formulation. Common O&M is separated into three Buckets: Programmatic Activities, which are activities performed by personnel located at the physical project site; Administrative and Technical Support, which are activities performed by personnel not located at the physical project site (e.g., District Office, Area Office, etc.); and Legal and Environmental Mandates, which includes all legal and environmental mandates (e.g., NAGPRA, BiOps, NEPA, etc.)." ;
    skos:inScheme CECW-11-2-220: ;
    skos:prefLabel "Common Operation and Maintenance" .

CECW-11-2-220:Component_Renewal a wov:GlossaryTerm,
        skos:Concept ;
    rdfs:label "Component Renewal" ;
    dcterms:bibliographicCitation "https://www.publications.usace.army.mil/Portals/76/Users/182/86/2486/EC_11-2-220.pdf#page=272" ;
    pav:wasDerivedFrom "glossaries/CivilWorks/CECW-11-2-220.yaml#term[Component Renewal]" ;
    skos:definition "The renewal or replacement of major asset components (roofs, large HVAC, lock gates and mechanisms, spillways gates, etc.). The work almost always exceeds Capital thresholds and generally has a frequency of greater than seven to ten years but is not a capital improvement." ;
    skos:inScheme CECW-11-2-220: ;
    skos:prefLabel "Component Renewal" .

CECW-11-2-220:Corrective_Maintenance a wov:GlossaryTerm,
        skos:Concept ;
    rdfs:label "Corrective Maintenance" ;
    dcterms:bibliographicCitation "https://www.publications.usace.army.mil/Portals/76/Users/182/86/2486/EC_11-2-220.pdf#page=272" ;
    pav:wasDerivedFrom "glossaries/CivilWorks/CECW-11-2-220.yaml#term[Corrective Maintenance]" ;
    skos:definition "The repair or renewal of an item which has failed or is about to fail." ;
    skos:inScheme CECW-11-2-220: ;
    skos:prefLabel "Corrective Maintenance" .

CECW-11-2-220:Critical_Infrastructure_Protection_%26_Resilience_Program a wov:GlossaryTerm,
        skos:Concept ;
    rdfs:label "Critical Infrastructure Protection & Resilience Program" ;
    dcterms:bibliographicCitation "https://www.publications.usace.army.mil/Portals/76/Users/182/86/2486/EC_11-2-220.pdf#page=273" ;
    pav:wasDerivedFrom "glossaries/CivilWorks/CECW-11-2-220.yaml#term[Critical Infrastructure Protection & Resilience Program]" ;
    skos:definition "The CIPR program leads risk assessment and prioritization efforts for USACE critical infrastructure portfolio in order to enhance its protection and resilience. The program includes both common actions (security and operations personnel training, security patrol and monitoring, security equipment maintenance, security risk assessments, blast damage assessment studies, dam security exercises, operating interim risk reduction measures, and physical security inspections) and Specific Work Activities (protection and operational interim risk reduction measures, physical security implementation, construction retrofits/hardening for vulnerability mitigation, surge in protective measures due to increased threat levels). For more information, see Annex III, paragraph III-2-7." ;
    skos:inScheme CECW-11-2-220: ;
    skos:prefLabel "Critical Infrastructure Protection & Resilience Program" .

CECW-11-2-220:Critical_Work_Activities%2FPackages a wov:GlossaryTerm,
        skos:Concept ;
    rdfs:label "Critical Work Activities/Packages" ;
    dcterms:bibliographicCitation "https://www.publications.usace.army.mil/Portals/76/Users/182/86/2486/EC_11-2-220.pdf#page=272" ;
    pav:wasDerivedFrom "glossaries/CivilWorks/CECW-11-2-220.yaml#term[Critical Work Activities/Packages]" ;
    skos:definition "Each MSC is responsible for evaluating individual work activities/packages to determine their level of importance with regard to funding in the BY budget. In addition, MSCs must be able to fully justify work activities/packages that are identified as \"critical\" to their needs. The supporting justification for critical work activities/packages must demonstrate failure to perform the work would be critical to the functioning of the project to accomplish its mission; would endanger the health and safety of the public or project employees, or would result in substantial losses. Equipment, assets, facilities or components where failure would directly impede the accomplishment of the assigned mission; would endanger the health and safety of the public or project employees; or would result in substantial losses are considered critical assets. The justification for critical work activities/packages must be supported by a risk vs consequence type analysis. All \"operation\", \"maintenance\" and \"joint cost\" work activities/packages in the budget that are identified as \"critical\", whether Common O&M or Specific Work Activities, should be capable of meeting this requirement. " ;
    skos:inScheme CECW-11-2-220: ;
    skos:prefLabel "Critical Work Activities/Packages" .

CECW-11-2-220:Cyclical_Maintenance a wov:GlossaryTerm,
        skos:Concept ;
    rdfs:label "Cyclical Maintenance" ;
    dcterms:bibliographicCitation "https://www.publications.usace.army.mil/Portals/76/Users/182/86/2486/EC_11-2-220.pdf#page=273" ;
    pav:wasDerivedFrom "glossaries/CivilWorks/CECW-11-2-220.yaml#term[Cyclical Maintenance]" ;
    skos:definition "The replacement or renewal of items that are required on a recurring basis, with a frequency of greater than one year and less than seven to ten years. Examples are channel dredging, painting, floor coverings, engine overhauls, etc. These generally fall below Capital thresholds. These are also the items that are frequently deferred. Cyclical Maintenance is also referred to as Recurring Maintenance." ;
    skos:inScheme CECW-11-2-220: ;
    skos:prefLabel "Cyclical Maintenance" .

CECW-11-2-220:Enterprise-Wide_Capability_for_Allocation_Strategy a wov:GlossaryTerm,
        skos:Concept ;
    rdfs:label "Enterprise-Wide Capability for Allocation Strategy" ;
    dcterms:bibliographicCitation "https://www.publications.usace.army.mil/Portals/76/Users/182/86/2486/EC_11-2-220.pdf#page=273" ;
    pav:wasDerivedFrom "glossaries/CivilWorks/CECW-11-2-220.yaml#term[Enterprise-Wide Capability for Allocation Strategy]" ;
    skos:definition """Enterprise-wide capability, or execution capacity, is the maximum amount of project capabilities that the MSC or FOA can execute in the applicable fiscal year. It is recognized that each enterprise, while it can execute the project capabilities on some of its projects, cannot execute the project capabilities on all of its projects. Enterprise-wide capability is less than the sum of project capabilities. Appropriations Committee staffs are interested in USACE enterprise- wide capabilities, particularly by business line or line item of additional funding, for the allocation Strategy (BY-1). This paragraph provides guidance on how each MSC or FOA states its enterprise-wide capability in the Allocation Strategy.
(i) The Explanatory Statements accompanying recent energy and water development appropriations acts have provided line items of additional funding that span all authorized business lines and functions, including those of lower budget priority such as bank protection and environmental infrastructure. Accordingly, enterprise-wide capability should represent a balanced mix of business lines and functions. In other words, within each business line or function a reasonable portion of work packages should be within enterprise-wide capability, and others should be beyond enterprise-wide capability. The mix is more or less governed by expectations (based on recent Explanatory Statements and House and Senate Reports) for funding of budgeted work and the line items of additional funding. (ii) The MSC or FOA should use performance to determine, within each business line or function, which work packages are within enterprise capability, and which are not. All budgeted work packages should be first-added within enterprise capability, and unbudgeted work packages should be next-added.
(iii) The MSC or FOA should signify which work packages are within enterprise-wide capability, or not, by checking the "Funding Pot" box, or not, in the "Recommended for Funding" field under the Funding tab in the Civil Works Integrated Funding Database (CWIFD). To respond to Congressional inquiries for USACE-wide enterprise capability for a business line or function, HQUSACE will aggregate across USACE the capabilities of work packages in that business line or function that have the Funding Pot box checked.""" ;
    skos:inScheme CECW-11-2-220: ;
    skos:prefLabel "Enterprise-Wide Capability for Allocation Strategy" .

CECW-11-2-220:FEM_Work_Order_Number a wov:GlossaryTerm,
        skos:Concept ;
    rdfs:label "FEM Work Order Number" ;
    dcterms:bibliographicCitation "https://www.publications.usace.army.mil/Portals/76/Users/182/86/2486/EC_11-2-220.pdf#page=274" ;
    pav:wasDerivedFrom "glossaries/CivilWorks/CECW-11-2-220.yaml#term[FEM Work Order Number]" ;
    skos:altLabel "FEM WON",
        "WON" ;
    skos:definition """A FEM WON is an alpha-numeric field from the FEM (Facilities and Equipment Maintenance) program that is a unique identifier connecting the budget work package to budget execution via the USACE Facilities and Equipment Management system (FEM). A FEM WON is required for all Specific Work Activity budget work packages in CWIF-D for all BLs and should be assigned at the appropriate asset level. Note that a data field has been established in CWIF-D for entering the FEM WON. Selection of the specific work order numbering schema is at the discretion of the activity submitting the budget work package. All project deficiencies and needs captured on FEM Work orders, according to Phase 3 of the Maintenance Management Improvement Plan (MMIP), should serve as input to developing work packages. Additionally, it is required that in FEM the Work Order:
(i) description should mirror the work package and associated Work Category Code descriptions and be preceded by "FY19 SWA". If a work package was created in FEM in previous years, was not funded, and will be resubmitted for FY19, the Work Order description may be updated as necessary.
(ii) the FEM work order long description field should contain exactly the same Information as the budget work package description and the associated Work Category Code.
(iii) type should be "SWA," Specific Work Activity.
(iv) the Command Work Type should be Deferred Maintenance (DM).""" ;
    skos:inScheme CECW-11-2-220: ;
    skos:prefLabel "FEM Work Order Number" .

CECW-11-2-220:FUSRAP a wov:GlossaryTerm,
        skos:Concept ;
    rdfs:label "FUSRAP" ;
    dcterms:bibliographicCitation "https://www.publications.usace.army.mil/Portals/76/Users/182/86/2486/EC_11-2-220.pdf#page=15" ;
    pav:wasDerivedFrom "glossaries/CivilWorks/CECW-11-2-220.yaml#term[FUSRAP]" ;
    skos:altLabel "Formerly Utilized Sites Remedial Action Program" ;
    skos:definition "The FUSRAP program is to protect human health and the environment from residual radioactive contamination at sites formerly utilized by the Manhattan Engineer District for the Nation's early atomic energy program. The major objectives of the FUSRAP program are to evaluate and remediate, as necessary, sites identified by the Department of Energy - Office of Legacy Management (DOE-LM) as eligible for consideration under FUSRAP." ;
    skos:inScheme CECW-11-2-220: ;
    skos:prefLabel "FUSRAP" .

CECW-11-2-220:Facility_Operation a wov:GlossaryTerm,
        skos:Concept ;
    rdfs:label "Facility Operation" ;
    dcterms:bibliographicCitation "https://www.publications.usace.army.mil/Portals/76/Users/182/86/2486/EC_11-2-220.pdf#page=274" ;
    pav:wasDerivedFrom "glossaries/CivilWorks/CECW-11-2-220.yaml#term[Facility Operation]" ;
    skos:definition "The day-to-day activities that allow for the continued use of facilities but are not considered part of the maintenance regimen that directly extends the life of the asset, facility or component. Examples include things such as security, custodial services, removing ice and snow, mowing, debris, trash, cleaning; or replacing lighting fixtures." ;
    skos:inScheme CECW-11-2-220: ;
    skos:prefLabel "Facility Operation" .

CECW-11-2-220:General_Reevaluation_Study a wov:GlossaryTerm,
        skos:Concept ;
    rdfs:label "General Reevaluation Study" ;
    dcterms:bibliographicCitation "https://www.publications.usace.army.mil/Portals/76/Users/182/86/2486/EC_11-2-220.pdf#page=274" ;
    pav:wasDerivedFrom "glossaries/CivilWorks/CECW-11-2-220.yaml#term[General Reevaluation Study]" ;
    skos:altLabel "GRR" ;
    skos:definition "This is a study that involves reformulation of alternatives from a previously completed Feasibility Study. The addition of separable element(s) or separable implementable features may be included in a General Reevaluation Study so long as reformulation of the already- recommended or already-authorized alternative is included. The phase activity code is GR." ;
    skos:inScheme CECW-11-2-220: ;
    skos:prefLabel "General Reevaluation Study" .

CECW-11-2-220:Inactive_Facility a wov:GlossaryTerm,
        skos:Concept ;
    rdfs:label "Inactive Facility" ;
    dcterms:bibliographicCitation "https://www.publications.usace.army.mil/Portals/76/Users/182/86/2486/EC_11-2-220.pdf#page=274" ;
    pav:wasDerivedFrom "glossaries/CivilWorks/CECW-11-2-220.yaml#term[Inactive Facility]" ;
    skos:definition """A facility that does not have a specific current or near-term program or mission requirement is considered "Inactive". Inactive facilities or parts of facilities are assets not currently needed to support the agency's mission or function but will have a planned need in the future. Inactive facilities may be classified by status: Standby or Mothball, corresponding to the Federal Real Property Council Indicator status inactive. The following conditions characterize all inactive facilities or parts of facilities that are inactive: No personnel occupy the facility.
2. Utilities are curtailed, other than as required for fire prevention, security, or safety. 3. The facility is secured to prevent unauthorized access and injury to personnel.
4. The facility does not receive funding for renewal or other significant improvement.""" ;
    skos:inScheme CECW-11-2-220: ;
    skos:prefLabel "Inactive Facility" .

CECW-11-2-220:Level_of_Performance a wov:GlossaryTerm,
        skos:Concept ;
    rdfs:label "Level of Performance" ;
    dcterms:bibliographicCitation "https://www.publications.usace.army.mil/Portals/76/Users/182/86/2486/EC_11-2-220.pdf#page=275" ;
    pav:wasDerivedFrom "glossaries/CivilWorks/CECW-11-2-220.yaml#term[Level of Performance]" ;
    skos:altLabel "LOP" ;
    skos:definition "LoP is a management decision in the context of the available maintenance resources, maintenance demands of an asset, and asset service demands or capacity. If formally established, the asset''s formally determined Level of Service (LoS), may be used in considering asset demand/capacity. Managers should understand the minimum funding levels necessary to meet regulatory and safety requirements as caretaker of the facility/asset. Beyond this, a range of facility performance levels are available. In the budget context, LoP's may be broadly grouped No Mission (Red), Partial Mission (Yellow), Full Mission (Green). Managers must understand the range of performance available for the facility and the associated investments required to achieve various performance levels. Work packages are formulated to express the investment necessary to achieve a given performance level for the facility/asset. Further definition of the three LOPs: No Mission LOP is funding required to simply own a project; Partial Mission represents the additional funding required to deliver the majority of project benefits, but not meet all requirements; and Full Mission includes the additional funding required to deliver all project benefits and fully preserve the facility for the foreseeable future." ;
    skos:inScheme CECW-11-2-220: ;
    skos:prefLabel "Level of Performance" .

CECW-11-2-220:Limited_Reevaluation_Study a wov:GlossaryTerm,
        skos:Concept ;
    rdfs:label "Limited Reevaluation Study" ;
    dcterms:bibliographicCitation "https://www.publications.usace.army.mil/Portals/76/Users/182/86/2486/EC_11-2-220.pdf#page=275" ;
    pav:wasDerivedFrom "glossaries/CivilWorks/CECW-11-2-220.yaml#term[Limited Reevaluation Study]" ;
    skos:altLabel "LRR" ;
    skos:definition "This is a reexamination of project justification, including the economics and/or environmental effects, which does not require reformulation of project alternatives for an ongoing study. No longer used, See Validation Studies and Annex I." ;
    skos:inScheme CECW-11-2-220: ;
    skos:prefLabel "Limited Reevaluation Study" .

CECW-11-2-220:Lowest_Sustainable_Investment a wov:GlossaryTerm,
        skos:Concept ;
    rdfs:label "Lowest Sustainable Investment" ;
    dcterms:bibliographicCitation "https://www.publications.usace.army.mil/Portals/76/Users/182/86/2486/EC_11-2-220.pdf#page=275" ;
    pav:wasDerivedFrom "glossaries/CivilWorks/CECW-11-2-220.yaml#term[Lowest Sustainable Investment]" ;
    skos:definition "The lowest overall investment level that a prudent manager would select, balancing between short and long term economics and considering overall availability of resources. Sustainability in this sense is crucial to ensure that project meets or exceeds project life-cycle expectations including meeting or exceeding changing environmental requirements for compliant operation." ;
    skos:inScheme CECW-11-2-220: ;
    skos:prefLabel "Lowest Sustainable Investment" .

CECW-11-2-220:MAX_%28OMB%29_Collection_and_Collaboration_Process a wov:GlossaryTerm,
        skos:Concept ;
    rdfs:label "MAX (OMB) Collection and Collaboration Process" ;
    dcterms:bibliographicCitation "https://www.publications.usace.army.mil/Portals/76/Users/182/86/2486/EC_11-2-220.pdf#page=276" ;
    pav:wasDerivedFrom "glossaries/CivilWorks/CECW-11-2-220.yaml#term[MAX (OMB) Collection and Collaboration Process]" ;
    skos:definition "Max Collect is a data collection and collaboration tool that allows HQUSACE to compile and publish the Congressional Budget Materials information into an easy to use web application." ;
    skos:inScheme CECW-11-2-220: ;
    skos:prefLabel "MAX (OMB) Collection and Collaboration Process" .

CECW-11-2-220:Maintenance a wov:GlossaryTerm,
        skos:Concept ;
    rdfs:label "Maintenance" ;
    dcterms:bibliographicCitation "https://www.publications.usace.army.mil/Portals/76/Users/182/86/2486/EC_11-2-220.pdf#page=276" ;
    pav:wasDerivedFrom "glossaries/CivilWorks/CECW-11-2-220.yaml#term[Maintenance]" ;
    skos:definition "Work to restore equipment, assets, facilities or components to design conditions or to conditions that have been determined to be sufficient to meet a prescribed level of performance (vice \"activities directed toward keeping assets in an acceptable condition\"); replacement of parts, systems, or components; preventive maintenance and inspection/monitoring of facilities or equipment (excluding formal inspection/monitoring of facilities or equipment required by USACE guidance such as ER 1110-2- 1156, ER 1110-2-111, and others); and other activities needed to preserve or maintain the asset. Maintenance and repairs, as distinguished from capital improvements, exclude activities directed towards expanding the capacity of an asset or otherwise upgrading it to serve needs different from, or significantly greater than, its current use. (SFFAS 40 & 6 maintenance on plant, property, and equipment (PP&E)) This activity involves \"maintenance\" as well as \"operation\" staff. However, Common O&M and Specific Work Activity maintenance or rehabilitations are maintenance so long as the action does not expand the capacity, or alter use." ;
    skos:inScheme CECW-11-2-220: ;
    skos:prefLabel "Maintenance" .

CECW-11-2-220:Major_Maintenance a wov:GlossaryTerm,
        skos:Concept ;
    rdfs:label "Major Maintenance" ;
    dcterms:bibliographicCitation "https://www.publications.usace.army.mil/Portals/76/Users/182/86/2486/EC_11-2-220.pdf#page=275" ;
    pav:wasDerivedFrom "glossaries/CivilWorks/CECW-11-2-220.yaml#term[Major Maintenance]" ;
    skos:definition "Major maintenance is defined as a non-repetitive item of work or aggregate items of related work for which the total estimated cost exceeds $6,200,000, and which does not qualify as Major Rehabilitation. This designation is not applicable to dredging, but it is applicable to dredged material disposal facilities. The related items of work should include all items required to make the work effective for its desired purpose. Optional or casually-related work which is not essential to the major maintenance item should be programmed, prioritized, and justified as a separate work package, or part of another work package, as appropriate. Major Maintenance work packages are budgeted under the O&M account only." ;
    skos:inScheme CECW-11-2-220: ;
    skos:prefLabel "Major Maintenance" .

CECW-11-2-220:Major_Rehabilitation a wov:GlossaryTerm,
        skos:Concept ;
    rdfs:label "Major Rehabilitation" ;
    dcterms:bibliographicCitation "https://www.publications.usace.army.mil/Portals/76/Users/182/86/2486/EC_11-2-220.pdf#page=275" ;
    pav:wasDerivedFrom "glossaries/CivilWorks/CECW-11-2-220.yaml#term[Major Rehabilitation]" ;
    skos:definition """Rehabilitation projects are projects to restore or ensure continuation of project functions or outputs. Section 205 of P.L.102-580 defines rehabilitation with respect to inland waterway projects, as either:
1. Economically justified structural work for restoration of a major project feature that extends the life of the feature significantly and will take at least 2 years to complete, and has a capital cost of at least $8,000,000, adjusted for changes in price levels (reliability improvements). The updated threshold for (a) is $ 21 million.
2. Structural modifications that enhance operational efficiency and that have a capital cost of at least $1,000,000, adjusted for changes in price levels (efficiency improvements). Section 205 of P.L. 102-580 (WRDA 1992) was amended by Section 2006 of P.L. 113-121, WRRDA 2014, which increased the major rehabilitation threshold from $8,000,000 to $20,000,000. The updated threshold for 1. is 21.5 million and for 2. is 2.1 million. By policy these thresholds also apply to all Business Lines / Missions.""" ;
    skos:inScheme CECW-11-2-220: ;
    skos:prefLabel "Major Rehabilitation" .

CECW-11-2-220:Mothball_status a wov:GlossaryTerm,
        skos:Concept ;
    rdfs:label "Mothball status" ;
    dcterms:bibliographicCitation "https://www.publications.usace.army.mil/Portals/76/Users/182/86/2486/EC_11-2-220.pdf#page=276" ;
    pav:wasDerivedFrom "glossaries/CivilWorks/CECW-11-2-220.yaml#term[Mothball status]" ;
    skos:altLabel "long term inactive" ;
    skos:definition """An asset status applied to facilities when a decision has been made to suspend operations for an extended period of time and for which maintenance measures have been taken to prevent deterioration of essential systems. Mothballing generally results in higher first-year costs, but future annual costs are lower due to reduced maintenance and repair requirements. Mothball status is distinct from caretaker or standby status; corresponds to the Federal Real Property Indicator status inactive. Mothball status is defined at the project or project site level, not the feature level. The total time to deactivate and then to reactivate a facility, including the mothballed period, generally exceeds 36 months. In addition to the conditions indicated above, the following conditions characterize mothballed facilities:
1. Utility systems and collateral equipment have been properly prepared for long-term inactivation without significant deterioration. Selected systems, such as cathodic and fire detection systems are kept in operation and routinely inspected.
2. The facility interior is equipped with appropriate environmental control to prevent significant deterioration.
3. Hazardous materials have been removed.
4. The facility exterior envelope is inspected routinely and the integrity and appearance of the exterior shell are maintained.
5. Personal property is reported to the USACE Logistic Agency for reutilization.""" ;
    skos:inScheme CECW-11-2-220: ;
    skos:prefLabel "Mothball status" .

CECW-11-2-220:New_Investment a wov:GlossaryTerm,
        skos:Concept ;
    rdfs:label "New Investment" ;
    dcterms:bibliographicCitation "https://www.publications.usace.army.mil/Portals/76/Users/182/86/2486/EC_11-2-220.pdf#page=276" ;
    pav:wasDerivedFrom "glossaries/CivilWorks/CECW-11-2-220.yaml#term[New Investment]" ;
    skos:definition "A new investment decision is required for a study or project that is not a new start, but meets one of the following criteria: It is a new study phase of a study funded previously in the account; it is a resumption; study resumption or construction resumption." ;
    skos:inScheme CECW-11-2-220: ;
    skos:prefLabel "New Investment" .

CECW-11-2-220:Non-critical_Work_Activities%2FPackages a wov:GlossaryTerm,
        skos:Concept ;
    rdfs:label "Non-critical Work Activities/Packages" ;
    dcterms:bibliographicCitation "https://www.publications.usace.army.mil/Portals/76/Users/182/86/2486/EC_11-2-220.pdf#page=276" ;
    pav:wasDerivedFrom "glossaries/CivilWorks/CECW-11-2-220.yaml#term[Non-critical Work Activities/Packages]" ;
    skos:definition "Activities where failure to perform the work may cause considerable inconvenience but would not affect the accomplishment of the assigned mission; would not seriously affect the health and safety of the public or project personnel; or would cause moderate or insignificant losses." ;
    skos:inScheme CECW-11-2-220: ;
    skos:prefLabel "Non-critical Work Activities/Packages" .

CECW-11-2-220:Operation a wov:GlossaryTerm,
        skos:Concept ;
    rdfs:label "Operation" ;
    dcterms:bibliographicCitation "https://www.publications.usace.army.mil/Portals/76/Users/182/86/2486/EC_11-2-220.pdf#page=277" ;
    pav:wasDerivedFrom "glossaries/CivilWorks/CECW-11-2-220.yaml#term[Operation]" ;
    skos:definition """Work that is integral to the actual performance of an operating project that provides authorized benefits to the public. Operation includes facility operation necessary to keep equipment, assets and facilities functioning at a particular service level; examples include custodial services, removing snow and ice, debris removal (not required for dam safety), trash, cleaning, replacing lighting elements. This work is typically performed on an annual basis, typically by hired labor or small contract (service contract, purchase order, etc.)
""" ;
    skos:inScheme CECW-11-2-220: ;
    skos:prefLabel "Operation" .

CECW-11-2-220:Operation_and_Maintenance a wov:GlossaryTerm,
        skos:Concept ;
    rdfs:label "Operation and Maintenance" ;
    dcterms:bibliographicCitation "https://www.publications.usace.army.mil/Portals/76/Users/182/86/2486/EC_11-2-220.pdf#page=279" ;
    pav:wasDerivedFrom "glossaries/CivilWorks/CECW-11-2-220.yaml#term[Operation and Maintenance]" ;
    skos:altLabel "O&M" ;
    skos:definition "The Operation and Maintenance account funds operation, maintenance, and related activities at the water resources projects that the Corps operates and maintains. It also includes some activities at non-Federally owned/operated projects (levee safety activities). Work to be accomplished consists of dredging, maintenance, repair, and operation of structures and other facilities, as authorized in the various River and Harbor, Flood Control, and Water Resources Development Acts. Budget and Allocation Strategy information developed under the O&M Account are broken out as either 'O' or 'M' and further identified by Business Line (s). This account is also used to fund other work not directly chargeable to authorized projects and is collectively known as the Remaining Items Program." ;
    skos:inScheme CECW-11-2-220: ;
    skos:prefLabel "Operation and Maintenance" .

CECW-11-2-220:Post-Feasibility_Studies a wov:GlossaryTerm,
        skos:Concept ;
    rdfs:label "Post-Feasibility Studies" ;
    dcterms:bibliographicCitation "https://www.publications.usace.army.mil/Portals/76/Users/182/86/2486/EC_11-2-220.pdf#page=277" ;
    pav:wasDerivedFrom "glossaries/CivilWorks/CECW-11-2-220.yaml#term[Post-Feasibility Studies]" ;
    skos:definition "These types of studies involve reformulation of alternatives and project justification via economics and/or environmental effects." ;
    skos:inScheme CECW-11-2-220: ;
    skos:prefLabel "Post-Feasibility Studies" .

CECW-11-2-220:President%27s_Budget_Rank a wov:GlossaryTerm,
        skos:Concept ;
    rdfs:label "President's Budget Rank" ;
    dcterms:bibliographicCitation "https://www.publications.usace.army.mil/Portals/76/Users/182/86/2486/EC_11-2-220.pdf#page=277" ;
    pav:wasDerivedFrom "glossaries/CivilWorks/CECW-11-2-220.yaml#term[President's Budget Rank]" ;
    skos:altLabel "ARMY Rank",
        "HQ Rank" ;
    skos:definition "President's Budget rank identifies the level of funding assigned to individual work packages after OMB review (passback) and HQ finalization of the BY budget. The President's Budget rank is entered into the CWIF-D database by BLMs prior to submitting the budget to Congress. President's Budget Rankings are defined as follows: - President's Budget Rank 1 = IN the budget - President's Budget Rank 7 = NOT in the budget See also ARMY Rank and HQ Rank" ;
    skos:inScheme CECW-11-2-220: ;
    skos:prefLabel "President's Budget Rank" .

CECW-11-2-220:Preventive_Maintenance a wov:GlossaryTerm,
        skos:Concept ;
    rdfs:label "Preventive Maintenance" ;
    dcterms:bibliographicCitation "https://www.publications.usace.army.mil/Portals/76/Users/182/86/2486/EC_11-2-220.pdf#page=277" ;
    pav:wasDerivedFrom "glossaries/CivilWorks/CECW-11-2-220.yaml#term[Preventive Maintenance]" ;
    skos:definition "The systematic care, servicing, and inspection of assets, facilities, equipment and components for the purpose of detecting and correcting incipient failures and accomplishing minor maintenance (based on AR 420-1) Formal inspections and assessments explicitly required by current USACE guidance (i.e., ER 1110-2-1156, ER 1110-2-111, and others) are not considered preventive maintenance. The frequency of preventive maintenance is generally less than one year. Examples include things such as routine testing of lubricating and hydraulic oils; replacing packing in valves and glands; lubrication of equipment/components; replacing electrical brushes and touch-up painting, etc." ;
    skos:inScheme CECW-11-2-220: ;
    skos:prefLabel "Preventive Maintenance" .

<https://usace-data.com/civil-works/glossary/CECW-11-2-220#Program,_Project,_or_Activity> a wov:GlossaryTerm,
        skos:Concept ;
    rdfs:label "Program, Project, or Activity" ;
    dcterms:bibliographicCitation "https://www.publications.usace.army.mil/Portals/76/Users/182/86/2486/EC_11-2-220.pdf#page=277" ;
    pav:wasDerivedFrom "glossaries/CivilWorks/CECW-11-2-220.yaml#term[Program, Project, or Activity]" ;
    skos:altLabel "PPA" ;
    skos:definition """For any appropriation, a project, study, program, or other work that has received a Statutory Earmark and for which any Funding from the Program Year of the Statutory Earmark remains available for obligation.
(2) For the FUSRAP appropriation, any funded project.
(3) For the I, C, O&M, or MR&T appropriation, a project, program, project element, or study that has been funded through a First-Tier Line Item in a table of allocations in the Statement of Managers accompanying any Act, and for which any Funding from the Program Year of that Act remains available for obligation.
(4) For the I, C, O&M, or MR&T appropriation, a Specifically Authorized Project or Program (see definition). However, if the Specifically Authorized Project or Program is a component of a broader PPA funded as a First-Tier Line Item, then the component is not a PPA unless the component itself had been funded through a First-Tier Line Item and Funding from the applicable Program Year remains available for obligation.
(5) For the I, C, O&M, or MR&T appropriation, a study intended to lead to a new, Specifically Authorized Project or Program (see definition), including a spinoff sub-basin study from a basin-wide or comprehensive study, or a study for an unauthorized project that would incorporate or subsume an already-authorized project, such as a study for widening or deepening beyond authorized channel dimensions.""" ;
    skos:inScheme CECW-11-2-220: ;
    skos:prefLabel "Program, Project, or Activity" .

CECW-11-2-220:Program_Code a wov:GlossaryTerm,
        skos:Concept ;
    rdfs:label "Program Code" ;
    dcterms:bibliographicCitation "https://www.publications.usace.army.mil/Portals/76/Users/182/86/2486/EC_11-2-220.pdf#page=277" ;
    pav:wasDerivedFrom "glossaries/CivilWorks/CECW-11-2-220.yaml#term[Program Code]" ;
    skos:definition "A mandatory field in P2 used to store the unique Congressional line-item identifier." ;
    skos:inScheme CECW-11-2-220: ;
    skos:prefLabel "Program Code" .

CECW-11-2-220:Project_Partnership_Agreement%2FPartnership_Agreement a wov:GlossaryTerm,
        skos:Concept ;
    rdfs:label "Project Partnership Agreement/Partnership Agreement" ;
    dcterms:bibliographicCitation "https://www.publications.usace.army.mil/Portals/76/Users/182/86/2486/EC_11-2-220.pdf#page=278" ;
    pav:wasDerivedFrom "glossaries/CivilWorks/CECW-11-2-220.yaml#term[Project Partnership Agreement/Partnership Agreement]" ;
    skos:altLabel "PPA" ;
    skos:definition "Reference P.L. 110-114 (WRDA 2007) Conference Report, Section 2003(f)(2) entitled: References to Cooperation Agreements “ any reference in a law, regulation, document, or other paper of the United States to a cooperation agreement or project cooperation agreement will be deemed to be a reference to a partnership agreement or a project partnership agreement, (PPA), respectively." ;
    skos:inScheme CECW-11-2-220: ;
    skos:prefLabel "Project Partnership Agreement/Partnership Agreement" .

CECW-11-2-220:Recurring_Maintenance a wov:GlossaryTerm,
        skos:Concept ;
    rdfs:label "Recurring Maintenance" ;
    dcterms:bibliographicCitation "https://www.publications.usace.army.mil/Portals/76/Users/182/86/2486/EC_11-2-220.pdf#page=278" ;
    pav:wasDerivedFrom "glossaries/CivilWorks/CECW-11-2-220.yaml#term[Recurring Maintenance]" ;
    skos:definition "The replacement or renewal of items that are required on a recurring basis, with a frequency of greater than one year and less than seven to ten years. Examples are channel dredging, painting, floor coverings, engine overhauls, etc. These generally fall below Capital thresholds. These are also the items that are frequently deferred. Recurring Maintenance is also referred to as Cyclical Maintenance." ;
    skos:inScheme CECW-11-2-220: ;
    skos:prefLabel "Recurring Maintenance" .

CECW-11-2-220:Rehabilitation a wov:GlossaryTerm,
        skos:Concept ;
    rdfs:label "Rehabilitation" ;
    dcterms:bibliographicCitation "https://www.publications.usace.army.mil/Portals/76/Users/182/86/2486/EC_11-2-220.pdf#page=278" ;
    pav:wasDerivedFrom "glossaries/CivilWorks/CECW-11-2-220.yaml#term[Rehabilitation]" ;
    skos:definition "A budget category for Specific Work Activities which exceed cost thresholds of Section 205 of P.L. 102-580 (WRDA 1992) as amended by Section 2006 of P.L. 113-121, WRRDA 2014." ;
    skos:inScheme CECW-11-2-220: ;
    skos:prefLabel "Rehabilitation" .

CECW-11-2-220:Remaining_Benefits_Remaining_Cost_Ratio a wov:GlossaryTerm,
        skos:Concept ;
    rdfs:label "Remaining Benefits Remaining Cost Ratio" ;
    dcterms:bibliographicCitation "https://www.publications.usace.army.mil/Portals/76/Users/182/86/2486/EC_11-2-220.pdf#page=278" ;
    pav:wasDerivedFrom "glossaries/CivilWorks/CECW-11-2-220.yaml#term[Remaining Benefits Remaining Cost Ratio]" ;
    skos:altLabel "RBRCR" ;
    skos:definition """Compute the RBRCR at the applicable interest rate, the current interest rate, and the OMB prescribed 7% interest rate for projects and separable elements other than design or construction deficiency correction projects, safety of dams projects, and aquatic ecosystem restoration projects.
(1) Remaining Costs. Consider anticipated Federal and non-Federal allocations and other non- Federal costs through the BY-1 as sunk, and exclude them from the RBRCR computation. The remaining costs will be the Federal and non-Federal allocations as of the end of BY-1 based on the current project cost estimate and allocations from prior years and on the President's Budget for BY-2 in October 2017 dollars. Where the project includes completed separable elements, independent units and/or useful increments, OMRR&R costs for completed units/increments will also be considered sunk, and only OMRR&R for remaining units/increments will be considered in remaining project costs. The remaining costs should include any reimbursements still needing to be paid for work already completed.
(2) Remaining Benefits. Where the project includes completed separable elements, independent units and/or useful increments, the amount of annual benefits that would be expected to accrue over the period of analysis for completed or functioning components of the total project will be considered sunk and excluded from the RBRCR computation. Sunk benefits for projects that have reimbursable features should be estimated based on the reimbursable costs expended and an estimate on the amount of sunk benefits that would be associated with that level of expenditure. Remaining benefits are those that will be attainable in the BY or thereafter only if project features not completed with allocations through BY-1 are completed and operated and maintained.""" ;
    skos:inScheme CECW-11-2-220: ;
    skos:prefLabel "Remaining Benefits Remaining Cost Ratio" .

CECW-11-2-220:Resumption-_Construction a wov:GlossaryTerm,
        skos:Concept ;
    rdfs:label "Resumption- Construction" ;
    dcterms:bibliographicCitation "https://www.publications.usace.army.mil/Portals/76/Users/182/86/2486/EC_11-2-220.pdf#page=278" ;
    pav:wasDerivedFrom "glossaries/CivilWorks/CECW-11-2-220.yaml#term[Resumption- Construction]" ;
    skos:altLabel "Construction" ;
    skos:definition "A construction resumption is renewal of physical construction activities on a project or separable element on which physical construction under a construction contract has not been performed in any of the three most recent fiscal years before the fiscal year in question. However, in the case of a construction project with intermittent construction activities, such as phases, levee lifts, or renourishment cycles, initiation of the next intermittent construction activity is not a resumption." ;
    skos:inScheme CECW-11-2-220: ;
    skos:prefLabel "Resumption- Construction" .

CECW-11-2-220:Resumption-_Study a wov:GlossaryTerm,
        skos:Concept ;
    rdfs:label "Resumption- Study" ;
    dcterms:bibliographicCitation "https://www.publications.usace.army.mil/Portals/76/Users/182/86/2486/EC_11-2-220.pdf#page=278" ;
    pav:wasDerivedFrom "glossaries/CivilWorks/CECW-11-2-220.yaml#term[Resumption- Study]" ;
    skos:altLabel "Investigation" ;
    skos:definition "A study resumption is the renewal of study activities on a study that has not been funded in any of the three most recent fiscal years before the fiscal year in question." ;
    skos:inScheme CECW-11-2-220: ;
    skos:prefLabel "Resumption- Study" .

CECW-11-2-220:Rounding a wov:GlossaryTerm,
        skos:Concept ;
    rdfs:label "Rounding" ;
    dcterms:bibliographicCitation "https://www.publications.usace.army.mil/Portals/76/Users/182/86/2486/EC_11-2-220.pdf#page=278" ;
    pav:wasDerivedFrom "glossaries/CivilWorks/CECW-11-2-220.yaml#term[Rounding]" ;
    skos:definition "All cost estimates will be rounded to the nearest one thousand dollar ($1000) unless otherwise specified." ;
    skos:inScheme CECW-11-2-220: ;
    skos:prefLabel "Rounding" .

CECW-11-2-220:Section_902_Post_Authorization_Study a wov:GlossaryTerm,
        skos:Concept ;
    rdfs:label "Section 902 Post Authorization Study" ;
    dcterms:bibliographicCitation "https://www.publications.usace.army.mil/Portals/76/Users/182/86/2486/EC_11-2-220.pdf#page=278" ;
    pav:wasDerivedFrom "glossaries/CivilWorks/CECW-11-2-220.yaml#term[Section 902 Post Authorization Study]" ;
    skos:definition "This is a type of Validation Study. Section 902 Post Authorization Reports are reviewed and approved at HQUSACE and may require additional Authorization." ;
    skos:inScheme CECW-11-2-220: ;
    skos:prefLabel "Section 902 Post Authorization Study" .

CECW-11-2-220:Smart_Use_of_Systems a wov:GlossaryTerm,
        skos:Concept ;
    rdfs:label "Smart Use of Systems" ;
    dcterms:bibliographicCitation "https://www.publications.usace.army.mil/Portals/76/Users/182/86/2486/EC_11-2-220.pdf#page=279" ;
    pav:wasDerivedFrom "glossaries/CivilWorks/CECW-11-2-220.yaml#term[Smart Use of Systems]" ;
    skos:definition "The objective of the Smart Use of Systems is to make efficient and consistent use of the various tools currently being used within the Corps of Engineers Civil Works program for project and program data. CWIF-D is the tool that will be used to collect project/program data from the various other data sources within the Corps and then provide an intuitive and user friendly platform for users to enter and manage the project and program data needed for budget and work plan development." ;
    skos:inScheme CECW-11-2-220: ;
    skos:prefLabel "Smart Use of Systems" .

CECW-11-2-220:Specific_Work_Activities a wov:GlossaryTerm,
        skos:Concept ;
    rdfs:label "Specific Work Activities" ;
    dcterms:bibliographicCitation "https://www.publications.usace.army.mil/Portals/76/Users/182/86/2486/EC_11-2-220.pdf#page=279" ;
    pav:wasDerivedFrom "glossaries/CivilWorks/CECW-11-2-220.yaml#term[Specific Work Activities]" ;
    skos:definition "Typically includes scoping, cost estimates, Project Management Plans and/or contract actions, and larger scale planned operations or planned component renewals related efforts such as unique operation and maintenance actions with a specific beginning and end that require a greater level of rigor and documentation. Each Specific Work Activity must be shown separately to allow for individual funding decisions based on performance metrics and risk-based indices. The entire cost for all project-specific marine construction work or fleet work, including dredging and revetment work, whether by contract or hired labor, must be visible in this category, along with full Recurring (cyclical) and Component Renewal maintenance requirements to support anticipated mission delivery or to meet anticipated levels of service in subsequent budget years, including major maintenance level packages. Recapitalization (including betterments) actions including rehabilitation, Major Maintenance and Major Rehabilitations studies or evaluations should be requested as Specific Work Activities. Also, estimated corrective maintenance (proactive) resourcing for commonly occurring breakdown maintenance should be requested as Specific Work Activities. It is a budget category for unique operation and maintenance actions with a specific beginning and end, which require a greater level of rigor and documentation in the form of planning, scoping, contracting, etc. Each Specific Work Activity must be shown separately to allow for individual funding decisions based on performance metrics and risk-based indices." ;
    skos:inScheme CECW-11-2-220: ;
    skos:prefLabel "Specific Work Activities" .

CECW-11-2-220:Spin-off_Studies a wov:GlossaryTerm,
        skos:Concept ;
    rdfs:label "Spin-off Studies" ;
    dcterms:bibliographicCitation "https://www.publications.usace.army.mil/Portals/76/Users/182/86/2486/EC_11-2-220.pdf#page=279" ;
    pav:wasDerivedFrom "glossaries/CivilWorks/CECW-11-2-220.yaml#term[Spin-off Studies]" ;
    skos:altLabel "SS" ;
    skos:definition "A Feasibility Study that is specifically identified in a final report from a Comprehensive or Basin-wide Study and that would be carried out under the same study authority as the Comprehensive or Basin-wide, if provided for by that authority, is termed a Spin-off Study." ;
    skos:inScheme CECW-11-2-220: ;
    skos:prefLabel "Spin-off Studies" .

CECW-11-2-220:Systems a wov:GlossaryTerm,
        skos:Concept ;
    rdfs:label "Systems" ;
    dcterms:bibliographicCitation "https://www.publications.usace.army.mil/Portals/76/Users/182/86/2486/EC_11-2-220.pdf#page=279" ;
    pav:wasDerivedFrom "glossaries/CivilWorks/CECW-11-2-220.yaml#term[Systems]" ;
    skos:definition "Is an area with a common function, such as a coastal system, navigation system or ecosystem. A system boundary is not a true drainage boundary, but does have hydrological function considerations. The term watershed will be used throughout this budget EC, and will refer to both watersheds and coastal systems." ;
    skos:inScheme CECW-11-2-220: ;
    skos:prefLabel "Systems" .

CECW-11-2-220:Systems-Based_Budgeting a wov:GlossaryTerm,
        skos:Concept ;
    rdfs:label "Systems-Based Budgeting" ;
    dcterms:bibliographicCitation "https://www.publications.usace.army.mil/Portals/76/Users/182/86/2486/EC_11-2-220.pdf#page=279" ;
    pav:wasDerivedFrom "glossaries/CivilWorks/CECW-11-2-220.yaml#term[Systems-Based Budgeting]" ;
    skos:altLabel "SBB" ;
    skos:definition "(SBB) explicitly acknowledges that the projects and work packages included in each year's budget submission are interconnected, within the context of systems and watersheds in which they operate. As such, the decision to fund (or not to fund) any given project or work package influences both the stand-alone project and system as a whole. Systems-based budgeting accounts for the interconnected performance of projects within watersheds and systems, in order to provide decision makers with a more clearly articulated description of work packages and project Value to Nation." ;
    skos:inScheme CECW-11-2-220: ;
    skos:prefLabel "Systems-Based Budgeting" .

CECW-11-2-220:Validation_Study a wov:GlossaryTerm,
        skos:Concept ;
    rdfs:label "Validation Study" ;
    dcterms:bibliographicCitation "https://www.publications.usace.army.mil/Portals/76/Users/182/86/2486/EC_11-2-220.pdf#page=279" ;
    pav:wasDerivedFrom "glossaries/CivilWorks/CECW-11-2-220.yaml#term[Validation Study]" ;
    skos:altLabel "VS" ;
    skos:definition "This is a reexamination of project justification, including the economics and/or environmental effects that does not require reformulation of alternatives. A Validation Study may be carried out using any funds appropriated for the project and the cost of the Validation Study is shared under the applicable Design Agreement or Project Partnership Agreement." ;
    skos:inScheme CECW-11-2-220: ;
    skos:prefLabel "Validation Study" .

CECW-11-2-220:Value_to_the_Nation a wov:GlossaryTerm,
        skos:Concept ;
    rdfs:label "Value to the Nation" ;
    dcterms:bibliographicCitation "https://www.publications.usace.army.mil/Portals/76/Users/182/86/2486/EC_11-2-220.pdf#page=279" ;
    pav:wasDerivedFrom "glossaries/CivilWorks/CECW-11-2-220.yaml#term[Value to the Nation]" ;
    skos:altLabel "VTN" ;
    skos:definition "Is defined broadly as improving economic growth, protecting the environment, and providing for the social well-being of the Nation." ;
    skos:inScheme CECW-11-2-220: ;
    skos:prefLabel "Value to the Nation" .

CECW-11-2-220:Watershed a wov:GlossaryTerm,
        skos:Concept ;
    rdfs:label "Watershed" ;
    dcterms:bibliographicCitation "https://www.publications.usace.army.mil/Portals/76/Users/182/86/2486/EC_11-2-220.pdf#page=279" ;
    pav:wasDerivedFrom "glossaries/CivilWorks/CECW-11-2-220.yaml#term[Watershed]" ;
    skos:definition "Is a geographic area which drains to a common river or body of water. Looking at water resource infrastructure and activities is called watershed management. Watershed management takes a comprehensive look at natural and man-made functions of the hydrologic system and impacts to that system." ;
    skos:inScheme CECW-11-2-220: ;
    skos:prefLabel "Watershed" .

CECW-11-2-220:Work_Increment a wov:GlossaryTerm,
        skos:Concept ;
    rdfs:label "Work Increment" ;
    dcterms:bibliographicCitation "https://www.publications.usace.army.mil/Portals/76/Users/182/86/2486/EC_11-2-220.pdf#page=279" ;
    pav:wasDerivedFrom "glossaries/CivilWorks/CECW-11-2-220.yaml#term[Work Increment]" ;
    skos:definition "A work increment is a discrete amount of work identified by an activity or a set of activities with specific resource requirements and a schedule." ;
    skos:inScheme CECW-11-2-220: ;
    skos:prefLabel "Work Increment" .

CECW-11-2-220: a wov:Glossary,
        owl:Ontology,
        skos:ConceptScheme,
        voaf:Vocabulary ;
    rdfs:label "Civil Works Direct Program Development Policy Guidance CECW-IP No. 11-2-220" ;
    dcterms:created "2024-07-16T04:22:43.789240+00:00"^^xsd:dateTime ;
    dcterms:description "The Civil Works Direct Program Development Policy Guidance (Circular CECW-IP No. 11-2-220) defines various acronyms and terms commonly used in this circular to describe policie guidance, budget activities and allocation strategy. These terms are defined in the glossary section of the circular." ;
    dcterms:publisher "None" ;
    dcterms:rights "MIT" ;
    dcterms:title "Civil Works Direct Program Development Policy Guidance CECW-IP No. 11-2-220" ;
    pav:ImportedFrom "glossaries/CivilWorks/CECW-11-2-220.yaml" ;
    pav:createdOn "2024-07-16T04:22:43.789240+00:00"^^xsd:dateTime ;
    pav:createdWith "gloss" ;
    pav:wasInfluencedBy "Civil Works Direct Program Development Policy Guidance CECW-IP No. 11-2-220" ;
    vann:preferredNamespaceUri "https://usace-data.com/civil-works/glossary/CECW-11-2-220#" ;
    skos:hasTopConcept CECW-11-2-220:Activity,
        CECW-11-2-220:Benefit_Cost_Ratio,
        CECW-11-2-220:Capability,
        CECW-11-2-220:Caretaker_Status,
        CECW-11-2-220:Civil_Works_Integrated_Funding_Database,
        CECW-11-2-220:Common_Operation_and_Maintenance,
        CECW-11-2-220:Component_Renewal,
        CECW-11-2-220:Corrective_Maintenance,
        CECW-11-2-220:Critical_Infrastructure_Protection_%26_Resilience_Program,
        CECW-11-2-220:Critical_Work_Activities%2FPackages,
        CECW-11-2-220:Cyclical_Maintenance,
        CECW-11-2-220:Enterprise-Wide_Capability_for_Allocation_Strategy,
        CECW-11-2-220:FEM_Work_Order_Number,
        CECW-11-2-220:FUSRAP,
        CECW-11-2-220:Facility_Operation,
        CECW-11-2-220:General_Reevaluation_Study,
        CECW-11-2-220:Inactive_Facility,
        CECW-11-2-220:Level_of_Performance,
        CECW-11-2-220:Limited_Reevaluation_Study,
        CECW-11-2-220:Lowest_Sustainable_Investment,
        CECW-11-2-220:MAX_%28OMB%29_Collection_and_Collaboration_Process,
        CECW-11-2-220:Maintenance,
        CECW-11-2-220:Major_Maintenance,
        CECW-11-2-220:Major_Rehabilitation,
        CECW-11-2-220:Mothball_status,
        CECW-11-2-220:New_Investment,
        CECW-11-2-220:Non-critical_Work_Activities%2FPackages,
        CECW-11-2-220:Operation,
        CECW-11-2-220:Operation_and_Maintenance,
        CECW-11-2-220:Post-Feasibility_Studies,
        CECW-11-2-220:President%27s_Budget_Rank,
        CECW-11-2-220:Preventive_Maintenance,
        <https://usace-data.com/civil-works/glossary/CECW-11-2-220#Program,_Project,_or_Activity>,
        CECW-11-2-220:Program_Code,
        CECW-11-2-220:Project_Partnership_Agreement%2FPartnership_Agreement,
        CECW-11-2-220:Recurring_Maintenance,
        CECW-11-2-220:Rehabilitation,
        CECW-11-2-220:Remaining_Benefits_Remaining_Cost_Ratio,
        CECW-11-2-220:Resumption-_Construction,
        CECW-11-2-220:Resumption-_Study,
        CECW-11-2-220:Rounding,
        CECW-11-2-220:Section_902_Post_Authorization_Study,
        CECW-11-2-220:Smart_Use_of_Systems,
        CECW-11-2-220:Specific_Work_Activities,
        CECW-11-2-220:Spin-off_Studies,
        CECW-11-2-220:Systems,
        CECW-11-2-220:Systems-Based_Budgeting,
        CECW-11-2-220:Validation_Study,
        CECW-11-2-220:Value_to_the_Nation,
        CECW-11-2-220:Watershed,
        CECW-11-2-220:Work_Increment .

