@prefix CFR-33-238-4: <https://usace-data.com/civil-works/glossary/CFR-33-238-4#> .
@prefix dcterms: <http://purl.org/dc/terms/> .
@prefix owl: <http://www.w3.org/2002/07/owl#> .
@prefix pav: <http://purl.org/pav#> .
@prefix rdfs: <http://www.w3.org/2000/01/rdf-schema#> .
@prefix skos: <http://www.w3.org/2004/02/skos/core#> .
@prefix vann: <http://purl.org/vocab/vann/> .
@prefix voaf: <https://lov.linkeddata.es/vocommons/voaf/v2.0/voaf_v2.0.rdf#> .
@prefix wov: <http://www.knowledgesmarts.com/ontologies/wov#> .
@prefix xsd: <http://www.w3.org/2001/XMLSchema#> .

CFR-33-238-4:Flood_damage_reduction_works_in_urban_areas a wov:GlossaryTerm,
        skos:Concept ;
    rdfs:label "Flood damage reduction works in urban areas" ;
    dcterms:bibliographicCitation "33 CFR 238.4" ;
    pav:wasDerivedFrom "glossaries/CivilWorks/CFR-33-238-4.yaml#term[Flood damage reduction works in urban areas]" ;
    skos:definition "are the adjustments in land use and the facilities (structural and non-structural) designed to reduce flood damages in urban areas from overflow or backwater due to major storms and snowmelt. They include structural and other engineering modifications to natural streams or to previously modified natural waterways. Flood damage reduction works are designed to modify flood behavior typified by temporary conditions of inundation of normally dry land from the overflow of rivers and streams or from abnormally high coastal waters due to sever storms." ;
    skos:inScheme CFR-33-238-4: ;
    skos:prefLabel "Flood damage reduction works in urban areas" .

CFR-33-238-4:Storm_sewer_systems a wov:GlossaryTerm,
        skos:Concept ;
    rdfs:label "Storm sewer systems" ;
    dcterms:bibliographicCitation "33 CFR 238.4" ;
    pav:wasDerivedFrom "glossaries/CivilWorks/CFR-33-238-4.yaml#term[Storm sewer systems]" ;
    skos:definition "are the facilities in urban areas designed to collect and convey runoff from rainfall or snowmelt in the urban area to natural water courses or to previously modified natural waterways. They include storm drains, inlets, manholes, pipes, culverts, conduits, sewers and sewer appurtenances, on-site storage and detention basins, curbs and gutters, and other small drainageways that remove or help to manage runoff in urban areas. Storm sewer systems are designed to solve storm drainage problems, which are typified by excessive accumulation of runoff in depressions; overland sheet flow resulting from rapid snowmelt or rainfall; and excessive accumulation of water at the facilities listed in this paragraph because of their limited capacity." ;
    skos:inScheme CFR-33-238-4: ;
    skos:prefLabel "Storm sewer systems" .

CFR-33-238-4:Urban_areas a wov:GlossaryTerm,
        skos:Concept ;
    rdfs:label "Urban areas" ;
    dcterms:bibliographicCitation "33 CFR 238.4" ;
    pav:wasDerivedFrom "glossaries/CivilWorks/CFR-33-238-4.yaml#term[Urban areas]" ;
    skos:definition """are cities, towns, or other incorporated or unincorporated political subdivisions of States that: 
(1) Provide general local government for specific population concentrations, and, 
(2) Occupy an essentially continuous area of developed land, containing such structures as residences, public and commercial buildings, and industrial sites.""" ;
    skos:inScheme CFR-33-238-4: ;
    skos:prefLabel "Urban areas" .

CFR-33-238-4: a wov:Glossary,
        owl:Ontology,
        skos:ConceptScheme,
        voaf:Vocabulary ;
    rdfs:label "Code of Federal Regulations - Title 33, Chapter-II, Part 238, Section-238.4" ;
    dcterms:created "2024-07-16T04:23:15.370289+00:00"^^xsd:dateTime ;
    dcterms:description "33-CFR-2038.4 Term definitions are applicable throughout part 238" ;
    dcterms:publisher "None" ;
    dcterms:rights "MIT" ;
    dcterms:title "Code of Federal Regulations - Title 33, Chapter-II, Part 238, Section-238.4" ;
    pav:ImportedFrom "glossaries/CivilWorks/CFR-33-238-4.yaml" ;
    pav:createdOn "2024-07-16T04:23:15.370289+00:00"^^xsd:dateTime ;
    pav:createdWith "gloss" ;
    pav:wasInfluencedBy "33 CFR 238.4" ;
    vann:preferredNamespaceUri "https://usace-data.com/civil-works/glossary/CFR-33-238-4#" ;
    skos:hasTopConcept CFR-33-238-4:Flood_damage_reduction_works_in_urban_areas,
        CFR-33-238-4:Storm_sewer_systems,
        CFR-33-238-4:Urban_areas .

