@prefix CFR-33-203-15: <https://usace-data.com/civil-works/glossary/CFR-33-203-15#> .
@prefix dcterms: <http://purl.org/dc/terms/> .
@prefix owl: <http://www.w3.org/2002/07/owl#> .
@prefix pav: <http://purl.org/pav#> .
@prefix rdfs: <http://www.w3.org/2000/01/rdf-schema#> .
@prefix skos: <http://www.w3.org/2004/02/skos/core#> .
@prefix vann: <http://purl.org/vocab/vann/> .
@prefix voaf: <https://lov.linkeddata.es/vocommons/voaf/v2.0/voaf_v2.0.rdf#> .
@prefix wov: <http://www.knowledgesmarts.com/ontologies/wov#> .
@prefix xsd: <http://www.w3.org/2001/XMLSchema#> .

CFR-33-203-15:Federal_project a wov:GlossaryTerm,
        skos:Concept ;
    rdfs:label "Federal project" ;
    dcterms:bibliographicCitation "https://www.ecfr.gov/title-33/part-203/section-203.15/#p-203.15Federal_project" ;
    pav:wasDerivedFrom "glossaries/CivilWorks/CFR-33-203-15.yaml#term[Federal project]" ;
    skos:definition "A project constructed by the Corps, and subsequently turned over to a local sponsor for operations and maintenance responsibility. This definition also includes any project specifically designated as a Federal project by an Act of Congress." ;
    skos:inScheme CFR-33-203-15: ;
    skos:prefLabel "Federal project" .

CFR-33-203-15:Flood_control_project%3A_A_project_designed_and_constructed_to_have_appreciable_and_dependable_effects_in_preventing_damage_from_irregular_and_unusual_rises_in_water_level a wov:GlossaryTerm,
        skos:Concept ;
    rdfs:label "Flood control project: A project designed and constructed to have appreciable and dependable effects in preventing damage from irregular and unusual rises in water level" ;
    dcterms:bibliographicCitation "https://www.ecfr.gov/title-33/part-203/section-203.15/#p-203.15Flood_control_project%3A_A_project_designed_and_constructed_to_have_appreciable_and_dependable_effects_in_preventing_damage_from_irregular_and_unusual_rises_in_water_level" ;
    pav:wasDerivedFrom "glossaries/CivilWorks/CFR-33-203-15.yaml#term[Flood control project: A project designed and constructed to have appreciable and dependable effects in preventing damage from irregular and unusual rises in water level]" ;
    skos:definition "For a multipurpose project, only those components that are necessary for the flood control function are considered eligible for Rehabilitation Assistance." ;
    skos:inScheme CFR-33-203-15: ;
    skos:prefLabel "Flood control project: A project designed and constructed to have appreciable and dependable effects in preventing damage from irregular and unusual rises in water level" .

CFR-33-203-15:Governor a wov:GlossaryTerm,
        skos:Concept ;
    rdfs:label "Governor" ;
    dcterms:bibliographicCitation "https://www.ecfr.gov/title-33/part-203/section-203.15/#p-203.15Governor" ;
    pav:wasDerivedFrom "glossaries/CivilWorks/CFR-33-203-15.yaml#term[Governor]" ;
    skos:definition "All references in part 203 to the Governor of a State also refer to: the Governors of United States commonwealths, territories, and possessions; and the Mayor of Washington, D.C." ;
    skos:inScheme CFR-33-203-15: ;
    skos:prefLabel "Governor" .

CFR-33-203-15:Hurricane%2FShore_Protection_Project_%28HSPP%29 a wov:GlossaryTerm,
        skos:Concept ;
    rdfs:label "Hurricane/Shore Protection Project (HSPP)" ;
    dcterms:bibliographicCitation "https://www.ecfr.gov/title-33/part-203/section-203.15/#p-203.15Hurricane%2FShore_Protection_Project_%28HSPP%29" ;
    pav:wasDerivedFrom "glossaries/CivilWorks/CFR-33-203-15.yaml#term[Hurricane/Shore Protection Project (HSPP)]" ;
    skos:altLabel "HSPP" ;
    skos:definition "A flood control project designed and constructed to have appreciable and predictable effects in preventing damage to developed areas from the impacts of hurricanes, tsunamis, and coastal storms. These effects are primarily to protect against wave action, storm surge, wind, and the complicating factors of extraordinary high tides. HSPP's include projects known as shore protection projects, shore protection structures, periodic nourishment projects, shore enhancement projects, and similar terms. Components of an HSPP may include both hard (permanent construction) and soft (sacrificial, i.e., sand) features." ;
    skos:inScheme CFR-33-203-15: ;
    skos:prefLabel "Hurricane/Shore Protection Project (HSPP)" .

CFR-33-203-15:Non-Federal_project a wov:GlossaryTerm,
        skos:Concept ;
    rdfs:label "Non-Federal project" ;
    dcterms:bibliographicCitation "https://www.ecfr.gov/title-33/part-203/section-203.15/#p-203.15Non-Federal_project" ;
    pav:wasDerivedFrom "glossaries/CivilWorks/CFR-33-203-15.yaml#term[Non-Federal project]" ;
    skos:definition "A project constructed with non-Federal funds, or a project constructed by tribal, State, local, or private interests, or a component of such a project. A project constructed under Federal emergency disaster authorities, such as Public Law 84-99 or the Robert T. Stafford Disaster Relief and Emergency Assistance Act, as amended (42 U.S.C. 5121, et seq.) (hereinafter referred to as the Stafford Act), is a non-Federal project unless it repairs or replaces an existing Federal project. Works Progress Administration (WPA) projects, and projects funded completely or partially by other (non-Corps) Federal agencies, are considered non-Federal projects for the application of Public Law 84-99 authority." ;
    skos:inScheme CFR-33-203-15: ;
    skos:prefLabel "Non-Federal project" .

CFR-33-203-15:Non-Federal_sponsor a wov:GlossaryTerm,
        skos:Concept ;
    rdfs:label "Non-Federal sponsor" ;
    dcterms:bibliographicCitation "https://www.ecfr.gov/title-33/part-203/section-203.15/#p-203.15Non-Federal_sponsor" ;
    pav:wasDerivedFrom "glossaries/CivilWorks/CFR-33-203-15.yaml#term[Non-Federal sponsor]" ;
    skos:definition "A non-Federal sponsor is a public entity that is a legally constituted public body with full authority and capability to perform the terms of its agreement as the non-Federal partner of the Corps for a project, and able to pay damages, if necessary, in the event of its failure to perform. A non-Federal sponsor may be a State, County, City, Town, Federally recognized Indian Tribe or tribal organization, Alaska Native Corporation, or any political subpart of a State or group of states that has the legal and financial authority and capability to provide the necessary cash contributions and LERRD's necessary for the project." ;
    skos:inScheme CFR-33-203-15: ;
    skos:prefLabel "Non-Federal sponsor" .

CFR-33-203-15:Repair_and_rehabilitation a wov:GlossaryTerm,
        skos:Concept ;
    rdfs:label "Repair and rehabilitation" ;
    dcterms:bibliographicCitation "https://www.ecfr.gov/title-33/part-203/section-203.15/#p-203.15Repair_and_rehabilitation" ;
    pav:wasDerivedFrom "glossaries/CivilWorks/CFR-33-203-15.yaml#term[Repair and rehabilitation]" ;
    skos:definition "The term repair and rehabilitation means the repair or rebuilding of a flood control structure, after the structure has been damaged by a flood, hurricane, or coastal storm, to the level of protection provided by the structure prior to the flood, hurricane, or coastal storm. Repair and rehabilitation does not include improvements (betterments) to the structure, nor does repair and rehabilitation include any repair or rebuilding of a flood control structure that, in the normal course of usage, has become structurally unsound and is no longer fit to provide the level of protection for which it was designed." ;
    skos:inScheme CFR-33-203-15: ;
    skos:prefLabel "Repair and rehabilitation" .

CFR-33-203-15: a wov:Glossary,
        owl:Ontology,
        skos:ConceptScheme,
        voaf:Vocabulary ;
    rdfs:label "Code of Federal Regulations - Title 33, Chapter-II, Part 203, Section-203.15" ;
    dcterms:created "2024-07-16T04:23:07.147908+00:00"^^xsd:dateTime ;
    dcterms:description "33-CFR-203.15 Term definitions are applicable throughout part 203" ;
    dcterms:publisher "None" ;
    dcterms:rights "MIT" ;
    dcterms:title "Code of Federal Regulations - Title 33, Chapter-II, Part 203, Section-203.15" ;
    pav:ImportedFrom "glossaries/CivilWorks/CFR-33-203-15.yaml" ;
    pav:createdOn "2024-07-16T04:23:07.147908+00:00"^^xsd:dateTime ;
    pav:createdWith "gloss" ;
    pav:wasInfluencedBy "CFR 203.15 Definitions" ;
    vann:preferredNamespaceUri "https://usace-data.com/civil-works/glossary/CFR-33-203-15#" ;
    skos:hasTopConcept CFR-33-203-15:Federal_project,
        CFR-33-203-15:Flood_control_project%3A_A_project_designed_and_constructed_to_have_appreciable_and_dependable_effects_in_preventing_damage_from_irregular_and_unusual_rises_in_water_level,
        CFR-33-203-15:Governor,
        CFR-33-203-15:Hurricane%2FShore_Protection_Project_%28HSPP%29,
        CFR-33-203-15:Non-Federal_project,
        CFR-33-203-15:Non-Federal_sponsor,
        CFR-33-203-15:Repair_and_rehabilitation .

