@prefix CFR-33-277-4: <https://usace-data.com/civil-works/glossary/CFR-33-277-4#> .
@prefix dcterms: <http://purl.org/dc/terms/> .
@prefix owl: <http://www.w3.org/2002/07/owl#> .
@prefix pav: <http://purl.org/pav#> .
@prefix rdfs: <http://www.w3.org/2000/01/rdf-schema#> .
@prefix skos: <http://www.w3.org/2004/02/skos/core#> .
@prefix vann: <http://purl.org/vocab/vann/> .
@prefix voaf: <https://lov.linkeddata.es/vocommons/voaf/v2.0/voaf_v2.0.rdf#> .
@prefix wov: <http://www.knowledgesmarts.com/ontologies/wov#> .
@prefix xsd: <http://www.w3.org/2001/XMLSchema#> .

CFR-33-277-4:Alteration a wov:GlossaryTerm,
        skos:Concept ;
    rdfs:label "Alteration" ;
    dcterms:bibliographicCitation "33 CFR 277.4" ;
    pav:wasDerivedFrom "glossaries/CivilWorks/CFR-33-277-4.yaml#term[Alteration]" ;
    skos:definition "The term alteration includes changes of any kind, reconstruction, or removal in whole or in part." ;
    skos:inScheme CFR-33-277-4: ;
    skos:prefLabel "Alteration" .

CFR-33-277-4:Bridge a wov:GlossaryTerm,
        skos:Concept ;
    rdfs:label "Bridge" ;
    dcterms:bibliographicCitation "33 CFR 277.4" ;
    pav:wasDerivedFrom "glossaries/CivilWorks/CFR-33-277-4.yaml#term[Bridge]" ;
    skos:definition "The term bridge means a lawful bridge over navigable waters of the United States, including approaches, fenders, and appurtenances thereto, which is used and operated for the purpose of carrying railroad traffic, or both railroad and highway traffic, or if a State, county, municipality, or other political subdivision is the owner or joint owner thereof, which is used and operated for the purpose of carrying highway traffic." ;
    skos:inScheme CFR-33-277-4: ;
    skos:prefLabel "Bridge" .

CFR-33-277-4:Bridge_owner a wov:GlossaryTerm,
        skos:Concept ;
    rdfs:label "Bridge owner" ;
    dcterms:bibliographicCitation "33 CFR 277.4" ;
    pav:wasDerivedFrom "glossaries/CivilWorks/CFR-33-277-4.yaml#term[Bridge owner]" ;
    skos:definition "Bridge owner means any State, county, municipality, or other political subdivision, or any corporation, association, partnership, or individual owning, or jointly owning, any bridge, and, when any bridge shall be in the possession or under the control of any trustee, receiver, trustee in bankruptcy, or lessee, such term shall include both the owner of the legal title and the person or the entity in possession or control of such bridge." ;
    skos:inScheme CFR-33-277-4: ;
    skos:prefLabel "Bridge owner" .

CFR-33-277-4:Navigable_waters a wov:GlossaryTerm,
        skos:Concept ;
    rdfs:label "Navigable waters" ;
    dcterms:bibliographicCitation "33 CFR 277.4" ;
    pav:wasDerivedFrom "glossaries/CivilWorks/CFR-33-277-4.yaml#term[Navigable waters]" ;
    skos:definition "Navigable waters of the United States means those waterbodies, except the territorial seas, which are subject to the ebb and flow of the tide, or are presently, or have been in the past, or may be in the future susceptible for use for purposes of interstate or foreign commerce." ;
    skos:inScheme CFR-33-277-4: ;
    skos:prefLabel "Navigable waters" .

CFR-33-277-4: a wov:Glossary,
        owl:Ontology,
        skos:ConceptScheme,
        voaf:Vocabulary ;
    rdfs:label "Code of Federal Regulations - Title 33, Chapter-II, Part 277, Section-277.4" ;
    dcterms:created "2024-07-16T04:23:41.276405+00:00"^^xsd:dateTime ;
    dcterms:description "33-CFR-277.4 Term definitions are applicable throughout part 277" ;
    dcterms:publisher "None" ;
    dcterms:rights "MIT" ;
    dcterms:title "Code of Federal Regulations - Title 33, Chapter-II, Part 277, Section-277.4" ;
    pav:ImportedFrom "glossaries/CivilWorks/CFR-33-277-4.yaml" ;
    pav:createdOn "2024-07-16T04:23:41.276405+00:00"^^xsd:dateTime ;
    pav:createdWith "gloss" ;
    pav:wasInfluencedBy "33 CFR 277.4" ;
    vann:preferredNamespaceUri "https://usace-data.com/civil-works/glossary/CFR-33-277-4#" ;
    skos:hasTopConcept CFR-33-277-4:Alteration,
        CFR-33-277-4:Bridge,
        CFR-33-277-4:Bridge_owner,
        CFR-33-277-4:Navigable_waters .

