@prefix CFR-33-330-2: <https://usace-data.com/civil-works/glossary/CFR-33-330-2#> .
@prefix dcterms: <http://purl.org/dc/terms/> .
@prefix owl: <http://www.w3.org/2002/07/owl#> .
@prefix pav: <http://purl.org/pav#> .
@prefix rdfs: <http://www.w3.org/2000/01/rdf-schema#> .
@prefix skos: <http://www.w3.org/2004/02/skos/core#> .
@prefix vann: <http://purl.org/vocab/vann/> .
@prefix voaf: <https://lov.linkeddata.es/vocommons/voaf/v2.0/voaf_v2.0.rdf#> .
@prefix wov: <http://www.knowledgesmarts.com/ontologies/wov#> .
@prefix xsd: <http://www.w3.org/2001/XMLSchema#> .

CFR-33-330-2:Authorization a wov:GlossaryTerm,
        skos:Concept ;
    rdfs:label "Authorization" ;
    dcterms:bibliographicCitation "https://www.ecfr.gov/current/title-33/chapter-II/part-330/section-330.2" ;
    pav:wasDerivedFrom "glossaries/CivilWorks/CFR-33-330-2.yaml#term[Authorization]" ;
    skos:definition "means that specific activities that qualify for an NWP may proceed, provided that the terms and conditions of the NWP are met. After determining that the activity complies with all applicable terms and conditions, the prospective permittee may assume an authorization under an NWP. This assumption is subject to the DE's authority to determine if an activity complies with the terms and conditions of an NWP. If requested by the permittee in writing, the DE will verify in writing that the permittee's proposed activity complies with the terms and conditions of the NWP. A written verification may contain activity-specific conditions and regional conditions which a permittee must satisfy for the authorization to be valid." ;
    skos:inScheme CFR-33-330-2: ;
    skos:prefLabel "Authorization" .

CFR-33-330-2:Discretionary_authority a wov:GlossaryTerm,
        skos:Concept ;
    rdfs:label "Discretionary authority" ;
    dcterms:bibliographicCitation "https://www.ecfr.gov/current/title-33/chapter-II/part-330/section-330.2" ;
    pav:wasDerivedFrom "glossaries/CivilWorks/CFR-33-330-2.yaml#term[Discretionary authority]" ;
    skos:definition "means the authority described in Â§Â§ 330.1(d) and 330.4(e) which the Chief of Engineers delegates to division or district engineers to modify an NWP authorization by adding conditions, to suspend an NWP authorization, or to revoke an NWP authorization and thus require individual permit authorization." ;
    skos:inScheme CFR-33-330-2: ;
    skos:prefLabel "Discretionary authority" .

CFR-33-330-2:Filled_area a wov:GlossaryTerm,
        skos:Concept ;
    rdfs:label "Filled area" ;
    dcterms:bibliographicCitation "https://www.ecfr.gov/current/title-33/chapter-II/part-330/section-330.2" ;
    pav:wasDerivedFrom "glossaries/CivilWorks/CFR-33-330-2.yaml#term[Filled area]" ;
    skos:definition "means the area within jurisdictional waters which is eliminated or covered as a direct result of the discharge (i.e., the area actually covered by the discharged material). It does not include areas excavated nor areas impacted as an indirect effect of the fill." ;
    skos:inScheme CFR-33-330-2: ;
    skos:prefLabel "Filled area" .

CFR-33-330-2:Headwaters a wov:GlossaryTerm,
        skos:Concept ;
    rdfs:label "Headwaters" ;
    dcterms:bibliographicCitation "https://www.ecfr.gov/current/title-33/chapter-II/part-330/section-330.2" ;
    pav:wasDerivedFrom "glossaries/CivilWorks/CFR-33-330-2.yaml#term[Headwaters]" ;
    skos:definition "means non-tidal rivers, streams, and their lakes and impoundments, including adjacent wetlands, that are part of a surface tributary system to an interstate or navigable water of the United States upstream of the point on the river or stream at which the average annual flow is less than five cubic feet per second. The DE may estimate this point from available data by using the mean annual area precipitation, area drainage basin maps, and the average runoff coefficient, or by similar means. For streams that are dry for long periods of the year, DEs may establish the point where headwaters begin as that point on the stream where a flow of five cubic feet per second is equaled or exceeded 50 percent of the time." ;
    skos:inScheme CFR-33-330-2: ;
    skos:prefLabel "Headwaters" .

CFR-33-330-2:Isolated_waters a wov:GlossaryTerm,
        skos:Concept ;
    rdfs:label "Isolated waters" ;
    dcterms:bibliographicCitation "https://www.ecfr.gov/current/title-33/chapter-II/part-330/section-330.2" ;
    pav:wasDerivedFrom "glossaries/CivilWorks/CFR-33-330-2.yaml#term[Isolated waters]" ;
    skos:definition """means those non-tidal waters of the United States that are: 
(1) Not part of a surface tributary system to interstate or navigable waters of the United States; and 
(2) Not adjacent to such tributary waterbodies.""" ;
    skos:inScheme CFR-33-330-2: ;
    skos:prefLabel "Isolated waters" .

CFR-33-330-2:Nationwide_Permit a wov:GlossaryTerm,
        skos:Concept ;
    rdfs:label "Nationwide Permit" ;
    dcterms:bibliographicCitation "https://www.ecfr.gov/current/title-33/chapter-II/part-330/section-330.2" ;
    pav:wasDerivedFrom "glossaries/CivilWorks/CFR-33-330-2.yaml#term[Nationwide Permit]" ;
    skos:definition "Nationwide  permit refers to a type of general permit which authorizes activities on a nationwide basis unless specifically limited. (Another type of general permit is a regional permit which is issued by division or district engineers on a regional basis in accordance with 33 CFR part 325). (See 33 CFR 322.2(f) and 323.2(h) for the definition of a general permit.)" ;
    skos:inScheme CFR-33-330-2: ;
    skos:prefLabel "Nationwide Permit" .

CFR-33-330-2:Single_and_complete_project a wov:GlossaryTerm,
        skos:Concept ;
    rdfs:label "Single and complete project" ;
    dcterms:bibliographicCitation "https://www.ecfr.gov/current/title-33/chapter-II/part-330/section-330.2" ;
    pav:wasDerivedFrom "glossaries/CivilWorks/CFR-33-330-2.yaml#term[Single and complete project]" ;
    skos:definition "means the total project proposed or accomplished by one owner/developer or partnership or other association of owners/developers. For example, if construction of a residential development affects several different areas of a headwater or isolated water, or several different headwaters or isolated waters, the cumulative total of all filled areas should be the basis for deciding whether or not the project will be covered by an NWP. For linear projects, the single and complete project (i.e., single and complete crossing) will apply to each crossing of a separate water of the United States (i.e., single waterbody) at that location; except that for linear projects crossing a single waterbody several times at separate and distant locations, each crossing is considered a single and complete project. However, individual channels in a braided stream or river, or individual arms of a large, irregularly-shaped wetland or lake, etc., are not separate waterbodies." ;
    skos:inScheme CFR-33-330-2: ;
    skos:prefLabel "Single and complete project" .

CFR-33-330-2:Special_aquatic_sites a wov:GlossaryTerm,
        skos:Concept ;
    rdfs:label "Special aquatic sites" ;
    dcterms:bibliographicCitation "https://www.ecfr.gov/current/title-33/chapter-II/part-330/section-330.2" ;
    pav:wasDerivedFrom "glossaries/CivilWorks/CFR-33-330-2.yaml#term[Special aquatic sites]" ;
    skos:definition "means wetlands, mudflats, vegetated shallows, coral reefs, riffle and pool complexes, sanctuaries, and refuges as defined at 40 CFR 230.40 through 230.45." ;
    skos:inScheme CFR-33-330-2: ;
    skos:prefLabel "Special aquatic sites" .

CFR-33-330-2:Terms_and_conditions a wov:GlossaryTerm,
        skos:Concept ;
    rdfs:label "Terms and conditions" ;
    dcterms:bibliographicCitation "https://www.ecfr.gov/current/title-33/chapter-II/part-330/section-330.2" ;
    pav:wasDerivedFrom "glossaries/CivilWorks/CFR-33-330-2.yaml#term[Terms and conditions]" ;
    skos:definition "The terms of an NWP are the limitations and provisions included in the description of the NWP itself. The conditions of NWPs are additional provisions which place restrictions or limitations on all of the NWPs. These are published with the NWPs. Other conditions may be imposed by district or division engineers on a geographic, category-of-activity, or activity-specific basis (See 33 CFR 330.4(e))." ;
    skos:inScheme CFR-33-330-2: ;
    skos:prefLabel "Terms and conditions" .

CFR-33-330-2: a wov:Glossary,
        owl:Ontology,
        skos:ConceptScheme,
        voaf:Vocabulary ;
    rdfs:label "Code of Federal Regulations - Title 33, Chapter-II, Part 330, Section-330.2" ;
    dcterms:created "2024-07-16T04:24:56.768521+00:00"^^xsd:dateTime ;
    dcterms:description "None" ;
    dcterms:publisher "None" ;
    dcterms:rights "MIT" ;
    dcterms:title "Code of Federal Regulations - Title 33, Chapter-II, Part 330, Section-330.2" ;
    pav:ImportedFrom "glossaries/CivilWorks/CFR-33-330-2.yaml" ;
    pav:createdOn "2024-07-16T04:24:56.768521+00:00"^^xsd:dateTime ;
    pav:createdWith "gloss" ;
    pav:wasInfluencedBy "33 CFR 330.2 Definitions" ;
    vann:preferredNamespaceUri "https://usace-data.com/civil-works/glossary/CFR-33-330-2#" ;
    skos:hasTopConcept CFR-33-330-2:Authorization,
        CFR-33-330-2:Discretionary_authority,
        CFR-33-330-2:Filled_area,
        CFR-33-330-2:Headwaters,
        CFR-33-330-2:Isolated_waters,
        CFR-33-330-2:Nationwide_Permit,
        CFR-33-330-2:Single_and_complete_project,
        CFR-33-330-2:Special_aquatic_sites,
        CFR-33-330-2:Terms_and_conditions .

