@prefix ER-1110-2-1156: <https://usace-data.com/civil-works/glossary/ER-1110-2-1156#> .
@prefix dcterms: <http://purl.org/dc/terms/> .
@prefix owl: <http://www.w3.org/2002/07/owl#> .
@prefix pav: <http://purl.org/pav#> .
@prefix rdfs: <http://www.w3.org/2000/01/rdf-schema#> .
@prefix skos: <http://www.w3.org/2004/02/skos/core#> .
@prefix vann: <http://purl.org/vocab/vann/> .
@prefix voaf: <https://lov.linkeddata.es/vocommons/voaf/v2.0/voaf_v2.0.rdf#> .
@prefix wov: <http://www.knowledgesmarts.com/ontologies/wov#> .
@prefix xsd: <http://www.w3.org/2001/XMLSchema#> .

ER-1110-2-1156:ATR_Team a wov:GlossaryTerm,
        skos:Concept ;
    rdfs:label "ATR Team" ;
    dcterms:bibliographicCitation "https://www.publications.usace.army.mil/Portals/76/Users/182/86/2486/er_1110-2-1156.pdf#page=487" ;
    pav:wasDerivedFrom "glossaries/CivilWorks/ER-1110-2-1156.yaml#term[ATR Team]" ;
    skos:definition "For dam safety studies, the ATR team must include members from and be coordinated with the RMC as well as recognized experts (internal and external to USACE) in the field of risk assessment. The ATR team findings will be vetted with the MSC DSO, Risk Management Center, and HQUSACE." ;
    skos:inScheme ER-1110-2-1156: ;
    skos:prefLabel "ATR Team" .

ER-1110-2-1156:Abutment a wov:GlossaryTerm,
        skos:Concept ;
    rdfs:label "Abutment" ;
    dcterms:bibliographicCitation "https://www.publications.usace.army.mil/Portals/76/Users/182/86/2486/er_1110-2-1156.pdf#page=487" ;
    pav:wasDerivedFrom "glossaries/CivilWorks/ER-1110-2-1156.yaml#term[Abutment]" ;
    skos:definition "That part of the valley side against which the dam is constructed. An artificial abutment is sometimes constructed as a concrete gravity section to take the thrust of an arch dam where there is no suitable natural abutment. The left and right abutments of dams are defined with the observer viewing the dam looking in the downstream direction, unless otherwise indicated." ;
    skos:inScheme ER-1110-2-1156: ;
    skos:prefLabel "Abutment" .

ER-1110-2-1156:Acceptable_Risk a wov:GlossaryTerm,
        skos:Concept ;
    rdfs:label "Acceptable Risk" ;
    dcterms:bibliographicCitation "https://www.publications.usace.army.mil/Portals/76/Users/182/86/2486/er_1110-2-1156.pdf#page=487" ;
    pav:wasDerivedFrom "glossaries/CivilWorks/ER-1110-2-1156.yaml#term[Acceptable Risk]" ;
    skos:definition "A risk, for the purposes of life or work, everyone who might be impacted is prepared to accept assuming no changes in risk control mechanisms. Such risk is regarded as insignificant and adequately controlled. Action to further reduce such risk is usually not required." ;
    skos:inScheme ER-1110-2-1156: ;
    skos:prefLabel "Acceptable Risk" .

ER-1110-2-1156:Acre-foot a wov:GlossaryTerm,
        skos:Concept ;
    rdfs:label "Acre-foot" ;
    dcterms:bibliographicCitation "https://www.publications.usace.army.mil/Portals/76/Users/182/86/2486/er_1110-2-1156.pdf#page=487" ;
    pav:wasDerivedFrom "glossaries/CivilWorks/ER-1110-2-1156.yaml#term[Acre-foot]" ;
    skos:definition "A unit of volumetric measure that would cover 1 acre to a depth of 1 foot. It is equal to 43,560 cubic feet. This is approximately 325,851.4 U.S. gallons." ;
    skos:inScheme ER-1110-2-1156: ;
    skos:prefLabel "Acre-foot" .

ER-1110-2-1156:Active_storage a wov:GlossaryTerm,
        skos:Concept ;
    rdfs:label "Active storage" ;
    dcterms:bibliographicCitation "https://www.publications.usace.army.mil/Portals/76/Users/182/86/2486/er_1110-2-1156.pdf#page=523" ;
    pav:wasDerivedFrom "glossaries/CivilWorks/ER-1110-2-1156.yaml#term[Active storage]" ;
    skos:definition "The volume of the reservoir that is available for some use such as power generation, irrigation, flood control, or water supply. The bottom elevation is the minimum operating level." ;
    skos:inScheme ER-1110-2-1156: ;
    skos:prefLabel "Active storage" .

ER-1110-2-1156:Adit a wov:GlossaryTerm,
        skos:Concept ;
    rdfs:label "Adit" ;
    dcterms:bibliographicCitation "https://www.publications.usace.army.mil/Portals/76/Users/182/86/2486/er_1110-2-1156.pdf#page=487" ;
    pav:wasDerivedFrom "glossaries/CivilWorks/ER-1110-2-1156.yaml#term[Adit]" ;
    skos:definition "A nearly horizontal underground excavation in an abutment having an opening in only one end, such as an opening in the face of a dam for access to galleries or operating chambers." ;
    skos:inScheme ER-1110-2-1156: ;
    skos:prefLabel "Adit" .

ER-1110-2-1156:Adverse_Consequences a wov:GlossaryTerm,
        skos:Concept ;
    rdfs:label "Adverse Consequences" ;
    dcterms:bibliographicCitation "https://www.publications.usace.army.mil/Portals/76/Users/182/86/2486/er_1110-2-1156.pdf#page=487" ;
    pav:wasDerivedFrom "glossaries/CivilWorks/ER-1110-2-1156.yaml#term[Adverse Consequences]" ;
    skos:definition "The outcome of the failure of a dam or its appurtenances, including immediate, short and long-term, direct and indirect losses and effects. Loss may include human casualties, project benefits, monetary and economic damages, and environmental impact (Adapted from USACE)." ;
    skos:inScheme ER-1110-2-1156: ;
    skos:prefLabel "Adverse Consequences" .

ER-1110-2-1156:Agency_Technical_Review_%28ATR%29 a wov:GlossaryTerm,
        skos:Concept ;
    rdfs:label "Agency Technical Review (ATR)" ;
    dcterms:bibliographicCitation "https://www.publications.usace.army.mil/Portals/76/Users/182/86/2486/er_1110-2-1156.pdf#page=487" ;
    pav:wasDerivedFrom "glossaries/CivilWorks/ER-1110-2-1156.yaml#term[Agency Technical Review (ATR)]" ;
    skos:altLabel "ATR" ;
    skos:definition "An independent in-depth review designed to ensure the proper application of clearly established criteria, regulations, laws, codes, principles and professional practices. The ATR team reviews the various work products and assures that all the parts fit together in a coherent whole." ;
    skos:inScheme ER-1110-2-1156: ;
    skos:prefLabel "Agency Technical Review (ATR)" .

ER-1110-2-1156:Annual_Inspections a wov:GlossaryTerm,
        skos:Concept ;
    rdfs:label "Annual Inspections" ;
    dcterms:bibliographicCitation "https://www.publications.usace.army.mil/Portals/76/Users/182/86/2486/er_1110-2-1156.pdf#page=487" ;
    pav:wasDerivedFrom "glossaries/CivilWorks/ER-1110-2-1156.yaml#term[Annual Inspections]" ;
    skos:definition "Inspections conducted annually by the Operating Project staff with technical experts from Engineering or Operations (reference ER 1130-2-500 (reference A.60)). The goal is to monitor the performance of the dam and note any evidence of changes in performance or needed dam safety related maintenance. Findings must be documented and reviewed in support of Periodic Inspections (PI's) and Periodic Assessments (PA's)." ;
    skos:inScheme ER-1110-2-1156: ;
    skos:prefLabel "Annual Inspections" .

ER-1110-2-1156:Annual_Probability_of_Failure_%28APF%29 a wov:GlossaryTerm,
        skos:Concept ;
    rdfs:label "Annual Probability of Failure (APF)" ;
    dcterms:bibliographicCitation "https://www.publications.usace.army.mil/Portals/76/Users/182/86/2486/er_1110-2-1156.pdf#page=487" ;
    pav:wasDerivedFrom "glossaries/CivilWorks/ER-1110-2-1156.yaml#term[Annual Probability of Failure (APF)]" ;
    skos:altLabel "APF" ;
    skos:definition "For dams the combined estimated annual probability of failure from all failure modes associated with all loading or initiating event types that result in an unintentional release of the reservoir." ;
    skos:inScheme ER-1110-2-1156: ;
    skos:prefLabel "Annual Probability of Failure (APF)" .

ER-1110-2-1156:Appurtenant_structure a wov:GlossaryTerm,
        skos:Concept ;
    rdfs:label "Appurtenant structure" ;
    dcterms:bibliographicCitation "https://www.publications.usace.army.mil/Portals/76/Users/182/86/2486/er_1110-2-1156.pdf#page=488" ;
    pav:wasDerivedFrom "glossaries/CivilWorks/ER-1110-2-1156.yaml#term[Appurtenant structure]" ;
    skos:definition "Ancillary features of a dam such as inlet and outlet works, spillways, tunnels, or power plants." ;
    skos:inScheme ER-1110-2-1156: ;
    skos:prefLabel "Appurtenant structure" .

ER-1110-2-1156:As-Low-As-Reasonably-Practicable_%28ALARP%29 a wov:GlossaryTerm,
        skos:Concept ;
    rdfs:label "As-Low-As-Reasonably-Practicable (ALARP)" ;
    dcterms:bibliographicCitation "https://www.publications.usace.army.mil/Portals/76/Users/182/86/2486/er_1110-2-1156.pdf#page=488" ;
    pav:wasDerivedFrom "glossaries/CivilWorks/ER-1110-2-1156.yaml#term[As-Low-As-Reasonably-Practicable (ALARP)]" ;
    skos:altLabel "ALARP" ;
    skos:definition "That principle which states that risks, lower than the limit of tolerability, are tolerable only if risk reduction is impracticable or if the next increment of risk reduction is not cost effective compared to the improvement gained." ;
    skos:inScheme ER-1110-2-1156: ;
    skos:prefLabel "As-Low-As-Reasonably-Practicable (ALARP)" .

ER-1110-2-1156:Automatically_Operated_System a wov:GlossaryTerm,
        skos:Concept ;
    rdfs:label "Automatically Operated System" ;
    dcterms:bibliographicCitation "https://www.publications.usace.army.mil/Portals/76/Users/182/86/2486/er_1110-2-1156.pdf#page=488" ;
    pav:wasDerivedFrom "glossaries/CivilWorks/ER-1110-2-1156.yaml#term[Automatically Operated System]" ;
    skos:definition "An automatically operated system is where operation is determined by automated means based on instrumentation data without requiring direct input from personnel." ;
    skos:inScheme ER-1110-2-1156: ;
    skos:prefLabel "Automatically Operated System" .

ER-1110-2-1156:Average_Annual_Life_Lost_%28AALL%29 a wov:GlossaryTerm,
        skos:Concept ;
    rdfs:label "Average Annual Life Lost (AALL)" ;
    dcterms:bibliographicCitation "https://www.publications.usace.army.mil/Portals/76/Users/182/86/2486/er_1110-2-1156.pdf#page=488" ;
    pav:wasDerivedFrom "glossaries/CivilWorks/ER-1110-2-1156.yaml#term[Average Annual Life Lost (AALL)]" ;
    skos:altLabel "AALL" ;
    skos:definition "As used in the f-N plot, the expected value (average) of potential life loss of the probability distribution of potential life loss from dam failure." ;
    skos:inScheme ER-1110-2-1156: ;
    skos:prefLabel "Average Annual Life Lost (AALL)" .

ER-1110-2-1156:Axis_of_dam a wov:GlossaryTerm,
        skos:Concept ;
    rdfs:label "Axis of dam" ;
    dcterms:bibliographicCitation "https://www.publications.usace.army.mil/Portals/76/Users/182/86/2486/er_1110-2-1156.pdf#page=488" ;
    pav:wasDerivedFrom "glossaries/CivilWorks/ER-1110-2-1156.yaml#term[Axis of dam]" ;
    skos:definition "The vertical plane or curved surface, chosen by a designer, which appears as a line, in plan, or in cross-section, from which the horizontal dimensions of the dam are referenced." ;
    skos:inScheme ER-1110-2-1156: ;
    skos:prefLabel "Axis of dam" .

ER-1110-2-1156:Baffle_block a wov:GlossaryTerm,
        skos:Concept ;
    rdfs:label "Baffle block" ;
    dcterms:bibliographicCitation "https://www.publications.usace.army.mil/Portals/76/Users/182/86/2486/er_1110-2-1156.pdf#page=488" ;
    pav:wasDerivedFrom "glossaries/CivilWorks/ER-1110-2-1156.yaml#term[Baffle block]" ;
    skos:definition "A block, usually of concrete, constructed in a channel or stilling basin to dissipate the energy of water flowing at high velocity." ;
    skos:inScheme ER-1110-2-1156: ;
    skos:prefLabel "Baffle block" .

ER-1110-2-1156:Bascule_gate a wov:GlossaryTerm,
        skos:Concept ;
    rdfs:label "Bascule gate" ;
    dcterms:bibliographicCitation "https://www.publications.usace.army.mil/Portals/76/Users/182/86/2486/er_1110-2-1156.pdf#page=506" ;
    pav:wasDerivedFrom "glossaries/CivilWorks/ER-1110-2-1156.yaml#term[Bascule gate]" ;
    skos:definition "See flap gate." ;
    skos:inScheme ER-1110-2-1156: ;
    skos:prefLabel "Bascule gate" .

ER-1110-2-1156:Base_thickness a wov:GlossaryTerm,
        skos:Concept ;
    rdfs:label "Base thickness" ;
    dcterms:bibliographicCitation "https://www.publications.usace.army.mil/Portals/76/Users/182/86/2486/er_1110-2-1156.pdf#page=488" ;
    pav:wasDerivedFrom "glossaries/CivilWorks/ER-1110-2-1156.yaml#term[Base thickness]" ;
    skos:definition "Also referred to as base width. The maximum thickness or width of the dam measured horizontally between upstream and downstream faces and normal to the axis of the dam, but excluding projections for outlets, or other appurtenant structures." ;
    skos:inScheme ER-1110-2-1156: ;
    skos:prefLabel "Base thickness" .

ER-1110-2-1156:Batter a wov:GlossaryTerm,
        skos:Concept ;
    rdfs:label "Batter" ;
    dcterms:bibliographicCitation "https://www.publications.usace.army.mil/Portals/76/Users/182/86/2486/er_1110-2-1156.pdf#page=488" ;
    pav:wasDerivedFrom "glossaries/CivilWorks/ER-1110-2-1156.yaml#term[Batter]" ;
    skos:definition "Angle of inclination from the vertical." ;
    skos:inScheme ER-1110-2-1156: ;
    skos:prefLabel "Batter" .

ER-1110-2-1156:Bedrock a wov:GlossaryTerm,
        skos:Concept ;
    rdfs:label "Bedrock" ;
    dcterms:bibliographicCitation "https://www.publications.usace.army.mil/Portals/76/Users/182/86/2486/er_1110-2-1156.pdf#page=488" ;
    pav:wasDerivedFrom "glossaries/CivilWorks/ER-1110-2-1156.yaml#term[Bedrock]" ;
    skos:definition "The consolidated body of natural solid mineral matter which underlies the overburden soils." ;
    skos:inScheme ER-1110-2-1156: ;
    skos:prefLabel "Bedrock" .

ER-1110-2-1156:Berm a wov:GlossaryTerm,
        skos:Concept ;
    rdfs:label "Berm" ;
    dcterms:bibliographicCitation "https://www.publications.usace.army.mil/Portals/76/Users/182/86/2486/er_1110-2-1156.pdf#page=488" ;
    pav:wasDerivedFrom "glossaries/CivilWorks/ER-1110-2-1156.yaml#term[Berm]" ;
    skos:definition "A nearly horizontal step in the sloping profile of an embankment dam. Also a step in a rock or earth cut." ;
    skos:inScheme ER-1110-2-1156: ;
    skos:prefLabel "Berm" .

ER-1110-2-1156:Borrow_Area a wov:GlossaryTerm,
        skos:Concept ;
    rdfs:label "Borrow Area" ;
    dcterms:bibliographicCitation "https://www.publications.usace.army.mil/Portals/76/Users/182/86/2486/er_1110-2-1156.pdf#page=488" ;
    pav:wasDerivedFrom "glossaries/CivilWorks/ER-1110-2-1156.yaml#term[Borrow Area]" ;
    skos:definition "The area from which natural materials, such as rock, gravel or soil, used for construction purposes is excavated." ;
    skos:inScheme ER-1110-2-1156: ;
    skos:prefLabel "Borrow Area" .

ER-1110-2-1156:Breach a wov:GlossaryTerm,
        skos:Concept ;
    rdfs:label "Breach" ;
    dcterms:bibliographicCitation "https://www.publications.usace.army.mil/Portals/76/Users/182/86/2486/er_1110-2-1156.pdf#page=488" ;
    pav:wasDerivedFrom "glossaries/CivilWorks/ER-1110-2-1156.yaml#term[Breach]" ;
    skos:definition "An opening through a dam that allows the uncontrolled draining of a reservoir. A controlled breach is a constructed opening. An uncontrolled breach is an unintentional opening caused by discharge from the reservoir. A breach is generally associated with the partial or total failure of the dam." ;
    skos:inScheme ER-1110-2-1156: ;
    skos:prefLabel "Breach" .

ER-1110-2-1156:Broadly_Acceptable_Risk a wov:GlossaryTerm,
        skos:Concept ;
    rdfs:label "Broadly Acceptable Risk" ;
    dcterms:bibliographicCitation "https://www.publications.usace.army.mil/Portals/76/Users/182/86/2486/er_1110-2-1156.pdf#page=488" ;
    pav:wasDerivedFrom "glossaries/CivilWorks/ER-1110-2-1156.yaml#term[Broadly Acceptable Risk]" ;
    skos:definition "\"Risks falling into this region are generally regarded as insignificant and adequately controlled. The levels of risk characterizing this region are comparable to those that people regard as insignificant or trivial in their daily lives. They are typical of the risk from activities that are inherently not very hazardous or from hazardous activities that can be, and are, readily controlled to produce very low risks\" (HSE, 2001 reference A.145). By the nature of the hazard that dams pose it is inappropriate to attempt to manage them as a broadly acceptable risk and therefore the concept of the broadly acceptable risk level or limit does not apply to dams." ;
    skos:inScheme ER-1110-2-1156: ;
    skos:prefLabel "Broadly Acceptable Risk" .

ER-1110-2-1156:Bulkhead_gate a wov:GlossaryTerm,
        skos:Concept ;
    rdfs:label "Bulkhead gate" ;
    dcterms:bibliographicCitation "https://www.publications.usace.army.mil/Portals/76/Users/182/86/2486/er_1110-2-1156.pdf#page=506" ;
    pav:wasDerivedFrom "glossaries/CivilWorks/ER-1110-2-1156.yaml#term[Bulkhead gate]" ;
    skos:definition "A gate used either for temporary closure of a channel or conduit before dewatering it for inspection or maintenance or for closure against flowing water when the head difference is small, e.g., for diversion tunnel closure." ;
    skos:inScheme ER-1110-2-1156: ;
    skos:prefLabel "Bulkhead gate" .

ER-1110-2-1156:Caretaker_Status a wov:GlossaryTerm,
        skos:Concept ;
    rdfs:label "Caretaker Status" ;
    dcterms:bibliographicCitation "https://www.publications.usace.army.mil/Portals/76/Users/182/86/2486/er_1110-2-1156.pdf#page=489" ;
    pav:wasDerivedFrom "glossaries/CivilWorks/ER-1110-2-1156.yaml#term[Caretaker Status]" ;
    skos:definition "Real or personal property at a project site, in part or in whole, which currently is not utilized or occupied for current program authorized purposes. This may also include property that is \"Inactive\" (Not currently being used but may have a future need) or \"Excess\" (Formally identified as having no further program use including pending disposition actions). This does not include property placed in Mothball status. Caretaker status is defined at the project or project site level, not the feature level.\"" ;
    skos:inScheme ER-1110-2-1156: ;
    skos:prefLabel "Caretaker Status" .

ER-1110-2-1156:Catastrophe a wov:GlossaryTerm,
        skos:Concept ;
    rdfs:label "Catastrophe" ;
    dcterms:bibliographicCitation "https://www.publications.usace.army.mil/Portals/76/Users/182/86/2486/er_1110-2-1156.pdf#page=489" ;
    pav:wasDerivedFrom "glossaries/CivilWorks/ER-1110-2-1156.yaml#term[Catastrophe]" ;
    skos:definition "A sudden and great disaster causing misfortune, destruction, or irreplaceable loss extensive enough to cripple activities in an area." ;
    skos:inScheme ER-1110-2-1156: ;
    skos:prefLabel "Catastrophe" .

ER-1110-2-1156:Channel a wov:GlossaryTerm,
        skos:Concept ;
    rdfs:label "Channel" ;
    dcterms:bibliographicCitation "https://www.publications.usace.army.mil/Portals/76/Users/182/86/2486/er_1110-2-1156.pdf#page=489" ;
    pav:wasDerivedFrom "glossaries/CivilWorks/ER-1110-2-1156.yaml#term[Channel]" ;
    skos:definition "A general term for any natural or artificial facility for conveying water." ;
    skos:inScheme ER-1110-2-1156: ;
    skos:prefLabel "Channel" .

ER-1110-2-1156:Cofferdam a wov:GlossaryTerm,
        skos:Concept ;
    rdfs:label "Cofferdam" ;
    dcterms:bibliographicCitation "https://www.publications.usace.army.mil/Portals/76/Users/182/86/2486/er_1110-2-1156.pdf#page=489" ;
    pav:wasDerivedFrom "glossaries/CivilWorks/ER-1110-2-1156.yaml#term[Cofferdam]" ;
    skos:definition "A temporary structure enclosing all or part of the construction area so that construction can proceed in the dry. A diversion cofferdam diverts a river into a pipe, channel, or tunnel." ;
    skos:inScheme ER-1110-2-1156: ;
    skos:prefLabel "Cofferdam" .

ER-1110-2-1156:Combined_Annual_Probability_of_all_Failure_Modes a wov:GlossaryTerm,
        skos:Concept ;
    rdfs:label "Combined Annual Probability of all Failure Modes" ;
    dcterms:bibliographicCitation "https://www.publications.usace.army.mil/Portals/76/Users/182/86/2486/er_1110-2-1156.pdf#page=489" ;
    pav:wasDerivedFrom "glossaries/CivilWorks/ER-1110-2-1156.yaml#term[Combined Annual Probability of all Failure Modes]" ;
    skos:definition "Combined estimated annual probability of failure from all failure modes associated with all loading or initiating event types." ;
    skos:inScheme ER-1110-2-1156: ;
    skos:prefLabel "Combined Annual Probability of all Failure Modes" .

ER-1110-2-1156:Compaction a wov:GlossaryTerm,
        skos:Concept ;
    rdfs:label "Compaction" ;
    dcterms:bibliographicCitation "https://www.publications.usace.army.mil/Portals/76/Users/182/86/2486/er_1110-2-1156.pdf#page=489" ;
    pav:wasDerivedFrom "glossaries/CivilWorks/ER-1110-2-1156.yaml#term[Compaction]" ;
    skos:definition "Mechanical action, which increases the density by reducing the voids in a material." ;
    skos:inScheme ER-1110-2-1156: ;
    skos:prefLabel "Compaction" .

ER-1110-2-1156:Component_Risks a wov:GlossaryTerm,
        skos:Concept ;
    rdfs:label "Component Risks" ;
    dcterms:bibliographicCitation "https://www.publications.usace.army.mil/Portals/76/Users/182/86/2486/er_1110-2-1156.pdf#page=489" ;
    pav:wasDerivedFrom "glossaries/CivilWorks/ER-1110-2-1156.yaml#term[Component Risks]" ;
    skos:definition "Estimates of risk contributed by the physical components of a dam undergoing failure mode analysis for a remediation alternative." ;
    skos:inScheme ER-1110-2-1156: ;
    skos:prefLabel "Component Risks" .

ER-1110-2-1156:Conditional_Load_Response_Probabilities a wov:GlossaryTerm,
        skos:Concept ;
    rdfs:label "Conditional Load Response Probabilities" ;
    dcterms:bibliographicCitation "https://www.publications.usace.army.mil/Portals/76/Users/182/86/2486/er_1110-2-1156.pdf#page=489" ;
    pav:wasDerivedFrom "glossaries/CivilWorks/ER-1110-2-1156.yaml#term[Conditional Load Response Probabilities]" ;
    skos:definition "Response probabilities (of failure) corresponding to the conditional load type and scenario under investigation." ;
    skos:inScheme ER-1110-2-1156: ;
    skos:prefLabel "Conditional Load Response Probabilities" .

ER-1110-2-1156:Conditional_System_Response_Probability_Estimates a wov:GlossaryTerm,
        skos:Concept ;
    rdfs:label "Conditional System Response Probability Estimates" ;
    dcterms:bibliographicCitation "https://www.publications.usace.army.mil/Portals/76/Users/182/86/2486/er_1110-2-1156.pdf#page=489" ;
    pav:wasDerivedFrom "glossaries/CivilWorks/ER-1110-2-1156.yaml#term[Conditional System Response Probability Estimates]" ;
    skos:definition "System response probabilities that are conditional on the specific loading condition analyzed (over the range of loading conditions to be studied)." ;
    skos:inScheme ER-1110-2-1156: ;
    skos:prefLabel "Conditional System Response Probability Estimates" .

ER-1110-2-1156:Conduit a wov:GlossaryTerm,
        skos:Concept ;
    rdfs:label "Conduit" ;
    dcterms:bibliographicCitation "https://www.publications.usace.army.mil/Portals/76/Users/182/86/2486/er_1110-2-1156.pdf#page=489" ;
    pav:wasDerivedFrom "glossaries/CivilWorks/ER-1110-2-1156.yaml#term[Conduit]" ;
    skos:definition "A closed channel to convey water through, around, or under a dam." ;
    skos:inScheme ER-1110-2-1156: ;
    skos:prefLabel "Conduit" .

ER-1110-2-1156:Confirmed_%28Unconfirmed%29 a wov:GlossaryTerm,
        skos:Concept ;
    rdfs:label "Confirmed (Unconfirmed)" ;
    dcterms:bibliographicCitation "https://www.publications.usace.army.mil/Portals/76/Users/182/86/2486/er_1110-2-1156.pdf#page=489" ;
    pav:wasDerivedFrom "glossaries/CivilWorks/ER-1110-2-1156.yaml#term[Confirmed (Unconfirmed)]" ;
    skos:definition "Through investigation or other means, Dam Safety issue is firmly established as of concern or not. Unconfirmed “ not confirmed." ;
    skos:inScheme ER-1110-2-1156: ;
    skos:prefLabel "Confirmed (Unconfirmed)" .

ER-1110-2-1156:Confirmed_Dam_Safety_Issues a wov:GlossaryTerm,
        skos:Concept ;
    rdfs:label "Confirmed Dam Safety Issues" ;
    dcterms:bibliographicCitation "https://www.publications.usace.army.mil/Portals/76/Users/182/86/2486/er_1110-2-1156.pdf#page=490" ;
    pav:wasDerivedFrom "glossaries/CivilWorks/ER-1110-2-1156.yaml#term[Confirmed Dam Safety Issues]" ;
    skos:definition "Manifested or obvious issues are those impacting the safe operation of a dam. Examples of confirmed issues can be described as performance concerns - lack of spillway or seismic capacity, or deficiencies that are demonstrated by signs of seepage and boils, obvious flaws or defects, component distress or malfunction, unusual settlement, unsatisfactory instrument readings, etc. that can be specifically linked to one or more potential failure modes." ;
    skos:inScheme ER-1110-2-1156: ;
    skos:prefLabel "Confirmed Dam Safety Issues" .

ER-1110-2-1156:Conservation_Pool a wov:GlossaryTerm,
        skos:Concept ;
    rdfs:label "Conservation Pool" ;
    dcterms:bibliographicCitation "https://www.publications.usace.army.mil/Portals/76/Users/182/86/2486/er_1110-2-1156.pdf#page=490" ;
    pav:wasDerivedFrom "glossaries/CivilWorks/ER-1110-2-1156.yaml#term[Conservation Pool]" ;
    skos:definition "The permanent pool that lies just below the flood storage pool in a reservoir." ;
    skos:inScheme ER-1110-2-1156: ;
    skos:prefLabel "Conservation Pool" .

ER-1110-2-1156:Constructability_evaluation_%28CE%29 a wov:GlossaryTerm,
        skos:Concept ;
    rdfs:label "Constructability evaluation (CE)" ;
    dcterms:bibliographicCitation "https://www.publications.usace.army.mil/Portals/76/Users/182/86/2486/er_1110-2-1156.pdf#page=490" ;
    pav:wasDerivedFrom "glossaries/CivilWorks/ER-1110-2-1156.yaml#term[Constructability evaluation (CE)]" ;
    skos:altLabel "CE" ;
    skos:definition "A project review that concentrates on schedule, cost, constructability, and risks that may be inherent to the construction of a project. This review is performed and documented by a team designated by the DSMMCX/DSPC. A CE report is prepared, briefed to the project PDT and approved by the DSPC. A CE will be performed at least during the steps of evaluation and comparison of alternatives in the plan formulation process and during PED prior to final design." ;
    skos:inScheme ER-1110-2-1156: ;
    skos:prefLabel "Constructability evaluation (CE)" .

ER-1110-2-1156:Construction_Joint a wov:GlossaryTerm,
        skos:Concept ;
    rdfs:label "Construction Joint" ;
    dcterms:bibliographicCitation "https://www.publications.usace.army.mil/Portals/76/Users/182/86/2486/er_1110-2-1156.pdf#page=490" ;
    pav:wasDerivedFrom "glossaries/CivilWorks/ER-1110-2-1156.yaml#term[Construction Joint]" ;
    skos:definition "The interface between two successive placings or pours of concrete where bond, and not permanent separation, is intended." ;
    skos:inScheme ER-1110-2-1156: ;
    skos:prefLabel "Construction Joint" .

ER-1110-2-1156:Contact_Grouting a wov:GlossaryTerm,
        skos:Concept ;
    rdfs:label "Contact Grouting" ;
    dcterms:bibliographicCitation "https://www.publications.usace.army.mil/Portals/76/Users/182/86/2486/er_1110-2-1156.pdf#page=490" ;
    pav:wasDerivedFrom "glossaries/CivilWorks/ER-1110-2-1156.yaml#term[Contact Grouting]" ;
    skos:definition "Filling, with cement grout, any voids existing at the contact of two zones of different materials, e.g., between a concrete tunnel lining and the surrounding rock." ;
    skos:inScheme ER-1110-2-1156: ;
    skos:prefLabel "Contact Grouting" .

ER-1110-2-1156:Contractor_Quality_Control_%28CQC%29 a wov:GlossaryTerm,
        skos:Concept ;
    rdfs:label "Contractor Quality Control (CQC)" ;
    dcterms:bibliographicCitation "https://www.publications.usace.army.mil/Portals/76/Users/182/86/2486/er_1110-2-1156.pdf#page=490" ;
    pav:wasDerivedFrom "glossaries/CivilWorks/ER-1110-2-1156.yaml#term[Contractor Quality Control (CQC)]" ;
    skos:altLabel "CQC" ;
    skos:definition "The construction contractor's system to manage, control, and document his own, his supplier's, and his subcontractor's activities to comply with contract requirements." ;
    skos:inScheme ER-1110-2-1156: ;
    skos:prefLabel "Contractor Quality Control (CQC)" .

ER-1110-2-1156:Core a wov:GlossaryTerm,
        skos:Concept ;
    rdfs:label "Core" ;
    dcterms:bibliographicCitation "https://www.publications.usace.army.mil/Portals/76/Users/182/86/2486/er_1110-2-1156.pdf#page=490" ;
    pav:wasDerivedFrom "glossaries/CivilWorks/ER-1110-2-1156.yaml#term[Core]" ;
    skos:definition "A zone of low permeability material in an embankment dam. The core is sometimes referred to as central core, inclined core, puddle clay core, rolled clay core, or impervious zone." ;
    skos:inScheme ER-1110-2-1156: ;
    skos:prefLabel "Core" .

ER-1110-2-1156:Core_Wall a wov:GlossaryTerm,
        skos:Concept ;
    rdfs:label "Core Wall" ;
    dcterms:bibliographicCitation "https://www.publications.usace.army.mil/Portals/76/Users/182/86/2486/er_1110-2-1156.pdf#page=490" ;
    pav:wasDerivedFrom "glossaries/CivilWorks/ER-1110-2-1156.yaml#term[Core Wall]" ;
    skos:definition "A wall built of relatively impervious material, usually of concrete or asphaltic concrete, in the body of an embankment dam to prevent seepage." ;
    skos:inScheme ER-1110-2-1156: ;
    skos:prefLabel "Core Wall" .

ER-1110-2-1156:Cost-to-Save-a-Statistical-Life_%28CSSL%29 a wov:GlossaryTerm,
        skos:Concept ;
    rdfs:label "Cost-to-Save-a-Statistical-Life (CSSL)" ;
    dcterms:bibliographicCitation "https://www.publications.usace.army.mil/Portals/76/Users/182/86/2486/er_1110-2-1156.pdf#page=490" ;
    pav:wasDerivedFrom "glossaries/CivilWorks/ER-1110-2-1156.yaml#term[Cost-to-Save-a-Statistical-Life (CSSL)]" ;
    skos:altLabel "CSSL" ;
    skos:definition "CSSL is the ratio of the cost of a proposed risk reduction measure divided by the consequent estimate of 'Statistical Lives Saved'." ;
    skos:inScheme ER-1110-2-1156: ;
    skos:prefLabel "Cost-to-Save-a-Statistical-Life (CSSL)" .

ER-1110-2-1156:Credible_Existing_and_Future_Without_Federal_Action_Risk_Estimate a wov:GlossaryTerm,
        skos:Concept ;
    rdfs:label "Credible Existing and Future Without Federal Action Risk Estimate" ;
    dcterms:bibliographicCitation "https://www.publications.usace.army.mil/Portals/76/Users/182/86/2486/er_1110-2-1156.pdf#page=490" ;
    pav:wasDerivedFrom "glossaries/CivilWorks/ER-1110-2-1156.yaml#term[Credible Existing and Future Without Federal Action Risk Estimate]" ;
    skos:definition "Occurs when the conditional load response probabilities and consequences used to estimate the residual project risk (incremental and non-breach) are supported by sufficient data, analysis, and performance history. The need for additional information, studies, and investigations to determine or resolve uncertainty should be determined after parametric studies are completed and insight is gained as to improvement in the confidence of the risk estimate by more accurately predicting conditional load response probabilities or life loss estimates. Typically, risk estimates for confirmed issues can be established with existing data and performance history because the physical manifestations are visual and measurable. Unconfirmed issues may require the collection of additional data if the concerns are less obvious or cannot be linked to a specific failure mode or observation. Credible Failure Mode “ A physically plausible failure mode." ;
    skos:inScheme ER-1110-2-1156: ;
    skos:prefLabel "Credible Existing and Future Without Federal Action Risk Estimate" .

ER-1110-2-1156:Crest_gate a wov:GlossaryTerm,
        skos:Concept ;
    rdfs:label "Crest gate" ;
    dcterms:bibliographicCitation "https://www.publications.usace.army.mil/Portals/76/Users/182/86/2486/er_1110-2-1156.pdf#page=506" ;
    pav:wasDerivedFrom "glossaries/CivilWorks/ER-1110-2-1156.yaml#term[Crest gate]" ;
    skos:altLabel "spillway gate" ;
    skos:definition "A gate on the crest of a spillway to control the discharge or reservoir water level." ;
    skos:inScheme ER-1110-2-1156: ;
    skos:prefLabel "Crest gate" .

ER-1110-2-1156:Crest_of_dam a wov:GlossaryTerm,
        skos:Concept ;
    rdfs:label "Crest of dam" ;
    dcterms:bibliographicCitation "https://www.publications.usace.army.mil/Portals/76/Users/182/86/2486/er_1110-2-1156.pdf#page=491" ;
    pav:wasDerivedFrom "glossaries/CivilWorks/ER-1110-2-1156.yaml#term[Crest of dam]" ;
    skos:definition "See top of dam." ;
    skos:inScheme ER-1110-2-1156: ;
    skos:prefLabel "Crest of dam" .

ER-1110-2-1156:Critical_feature a wov:GlossaryTerm,
        skos:Concept ;
    rdfs:label "Critical feature" ;
    dcterms:bibliographicCitation "https://www.publications.usace.army.mil/Portals/76/Users/182/86/2486/er_1110-2-1156.pdf#page=491" ;
    pav:wasDerivedFrom "glossaries/CivilWorks/ER-1110-2-1156.yaml#term[Critical feature]" ;
    skos:definition "For Seismic Evaluation “ Critical features are the engineered structures, natural site conditions, or operating equipment and utilities at high hazard projects whose failure during or immediately following an earthquake could result in loss of life." ;
    skos:inScheme ER-1110-2-1156: ;
    skos:prefLabel "Critical feature" .

ER-1110-2-1156:Critically_near_failure a wov:GlossaryTerm,
        skos:Concept ;
    rdfs:label "Critically near failure" ;
    dcterms:bibliographicCitation "https://www.publications.usace.army.mil/Portals/76/Users/182/86/2486/er_1110-2-1156.pdf#page=491" ;
    pav:wasDerivedFrom "glossaries/CivilWorks/ER-1110-2-1156.yaml#term[Critically near failure]" ;
    skos:definition "Failure sequence has been initiated and continues under normal loading. Without intervention (e.g., interim risk reduction measures or remediation), dam is expected to fail." ;
    skos:inScheme ER-1110-2-1156: ;
    skos:prefLabel "Critically near failure" .

ER-1110-2-1156:Cross_section a wov:GlossaryTerm,
        skos:Concept ;
    rdfs:label "Cross section" ;
    dcterms:bibliographicCitation "https://www.publications.usace.army.mil/Portals/76/Users/182/86/2486/er_1110-2-1156.pdf#page=491" ;
    pav:wasDerivedFrom "glossaries/CivilWorks/ER-1110-2-1156.yaml#term[Cross section]" ;
    skos:definition "An elevation view of a dam formed by passing a plane through the dam perpendicular to the axis." ;
    skos:inScheme ER-1110-2-1156: ;
    skos:prefLabel "Cross section" .

ER-1110-2-1156:Cutoff_trench a wov:GlossaryTerm,
        skos:Concept ;
    rdfs:label "Cutoff trench" ;
    dcterms:bibliographicCitation "https://www.publications.usace.army.mil/Portals/76/Users/182/86/2486/er_1110-2-1156.pdf#page=491" ;
    pav:wasDerivedFrom "glossaries/CivilWorks/ER-1110-2-1156.yaml#term[Cutoff trench]" ;
    skos:definition "A foundation excavation later to be filled with impervious material so as to limit seepage beneath a dam." ;
    skos:inScheme ER-1110-2-1156: ;
    skos:prefLabel "Cutoff trench" .

ER-1110-2-1156:Cutoff_wall a wov:GlossaryTerm,
        skos:Concept ;
    rdfs:label "Cutoff wall" ;
    dcterms:bibliographicCitation "https://www.publications.usace.army.mil/Portals/76/Users/182/86/2486/er_1110-2-1156.pdf#page=491" ;
    pav:wasDerivedFrom "glossaries/CivilWorks/ER-1110-2-1156.yaml#term[Cutoff wall]" ;
    skos:definition "A wall of impervious material usually of concrete, asphaltic concrete, or steel sheet piling constructed in the foundation and abutments to reduce seepage beneath and adjacent to the dam." ;
    skos:inScheme ER-1110-2-1156: ;
    skos:prefLabel "Cutoff wall" .

ER-1110-2-1156:DSAC_1_%28Very_High_Urgency%29 a wov:GlossaryTerm,
        skos:Concept ;
    rdfs:label "DSAC 1 (Very High Urgency)" ;
    dcterms:bibliographicCitation "https://www.publications.usace.army.mil/Portals/76/Users/182/86/2486/er_1110-2-1156.pdf#page=498" ;
    pav:wasDerivedFrom "glossaries/CivilWorks/ER-1110-2-1156.yaml#term[DSAC 1 (Very High Urgency)]" ;
    skos:definition "Dams where progression toward failure is confirmed to be taking place under normal operations and the dam is almost certain to fail under normal operations within a few years without intervention; or the incremental risk “ combination of life or economic consequences with likelihood of failure “ is very high. USACE considers this level of life-risk to be unacceptable except in extraordinary circumstances." ;
    skos:inScheme ER-1110-2-1156: ;
    skos:prefLabel "DSAC 1 (Very High Urgency)" .

ER-1110-2-1156:DSAC_2_%28High_Urgency%29 a wov:GlossaryTerm,
        skos:Concept ;
    rdfs:label "DSAC 2 (High Urgency)" ;
    dcterms:bibliographicCitation "https://www.publications.usace.army.mil/Portals/76/Users/182/86/2486/er_1110-2-1156.pdf#page=498" ;
    pav:wasDerivedFrom "glossaries/CivilWorks/ER-1110-2-1156.yaml#term[DSAC 2 (High Urgency)]" ;
    skos:definition "Dams where failure could begin during normal operations or be initiated by an event. The likelihood of failure from one of these occurrences, prior to remediation, is too high to assure public safety; or the incremental risk “ combination of life or economic consequences with likelihood of failure “ is high. USACE considers this level of life-risk to be unacceptable except in extraordinary circumstances." ;
    skos:inScheme ER-1110-2-1156: ;
    skos:prefLabel "DSAC 2 (High Urgency)" .

ER-1110-2-1156:DSAC_3_%28Moderate_Urgency%29 a wov:GlossaryTerm,
        skos:Concept ;
    rdfs:label "DSAC 3 (Moderate Urgency)" ;
    dcterms:bibliographicCitation "https://www.publications.usace.army.mil/Portals/76/Users/182/86/2486/er_1110-2-1156.pdf#page=498" ;
    pav:wasDerivedFrom "glossaries/CivilWorks/ER-1110-2-1156.yaml#term[DSAC 3 (Moderate Urgency)]" ;
    skos:definition "Dams in this class have issues where the incremental risk “ combination life, economic, or environmental consequences with likelihood of failure “ is moderate. USACE considers this level of life-risk to be unacceptable except in unusual circumstances." ;
    skos:inScheme ER-1110-2-1156: ;
    skos:prefLabel "DSAC 3 (Moderate Urgency)" .

ER-1110-2-1156:DSAC_4_%28Low_Urgency%29 a wov:GlossaryTerm,
        skos:Concept ;
    rdfs:label "DSAC 4 (Low Urgency)" ;
    dcterms:bibliographicCitation "https://www.publications.usace.army.mil/Portals/76/Users/182/86/2486/er_1110-2-1156.pdf#page=498" ;
    pav:wasDerivedFrom "glossaries/CivilWorks/ER-1110-2-1156.yaml#term[DSAC 4 (Low Urgency)]" ;
    skos:definition "Dams are inadequate with low incremental risk such that the incremental risk “ combination of life, economic, or environmental consequences with a likelihood of failure “ is low and the dam may not meet all essential USACE guidelines. USACE considers this level of life-risk to be in the range of tolerability but the dam does not meet all essential USACE guidelines." ;
    skos:inScheme ER-1110-2-1156: ;
    skos:prefLabel "DSAC 4 (Low Urgency)" .

ER-1110-2-1156:DSAC_5_%28Normal%29 a wov:GlossaryTerm,
        skos:Concept ;
    rdfs:label "DSAC 5 (Normal)" ;
    dcterms:bibliographicCitation "https://www.publications.usace.army.mil/Portals/76/Users/182/86/2486/er_1110-2-1156.pdf#page=498" ;
    pav:wasDerivedFrom "glossaries/CivilWorks/ER-1110-2-1156.yaml#term[DSAC 5 (Normal)]" ;
    skos:definition "Dams in this class are where the incremental risk - combination life, economic, or environmental consequences with likelihood of failure “ is very low and the dam meets all essential USACE guidelines (see Appendix F). USACE considers this Level of life-safety risk to be tolerable." ;
    skos:inScheme ER-1110-2-1156: ;
    skos:prefLabel "DSAC 5 (Normal)" .

ER-1110-2-1156:Dam a wov:GlossaryTerm,
        skos:Concept ;
    rdfs:label "Dam" ;
    dcterms:bibliographicCitation "https://www.publications.usace.army.mil/Portals/76/Users/182/86/2486/er_1110-2-1156.pdf#page=491" ;
    pav:wasDerivedFrom "glossaries/CivilWorks/ER-1110-2-1156.yaml#term[Dam]" ;
    skos:definition "An artificial barrier, including appurtenant works, constructed for the purpose of storage, control, or diversion of water, and which (1) is twenty-five feet or more in height from the natural bed of the stream or watercourse measured at the downstream toe of the barrier or from the lowest elevation of the outside limit of the barrier if it is not across a stream channel or watercourse, to the maximum water storage elevation or (2) has an impounding capacity at maximum water storage elevation of fifty acre-feet or more. Any such barrier which is under six feet in height regardless of storage capacity, or which has a storage capacity at maximum water storage elevation not in excess of fifteen acre-feet regardless of height is not considered a dam. This lower size limitation should be waived if there is a potentially significant downstream hazard. This definition applies whether the dam has a permanent reservoir or is a detention dam for temporary storage of floodwaters. The impounding capacity at maximum water storage elevation includes storage of floodwaters above the normal full storage elevation. Various types of dams include the following: a. Afterbay dam. See regulating dam.; b. Ambursen dam. A buttress dam in which the upstream part is a relatively thin flat slab usually made of reinforced concrete.; c. Arch dam. A concrete or masonry dam, which is curved upstream so as to transmit the major part of the water load to the abutments. d. Buttress dam. A dam consisting of a watertight part supported at intervals on the downstream side by a series of buttresses. A buttress dam can take many forms, such as a flat slab or a massive head buttress. e. Cofferdam. A temporary structure enclosing all or part of the construction area so that construction can proceed in the dry. A diversion cofferdam diverts a stream into a pipe, channel, tunnel, or other watercourse. f. Crib dam. A gravity dam built up of boxes, crossed timbers, or gabions filled with earth or rock. g. Diversion dam. A dam built to divert water from a waterway or stream into a different watercourse. h. Double curvature arch dam. An arch dam, which is curved vertically as well as horizontally. i. Earth dam. An embankment dam in which more than 50 percent of the total volume is formed of compacted earth material generally smaller than 3-inch size. j. Embankment dam. Any dam constructed of excavated natural materials or of industrial waste materials. k. Gravity dam. A dam constructed of concrete and/or masonry, which relies on its weight and internal strength for stability. l. Hollow gravity dam. A dam constructed of concrete and/or masonry on the outside but having a hollow interior and relying on its weight for stability. m. Hydraulic fill dam. An earth dam constructed of materials, often dredged, which are conveyed and placed by suspension in flowing water. n. Industrial waste dam. An embankment dam, usually built in stages, to create storage for the disposal of waste products from an industrial process. The waste products are conveyed as fine material suspended in water to the reservoir impounded by the embankment. The embankment may be built of conventional materials but sometimes incorporates suitable waste products. o. Masonry dam. Any dam constructed mainly of stone, brick, or concrete blocks jointed with mortar. A dam having only a masonry facing should not be referred to as a masonry dam. p. Mine tailings dam. An industrial waste dam in which the waste materials come from mining operations or mineral processing. q. Multiple arch dam. A buttress dam composed of a series of arches for the upstream face. r. Overflow dam. A dam designed to be overtopped. s. Regulating dam. A dam impounding a reservoir from which water is released to regulate the flow downstream. t. Rockfill dam. An embankment dam in which more than 50 percent of the total volume is composed of compacted or dumped cobbles, boulders, rock fragments, or quarried rock generally larger than 3-inch size. u. Roller-compacted concrete dam. A concrete gravity dam constructed by the use of a dry mix concrete transported by conventional construction equipment and compacted by rolling, usually with vibratory rollers. v. Rubble dam. A stone masonry dam in which the stones are unshaped or uncoursed. w. Saddle dam (or dike). A subsidiary dam of any type constructed across a saddle or low point on the perimeter of a reservoir. x. Tailings dam. See mine tailings dam." ;
    skos:inScheme ER-1110-2-1156: ;
    skos:prefLabel "Dam" .

ER-1110-2-1156:Dam_Safety a wov:GlossaryTerm,
        skos:Concept ;
    rdfs:label "Dam Safety" ;
    dcterms:bibliographicCitation "https://www.publications.usace.army.mil/Portals/76/Users/182/86/2486/er_1110-2-1156.pdf#page=493" ;
    pav:wasDerivedFrom "glossaries/CivilWorks/ER-1110-2-1156.yaml#term[Dam Safety]" ;
    skos:definition "Dam safety is the art and science of ensuring the integrity and viability of dams such that they do not present unacceptable risks to the public, property, and the environment. It requires the collective application of engineering principles and experience, and a philosophy of risk management that recognizes that a dam is a structure whose safe functioning is not explicitly determined by its original design and construction. It also includes all actions taken to routinely monitor, evaluate, identify or predict dam safety issues and consequences related to failure including ensuring all reservoir regulation activities are performed in accordance with established water control plans in support of dam safety concerns. These actions are to be performed in concert with activities to document, publicize, and reduce, eliminate, or remediate, to the extent reasonably practicable, any unacceptable risks." ;
    skos:inScheme ER-1110-2-1156: ;
    skos:prefLabel "Dam Safety" .

ER-1110-2-1156:Dam_Safety_Action_Classification_%28DSAC%29_System a wov:GlossaryTerm,
        skos:Concept ;
    rdfs:label "Dam Safety Action Classification (DSAC) System" ;
    dcterms:bibliographicCitation "https://www.publications.usace.army.mil/Portals/76/Users/182/86/2486/er_1110-2-1156.pdf#page=494" ;
    pav:wasDerivedFrom "glossaries/CivilWorks/ER-1110-2-1156.yaml#term[Dam Safety Action Classification (DSAC) System]" ;
    skos:altLabel "DSAC System" ;
    skos:definition "The Dam Safety Action Classification system is intended to provide consistent and systematic guidelines for appropriate actions to address the dam safety issues and deficiencies of USACE dams. USACE dams are assigned a DSAC class informed by their incremental flood risk considered as a combination of probability of failure and potential life safety, economic, environmental, or other consequences. The DSAC table presents different levels and urgencies of actions that are commensurate with the different levels of incremental flood risk associated with USACE dams. These actions range from immediate recognition of a very high urgency requiring extraordinary and immediate action for dams considered critically near failure or dams with very high incremental flood risk through normal level of urgency for the operations and dam safety activities for dams with very low incremental flood risk and that meet all essential USACE guideline." ;
    skos:inScheme ER-1110-2-1156: ;
    skos:prefLabel "Dam Safety Action Classification (DSAC) System" .

ER-1110-2-1156:Dam_Safety_Committee a wov:GlossaryTerm,
        skos:Concept ;
    rdfs:label "Dam Safety Committee" ;
    dcterms:bibliographicCitation "https://www.publications.usace.army.mil/Portals/76/Users/182/86/2486/er_1110-2-1156.pdf#page=494" ;
    pav:wasDerivedFrom "glossaries/CivilWorks/ER-1110-2-1156.yaml#term[Dam Safety Committee]" ;
    skos:definition "The Dam Safety Committee includes the Dam Safety Officer (DSO) and the Dam Safety Program Manager (DSPM) plus additional members as required. The members should include various technical engineering disciplines from within the district. Other disciplines and areas of expertise may be represented, as required by the DSO or Commander. There is a standing Dam Safety Committee at each level of the decentralized USACE program (districts, divisions, and HQ), who convening regularly to discuss dam safety project and program matters, and advice the Commander on critical dam safety related decisions." ;
    skos:inScheme ER-1110-2-1156: ;
    skos:prefLabel "Dam Safety Committee" .

ER-1110-2-1156:Dam_Safety_Deficiency a wov:GlossaryTerm,
        skos:Concept ;
    rdfs:label "Dam Safety Deficiency" ;
    dcterms:bibliographicCitation "https://www.publications.usace.army.mil/Portals/76/Users/182/86/2486/er_1110-2-1156.pdf#page=494" ;
    pav:wasDerivedFrom "glossaries/CivilWorks/ER-1110-2-1156.yaml#term[Dam Safety Deficiency]" ;
    skos:definition "A material defect or load capacity limit that threatens a dam failure." ;
    skos:inScheme ER-1110-2-1156: ;
    skos:prefLabel "Dam Safety Deficiency" .

ER-1110-2-1156:Dam_Safety_Issue a wov:GlossaryTerm,
        skos:Concept ;
    rdfs:label "Dam Safety Issue" ;
    dcterms:bibliographicCitation "https://www.publications.usace.army.mil/Portals/76/Users/182/86/2486/er_1110-2-1156.pdf#page=494" ;
    pav:wasDerivedFrom "glossaries/CivilWorks/ER-1110-2-1156.yaml#term[Dam Safety Issue]" ;
    skos:definition "Any confirmed or not yet confirmed condition at a dam that could result in intolerable life safety, economic, and environmental risks." ;
    skos:inScheme ER-1110-2-1156: ;
    skos:prefLabel "Dam Safety Issue" .

ER-1110-2-1156:Dam_Safety_Modification a wov:GlossaryTerm,
        skos:Concept ;
    rdfs:label "Dam Safety Modification" ;
    dcterms:bibliographicCitation "https://www.publications.usace.army.mil/Portals/76/Users/182/86/2486/er_1110-2-1156.pdf#page=494" ;
    pav:wasDerivedFrom "glossaries/CivilWorks/ER-1110-2-1156.yaml#term[Dam Safety Modification]" ;
    skos:definition "A Dam Safety Modification is any planning, design, or construAction activity whose execution or improper execution could significantly impact the project's ability to operate as intended. The following activities will normally be considered dam safety modifications: all dam safety modification studies to bring projects within tolerable risks, all drilling and or grouting activities for a dam, replacement of hydraulic steel structures with new or significantly altered designs, installation of relief wells and collector systems, any drilling within or immediately adjacent to the dam, replacement of operating machinery other than like kind and similar activities. The following activities will normally be considered as routine and are not dam safety modifications: routine cleaning of drains, normal maintenance and repair of existing operating machinery, replacement of hydraulic steel structures and operating equipment with like kind components and similar routine activities performed by the district staff." ;
    skos:inScheme ER-1110-2-1156: ;
    skos:prefLabel "Dam Safety Modification" .

ER-1110-2-1156:Dam_Safety_Modification_%28DSM%29_Lead_Engineer a wov:GlossaryTerm,
        skos:Concept ;
    rdfs:label "Dam Safety Modification (DSM) Lead Engineer" ;
    dcterms:bibliographicCitation "https://www.publications.usace.army.mil/Portals/76/Users/182/86/2486/er_1110-2-1156.pdf#page=495" ;
    pav:wasDerivedFrom "glossaries/CivilWorks/ER-1110-2-1156.yaml#term[Dam Safety Modification (DSM) Lead Engineer]" ;
    skos:altLabel "DSM Lead Engineer" ;
    skos:definition "The DSM lead engineer must be a senior level registered professional engineer (typically a civil, geotechnical, or structural engineer) or engineering geologist with extensive knowledge and skills related to the primary features associated with the project. The engineering geologist is required to be a registered professional engineer.Dam Safety Modification (DSM) Lead Engineer - The DSM lead engineer for all dam safety modification studies, designs, plans and specification, and engineering during construction must be assigned by the Director of the Dam Safety Production Center in consultation with the district DSO" ;
    skos:inScheme ER-1110-2-1156: ;
    skos:prefLabel "Dam Safety Modification (DSM) Lead Engineer" .

ER-1110-2-1156:Dam_Safety_Modification_Risk_Assessment a wov:GlossaryTerm,
        skos:Concept ;
    rdfs:label "Dam Safety Modification Risk Assessment" ;
    dcterms:bibliographicCitation "https://www.publications.usace.army.mil/Portals/76/Users/182/86/2486/er_1110-2-1156.pdf#page=495" ;
    pav:wasDerivedFrom "glossaries/CivilWorks/ER-1110-2-1156.yaml#term[Dam Safety Modification Risk Assessment]" ;
    skos:definition "The risk assessment addresses the life safety, economic, and environmental risks associated with the identified potential failure modes and the risk reduction that can be achieved with risk reduction measures, including potential staged implementation options." ;
    skos:inScheme ER-1110-2-1156: ;
    skos:prefLabel "Dam Safety Modification Risk Assessment" .

ER-1110-2-1156:Dam_Safety_Modification_Study a wov:GlossaryTerm,
        skos:Concept ;
    rdfs:label "Dam Safety Modification Study" ;
    dcterms:bibliographicCitation "https://www.publications.usace.army.mil/Portals/76/Users/182/86/2486/er_1110-2-1156.pdf#page=495" ;
    pav:wasDerivedFrom "glossaries/CivilWorks/ER-1110-2-1156.yaml#term[Dam Safety Modification Study]" ;
    skos:definition "The safety case that presents the investigation, documentation, and rationale for modifications for dam safety at completed USACE projects. The report presents the formulation and evaluation for a full range of risk reduction alternatives with preliminary level cost estimates. A detailed risk assessment is required to look at incremental risk reduction alternatives that together meet the tolerable risk guidelines and cost effectiveness of reducing the risk to and below the minimum safety criteria. However, the level of detail should only be what is needed to justify the modification decision. Related NEPA (reference A.6) and ESA (reference A.10) studies will be conducted during the Modification Study, in support of the recommended risk reduction measures. The resultant Dam Safety Modification Decision Document will present a comparison of alternatives and the recommended risk management plan to include actions, components, risk reduction by increments or stages, implementation plan, detailed cost estimate, NEPA, and ESA determinations." ;
    skos:inScheme ER-1110-2-1156: ;
    skos:prefLabel "Dam Safety Modification Study" .

ER-1110-2-1156:Dam_Safety_Officer a wov:GlossaryTerm,
        skos:Concept ;
    rdfs:label "Dam Safety Officer" ;
    dcterms:bibliographicCitation "https://www.publications.usace.army.mil/Portals/76/Users/182/86/2486/er_1110-2-1156.pdf#page=495" ;
    pav:wasDerivedFrom "glossaries/CivilWorks/ER-1110-2-1156.yaml#term[Dam Safety Officer]" ;
    skos:definition "A registered professional engineer with civil engineering background and with management abilities who is competent in the areas related to the design, construction, operation, inspection or evaluation of dams. They must understand adverse dam incidents and the potential causes and consequences of dam failure. The DSO is the highest-ranking Registered Professional Engineer in each level of USACE responsible for implementing the dam safety program of that organization. The Commander must ensure the DSO meets the technical qualifications and experience. The DSO is the Chair of the Dam Safety Committee." ;
    skos:inScheme ER-1110-2-1156: ;
    skos:prefLabel "Dam Safety Officer" .

ER-1110-2-1156:Dam_Safety_Portfolio_Risk_Management a wov:GlossaryTerm,
        skos:Concept ;
    rdfs:label "Dam Safety Portfolio Risk Management" ;
    dcterms:bibliographicCitation "https://www.publications.usace.army.mil/Portals/76/Users/182/86/2486/er_1110-2-1156.pdf#page=496" ;
    pav:wasDerivedFrom "glossaries/CivilWorks/ER-1110-2-1156.yaml#term[Dam Safety Portfolio Risk Management]" ;
    skos:definition "The management process shown generally on Figure 2.3 and for USACE in detail on Figure 3.1. It is a risk-informed USACE-wide portfolio perspective process applied to all features of all dams on a continuing basis. Dam Safety Program “ The purposes of a dam safety program are to protect life, property, and the environment by ensuring that all dams are designed, constructed, operated, and maintained as safely and effectively as is reasonably possible. Accomplishing these purposes require commitments to continually inspect, evaluate, and document the design, construction, operations, maintenance, rehabilitation, and emergency preparedness of each dam and the associated public. It also requires the archiving of documents on the inspections and history of dams and the training of personnel who inspect, evaluate, operate, and maintain them. Programs must instill an awareness of dams and the potential hazard that they may present in the owners, the users, the public, and the local and national decision-makers. On both local and national scales, program purposes also include periodic reporting on the degree of program implementation. Key to accomplishing these purposes is to attract, train, and retain a staff proficient in the art and science of dam design." ;
    skos:inScheme ER-1110-2-1156: ;
    skos:prefLabel "Dam Safety Portfolio Risk Management" .

ER-1110-2-1156:Dam_Safety_Program_Management_Tools a wov:GlossaryTerm,
        skos:Concept ;
    rdfs:label "Dam Safety Program Management Tools" ;
    dcterms:bibliographicCitation "https://www.publications.usace.army.mil/Portals/76/Users/182/86/2486/er_1110-2-1156.pdf#page=496" ;
    pav:wasDerivedFrom "glossaries/CivilWorks/ER-1110-2-1156.yaml#term[Dam Safety Program Management Tools]" ;
    skos:definition "A shared software database, developed and maintained by USACE on behalf of FEMA, used for managing and monitoring Dam Safety Programs. It is used by multiple Federal and State agencies, to track program accomplishments, including entering data for the National Inventory of Dams and preparing the Federal Dam Safety Biennial Report to Congress." ;
    skos:inScheme ER-1110-2-1156: ;
    skos:prefLabel "Dam Safety Program Management Tools" .

ER-1110-2-1156:Dam_Safety_Program_Manager_%28DSPM%29 a wov:GlossaryTerm,
        skos:Concept ;
    rdfs:label "Dam Safety Program Manager (DSPM)" ;
    dcterms:bibliographicCitation "https://www.publications.usace.army.mil/Portals/76/Users/182/86/2486/er_1110-2-1156.pdf#page=496" ;
    pav:wasDerivedFrom "glossaries/CivilWorks/ER-1110-2-1156.yaml#term[Dam Safety Program Manager (DSPM)]" ;
    skos:altLabel "DSPM" ;
    skos:definition "Dam Safety officials at the HQUSACE, MSC, and district level responsible for the overall daily management of the Dam Safety program. These managers normally support and report to the Dam Safety Officer at their respective level." ;
    skos:inScheme ER-1110-2-1156: ;
    skos:prefLabel "Dam Safety Program Manager (DSPM)" .

ER-1110-2-1156:Dam_Safety_Steering_Committee_%28DSSC%29 a wov:GlossaryTerm,
        skos:Concept ;
    rdfs:label "Dam Safety Steering Committee (DSSC)" ;
    dcterms:bibliographicCitation "https://www.publications.usace.army.mil/Portals/76/Users/182/86/2486/er_1110-2-1156.pdf#page=494" ;
    pav:wasDerivedFrom "glossaries/CivilWorks/ER-1110-2-1156.yaml#term[Dam Safety Steering Committee (DSSC)]" ;
    skos:altLabel "DSSC" ;
    skos:definition "A committee charged with facilitating and promoting dam safety as a fundamental USACE mission in all levels of the organization, promoting dam safety career development, disseminating pertinent information throughout USACE, and reviewing and evaluating policy, technical criteria and practices, administrative procedures, and regulatory functions to support the USACE dam safety program. The DSSC reviews experience and qualifications of dam safety staffing at all levels within the USACE to assess competency, serves as a resource for sharing information and project specific Lessons Learned, and makes recommendations for future research and development in areas related to dam safety. The team meets as required, and provides advice and information to the Special Assistant for Dam and Levee Safety." ;
    skos:inScheme ER-1110-2-1156: ;
    skos:prefLabel "Dam Safety Steering Committee (DSSC)" .

ER-1110-2-1156:Dam_Senior_Oversight_Group_%28DSOG%29 a wov:GlossaryTerm,
        skos:Concept ;
    rdfs:label "Dam Senior Oversight Group (DSOG)" ;
    dcterms:bibliographicCitation "https://www.publications.usace.army.mil/Portals/76/Users/182/86/2486/er_1110-2-1156.pdf#page=496" ;
    pav:wasDerivedFrom "glossaries/CivilWorks/ER-1110-2-1156.yaml#term[Dam Senior Oversight Group (DSOG)]" ;
    skos:altLabel "DSOG" ;
    skos:definition "Designated USACE dam safety senior headquarters and field staff team that performs an oversight function for the Dam Safety program. The DSOG meets periodically to advise the Dam Safety Officer on key issues related to the program, such as determining Dam Safety Action Classifications. The DSOG generally consists of the following members: Special Assistant for Dam and Levee Safety (Chair); USACE CoP leaders (for Geotechnical, Structural and H&H technical disciplines); Regional representatives determined by Special Assistant for Dam and Levee Safety; USACE Business Line & Program Representatives to include USACE DSPM, Flood Damage Reduction, Navigation, Programs, and Risk Management Center Director; and any other Representatives determined by the Special Assistant for Dam and Levee Safety. The Senior Oversight Group is established to vet the findings of the Regional Risk Cadres and confirm dam safety work priorities based on portfolio risk findings." ;
    skos:inScheme ER-1110-2-1156: ;
    skos:prefLabel "Dam Senior Oversight Group (DSOG)" .

ER-1110-2-1156:Dam_failure a wov:GlossaryTerm,
        skos:Concept ;
    rdfs:label "Dam failure" ;
    dcterms:bibliographicCitation "https://www.publications.usace.army.mil/Portals/76/Users/182/86/2486/er_1110-2-1156.pdf#page=493" ;
    pav:wasDerivedFrom "glossaries/CivilWorks/ER-1110-2-1156.yaml#term[Dam failure]" ;
    skos:definition "Failure characterized by the sudden, rapid, and uncontrolled release of impounded water. It is recognized that there are lesser degrees of failure and that any malfunction or abnormality outside the design assumptions and parameters that adversely affect a dam's primary function of impounding water is properly considered a failure. These lesser degrees of failure can lead to loss of services and progressively lead to or heighten the risk of a catastrophic failure." ;
    skos:inScheme ER-1110-2-1156: ;
    skos:prefLabel "Dam failure" .

ER-1110-2-1156:Dam_safety_preparedness a wov:GlossaryTerm,
        skos:Concept ;
    rdfs:label "Dam safety preparedness" ;
    dcterms:bibliographicCitation "https://www.publications.usace.army.mil/Portals/76/Users/182/86/2486/er_1110-2-1156.pdf#page=496" ;
    pav:wasDerivedFrom "glossaries/CivilWorks/ER-1110-2-1156.yaml#term[Dam safety preparedness]" ;
    skos:definition "The quality or state of being prepared to deal with emergency conditions which endanger the structural integrity of the dam and/or downstream property and human life." ;
    skos:inScheme ER-1110-2-1156: ;
    skos:prefLabel "Dam safety preparedness" .

ER-1110-2-1156:Damming_Surface a wov:GlossaryTerm,
        skos:Concept ;
    rdfs:label "Damming Surface" ;
    dcterms:bibliographicCitation "https://www.publications.usace.army.mil/Portals/76/Users/182/86/2486/er_1110-2-1156.pdf#page=497" ;
    pav:wasDerivedFrom "glossaries/CivilWorks/ER-1110-2-1156.yaml#term[Damming Surface]" ;
    skos:definition "Any surface of the structure that hold back water. In the case of a navigation lock, the damming surface could include the miter gates and lock walls. In the case of a hydropower unit, the damming surface could be the head gates on the penstocks" ;
    skos:inScheme ER-1110-2-1156: ;
    skos:prefLabel "Damming Surface" .

ER-1110-2-1156:Dead_storage a wov:GlossaryTerm,
        skos:Concept ;
    rdfs:label "Dead storage" ;
    dcterms:bibliographicCitation "https://www.publications.usace.army.mil/Portals/76/Users/182/86/2486/er_1110-2-1156.pdf#page=523" ;
    pav:wasDerivedFrom "glossaries/CivilWorks/ER-1110-2-1156.yaml#term[Dead storage]" ;
    skos:definition "The storage that lies below the invert of the lowest outlet and that, therefore, cannot readily be withdrawn from the reservoir." ;
    skos:inScheme ER-1110-2-1156: ;
    skos:prefLabel "Dead storage" .

ER-1110-2-1156:Design_Structural_Capacity a wov:GlossaryTerm,
        skos:Concept ;
    rdfs:label "Design Structural Capacity" ;
    dcterms:bibliographicCitation "https://www.publications.usace.army.mil/Portals/76/Users/182/86/2486/er_1110-2-1156.pdf#page=497" ;
    pav:wasDerivedFrom "glossaries/CivilWorks/ER-1110-2-1156.yaml#term[Design Structural Capacity]" ;
    skos:definition "The maximum loading condition that the project was planned to withstand, although the project may fail at a lesser loading condition" ;
    skos:inScheme ER-1110-2-1156: ;
    skos:prefLabel "Design Structural Capacity" .

ER-1110-2-1156:Design_water_level a wov:GlossaryTerm,
        skos:Concept ;
    rdfs:label "Design water level" ;
    dcterms:bibliographicCitation "https://www.publications.usace.army.mil/Portals/76/Users/182/86/2486/er_1110-2-1156.pdf#page=497" ;
    pav:wasDerivedFrom "glossaries/CivilWorks/ER-1110-2-1156.yaml#term[Design water level]" ;
    skos:definition "The maximum water elevation including the flood surcharge that a dam is designed to withstand." ;
    skos:inScheme ER-1110-2-1156: ;
    skos:prefLabel "Design water level" .

ER-1110-2-1156:Design_wind a wov:GlossaryTerm,
        skos:Concept ;
    rdfs:label "Design wind" ;
    dcterms:bibliographicCitation "https://www.publications.usace.army.mil/Portals/76/Users/182/86/2486/er_1110-2-1156.pdf#page=497" ;
    pav:wasDerivedFrom "glossaries/CivilWorks/ER-1110-2-1156.yaml#term[Design wind]" ;
    skos:definition "The most severe wind that is reasonably possible at a particular reservoir for generating wind setup and run-up. The determination will generally include the results of meteorological studies, which combine wind velocity, duration, direction, and seasonal distribution characteristics in a realistic manner." ;
    skos:inScheme ER-1110-2-1156: ;
    skos:prefLabel "Design wind" .

ER-1110-2-1156:Diaphragm_wall a wov:GlossaryTerm,
        skos:Concept ;
    rdfs:label "Diaphragm wall" ;
    dcterms:bibliographicCitation "https://www.publications.usace.army.mil/Portals/76/Users/182/86/2486/er_1110-2-1156.pdf#page=497" ;
    pav:wasDerivedFrom "glossaries/CivilWorks/ER-1110-2-1156.yaml#term[Diaphragm wall]" ;
    skos:altLabel "membrane" ;
    skos:definition "A sheet, thin zone, or facing made of an impervious material such as concrete, steel, wood, or plastic. Also see core wall." ;
    skos:inScheme ER-1110-2-1156: ;
    skos:prefLabel "Diaphragm wall" .

ER-1110-2-1156:Dike a wov:GlossaryTerm,
        skos:Concept ;
    rdfs:label "Dike" ;
    dcterms:bibliographicCitation "https://www.publications.usace.army.mil/Portals/76/Users/182/86/2486/er_1110-2-1156.pdf#page=497" ;
    pav:wasDerivedFrom "glossaries/CivilWorks/ER-1110-2-1156.yaml#term[Dike]" ;
    skos:definition "See Dam, w. saddle dam." ;
    skos:inScheme ER-1110-2-1156: ;
    skos:prefLabel "Dike" .

ER-1110-2-1156:Direct_Economic_Losses a wov:GlossaryTerm,
        skos:Concept ;
    rdfs:label "Direct Economic Losses" ;
    dcterms:bibliographicCitation "https://www.publications.usace.army.mil/Portals/76/Users/182/86/2486/er_1110-2-1156.pdf#page=497" ;
    pav:wasDerivedFrom "glossaries/CivilWorks/ER-1110-2-1156.yaml#term[Direct Economic Losses]" ;
    skos:definition "Direct economic losses are the damage to property located downstream from the dam due to the failure. Items in this category include those commonly computed for the National Economic Development (NED) account in any USACE flood risk management study. These include damage to private and public buildings, contents of buildings, vehicles, public infrastructure such as roads and bridges, public utility infrastructure, agricultural crops, agricultural capital, and erosion losses to land." ;
    skos:inScheme ER-1110-2-1156: ;
    skos:prefLabel "Direct Economic Losses" .

<https://usace-data.com/civil-works/glossary/ER-1110-2-1156#Diversion_channel,_canal,_or_tunnel> a wov:GlossaryTerm,
        skos:Concept ;
    rdfs:label "Diversion channel, canal, or tunnel" ;
    dcterms:bibliographicCitation "https://www.publications.usace.army.mil/Portals/76/Users/182/86/2486/er_1110-2-1156.pdf#page=497" ;
    pav:wasDerivedFrom "glossaries/CivilWorks/ER-1110-2-1156.yaml#term[Diversion channel, canal, or tunnel]" ;
    skos:definition "A waterway used to divert water from its natural course. The term is generally applied to a temporary arrangement, e.g., to by-pass water around a dam site during construction. Channel is normally used instead of canal when the waterway is short." ;
    skos:inScheme ER-1110-2-1156: ;
    skos:prefLabel "Diversion channel, canal, or tunnel" .

<https://usace-data.com/civil-works/glossary/ER-1110-2-1156#Drain,_blanket> a wov:GlossaryTerm,
        skos:Concept ;
    rdfs:label "Drain, blanket" ;
    dcterms:bibliographicCitation "https://www.publications.usace.army.mil/Portals/76/Users/182/86/2486/er_1110-2-1156.pdf#page=497" ;
    pav:wasDerivedFrom "glossaries/CivilWorks/ER-1110-2-1156.yaml#term[Drain, blanket]" ;
    skos:definition "A layer of pervious material placed to facilitate drainage of the foundation and/or embankment." ;
    skos:inScheme ER-1110-2-1156: ;
    skos:prefLabel "Drain, blanket" .

<https://usace-data.com/civil-works/glossary/ER-1110-2-1156#Drain,_chimney> a wov:GlossaryTerm,
        skos:Concept ;
    rdfs:label "Drain, chimney" ;
    dcterms:bibliographicCitation "https://www.publications.usace.army.mil/Portals/76/Users/182/86/2486/er_1110-2-1156.pdf#page=497" ;
    pav:wasDerivedFrom "glossaries/CivilWorks/ER-1110-2-1156.yaml#term[Drain, chimney]" ;
    skos:definition "A vertical or inclined layer of pervious material in an embankment to facilitate and control drainage of the embankment fill." ;
    skos:inScheme ER-1110-2-1156: ;
    skos:prefLabel "Drain, chimney" .

<https://usace-data.com/civil-works/glossary/ER-1110-2-1156#Drain,_toe> a wov:GlossaryTerm,
        skos:Concept ;
    rdfs:label "Drain, toe" ;
    dcterms:bibliographicCitation "https://www.publications.usace.army.mil/Portals/76/Users/182/86/2486/er_1110-2-1156.pdf#page=497" ;
    pav:wasDerivedFrom "glossaries/CivilWorks/ER-1110-2-1156.yaml#term[Drain, toe]" ;
    skos:definition "A system of pipe and/or pervious material along the downstream toe of a dam used to collect seepage from the foundation and embankment and convey it to a free outlet." ;
    skos:inScheme ER-1110-2-1156: ;
    skos:prefLabel "Drain, toe" .

ER-1110-2-1156:Drainage_area a wov:GlossaryTerm,
        skos:Concept ;
    rdfs:label "Drainage area" ;
    dcterms:bibliographicCitation "https://www.publications.usace.army.mil/Portals/76/Users/182/86/2486/er_1110-2-1156.pdf#page=497" ;
    pav:wasDerivedFrom "glossaries/CivilWorks/ER-1110-2-1156.yaml#term[Drainage area]" ;
    skos:definition "The area, which drains to a particular point on a river or stream." ;
    skos:inScheme ER-1110-2-1156: ;
    skos:prefLabel "Drainage area" .

ER-1110-2-1156:Drainage_curtain a wov:GlossaryTerm,
        skos:Concept ;
    rdfs:label "Drainage curtain" ;
    dcterms:bibliographicCitation "https://www.publications.usace.army.mil/Portals/76/Users/182/86/2486/er_1110-2-1156.pdf#page=498" ;
    pav:wasDerivedFrom "glossaries/CivilWorks/ER-1110-2-1156.yaml#term[Drainage curtain]" ;
    skos:definition "Also called drainage wells or relief wells. A line of vertical wells or boreholes placed to facilitate drainage of the foundation and abutments and to reduce water pressure." ;
    skos:inScheme ER-1110-2-1156: ;
    skos:prefLabel "Drainage curtain" .

ER-1110-2-1156:Drawdown a wov:GlossaryTerm,
        skos:Concept ;
    rdfs:label "Drawdown" ;
    dcterms:bibliographicCitation "https://www.publications.usace.army.mil/Portals/76/Users/182/86/2486/er_1110-2-1156.pdf#page=498" ;
    pav:wasDerivedFrom "glossaries/CivilWorks/ER-1110-2-1156.yaml#term[Drawdown]" ;
    skos:definition "The difference between a water level and a lower water level in a reservoir within a particular time. Used as a verb, it is the lowering of the water surface." ;
    skos:inScheme ER-1110-2-1156: ;
    skos:prefLabel "Drawdown" .

ER-1110-2-1156:Drum_gate a wov:GlossaryTerm,
        skos:Concept ;
    rdfs:label "Drum gate" ;
    dcterms:bibliographicCitation "https://www.publications.usace.army.mil/Portals/76/Users/182/86/2486/er_1110-2-1156.pdf#page=506" ;
    pav:wasDerivedFrom "glossaries/CivilWorks/ER-1110-2-1156.yaml#term[Drum gate]" ;
    skos:definition "A type of spillway gate consisting of a long hollow drum. The drum may be held in its raised position by the water pressure in a flotation chamber beneath the dam." ;
    skos:inScheme ER-1110-2-1156: ;
    skos:prefLabel "Drum gate" .

ER-1110-2-1156:Earthquake a wov:GlossaryTerm,
        skos:Concept ;
    rdfs:label "Earthquake" ;
    dcterms:bibliographicCitation "https://www.publications.usace.army.mil/Portals/76/Users/182/86/2486/er_1110-2-1156.pdf#page=498" ;
    pav:wasDerivedFrom "glossaries/CivilWorks/ER-1110-2-1156.yaml#term[Earthquake]" ;
    skos:definition "A sudden motion or trembling in the earth caused by the abrupt release of accumulated stress along a fault." ;
    skos:inScheme ER-1110-2-1156: ;
    skos:prefLabel "Earthquake" .

<https://usace-data.com/civil-works/glossary/ER-1110-2-1156#Earthquake,_Maximum_Credible_%28MCE%29> a wov:GlossaryTerm,
        skos:Concept ;
    rdfs:label "Earthquake, Maximum Credible (MCE)" ;
    dcterms:bibliographicCitation "https://www.publications.usace.army.mil/Portals/76/Users/182/86/2486/er_1110-2-1156.pdf#page=498" ;
    pav:wasDerivedFrom "glossaries/CivilWorks/ER-1110-2-1156.yaml#term[Earthquake, Maximum Credible (MCE)]" ;
    skos:altLabel "MCE" ;
    skos:definition "The MCE is defined as the greatest earthquake that can reasonably be expected to be generated by a specific source on the basis of seismological and geological evidence. Since a project site may be affected by earthquakes generated by various sources, each with its own fault mechanism, maximum earthquake magnitude, and distance from the site, multiple MCE's may be defined for the site, each with characteristic ground motion parameters and spectral shape. The MCE is determined by a DSHA and input from PSHA when site specific studies are performed." ;
    skos:inScheme ER-1110-2-1156: ;
    skos:prefLabel "Earthquake, Maximum Credible (MCE)" .

<https://usace-data.com/civil-works/glossary/ER-1110-2-1156#Earthquake,_Maximum_Design_%28MDE%29> a wov:GlossaryTerm,
        skos:Concept ;
    rdfs:label "Earthquake, Maximum Design (MDE)" ;
    dcterms:bibliographicCitation "https://www.publications.usace.army.mil/Portals/76/Users/182/86/2486/er_1110-2-1156.pdf#page=499" ;
    pav:wasDerivedFrom "glossaries/CivilWorks/ER-1110-2-1156.yaml#term[Earthquake, Maximum Design (MDE)]" ;
    skos:altLabel "MDE" ;
    skos:definition "The MDE is the maximum level of ground motion for which a structure is designed or evaluated. The associated performance requirement is that the project performs without catastrophic failure, such as uncontrolled release of a reservoir, although severe damage or economic loss may be tolerated. For critical features, the MDE is the same as the MCE. For all other features, the MDE must be selected as a minimum of event with a 10% probability of exceedance in 100 years. ( This corresponds to an average return period of 975 years). The longer or shorter return period for the non critical features can be use if warranted. The MDE can be characterized as a deterministic or probabilistic event." ;
    skos:inScheme ER-1110-2-1156: ;
    skos:prefLabel "Earthquake, Maximum Design (MDE)" .

<https://usace-data.com/civil-works/glossary/ER-1110-2-1156#Earthquake,_Operating_Basis_%28OBE%29> a wov:GlossaryTerm,
        skos:Concept ;
    rdfs:label "Earthquake, Operating Basis (OBE)" ;
    dcterms:bibliographicCitation "https://www.publications.usace.army.mil/Portals/76/Users/182/86/2486/er_1110-2-1156.pdf#page=499" ;
    pav:wasDerivedFrom "glossaries/CivilWorks/ER-1110-2-1156.yaml#term[Earthquake, Operating Basis (OBE)]" ;
    skos:altLabel "OBE" ;
    skos:definition "The OBE is considered to be an earthquake that has a 50 percent chance of being exceeded in 100 years (or a 144-year return period)." ;
    skos:inScheme ER-1110-2-1156: ;
    skos:prefLabel "Earthquake, Operating Basis (OBE)" .

<https://usace-data.com/civil-works/glossary/ER-1110-2-1156#Earthquake,_Safety_Evaluation_%28SEE%29> a wov:GlossaryTerm,
        skos:Concept ;
    rdfs:label "Earthquake, Safety Evaluation (SEE)" ;
    dcterms:bibliographicCitation "https://www.publications.usace.army.mil/Portals/76/Users/182/86/2486/er_1110-2-1156.pdf#page=499" ;
    pav:wasDerivedFrom "glossaries/CivilWorks/ER-1110-2-1156.yaml#term[Earthquake, Safety Evaluation (SEE)]" ;
    skos:altLabel "SEE" ;
    skos:definition "The earthquake, expressed in terms of magnitude and closest distance from the dam site or in terms of the characteristics of the time history of free-field ground motions, for which the safety of the dam and critical structures associated with the dam are to be evaluated. In many cases, this earthquake will be the maximum credible earthquake to which the dam will be exposed. However, in other cases where the possible sources of ground motion are not easily apparent, it may be a motion with prescribed characteristics selected on the basis of a probabilistic assessment of the ground motions that may occur in the vicinity of the dam. To be considered safe, it should be demonstrated that the dam can withstand this level of earthquake shaking without release of water from the reservoir." ;
    skos:inScheme ER-1110-2-1156: ;
    skos:prefLabel "Earthquake, Safety Evaluation (SEE)" .

<https://usace-data.com/civil-works/glossary/ER-1110-2-1156#Earthquake,_synthetic> a wov:GlossaryTerm,
        skos:Concept ;
    rdfs:label "Earthquake, synthetic" ;
    dcterms:bibliographicCitation "https://www.publications.usace.army.mil/Portals/76/Users/182/86/2486/er_1110-2-1156.pdf#page=499" ;
    pav:wasDerivedFrom "glossaries/CivilWorks/ER-1110-2-1156.yaml#term[Earthquake, synthetic]" ;
    skos:definition "Earthquake time history records developed from mathematical models that use white noise, filtered white noise, and stationary and non-stationary filtered white noise, or theoretical seismic source models of failure in the fault zone. (White noise is random energy containing all frequency components in equal proportions. Stationary white noise is random energy with statistical characteristics that do not vary with time)." ;
    skos:inScheme ER-1110-2-1156: ;
    skos:prefLabel "Earthquake, synthetic" .

ER-1110-2-1156:Economic_Consequences a wov:GlossaryTerm,
        skos:Concept ;
    rdfs:label "Economic Consequences" ;
    dcterms:bibliographicCitation "https://www.publications.usace.army.mil/Portals/76/Users/182/86/2486/er_1110-2-1156.pdf#page=499" ;
    pav:wasDerivedFrom "glossaries/CivilWorks/ER-1110-2-1156.yaml#term[Economic Consequences]" ;
    skos:definition "Direct and indirect losses of the failure of a dam and other economic impacts on the regional or national economy. Part of the direct losses is the damage to property located downstream from the dam due to the failure. Items in this category include those commonly computed for the National Economic Development (NED) account in any USACE flood risk management study." ;
    skos:inScheme ER-1110-2-1156: ;
    skos:prefLabel "Economic Consequences" .

ER-1110-2-1156:Economic_Damages a wov:GlossaryTerm,
        skos:Concept ;
    rdfs:label "Economic Damages" ;
    dcterms:bibliographicCitation "https://www.publications.usace.army.mil/Portals/76/Users/182/86/2486/er_1110-2-1156.pdf#page=499" ;
    pav:wasDerivedFrom "glossaries/CivilWorks/ER-1110-2-1156.yaml#term[Economic Damages]" ;
    skos:definition "These include damage to private and public buildings, contents of buildings, vehicles, public infrastructure such as roads and bridges, public utility infrastructure, agricultural crops, agricultural capital, and erosion losses to land." ;
    skos:inScheme ER-1110-2-1156: ;
    skos:prefLabel "Economic Damages" .

ER-1110-2-1156:Economic_Regret a wov:GlossaryTerm,
        skos:Concept ;
    rdfs:label "Economic Regret" ;
    dcterms:bibliographicCitation "https://www.publications.usace.army.mil/Portals/76/Users/182/86/2486/er_1110-2-1156.pdf#page=499" ;
    pav:wasDerivedFrom "glossaries/CivilWorks/ER-1110-2-1156.yaml#term[Economic Regret]" ;
    skos:definition "Condition when the costs of making a wrong decision are deemed to be high. The basic concept of regret is the difference between the outcome of the \"best alternative for a future, uncertain state\" and outcome of each alternative evaluated for that state. So it is really the potential costs, if you choose an alternative as the best given some future scenario, and a different future actually happens. All regret values are determined by comparing each alternative to the best (e.g. maximum net benefits) for a scenario. So you end up with a regret matrix with scenarios as column headings and alternatives as row headings. There is nothing in the notion about regret about it being \"too high.\" The minimax principle is usually applied to regret to identify the plan or plans that are robust across multiple future scenarios." ;
    skos:inScheme ER-1110-2-1156: ;
    skos:prefLabel "Economic Regret" .

ER-1110-2-1156:Efficiency a wov:GlossaryTerm,
        skos:Concept ;
    rdfs:label "Efficiency" ;
    dcterms:bibliographicCitation "https://www.publications.usace.army.mil/Portals/76/Users/182/86/2486/er_1110-2-1156.pdf#page=500" ;
    pav:wasDerivedFrom "glossaries/CivilWorks/ER-1110-2-1156.yaml#term[Efficiency]" ;
    skos:definition "Efficiency is the need for society to distribute and use available resources so as to achieve the greatest benefit. For dam safety investments, this means ensuring that resources and expenditure directed to safety improvements are cost-effective and that an appropriate balance between the monetary and non-monetary benefits and the monetary and non-monetary costs is achieved." ;
    skos:inScheme ER-1110-2-1156: ;
    skos:prefLabel "Efficiency" .

ER-1110-2-1156:Embankment a wov:GlossaryTerm,
        skos:Concept ;
    rdfs:label "Embankment" ;
    dcterms:bibliographicCitation "https://www.publications.usace.army.mil/Portals/76/Users/182/86/2486/er_1110-2-1156.pdf#page=500" ;
    pav:wasDerivedFrom "glossaries/CivilWorks/ER-1110-2-1156.yaml#term[Embankment]" ;
    skos:definition "A raised structure of earth, rocks, or gravel, usually intended to retain water or carry a roadway." ;
    skos:inScheme ER-1110-2-1156: ;
    skos:prefLabel "Embankment" .

ER-1110-2-1156:Emergency a wov:GlossaryTerm,
        skos:Concept ;
    rdfs:label "Emergency" ;
    dcterms:bibliographicCitation "https://www.publications.usace.army.mil/Portals/76/Users/182/86/2486/er_1110-2-1156.pdf#page=500" ;
    pav:wasDerivedFrom "glossaries/CivilWorks/ER-1110-2-1156.yaml#term[Emergency]" ;
    skos:definition "An emergency, in terms of dam operation, is a condition, which develops unexpectedly, endangers the structural integrity of the dam and/or downstream property and human life, and requires immediate action." ;
    skos:inScheme ER-1110-2-1156: ;
    skos:prefLabel "Emergency" .

ER-1110-2-1156:Emergency_Action_Plan_%28EAP%29 a wov:GlossaryTerm,
        skos:Concept ;
    rdfs:label "Emergency Action Plan (EAP)" ;
    dcterms:bibliographicCitation "https://www.publications.usace.army.mil/Portals/76/Users/182/86/2486/er_1110-2-1156.pdf#page=500" ;
    pav:wasDerivedFrom "glossaries/CivilWorks/ER-1110-2-1156.yaml#term[Emergency Action Plan (EAP)]" ;
    skos:altLabel "EAP" ;
    skos:definition "An action plan that provides detailed instructions for agencies and individuals for responding to emergencies such as a potential dam failure. Plans typically include threat recognition, emergency action message formulation, message dissemination to authorities and the public, provisions for search and rescue, and early stages of recovery." ;
    skos:inScheme ER-1110-2-1156: ;
    skos:prefLabel "Emergency Action Plan (EAP)" .

ER-1110-2-1156:Emergency_Exercise a wov:GlossaryTerm,
        skos:Concept ;
    rdfs:label "Emergency Exercise" ;
    dcterms:bibliographicCitation "https://www.publications.usace.army.mil/Portals/76/Users/182/86/2486/er_1110-2-1156.pdf#page=500",
        "https://www.publications.usace.army.mil/Portals/76/Users/182/86/2486/er_1110-2-1156.pdf#page=501" ;
    pav:wasDerivedFrom "glossaries/CivilWorks/ER-1110-2-1156.yaml#term[Emergency Exercise]" ;
    skos:definition "Drill “ A drill is the lowest level exercise that involves an actual exercise. It tests, develops, or maintains skills in a single emergency response procedure. An example of a drill is an in-house exercise performed to verify the validity of telephone numbers and other means of communication along with the response of the entity responsible for the dam. A drill is considered a necessary part of ongoing training.",
        "Full Scale “ The full scale exercise is the most complex level of exercise. It evaluates the operational capability of all facets of the emergency management system (both dam operator and state and local emergency management agencies) interactively in a stressful environment with the actual mobilization of personnel and resources. It includes deployment to and movement in the field of personnel and equipment to demonstrate coordination and response capability. The participants actively \"play out\" their roles in a dynamic environment that provides the highest degree of realism possible for the simulated event. Actual evacuation of critical residents may be exercised if previously announced to the public.",
        "Functional “ The functional exercise is the highest level exercise that does not involve the full activation of the entity responsible for dam operation and state and local emergency management agency field personnel and facilities or test evacuation of residents downstream of the dam. It involves the various levels of the entity responsible for dam operation and state and local emergency management personnel that would be involved in an actual emergency. The functional exercise takes place in a stress-induced environment with time constraints and involves the simulation of a dam failure and other specified events. The participants \"act out\" their actual roles. The exercise is designed to evaluate both the internal capabilities and responses of the entity responsible for dam operation and the workability of the information in the EAP used by the emergency management officials to carry out their responsibilities. The functional exercise also is designed to evaluate the coordination activities between the entity responsible for dam operation and emergency management personnel.",
        "Orientation Seminar “ This exercise is a seminar that involves bringing together those with a role or interest in an EAP, i.e., entity responsible for dam operation and state and local emergency management agencies, to discuss the EAP and initial plans for an annual drill or more in-depth comprehensive exercise. The seminar does not involve an actual exercise of the EAP. Instead, it is a meeting that enables each participant to become familiar with the EAP and the roles, responsibilities, and procedures of those involved. An orientation seminar can also be used to discuss and describe technical matters with involved, non-technical personnel.",
        "Tabletop “ The tabletop exercise involves a meeting of the entity responsible for dam operation and the state and local emergency management officials in a conference room environment. The format is usually informal with minimum stress involved. The exercise begins with the description of a simulated event and proceeds with discussions by the participants to evaluate the EAP and response procedures and to resolve concerns regarding coordination and responsibilities." ;
    skos:inScheme ER-1110-2-1156: ;
    skos:prefLabel "Emergency Exercise" .

ER-1110-2-1156:Emergency_gate a wov:GlossaryTerm,
        skos:Concept ;
    rdfs:label "Emergency gate" ;
    dcterms:bibliographicCitation "https://www.publications.usace.army.mil/Portals/76/Users/182/86/2486/er_1110-2-1156.pdf#page=506" ;
    pav:wasDerivedFrom "glossaries/CivilWorks/ER-1110-2-1156.yaml#term[Emergency gate]" ;
    skos:definition "A standby or auxiliary gate used when the normal means of water control is not available. Sometimes referred to as guard gate." ;
    skos:inScheme ER-1110-2-1156: ;
    skos:prefLabel "Emergency gate" .

ER-1110-2-1156:Endangered_Species_Act_%28ESA%29 a wov:GlossaryTerm,
        skos:Concept ;
    rdfs:label "Endangered Species Act (ESA)" ;
    dcterms:bibliographicCitation "https://www.publications.usace.army.mil/Portals/76/Users/182/86/2486/er_1110-2-1156.pdf#page=501" ;
    pav:wasDerivedFrom "glossaries/CivilWorks/ER-1110-2-1156.yaml#term[Endangered Species Act (ESA)]" ;
    skos:altLabel "ESA" ;
    skos:definition "The Endangered Species Act of 1973 (7 U.S.C. Â§ 136, 16 U.S.C. Â§ 1531 et seq.) or ESA is the most wide-ranging of the dozens of United States environmental laws passed in the 1970s (references A.6, A.9, and A.10). As stated in section 2 of the act, it was designed to protect critically imperiled species from extinction as a \"consequence of economic growth and development untendered by adequate concern and conservation.\" See ER 1105-2-100 Appendix C (reference A.39) for detailed discussion." ;
    skos:inScheme ER-1110-2-1156: ;
    skos:prefLabel "Endangered Species Act (ESA)" .

ER-1110-2-1156:Energy_dissipater a wov:GlossaryTerm,
        skos:Concept ;
    rdfs:label "Energy dissipater" ;
    dcterms:bibliographicCitation "https://www.publications.usace.army.mil/Portals/76/Users/182/86/2486/er_1110-2-1156.pdf#page=501" ;
    pav:wasDerivedFrom "glossaries/CivilWorks/ER-1110-2-1156.yaml#term[Energy dissipater]" ;
    skos:definition "A device constructed in a waterway to reduce the kinetic energy of fast flowing water." ;
    skos:inScheme ER-1110-2-1156: ;
    skos:prefLabel "Energy dissipater" .

ER-1110-2-1156:Environmental_Impact_Statement_%28EIS%29 a wov:GlossaryTerm,
        skos:Concept ;
    rdfs:label "Environmental Impact Statement (EIS)" ;
    dcterms:bibliographicCitation "https://www.publications.usace.army.mil/Portals/76/Users/182/86/2486/er_1110-2-1156.pdf#page=502" ;
    pav:wasDerivedFrom "glossaries/CivilWorks/ER-1110-2-1156.yaml#term[Environmental Impact Statement (EIS)]" ;
    skos:altLabel "EIS" ;
    skos:definition "An environmental impact statement, in the United States, is a document that must be filed when the federal government takes a \"major Federal action significantly affecting the quality of the human environment.\" The law requiring this is the National Environmental Policy Act. See ER 200-2-2 (reference A.34) and ER 1105-2-100, Appendix C (reference A.39), for details on preparation of EIS." ;
    skos:inScheme ER-1110-2-1156: ;
    skos:prefLabel "Environmental Impact Statement (EIS)" .

ER-1110-2-1156:Environmental_and_other_Non-monetary_Consequences a wov:GlossaryTerm,
        skos:Concept ;
    rdfs:label "Environmental and other Non-monetary Consequences" ;
    dcterms:bibliographicCitation "https://www.publications.usace.army.mil/Portals/76/Users/182/86/2486/er_1110-2-1156.pdf#page=501" ;
    pav:wasDerivedFrom "glossaries/CivilWorks/ER-1110-2-1156.yaml#term[Environmental and other Non-monetary Consequences]" ;
    skos:definition "Direct and indirect consequences that cannot be measured in monetary terms. These stem from the impacts of the dam failure flood and loss of pool on environmental, cultural, and historic resources. In most cases, the assessment of the impacts of dam failure will be the reporting of area and type of habitat impacted, habitat of threatened and endangered species impacted, number and type of historic sites and the cultural significance areas impacted. An indirect non-monetary consequence could be the exposure of people and the ecosystem to hazardous and toxic material released from landfills, warehouses, and other facilities. An estimate of the locations and quantities should be compiled identifying where significant quantities are concentrated." ;
    skos:inScheme ER-1110-2-1156: ;
    skos:prefLabel "Environmental and other Non-monetary Consequences" .

ER-1110-2-1156:Epicenter a wov:GlossaryTerm,
        skos:Concept ;
    rdfs:label "Epicenter" ;
    dcterms:bibliographicCitation "https://www.publications.usace.army.mil/Portals/76/Users/182/86/2486/er_1110-2-1156.pdf#page=502" ;
    pav:wasDerivedFrom "glossaries/CivilWorks/ER-1110-2-1156.yaml#term[Epicenter]" ;
    skos:definition "The point on the earth's surface located vertically above the point of origin of an earthquake." ;
    skos:inScheme ER-1110-2-1156: ;
    skos:prefLabel "Epicenter" .

ER-1110-2-1156:Equity_in_Risk_Management a wov:GlossaryTerm,
        skos:Concept ;
    rdfs:label "Equity in Risk Management" ;
    dcterms:bibliographicCitation "https://www.publications.usace.army.mil/Portals/76/Users/182/86/2486/er_1110-2-1156.pdf#page=502" ;
    pav:wasDerivedFrom "glossaries/CivilWorks/ER-1110-2-1156.yaml#term[Equity in Risk Management]" ;
    skos:definition "Equity, in the risk management context, is the right of individuals and society to be protected, and the right that the interests of all are treated with fairness, placing all members of society on a (more) equal footing in terms of levels of risk faced. The equity objective is addressed by requiring that all risks higher than a limit value be brought down below the limit, except in extraordinary circumstances." ;
    skos:inScheme ER-1110-2-1156: ;
    skos:prefLabel "Equity in Risk Management" .

ER-1110-2-1156:Essential_Agency_Guidelines a wov:GlossaryTerm,
        skos:Concept ;
    rdfs:label "Essential Agency Guidelines" ;
    dcterms:bibliographicCitation "https://www.publications.usace.army.mil/Portals/76/Users/182/86/2486/er_1110-2-1156.pdf#page=502" ;
    pav:wasDerivedFrom "glossaries/CivilWorks/ER-1110-2-1156.yaml#term[Essential Agency Guidelines]" ;
    skos:definition "The state-of-practice for design, construction, operation, and maintenance of USACE dams as documented in current USACE regulations. The requirements specified in these USACE regulations must be met for a dam to achieve DSAC 5 (Normal) classification status. These regulations include: Engineer Circulars, Engineer Regulations, Engineer Manuals, Engineer Pamphlets and Engineer Technical Letters; and Engineering and Construction Bulletins, and other official HQUSACE dam safety-related Policy Letters and guidance. Current state-of-practice guidance is summarized in Appendix F." ;
    skos:inScheme ER-1110-2-1156: ;
    skos:prefLabel "Essential Agency Guidelines" .

ER-1110-2-1156:Event_Tree%28s%29 a wov:GlossaryTerm,
        skos:Concept ;
    rdfs:label "Event Tree(s)" ;
    dcterms:bibliographicCitation "https://www.publications.usace.army.mil/Portals/76/Users/182/86/2486/er_1110-2-1156.pdf#page=502" ;
    pav:wasDerivedFrom "glossaries/CivilWorks/ER-1110-2-1156.yaml#term[Event Tree(s)]" ;
    skos:definition "An event tree serves as a model of the physical dam system in which each node represents an identifiable behavior of the dam or its physical components and each event should be something that happens in space or time (Hartford and Baecher, 2004). An event tree begins with a single initiating branch on the left hand side and progress toward more detailed events to the right hand side. Starting with an initiating event branch (e.g. a severe flood, an earthquake or other natural or human caused hazards), each node is divided at various nodes to generate all possible subsequent events. Each node is an origin of possible subsequent events and each branch is a possible event that is a logical consequence of the one before it, and a necessary precursor of the one that follows. As the number of events increases, structure fans outs like the branches of a tree until each event tree chain comes to a terminal branch. Terminal branches are the system outcome or system effect of an initiating event which leads to adverse consequences or failure of the system completely or partially. The tree may be extended to represent the economic damages and life loss consequences associated with the terminal branches." ;
    skos:inScheme ER-1110-2-1156: ;
    skos:prefLabel "Event Tree(s)" .

ER-1110-2-1156:Existing_Condition_Component_Risk_Estimates a wov:GlossaryTerm,
        skos:Concept ;
    rdfs:label "Existing Condition Component Risk Estimates" ;
    dcterms:bibliographicCitation "https://www.publications.usace.army.mil/Portals/76/Users/182/86/2486/er_1110-2-1156.pdf#page=503" ;
    pav:wasDerivedFrom "glossaries/CivilWorks/ER-1110-2-1156.yaml#term[Existing Condition Component Risk Estimates]" ;
    skos:definition "An Estimate of risk contributed by an individual credible failure mode that is associated with a dam for given load combinations." ;
    skos:inScheme ER-1110-2-1156: ;
    skos:prefLabel "Existing Condition Component Risk Estimates" .

ER-1110-2-1156:Existing_Condition_Risk_Estimate a wov:GlossaryTerm,
        skos:Concept ;
    rdfs:label "Existing Condition Risk Estimate" ;
    dcterms:bibliographicCitation "https://www.publications.usace.army.mil/Portals/76/Users/182/86/2486/er_1110-2-1156.pdf#page=503" ;
    pav:wasDerivedFrom "glossaries/CivilWorks/ER-1110-2-1156.yaml#term[Existing Condition Risk Estimate]" ;
    skos:definition "The risk estimate at a point in time." ;
    skos:inScheme ER-1110-2-1156: ;
    skos:prefLabel "Existing Condition Risk Estimate" .

ER-1110-2-1156:Existing_and_Future_Condition_Without_Federal_Action_Consequence_Analysis a wov:GlossaryTerm,
        skos:Concept ;
    rdfs:label "Existing and Future Condition Without Federal Action Consequence Analysis" ;
    dcterms:bibliographicCitation "https://www.publications.usace.army.mil/Portals/76/Users/182/86/2486/er_1110-2-1156.pdf#page=503" ;
    pav:wasDerivedFrom "glossaries/CivilWorks/ER-1110-2-1156.yaml#term[Existing and Future Condition Without Federal Action Consequence Analysis]" ;
    skos:definition "Analysis of existing and future without Federal remediation project consequences." ;
    skos:inScheme ER-1110-2-1156: ;
    skos:prefLabel "Existing and Future Condition Without Federal Action Consequence Analysis" .

ER-1110-2-1156:Exposure_Assessment a wov:GlossaryTerm,
        skos:Concept ;
    rdfs:label "Exposure Assessment" ;
    dcterms:bibliographicCitation "https://www.publications.usace.army.mil/Portals/76/Users/182/86/2486/er_1110-2-1156.pdf#page=503" ;
    pav:wasDerivedFrom "glossaries/CivilWorks/ER-1110-2-1156.yaml#term[Exposure Assessment]" ;
    skos:definition "Exposure occurs when a susceptible asset comes in contact with a hazard. An exposure assessment, then, is the determination or estimation (which may be qualitative or quantitative) of the magnitude, frequency, or duration, and route of exposure." ;
    skos:inScheme ER-1110-2-1156: ;
    skos:prefLabel "Exposure Assessment" .

ER-1110-2-1156:F-N_chart a wov:GlossaryTerm,
        skos:Concept ;
    rdfs:label "F-N chart" ;
    dcterms:bibliographicCitation "https://www.publications.usace.army.mil/Portals/76/Users/182/86/2486/er_1110-2-1156.pdf#page=505" ;
    pav:wasDerivedFrom "glossaries/CivilWorks/ER-1110-2-1156.yaml#term[F-N chart]" ;
    skos:altLabel "Plot" ;
    skos:definition "This chart is a plot of the annual probability of exceedance (greater than or equal to) of potential life loss (F) vs. incremental potential loss of life (N) due to failure compared to the no failure condition. Thus, the F-N chart displays the entire estimated probability distribution of life loss for a reservoir encompassing all failure modes and all population exposure scenarios for a particular reservoir. See figure 5.4.b." ;
    skos:inScheme ER-1110-2-1156: ;
    skos:prefLabel "F-N chart" .

ER-1110-2-1156:Failure_Mode a wov:GlossaryTerm,
        skos:Concept ;
    rdfs:label "Failure Mode" ;
    dcterms:bibliographicCitation "https://www.publications.usace.army.mil/Portals/76/Users/182/86/2486/er_1110-2-1156.pdf#page=503" ;
    pav:wasDerivedFrom "glossaries/CivilWorks/ER-1110-2-1156.yaml#term[Failure Mode]" ;
    skos:definition "A way that failure can occur, described by the means by which element or component failures must occur to cause loss of the sub-system or system function of a dam that could result in failure." ;
    skos:inScheme ER-1110-2-1156: ;
    skos:prefLabel "Failure Mode" .

ER-1110-2-1156:Failure_of_a_Water_Control_System a wov:GlossaryTerm,
        skos:Concept ;
    rdfs:label "Failure of a Water Control System" ;
    dcterms:bibliographicCitation "https://www.publications.usace.army.mil/Portals/76/Users/182/86/2486/er_1110-2-1156.pdf#page=503" ;
    pav:wasDerivedFrom "glossaries/CivilWorks/ER-1110-2-1156.yaml#term[Failure of a Water Control System]" ;
    skos:definition "A water control system failure is any condition that results in the uncontrolled release or discharge of water. This might include misoperation involving improper or unintended opening or closing of gates, valves, operation of pumps, etc. Misoperation leading to systems not operating when needed or intended (i.e. gates fail to open on demand) might also lead to failure. Another example could be structural failure involving partial or total collapse of a gate." ;
    skos:inScheme ER-1110-2-1156: ;
    skos:prefLabel "Failure of a Water Control System" .

ER-1110-2-1156:Fault a wov:GlossaryTerm,
        skos:Concept ;
    rdfs:label "Fault" ;
    dcterms:bibliographicCitation "https://www.publications.usace.army.mil/Portals/76/Users/182/86/2486/er_1110-2-1156.pdf#page=503" ;
    pav:wasDerivedFrom "glossaries/CivilWorks/ER-1110-2-1156.yaml#term[Fault]" ;
    skos:definition "A fracture or fracture zone in the earth crust along which there has been displacement of the two sides relative to one another." ;
    skos:inScheme ER-1110-2-1156: ;
    skos:prefLabel "Fault" .

<https://usace-data.com/civil-works/glossary/ER-1110-2-1156#Fault,_active> a wov:GlossaryTerm,
        skos:Concept ;
    rdfs:label "Fault, active" ;
    dcterms:bibliographicCitation "https://www.publications.usace.army.mil/Portals/76/Users/182/86/2486/er_1110-2-1156.pdf#page=503" ;
    pav:wasDerivedFrom "glossaries/CivilWorks/ER-1110-2-1156.yaml#term[Fault, active]" ;
    skos:definition "A fault which, because of its present tectonic setting, can undergo movement from time to time in the immediate geologic future." ;
    skos:inScheme ER-1110-2-1156: ;
    skos:prefLabel "Fault, active" .

<https://usace-data.com/civil-works/glossary/ER-1110-2-1156#Fault,_capable> a wov:GlossaryTerm,
        skos:Concept ;
    rdfs:label "Fault, capable" ;
    dcterms:bibliographicCitation "https://www.publications.usace.army.mil/Portals/76/Users/182/86/2486/er_1110-2-1156.pdf#page=503" ;
    pav:wasDerivedFrom "glossaries/CivilWorks/ER-1110-2-1156.yaml#term[Fault, capable]" ;
    skos:definition "An active fault that is judged capable of producing macro earthquakes and exhibits one or more of the following characteristics: years. a. Movement at or near the ground surface at least once within the past 35,000 b. Macroseismicity (3.5 magnitude Richter or greater) instrumentally determined with records of sufficient precision to demonstrate a direct relationship with the fault. c. A structural relationship to a capable fault such that movement on one fault could be reasonably expected to cause movement on the other. d. Established patterns of microseismicity, which define a fault, with historic macroseismicity that can reasonably, be associated with the fault." ;
    skos:inScheme ER-1110-2-1156: ;
    skos:prefLabel "Fault, capable" .

ER-1110-2-1156:Fetch a wov:GlossaryTerm,
        skos:Concept ;
    rdfs:label "Fetch" ;
    dcterms:bibliographicCitation "https://www.publications.usace.army.mil/Portals/76/Users/182/86/2486/er_1110-2-1156.pdf#page=504" ;
    pav:wasDerivedFrom "glossaries/CivilWorks/ER-1110-2-1156.yaml#term[Fetch]" ;
    skos:definition "The straight-line distance across a body of water subject to wind forces. The fetch is one of the factors used in calculating wave heights in a reservoir." ;
    skos:inScheme ER-1110-2-1156: ;
    skos:prefLabel "Fetch" .

ER-1110-2-1156:Filter_%28filter_zone%29 a wov:GlossaryTerm,
        skos:Concept ;
    rdfs:label "Filter (filter zone)" ;
    dcterms:bibliographicCitation "https://www.publications.usace.army.mil/Portals/76/Users/182/86/2486/er_1110-2-1156.pdf#page=504" ;
    pav:wasDerivedFrom "glossaries/CivilWorks/ER-1110-2-1156.yaml#term[Filter (filter zone)]" ;
    skos:definition "One or more layers of granular material graded (either naturally or by selection) so as to allow seepage through or within the layers while preventing the migration of material from adjacent zones." ;
    skos:inScheme ER-1110-2-1156: ;
    skos:prefLabel "Filter (filter zone)" .

ER-1110-2-1156:Fixed_wheel_gate a wov:GlossaryTerm,
        skos:Concept ;
    rdfs:label "Fixed wheel gate" ;
    dcterms:bibliographicCitation "https://www.publications.usace.army.mil/Portals/76/Users/182/86/2486/er_1110-2-1156.pdf#page=506" ;
    pav:wasDerivedFrom "glossaries/CivilWorks/ER-1110-2-1156.yaml#term[Fixed wheel gate]" ;
    skos:altLabel "fixed axle gate",
        "fixed roller gate" ;
    skos:definition "A gate having wheels or rollers mounted on the end posts of the gate. The wheels bear against rails fixed in side grooves or gate guides." ;
    skos:inScheme ER-1110-2-1156: ;
    skos:prefLabel "Fixed wheel gate" .

ER-1110-2-1156:Flap_gate a wov:GlossaryTerm,
        skos:Concept ;
    rdfs:label "Flap gate" ;
    dcterms:bibliographicCitation "https://www.publications.usace.army.mil/Portals/76/Users/182/86/2486/er_1110-2-1156.pdf#page=506" ;
    pav:wasDerivedFrom "glossaries/CivilWorks/ER-1110-2-1156.yaml#term[Flap gate]" ;
    skos:definition "A gate hinged along one edge, usually either the top or bottom edge. Examples of bottom-hinged flap gates are tilting gates and fish belly gates so called from their shape in cross section." ;
    skos:inScheme ER-1110-2-1156: ;
    skos:prefLabel "Flap gate" .

ER-1110-2-1156:Flashboards a wov:GlossaryTerm,
        skos:Concept ;
    rdfs:label "Flashboards" ;
    dcterms:bibliographicCitation "https://www.publications.usace.army.mil/Portals/76/Users/182/86/2486/er_1110-2-1156.pdf#page=504" ;
    pav:wasDerivedFrom "glossaries/CivilWorks/ER-1110-2-1156.yaml#term[Flashboards]" ;
    skos:definition "Structural members of timber, concrete, or steel placed in channels or on the crest of a spillway to raise the reservoir water level but that may be quickly removed in the event of a flood." ;
    skos:inScheme ER-1110-2-1156: ;
    skos:prefLabel "Flashboards" .

ER-1110-2-1156:Flip_bucket a wov:GlossaryTerm,
        skos:Concept ;
    rdfs:label "Flip bucket" ;
    dcterms:bibliographicCitation "https://www.publications.usace.army.mil/Portals/76/Users/182/86/2486/er_1110-2-1156.pdf#page=504" ;
    pav:wasDerivedFrom "glossaries/CivilWorks/ER-1110-2-1156.yaml#term[Flip bucket]" ;
    skos:definition "An energy dissipater located at the downstream end of a spillway and shaped so that water flowing at a high velocity is deflected upwards in a trajectory away from the foundation of the spillway." ;
    skos:inScheme ER-1110-2-1156: ;
    skos:prefLabel "Flip bucket" .

ER-1110-2-1156:Flood a wov:GlossaryTerm,
        skos:Concept ;
    rdfs:label "Flood" ;
    dcterms:bibliographicCitation "https://www.publications.usace.army.mil/Portals/76/Users/182/86/2486/er_1110-2-1156.pdf#page=504" ;
    pav:wasDerivedFrom "glossaries/CivilWorks/ER-1110-2-1156.yaml#term[Flood]" ;
    skos:definition "A general and temporary condition of partial or complete inundation of two or more acres of normally dry land area or of two or more properties from: (1) overflow of inland or tidal waters; (2) unusual and rapid accumulation or runoff of surface waters from any source; (3) mudflow; or (4) collapse or subsidence of land along the shore of a lake or similar body of water as a result of erosion or undermining caused by waves or currents of water exceeding anticipated cyclical levels that result in a flood as defined above. The four terms below are used to further define flooding and efforts to prevent flooding." ;
    skos:inScheme ER-1110-2-1156: ;
    skos:prefLabel "Flood" .

<https://usace-data.com/civil-works/glossary/ER-1110-2-1156#Flood,_Inflow_Design_%28IDF%29> a wov:GlossaryTerm,
        skos:Concept ;
    rdfs:label "Flood, Inflow Design (IDF)" ;
    dcterms:bibliographicCitation "https://www.publications.usace.army.mil/Portals/76/Users/182/86/2486/er_1110-2-1156.pdf#page=505" ;
    pav:wasDerivedFrom "glossaries/CivilWorks/ER-1110-2-1156.yaml#term[Flood, Inflow Design (IDF)]" ;
    skos:altLabel "IDF" ;
    skos:definition "The flood used in the design of a dam and its appurtenant works particularly for sizing the spillway and outlet works, and for determining maximum temporary storage and height of dam requirements." ;
    skos:inScheme ER-1110-2-1156: ;
    skos:prefLabel "Flood, Inflow Design (IDF)" .

<https://usace-data.com/civil-works/glossary/ER-1110-2-1156#Flood,_Probable_Maximum_%28PMF%29> a wov:GlossaryTerm,
        skos:Concept ;
    rdfs:label "Flood, Probable Maximum (PMF)" ;
    dcterms:bibliographicCitation "https://www.publications.usace.army.mil/Portals/76/Users/182/86/2486/er_1110-2-1156.pdf#page=505" ;
    pav:wasDerivedFrom "glossaries/CivilWorks/ER-1110-2-1156.yaml#term[Flood, Probable Maximum (PMF)]" ;
    skos:altLabel "PMF" ;
    skos:definition "The most severe flood that is considered reasonably possible at a site as a result of meteorological and hydrologic conditions." ;
    skos:inScheme ER-1110-2-1156: ;
    skos:prefLabel "Flood, Probable Maximum (PMF)" .

<https://usace-data.com/civil-works/glossary/ER-1110-2-1156#Flood,_Safety_Evaluation_%28SEF%29> a wov:GlossaryTerm,
        skos:Concept ;
    rdfs:label "Flood, Safety Evaluation (SEF)" ;
    dcterms:bibliographicCitation "https://www.publications.usace.army.mil/Portals/76/Users/182/86/2486/er_1110-2-1156.pdf#page=505" ;
    pav:wasDerivedFrom "glossaries/CivilWorks/ER-1110-2-1156.yaml#term[Flood, Safety Evaluation (SEF)]" ;
    skos:altLabel "SEF" ;
    skos:definition "The largest flood for which the safety of a dam and appurtenant structure is to be evaluated." ;
    skos:inScheme ER-1110-2-1156: ;
    skos:prefLabel "Flood, Safety Evaluation (SEF)" .

<https://usace-data.com/civil-works/glossary/ER-1110-2-1156#Flood,_antecedent> a wov:GlossaryTerm,
        skos:Concept ;
    rdfs:label "Flood, antecedent" ;
    dcterms:bibliographicCitation "https://www.publications.usace.army.mil/Portals/76/Users/182/86/2486/er_1110-2-1156.pdf#page=505" ;
    pav:wasDerivedFrom "glossaries/CivilWorks/ER-1110-2-1156.yaml#term[Flood, antecedent]" ;
    skos:definition "A flood or series of floods assumed to occur prior to the occurrence of an inflow design flood." ;
    skos:inScheme ER-1110-2-1156: ;
    skos:prefLabel "Flood, antecedent" .

<https://usace-data.com/civil-works/glossary/ER-1110-2-1156#Flood,_base_safety_standard_%28BSS%29> a wov:GlossaryTerm,
        skos:Concept ;
    rdfs:label "Flood, base safety standard (BSS)" ;
    dcterms:bibliographicCitation "https://www.publications.usace.army.mil/Portals/76/Users/182/86/2486/er_1110-2-1156.pdf#page=505" ;
    pav:wasDerivedFrom "glossaries/CivilWorks/ER-1110-2-1156.yaml#term[Flood, base safety standard (BSS)]" ;
    skos:altLabel "BSS" ;
    skos:definition "The inflow design flood where there is no significant increase in adverse consequences from dam failure compared to non-failure adverse consequences." ;
    skos:inScheme ER-1110-2-1156: ;
    skos:prefLabel "Flood, base safety standard (BSS)" .

ER-1110-2-1156:Flood_Control a wov:GlossaryTerm,
        skos:Concept ;
    rdfs:label "Flood Control" ;
    dcterms:bibliographicCitation "https://www.publications.usace.army.mil/Portals/76/Users/182/86/2486/er_1110-2-1156.pdf#page=504" ;
    pav:wasDerivedFrom "glossaries/CivilWorks/ER-1110-2-1156.yaml#term[Flood Control]" ;
    skos:definition "The Flood Control Act of 1936 declared that flood control was a national priority since floods constituted a menace to the national welfare. This act authorized the construction of levees, floodwalls, channel improvements, and reservoirs to control flooding.Flood Control" ;
    skos:inScheme ER-1110-2-1156: ;
    skos:prefLabel "Flood Control" .

ER-1110-2-1156:Flood_Damage_Reduction a wov:GlossaryTerm,
        skos:Concept ;
    rdfs:label "Flood Damage Reduction" ;
    dcterms:bibliographicCitation "https://www.publications.usace.army.mil/Portals/76/Users/182/86/2486/er_1110-2-1156.pdf#page=504" ;
    pav:wasDerivedFrom "glossaries/CivilWorks/ER-1110-2-1156.yaml#term[Flood Damage Reduction]" ;
    skos:definition "The term flood damage reduction was adopted in recognition that the structures built for flood control only reduced the level of flooding and did not totally control all floods. Projects developed for flood damage reduction also include non-structural elements.Flood Damage Reduction" ;
    skos:inScheme ER-1110-2-1156: ;
    skos:prefLabel "Flood Damage Reduction" .

ER-1110-2-1156:Flood_Level a wov:GlossaryTerm,
        skos:Concept ;
    rdfs:label "Flood Level" ;
    dcterms:bibliographicCitation "https://www.publications.usace.army.mil/Portals/76/Users/182/86/2486/er_1110-2-1156.pdf#page=504" ;
    pav:wasDerivedFrom "glossaries/CivilWorks/ER-1110-2-1156.yaml#term[Flood Level]" ;
    skos:definition "The size of a flood may be expressed in terms of probability, of exceedance per year such as one percent chance flood or expressed as a fraction of the probable maximum flood or other reference flood.Flood Level" ;
    skos:inScheme ER-1110-2-1156: ;
    skos:prefLabel "Flood Level" .

ER-1110-2-1156:Flood_Risk_Management a wov:GlossaryTerm,
        skos:Concept ;
    rdfs:label "Flood Risk Management" ;
    dcterms:bibliographicCitation "https://www.publications.usace.army.mil/Portals/76/Users/182/86/2486/er_1110-2-1156.pdf#page=504" ;
    pav:wasDerivedFrom "glossaries/CivilWorks/ER-1110-2-1156.yaml#term[Flood Risk Management]" ;
    skos:definition "This term recognizes that there are different levels of risks in flood control works and in flood damage reduction activities. Since all flood management structures and other features have a risk of failure, the current practice is to seek to reduce the risk to a tolerable level that the public is willing to accept.Flood Risk Management" ;
    skos:inScheme ER-1110-2-1156: ;
    skos:prefLabel "Flood Risk Management" .

ER-1110-2-1156:Flood_gate a wov:GlossaryTerm,
        skos:Concept ;
    rdfs:label "Flood gate" ;
    dcterms:bibliographicCitation "https://www.publications.usace.army.mil/Portals/76/Users/182/86/2486/er_1110-2-1156.pdf#page=506" ;
    pav:wasDerivedFrom "glossaries/CivilWorks/ER-1110-2-1156.yaml#term[Flood gate]" ;
    skos:definition "A gate to control flood release from a reservoir." ;
    skos:inScheme ER-1110-2-1156: ;
    skos:prefLabel "Flood gate" .

ER-1110-2-1156:Flood_routing a wov:GlossaryTerm,
        skos:Concept ;
    rdfs:label "Flood routing" ;
    dcterms:bibliographicCitation "https://www.publications.usace.army.mil/Portals/76/Users/182/86/2486/er_1110-2-1156.pdf#page=505" ;
    pav:wasDerivedFrom "glossaries/CivilWorks/ER-1110-2-1156.yaml#term[Flood routing]" ;
    skos:definition "A process of determining progressively over time the amplitude of a flood wave as it moves past a dam or downstream to successive points along a river or stream." ;
    skos:inScheme ER-1110-2-1156: ;
    skos:prefLabel "Flood routing" .

ER-1110-2-1156:Flood_surcharge a wov:GlossaryTerm,
        skos:Concept ;
    rdfs:label "Flood surcharge" ;
    dcterms:bibliographicCitation "https://www.publications.usace.army.mil/Portals/76/Users/182/86/2486/er_1110-2-1156.pdf#page=523" ;
    pav:wasDerivedFrom "glossaries/CivilWorks/ER-1110-2-1156.yaml#term[Flood surcharge]" ;
    skos:definition "The storage volume between the top of the active storage and the design water level." ;
    skos:inScheme ER-1110-2-1156: ;
    skos:prefLabel "Flood surcharge" .

ER-1110-2-1156:Floodplain a wov:GlossaryTerm,
        skos:Concept ;
    rdfs:label "Floodplain" ;
    dcterms:bibliographicCitation "https://www.publications.usace.army.mil/Portals/76/Users/182/86/2486/er_1110-2-1156.pdf#page=505" ;
    pav:wasDerivedFrom "glossaries/CivilWorks/ER-1110-2-1156.yaml#term[Floodplain]" ;
    skos:definition "An area adjoining a body of water or natural stream that has been or may be covered by floodwater." ;
    skos:inScheme ER-1110-2-1156: ;
    skos:prefLabel "Floodplain" .

ER-1110-2-1156:Freeboard a wov:GlossaryTerm,
        skos:Concept ;
    rdfs:label "Freeboard" ;
    dcterms:bibliographicCitation "https://www.publications.usace.army.mil/Portals/76/Users/182/86/2486/er_1110-2-1156.pdf#page=505" ;
    pav:wasDerivedFrom "glossaries/CivilWorks/ER-1110-2-1156.yaml#term[Freeboard]" ;
    skos:definition "Vertical distance between the design water level and the top of dam." ;
    skos:inScheme ER-1110-2-1156: ;
    skos:prefLabel "Freeboard" .

ER-1110-2-1156:Full_pool a wov:GlossaryTerm,
        skos:Concept ;
    rdfs:label "Full pool" ;
    dcterms:bibliographicCitation "https://www.publications.usace.army.mil/Portals/76/Users/182/86/2486/er_1110-2-1156.pdf#page=505" ;
    pav:wasDerivedFrom "glossaries/CivilWorks/ER-1110-2-1156.yaml#term[Full pool]" ;
    skos:definition "The reservoir level that would be attained when the reservoir is fully utilized for all project purposes, including flood control." ;
    skos:inScheme ER-1110-2-1156: ;
    skos:prefLabel "Full pool" .

ER-1110-2-1156:Future_Without_Federal_Action_Condition a wov:GlossaryTerm,
        skos:Concept ;
    rdfs:label "Future Without Federal Action Condition" ;
    dcterms:bibliographicCitation "https://www.publications.usace.army.mil/Portals/76/Users/182/86/2486/er_1110-2-1156.pdf#page=505" ;
    pav:wasDerivedFrom "glossaries/CivilWorks/ER-1110-2-1156.yaml#term[Future Without Federal Action Condition]" ;
    skos:definition "The condition, data, or other representations of the topic of interest to be used for comparison of changes which may occur without intervention or as a result of a remediation alternative remediation. It is comprised of the existing conditions and such future projected conditions as chosen to be relevant for the comparison." ;
    skos:inScheme ER-1110-2-1156: ;
    skos:prefLabel "Future Without Federal Action Condition" .

ER-1110-2-1156:Gallery a wov:GlossaryTerm,
        skos:Concept ;
    rdfs:label "Gallery" ;
    dcterms:bibliographicCitation "https://www.publications.usace.army.mil/Portals/76/Users/182/86/2486/er_1110-2-1156.pdf#page=505" ;
    pav:wasDerivedFrom "glossaries/CivilWorks/ER-1110-2-1156.yaml#term[Gallery]" ;
    skos:definition "A passageway in the body of a dam used for inspection, foundation grouting, and/or drainage." ;
    skos:inScheme ER-1110-2-1156: ;
    skos:prefLabel "Gallery" .

ER-1110-2-1156:Gantry_crane a wov:GlossaryTerm,
        skos:Concept ;
    rdfs:label "Gantry crane" ;
    dcterms:bibliographicCitation "https://www.publications.usace.army.mil/Portals/76/Users/182/86/2486/er_1110-2-1156.pdf#page=505" ;
    pav:wasDerivedFrom "glossaries/CivilWorks/ER-1110-2-1156.yaml#term[Gantry crane]" ;
    skos:definition "A fixed or traveling bent-supported crane for handling heavy equipment." ;
    skos:inScheme ER-1110-2-1156: ;
    skos:prefLabel "Gantry crane" .

ER-1110-2-1156:Gate a wov:GlossaryTerm,
        skos:Concept ;
    rdfs:label "Gate" ;
    dcterms:bibliographicCitation "https://www.publications.usace.army.mil/Portals/76/Users/182/86/2486/er_1110-2-1156.pdf#page=506" ;
    pav:wasDerivedFrom "glossaries/CivilWorks/ER-1110-2-1156.yaml#term[Gate]" ;
    skos:definition "A movable, watertight barrier for the control of water in a waterway. Types of gate include the following:" ;
    skos:inScheme ER-1110-2-1156: ;
    skos:prefLabel "Gate" .

ER-1110-2-1156:Gate_chamber a wov:GlossaryTerm,
        skos:Concept ;
    rdfs:label "Gate chamber" ;
    dcterms:bibliographicCitation "https://www.publications.usace.army.mil/Portals/76/Users/182/86/2486/er_1110-2-1156.pdf#page=507" ;
    pav:wasDerivedFrom "glossaries/CivilWorks/ER-1110-2-1156.yaml#term[Gate chamber]" ;
    skos:definition "Also called valve chamber. A room from which a gate or valve can be operated, or sometimes in which the gate is located." ;
    skos:inScheme ER-1110-2-1156: ;
    skos:prefLabel "Gate chamber" .

ER-1110-2-1156:Geotextiles a wov:GlossaryTerm,
        skos:Concept ;
    rdfs:label "Geotextiles" ;
    dcterms:bibliographicCitation "https://www.publications.usace.army.mil/Portals/76/Users/182/86/2486/er_1110-2-1156.pdf#page=507" ;
    pav:wasDerivedFrom "glossaries/CivilWorks/ER-1110-2-1156.yaml#term[Geotextiles]" ;
    skos:definition "Any fabric or textile (natural or synthetic) when used as an engineering material in conjunction with soil, foundations, or rock. Geotextiles have the following uses: drainage, filtration, separation of materials, reinforcement, moisture barriers, and erosion protection." ;
    skos:inScheme ER-1110-2-1156: ;
    skos:prefLabel "Geotextiles" .

ER-1110-2-1156:Groin a wov:GlossaryTerm,
        skos:Concept ;
    rdfs:label "Groin" ;
    dcterms:bibliographicCitation "https://www.publications.usace.army.mil/Portals/76/Users/182/86/2486/er_1110-2-1156.pdf#page=507" ;
    pav:wasDerivedFrom "glossaries/CivilWorks/ER-1110-2-1156.yaml#term[Groin]" ;
    skos:definition "The area along the contact (or intersection) of the face of a dam with the abutments." ;
    skos:inScheme ER-1110-2-1156: ;
    skos:prefLabel "Groin" .

ER-1110-2-1156:Grout a wov:GlossaryTerm,
        skos:Concept ;
    rdfs:label "Grout" ;
    dcterms:bibliographicCitation "https://www.publications.usace.army.mil/Portals/76/Users/182/86/2486/er_1110-2-1156.pdf#page=507" ;
    pav:wasDerivedFrom "glossaries/CivilWorks/ER-1110-2-1156.yaml#term[Grout]" ;
    skos:definition "A fluidized material that is injected into soil, rock, concrete, or other construction material to seal openings and to lower the permeability and/or provide additional structural strength. There are four major types of grouting materials: chemical, cement, clay, and bitumen." ;
    skos:inScheme ER-1110-2-1156: ;
    skos:prefLabel "Grout" .

ER-1110-2-1156:Grout_blanket a wov:GlossaryTerm,
        skos:Concept ;
    rdfs:label "Grout blanket" ;
    dcterms:bibliographicCitation "https://www.publications.usace.army.mil/Portals/76/Users/182/86/2486/er_1110-2-1156.pdf#page=507" ;
    pav:wasDerivedFrom "glossaries/CivilWorks/ER-1110-2-1156.yaml#term[Grout blanket]" ;
    skos:definition "An area of the foundation systematically grouted to a uniform shallow depth." ;
    skos:inScheme ER-1110-2-1156: ;
    skos:prefLabel "Grout blanket" .

ER-1110-2-1156:Grout_cap a wov:GlossaryTerm,
        skos:Concept ;
    rdfs:label "Grout cap" ;
    dcterms:bibliographicCitation "https://www.publications.usace.army.mil/Portals/76/Users/182/86/2486/er_1110-2-1156.pdf#page=507" ;
    pav:wasDerivedFrom "glossaries/CivilWorks/ER-1110-2-1156.yaml#term[Grout cap]" ;
    skos:definition "A concrete pad constructed to facilitate subsequent pressure grouting of the grout curtain." ;
    skos:inScheme ER-1110-2-1156: ;
    skos:prefLabel "Grout cap" .

ER-1110-2-1156:Grout_curtain a wov:GlossaryTerm,
        skos:Concept ;
    rdfs:label "Grout curtain" ;
    dcterms:bibliographicCitation "https://www.publications.usace.army.mil/Portals/76/Users/182/86/2486/er_1110-2-1156.pdf#page=507" ;
    pav:wasDerivedFrom "glossaries/CivilWorks/ER-1110-2-1156.yaml#term[Grout curtain]" ;
    skos:definition "One or more zones, usually thin, in the foundation into which grout is injected to reduce seepage under or around a dam." ;
    skos:inScheme ER-1110-2-1156: ;
    skos:prefLabel "Grout curtain" .

ER-1110-2-1156:HAZUS a wov:GlossaryTerm,
        skos:Concept ;
    rdfs:label "HAZUS" ;
    dcterms:bibliographicCitation "https://www.publications.usace.army.mil/Portals/76/Users/182/86/2486/er_1110-2-1156.pdf#page=508" ;
    pav:wasDerivedFrom "glossaries/CivilWorks/ER-1110-2-1156.yaml#term[HAZUS]" ;
    skos:definition "A database and software system sponsored by the Federal Emergency Management Agency (FEMA) for performing a range of hazard analysis, including flood loss and impacts, for a variety of levels of detail regional wherein analysis supported by national databases; and site specific wherein local data be substituted for data that would come from national databases." ;
    skos:inScheme ER-1110-2-1156: ;
    skos:prefLabel "HAZUS" .

ER-1110-2-1156:Hazard a wov:GlossaryTerm,
        skos:Concept ;
    rdfs:label "Hazard" ;
    dcterms:bibliographicCitation "https://www.publications.usace.army.mil/Portals/76/Users/182/86/2486/er_1110-2-1156.pdf#page=507" ;
    pav:wasDerivedFrom "glossaries/CivilWorks/ER-1110-2-1156.yaml#term[Hazard]" ;
    skos:definition "Hazard is anything that is a potential source of harm to a valued asset (human, animal, natural, economic, social)." ;
    skos:inScheme ER-1110-2-1156: ;
    skos:prefLabel "Hazard" .

ER-1110-2-1156:Hazard_Characterization a wov:GlossaryTerm,
        skos:Concept ;
    rdfs:label "Hazard Characterization" ;
    dcterms:bibliographicCitation "https://www.publications.usace.army.mil/Portals/76/Users/182/86/2486/er_1110-2-1156.pdf#page=507" ;
    pav:wasDerivedFrom "glossaries/CivilWorks/ER-1110-2-1156.yaml#term[Hazard Characterization]" ;
    skos:definition "Hazard Characterization is the qualitative and/or quantitative evaluation of the nature of the adverse effects associated with the identified hazard(s), which may be present in the situation of interest." ;
    skos:inScheme ER-1110-2-1156: ;
    skos:prefLabel "Hazard Characterization" .

ER-1110-2-1156:Hazard_Identification a wov:GlossaryTerm,
        skos:Concept ;
    rdfs:label "Hazard Identification" ;
    dcterms:bibliographicCitation "https://www.publications.usace.army.mil/Portals/76/Users/182/86/2486/er_1110-2-1156.pdf#page=507" ;
    pav:wasDerivedFrom "glossaries/CivilWorks/ER-1110-2-1156.yaml#term[Hazard Identification]" ;
    skos:definition "Hazard Identification identifies all biological, chemical, social, economic, and physical agents or natural/anthropogenic events capable of causing adverse effects on people, property, economy, culture, social structure, or environment." ;
    skos:inScheme ER-1110-2-1156: ;
    skos:prefLabel "Hazard Identification" .

ER-1110-2-1156:Hazard_potential_classification a wov:GlossaryTerm,
        skos:Concept ;
    rdfs:label "Hazard potential classification" ;
    dcterms:bibliographicCitation "https://www.publications.usace.army.mil/Portals/76/Users/182/86/2486/er_1110-2-1156.pdf#page=507" ;
    pav:wasDerivedFrom "glossaries/CivilWorks/ER-1110-2-1156.yaml#term[Hazard potential classification]" ;
    skos:definition "The rating for a dam based on the potential consequences of failure. The rating is based on potential for loss of life and damage to property that failure of that dam could cause. Such classification is related to the amount of development downstream of a dam." ;
    skos:inScheme ER-1110-2-1156: ;
    skos:prefLabel "Hazard potential classification" .

<https://usace-data.com/civil-works/glossary/ER-1110-2-1156#Head,_static> a wov:GlossaryTerm,
        skos:Concept ;
    rdfs:label "Head, static" ;
    dcterms:bibliographicCitation "https://www.publications.usace.army.mil/Portals/76/Users/182/86/2486/er_1110-2-1156.pdf#page=508" ;
    pav:wasDerivedFrom "glossaries/CivilWorks/ER-1110-2-1156.yaml#term[Head, static]" ;
    skos:definition "The vertical distance between two points in a fluid." ;
    skos:inScheme ER-1110-2-1156: ;
    skos:prefLabel "Head, static" .

<https://usace-data.com/civil-works/glossary/ER-1110-2-1156#Head,_velocity> a wov:GlossaryTerm,
        skos:Concept ;
    rdfs:label "Head, velocity" ;
    dcterms:bibliographicCitation "https://www.publications.usace.army.mil/Portals/76/Users/182/86/2486/er_1110-2-1156.pdf#page=508" ;
    pav:wasDerivedFrom "glossaries/CivilWorks/ER-1110-2-1156.yaml#term[Head, velocity]" ;
    skos:definition "The vertical distance that would statically result from the velocity of a moving fluid." ;
    skos:inScheme ER-1110-2-1156: ;
    skos:prefLabel "Head, velocity" .

ER-1110-2-1156:Headrace a wov:GlossaryTerm,
        skos:Concept ;
    rdfs:label "Headrace" ;
    dcterms:bibliographicCitation "https://www.publications.usace.army.mil/Portals/76/Users/182/86/2486/er_1110-2-1156.pdf#page=508" ;
    pav:wasDerivedFrom "glossaries/CivilWorks/ER-1110-2-1156.yaml#term[Headrace]" ;
    skos:definition "A free-flow tunnel or open channel that conveys water to the upper end of a penstock; hence, the terms 'headrace tunnel' and 'headrace canal'." ;
    skos:inScheme ER-1110-2-1156: ;
    skos:prefLabel "Headrace" .

ER-1110-2-1156:Heel a wov:GlossaryTerm,
        skos:Concept ;
    rdfs:label "Heel" ;
    dcterms:bibliographicCitation "https://www.publications.usace.army.mil/Portals/76/Users/182/86/2486/er_1110-2-1156.pdf#page=508" ;
    pav:wasDerivedFrom "glossaries/CivilWorks/ER-1110-2-1156.yaml#term[Heel]" ;
    skos:definition "The junction of the upstream face of a gravity or arch dam with the ground surface. For an embankment dam the junction is referred to as the upstream toe of the dam." ;
    skos:inScheme ER-1110-2-1156: ;
    skos:prefLabel "Heel" .

<https://usace-data.com/civil-works/glossary/ER-1110-2-1156#Height,_above_ground> a wov:GlossaryTerm,
        skos:Concept ;
    rdfs:label "Height, above ground" ;
    dcterms:bibliographicCitation "https://www.publications.usace.army.mil/Portals/76/Users/182/86/2486/er_1110-2-1156.pdf#page=508" ;
    pav:wasDerivedFrom "glossaries/CivilWorks/ER-1110-2-1156.yaml#term[Height, above ground]" ;
    skos:definition "The maximum height from natural ground surface to the top of a dam." ;
    skos:inScheme ER-1110-2-1156: ;
    skos:prefLabel "Height, above ground" .

<https://usace-data.com/civil-works/glossary/ER-1110-2-1156#Height,_dam> a wov:GlossaryTerm,
        skos:Concept ;
    rdfs:label "Height, dam" ;
    dcterms:bibliographicCitation "https://www.publications.usace.army.mil/Portals/76/Users/182/86/2486/er_1110-2-1156.pdf#page=508" ;
    pav:wasDerivedFrom "glossaries/CivilWorks/ER-1110-2-1156.yaml#term[Height, dam]" ;
    skos:definition "The dam height is the vertical distance between the lowest point on the crest of the dam and the lowest point in the original streambed." ;
    skos:inScheme ER-1110-2-1156: ;
    skos:prefLabel "Height, dam" .

<https://usace-data.com/civil-works/glossary/ER-1110-2-1156#Height,_hydraulic> a wov:GlossaryTerm,
        skos:Concept ;
    rdfs:label "Height, hydraulic" ;
    dcterms:bibliographicCitation "https://www.publications.usace.army.mil/Portals/76/Users/182/86/2486/er_1110-2-1156.pdf#page=508" ;
    pav:wasDerivedFrom "glossaries/CivilWorks/ER-1110-2-1156.yaml#term[Height, hydraulic]" ;
    skos:definition "The vertical difference between the maximum design water level and the lowest point in the original streambed." ;
    skos:inScheme ER-1110-2-1156: ;
    skos:prefLabel "Height, hydraulic" .

<https://usace-data.com/civil-works/glossary/ER-1110-2-1156#Height,_structural> a wov:GlossaryTerm,
        skos:Concept ;
    rdfs:label "Height, structural" ;
    dcterms:bibliographicCitation "https://www.publications.usace.army.mil/Portals/76/Users/182/86/2486/er_1110-2-1156.pdf#page=508" ;
    pav:wasDerivedFrom "glossaries/CivilWorks/ER-1110-2-1156.yaml#term[Height, structural]" ;
    skos:definition "The vertical distance between the lowest point of the excavated foundation to the top of the dam." ;
    skos:inScheme ER-1110-2-1156: ;
    skos:prefLabel "Height, structural" .

ER-1110-2-1156:Hollow_jet_valve a wov:GlossaryTerm,
        skos:Concept ;
    rdfs:label "Hollow jet valve" ;
    dcterms:bibliographicCitation "https://www.publications.usace.army.mil/Portals/76/Users/182/86/2486/er_1110-2-1156.pdf#page=525" ;
    pav:wasDerivedFrom "glossaries/CivilWorks/ER-1110-2-1156.yaml#term[Hollow jet valve]" ;
    skos:definition "A device for regulating high-pressure outlets. Essentially, it is half a needle valve in which the needle closure member moves upstream toward the inlet end of the valve to shut off flow. As there is no convergence at the outlet end, the flow emerges in the form of an annular cylinder, segmented by several splitter ribs for admitting air into the jet interior to prevent jet instability." ;
    skos:inScheme ER-1110-2-1156: ;
    skos:prefLabel "Hollow jet valve" .

ER-1110-2-1156:Inactive_storage a wov:GlossaryTerm,
        skos:Concept ;
    rdfs:label "Inactive storage" ;
    dcterms:bibliographicCitation "https://www.publications.usace.army.mil/Portals/76/Users/182/86/2486/er_1110-2-1156.pdf#page=523" ;
    pav:wasDerivedFrom "glossaries/CivilWorks/ER-1110-2-1156.yaml#term[Inactive storage]" ;
    skos:definition "The storage volume of a reservoir between the crest of the invert of the lowest outlet and the minimum operating level." ;
    skos:inScheme ER-1110-2-1156: ;
    skos:prefLabel "Inactive storage" .

ER-1110-2-1156:Incident a wov:GlossaryTerm,
        skos:Concept ;
    rdfs:label "Incident" ;
    dcterms:bibliographicCitation "https://www.publications.usace.army.mil/Portals/76/Users/182/86/2486/er_1110-2-1156.pdf#page=508" ;
    pav:wasDerivedFrom "glossaries/CivilWorks/ER-1110-2-1156.yaml#term[Incident]" ;
    skos:definition "An event occurrence at a dam that could potentially result in a dam safety issue, such as a spillway flood, seismic event, gate operation failure, etc. that should be documented and trigger an investigation." ;
    skos:inScheme ER-1110-2-1156: ;
    skos:prefLabel "Incident" .

ER-1110-2-1156:Inclinometer a wov:GlossaryTerm,
        skos:Concept ;
    rdfs:label "Inclinometer" ;
    dcterms:bibliographicCitation "https://www.publications.usace.army.mil/Portals/76/Users/182/86/2486/er_1110-2-1156.pdf#page=508" ;
    pav:wasDerivedFrom "glossaries/CivilWorks/ER-1110-2-1156.yaml#term[Inclinometer]" ;
    skos:definition "An instrument, usually consisting of a metal or plastic tube inserted in a drill hole and a sensitized monitor either lowered into the tube or fixed within the tube. This measures at different points the tube's inclination to the vertical. By integration, the lateral position at different Levels of the tube may be found relative to a point, usually the top or bottom of the tube, assumed to be fixed. The system may be used to measure settlement during embankment construction (Bartholomew, Murray, and Goins 1987). A reference benchmark is used to establish the top of the inclinometer casing. The instrument probe is lowered to each slip joint in the casing, and the depth to each joint is read directly off the tape. Settlement measurements are made as each section of casing is added during embankment construction." ;
    skos:inScheme ER-1110-2-1156: ;
    skos:prefLabel "Inclinometer" .

ER-1110-2-1156:Incremental_consequences a wov:GlossaryTerm,
        skos:Concept ;
    rdfs:label "Incremental consequences" ;
    dcterms:bibliographicCitation "https://www.publications.usace.army.mil/Portals/76/Users/182/86/2486/er_1110-2-1156.pdf#page=509" ;
    pav:wasDerivedFrom "glossaries/CivilWorks/ER-1110-2-1156.yaml#term[Incremental consequences]" ;
    skos:definition "Incremental consequences are associated with a failure of the project to provide the planned level of public protection plus any additional risk created by the project due to dam failure. Incremental consequences = (Consequences associated with the estimated performance of the project including failure) - (Consequence associated with the estimated performance of the project hypothetically without failure)." ;
    skos:inScheme ER-1110-2-1156: ;
    skos:prefLabel "Incremental consequences" .

ER-1110-2-1156:Independent_External_Peer_Review_Team a wov:GlossaryTerm,
        skos:Concept ;
    rdfs:label "Independent External Peer Review Team" ;
    dcterms:bibliographicCitation "https://www.publications.usace.army.mil/Portals/76/Users/182/86/2486/er_1110-2-1156.pdf#page=509" ;
    pav:wasDerivedFrom "glossaries/CivilWorks/ER-1110-2-1156.yaml#term[Independent External Peer Review Team]" ;
    skos:definition "A team of experts selected in accordance with Section 2034 and/ Section 2035 of the Water Resources Development Act of 2007 (Public Law 110-114) to review proposed Civil Works projects and projects under construction." ;
    skos:inScheme ER-1110-2-1156: ;
    skos:prefLabel "Independent External Peer Review Team" .

ER-1110-2-1156:Independent_Technical_Review_%28ITR%29 a wov:GlossaryTerm,
        skos:Concept ;
    rdfs:label "Independent Technical Review (ITR)" ;
    dcterms:bibliographicCitation "https://www.publications.usace.army.mil/Portals/76/Users/182/86/2486/er_1110-2-1156.pdf#page=509" ;
    pav:wasDerivedFrom "glossaries/CivilWorks/ER-1110-2-1156.yaml#term[Independent Technical Review (ITR)]" ;
    skos:altLabel "ITR" ;
    skos:definition "A comprehensive independent review of a technical product (design and construction documents). .The ITR was replaced by an ATR level of review in 2009." ;
    skos:inScheme ER-1110-2-1156: ;
    skos:prefLabel "Independent Technical Review (ITR)" .

ER-1110-2-1156:Indirect_Economic_Impacts a wov:GlossaryTerm,
        skos:Concept ;
    rdfs:label "Indirect Economic Impacts" ;
    dcterms:bibliographicCitation "https://www.publications.usace.army.mil/Portals/76/Users/182/86/2486/er_1110-2-1156.pdf#page=509" ;
    pav:wasDerivedFrom "glossaries/CivilWorks/ER-1110-2-1156.yaml#term[Indirect Economic Impacts]" ;
    skos:definition "Impacts associated with the destruction of property and the displacement of people due to the failure. The destruction due to the failure flood can have significant impacts on the local and regional economy as businesses at least temporarily close resulting in loss of employment and income. Similarly, economic activity linked to the services provided by the dam will also have consequences. All these indirect losses then have ripple or multiplier effects in the rest of the regional and national economy due to the resulting reduction in spending on goods and services in the region. These losses are the increment to flood losses above those that would have would have occurred had the dam not failed." ;
    skos:inScheme ER-1110-2-1156: ;
    skos:prefLabel "Indirect Economic Impacts" .

ER-1110-2-1156:Individual_Risk a wov:GlossaryTerm,
        skos:Concept ;
    rdfs:label "Individual Risk" ;
    dcterms:bibliographicCitation "https://www.publications.usace.army.mil/Portals/76/Users/182/86/2486/er_1110-2-1156.pdf#page=509" ;
    pav:wasDerivedFrom "glossaries/CivilWorks/ER-1110-2-1156.yaml#term[Individual Risk]" ;
    skos:definition "The increment of risk imposed on a particular individual by the existence of a hazardous facility. This increment of risk is an addition to the background risk to life, which the person would live with on a daily basis if the facility did not exist. (ANCOLD October 2003) (reference A.130)." ;
    skos:inScheme ER-1110-2-1156: ;
    skos:prefLabel "Individual Risk" .

ER-1110-2-1156:Individual_incremental_life_safety_tolerable_risk_guideline_%28ANCOLD%29 a wov:GlossaryTerm,
        skos:Concept ;
    rdfs:label "Individual incremental life safety tolerable risk guideline (ANCOLD)" ;
    dcterms:bibliographicCitation "https://www.publications.usace.army.mil/Portals/76/Users/182/86/2486/er_1110-2-1156.pdf#page=509" ;
    pav:wasDerivedFrom "glossaries/CivilWorks/ER-1110-2-1156.yaml#term[Individual incremental life safety tolerable risk guideline (ANCOLD)]" ;
    skos:altLabel "ANCOLD" ;
    skos:definition "For existing dams, the individual risk to the person or group, which is most at risk, should be less than a limit value of 1 in 10,000 per year, except in extraordinary circumstances, following the ANCOLD (2003) (reference A.130) individual life safety risk guideline. For new dams or major augmentations , the individual risk to the person or group, which is most at risk, should be less than a limit value of 1 in 100,000 per year, except in extraordinary circumstances, following the ANCOLD (2003) (reference A.130) individual life safety risk guideline. In the case of existing dams and new dams or major augmentations, individual risks are to be lower than the limit values to an extent determined in accordance with the ALARP principle." ;
    skos:inScheme ER-1110-2-1156: ;
    skos:prefLabel "Individual incremental life safety tolerable risk guideline (ANCOLD)" .

ER-1110-2-1156:Initial_reservoir_filling a wov:GlossaryTerm,
        skos:Concept ;
    rdfs:label "Initial reservoir filling" ;
    dcterms:bibliographicCitation "https://www.publications.usace.army.mil/Portals/76/Users/182/86/2486/er_1110-2-1156.pdf#page=509" ;
    pav:wasDerivedFrom "glossaries/CivilWorks/ER-1110-2-1156.yaml#term[Initial reservoir filling]" ;
    skos:definition "A deliberate impoundment to meet project purposes (a continuing process as successively higher pools are attained for flood control projects)." ;
    skos:inScheme ER-1110-2-1156: ;
    skos:prefLabel "Initial reservoir filling" .

ER-1110-2-1156:Institute_for_Water_Resources a wov:GlossaryTerm,
        skos:Concept ;
    rdfs:label "Institute for Water Resources" ;
    dcterms:bibliographicCitation "https://www.publications.usace.army.mil/Portals/76/Users/182/86/2486/er_1110-2-1156.pdf#page=510" ;
    pav:wasDerivedFrom "glossaries/CivilWorks/ER-1110-2-1156.yaml#term[Institute for Water Resources]" ;
    skos:definition "The U.S. Army Engineer Institute for Water Resources (IWR) was formed to provide forward-looking analysis and research in developing planning methodologies to aid the Civil Works program. Since its beginnings in 1969, the Institute was envisioned to provide USACE with long-range planning capabilities to assist in improving the civil works planning process. Today the Institute continues to provide the Civil Works program with a variety of products to enhance the U.S. Army Engineer Institute for Water Resources development planning. IWR is comprised of several semi-independent Centers, and a senior staff of planning and policy experts. See http://www.iwr.usace.army.mil." ;
    skos:inScheme ER-1110-2-1156: ;
    skos:prefLabel "Institute for Water Resources" .

ER-1110-2-1156:Instrumentation a wov:GlossaryTerm,
        skos:Concept ;
    rdfs:label "Instrumentation" ;
    dcterms:bibliographicCitation "https://www.publications.usace.army.mil/Portals/76/Users/182/86/2486/er_1110-2-1156.pdf#page=510" ;
    pav:wasDerivedFrom "glossaries/CivilWorks/ER-1110-2-1156.yaml#term[Instrumentation]" ;
    skos:definition "An arrangement of devices installed into or near dams (i.e., piezometers, inclinometers, strain gages, measurement points, etc.), which provide for measurements that can be used to evaluate the structural behavior and performance parameters of the structure." ;
    skos:inScheme ER-1110-2-1156: ;
    skos:prefLabel "Instrumentation" .

ER-1110-2-1156:Intake a wov:GlossaryTerm,
        skos:Concept ;
    rdfs:label "Intake" ;
    dcterms:bibliographicCitation "https://www.publications.usace.army.mil/Portals/76/Users/182/86/2486/er_1110-2-1156.pdf#page=510" ;
    pav:wasDerivedFrom "glossaries/CivilWorks/ER-1110-2-1156.yaml#term[Intake]" ;
    skos:definition "Any structure in a reservoir, dam, or river through which water can be discharged. Placed at the beginning of an outlet-works waterway (power conduit, water supply conduit), the intake establishes the ultimate drawdown level of the reservoir by the position and size of its opening(s) to the outlet works. The intake may be vertical or inclined towers, drop inlets, or submerged, box-shaped structures." ;
    skos:inScheme ER-1110-2-1156: ;
    skos:prefLabel "Intake" .

ER-1110-2-1156:Intangible_Consequences a wov:GlossaryTerm,
        skos:Concept ;
    rdfs:label "Intangible Consequences" ;
    dcterms:bibliographicCitation "https://www.publications.usace.army.mil/Portals/76/Users/182/86/2486/er_1110-2-1156.pdf#page=510" ;
    pav:wasDerivedFrom "glossaries/CivilWorks/ER-1110-2-1156.yaml#term[Intangible Consequences]" ;
    skos:definition "These are consequences that have no directly observable physical dimensions but exist in the minds, individually and collectively, of those affected. Such consequences are real and can support decisions. Intangible consequences identified in ANCOLD (2003) (reference A.130) include such things as: the grief and loss suffered by relatives and friends of those who die; the impact of multiple deaths on the psyche of the community in which they lived; the stress involved in arranging alternative accommodations and income; the sense of loss by those who enjoyed the natural landscape destroyed; and the fear of lost status and reputation of the dam owning organization and its technical staff (see discussion at paragraph 5.3.10.3 and ANCOLD (2003) (reference A-130). The affect of these intangible consequences can be observed more tangibly in terms of increased mental health expenditures and increased suicides." ;
    skos:inScheme ER-1110-2-1156: ;
    skos:prefLabel "Intangible Consequences" .

ER-1110-2-1156:Interagency_Committee_on_Dam_Safety a wov:GlossaryTerm,
        skos:Concept ;
    rdfs:label "Interagency Committee on Dam Safety" ;
    dcterms:bibliographicCitation "https://www.publications.usace.army.mil/Portals/76/Users/182/86/2486/er_1110-2-1156.pdf#page=510" ;
    pav:wasDerivedFrom "glossaries/CivilWorks/ER-1110-2-1156.yaml#term[Interagency Committee on Dam Safety]" ;
    skos:definition "The Interagency Committee on Dam Safety (ICODS) is comprised of a representative of each of the Department of Agriculture, the Department of Defense, the Department of Energy, the Department of the Interior, the Department of Labor, the Federal Emergency Management Agency, the Federal Energy Regulatory Commission, the Nuclear Regulatory Commission, the Tennessee Valley Authority, and the United States Section of the International Boundary Commission. ICODS encourages the establishment and maintenance of effective Federal programs, policies, and guidelines intended to enhance dam safety for the protection of human life and property through coordination and information exchange among Federal agencies concerning implementation of the Federal Guidelines for Dam Safety (reference A.114)." ;
    skos:inScheme ER-1110-2-1156: ;
    skos:prefLabel "Interagency Committee on Dam Safety" .

ER-1110-2-1156:Interim_Risk_Reduction_Measure_%28IRRM%29 a wov:GlossaryTerm,
        skos:Concept ;
    rdfs:label "Interim Risk Reduction Measure (IRRM)" ;
    dcterms:bibliographicCitation "https://www.publications.usace.army.mil/Portals/76/Users/182/86/2486/er_1110-2-1156.pdf#page=511" ;
    pav:wasDerivedFrom "glossaries/CivilWorks/ER-1110-2-1156.yaml#term[Interim Risk Reduction Measure (IRRM)]" ;
    skos:altLabel "IRRM" ;
    skos:definition "Dam Safety Risk Reduction Measures that are to be formulated and undertaken for dams that are not considered to be tolerably safe and are intended as interim until more permanent remediation measures are implemented. Increased monitoring and reservoir restrictions are examples of interim measures that can be taken at a project." ;
    skos:inScheme ER-1110-2-1156: ;
    skos:prefLabel "Interim Risk Reduction Measure (IRRM)" .

ER-1110-2-1156:Interim_Risk_Reduction_Measures_Plans_%28IRRMP%29 a wov:GlossaryTerm,
        skos:Concept ;
    rdfs:label "Interim Risk Reduction Measures Plans (IRRMP)" ;
    dcterms:bibliographicCitation "https://www.publications.usace.army.mil/Portals/76/Users/182/86/2486/er_1110-2-1156.pdf#page=511" ;
    pav:wasDerivedFrom "glossaries/CivilWorks/ER-1110-2-1156.yaml#term[Interim Risk Reduction Measures Plans (IRRMP)]" ;
    skos:altLabel "IRRMP" ;
    skos:definition "Plans prepared by the districts for all DSAC Class I, 2, and 3 dams. The urgency of submittal corresponds to the DSAC Class. In general, the plans will describe the project and area, dam safety issues, failure modes and analysis, interim risk reduction plans, consequences with and without the plan, schedule, cost, coordination and review documentation, updated emergency action plan, and communications plan." ;
    skos:inScheme ER-1110-2-1156: ;
    skos:prefLabel "Interim Risk Reduction Measures Plans (IRRMP)" .

ER-1110-2-1156:Interlock a wov:GlossaryTerm,
        skos:Concept ;
    rdfs:label "Interlock" ;
    dcterms:bibliographicCitation "https://www.publications.usace.army.mil/Portals/76/Users/182/86/2486/er_1110-2-1156.pdf#page=511" ;
    pav:wasDerivedFrom "glossaries/CivilWorks/ER-1110-2-1156.yaml#term[Interlock]" ;
    skos:definition "A device for preventing a mechanism from being set in motion when another mechanism is in such a position that the two operating simultaneously might produce undesirable results." ;
    skos:inScheme ER-1110-2-1156: ;
    skos:prefLabel "Interlock" .

ER-1110-2-1156:Internal_Erosion a wov:GlossaryTerm,
        skos:Concept ;
    rdfs:label "Internal Erosion" ;
    dcterms:bibliographicCitation "https://www.publications.usace.army.mil/Portals/76/Users/182/86/2486/er_1110-2-1156.pdf#page=511" ;
    pav:wasDerivedFrom "glossaries/CivilWorks/ER-1110-2-1156.yaml#term[Internal Erosion]" ;
    skos:definition "Internal erosion development leading to dam failure can be represented by four phases: initiation, continuation, progression, and breach.Internal Erosion: Removal of soil particles within an embankment dam or its foundation by seepage or leakage" ;
    skos:inScheme ER-1110-2-1156: ;
    skos:prefLabel "Internal Erosion" .

ER-1110-2-1156:Intervention a wov:GlossaryTerm,
        skos:Concept ;
    rdfs:label "Intervention" ;
    dcterms:bibliographicCitation "https://www.publications.usace.army.mil/Portals/76/Users/182/86/2486/er_1110-2-1156.pdf#page=511" ;
    pav:wasDerivedFrom "glossaries/CivilWorks/ER-1110-2-1156.yaml#term[Intervention]" ;
    skos:definition "An action taken during the sequence of any failure mechanism either when failure has been initiated or later to prevent or delay completion of failure progression." ;
    skos:inScheme ER-1110-2-1156: ;
    skos:prefLabel "Intervention" .

ER-1110-2-1156:Inundation_map a wov:GlossaryTerm,
        skos:Concept ;
    rdfs:label "Inundation map" ;
    dcterms:bibliographicCitation "https://www.publications.usace.army.mil/Portals/76/Users/182/86/2486/er_1110-2-1156.pdf#page=511" ;
    pav:wasDerivedFrom "glossaries/CivilWorks/ER-1110-2-1156.yaml#term[Inundation map]" ;
    skos:definition "Inundation Map: A map showing either the actual or predicted extent of flood water within a study area for future pre-determined flood events, ongoing flood events, or past flood events. For dams, a map showing the predicted extent of inundation from controlled or uncontrolled reservoir releases for a pre-determined event scenario or scenarios. Releases may be a result of normal reservoir operation, a result of structural failure or a result of misoperation. An example of a controlled release is flood-inducing spillway discharge. An example of an uncontrolled release is overtopping and/or structural failure. For levees, a map showing the predicted extent of leveed area inundation due to breach of the levee system prior to or during overtopping, levee overtopping without breach, or misoperation of a levee system component for a pre-determined event scenario. An inundation map is sometimes referred to as a flood inundation map. The policy on release of inundation maps is provided in EC 1165-2- 215 (reference A.97)." ;
    skos:inScheme ER-1110-2-1156: ;
    skos:prefLabel "Inundation map" .

ER-1110-2-1156:Issue_Evaluation_Studies a wov:GlossaryTerm,
        skos:Concept ;
    rdfs:label "Issue Evaluation Studies" ;
    dcterms:bibliographicCitation "https://www.publications.usace.army.mil/Portals/76/Users/182/86/2486/er_1110-2-1156.pdf#page=511" ;
    pav:wasDerivedFrom "glossaries/CivilWorks/ER-1110-2-1156.yaml#term[Issue Evaluation Studies]" ;
    skos:definition "Issue Evaluation studies for dams classified in DSAC Classes 2, 3, and 4 are studies to better determine the nature of the dam safety issue and the degree of urgency for action within the context of the full USACE inventory of dams. The intent of an Issue Evaluation Study is to perform a more robust and detailed level of risk assessment, than used in the SPRA that will enable informed decisions about the need for further investigations, the DSAC classification, and interim risk reduction measures implementation. However the level of detail should only be what is needed to justify the decision to pursue or not to pursue a dam safety modification study." ;
    skos:inScheme ER-1110-2-1156: ;
    skos:prefLabel "Issue Evaluation Studies" .

ER-1110-2-1156:Lead_Engineer a wov:GlossaryTerm,
        skos:Concept ;
    rdfs:label "Lead Engineer" ;
    dcterms:bibliographicCitation "https://www.publications.usace.army.mil/Portals/76/Users/182/86/2486/er_1110-2-1156.pdf#page=512" ;
    pav:wasDerivedFrom "glossaries/CivilWorks/ER-1110-2-1156.yaml#term[Lead Engineer]" ;
    skos:definition "A registered professional engineer (typically a civil, geotechnical, or structural engineer) or engineering geologist qualified through appropriate technical training and experience, assigned the responsibility to lead the technical team members of a product delivery team. The engineering geologist is required to be a registered professional engineer. The lead engineer is responsible for working closely with the Project Manager and insuring that all technical requirements are addressed in the Project Management Plan (PMP). The lead engineer insure that the necessary field investigations are completed during the study and design phases; that plans and specifications are reviewed; that the technical comments on the design are properly addressed; and that engineers on the PDT visit the project during the construction phase. When possible the same individual should function as the lead engineer from the start of the studies until the completion of the project. (See Dam Safety Modification Lead Engineer definition for dam safety modification projects.)" ;
    skos:inScheme ER-1110-2-1156: ;
    skos:prefLabel "Lead Engineer" .

ER-1110-2-1156:Leakage a wov:GlossaryTerm,
        skos:Concept ;
    rdfs:label "Leakage" ;
    dcterms:bibliographicCitation "https://www.publications.usace.army.mil/Portals/76/Users/182/86/2486/er_1110-2-1156.pdf#page=512" ;
    pav:wasDerivedFrom "glossaries/CivilWorks/ER-1110-2-1156.yaml#term[Leakage]" ;
    skos:definition "Concentrated flow through preferential paths (e.g., crack in cohesive soil, open rock defect)." ;
    skos:inScheme ER-1110-2-1156: ;
    skos:prefLabel "Leakage" .

ER-1110-2-1156:Length_of_dam a wov:GlossaryTerm,
        skos:Concept ;
    rdfs:label "Length of dam" ;
    dcterms:bibliographicCitation "https://www.publications.usace.army.mil/Portals/76/Users/182/86/2486/er_1110-2-1156.pdf#page=512" ;
    pav:wasDerivedFrom "glossaries/CivilWorks/ER-1110-2-1156.yaml#term[Length of dam]" ;
    skos:definition "The length along the top of the dam. This also includes the spillway, power plant, navigation lock, fish pass, etc., where these form part of the length of the dam. If detached from the dam these structures should not be included." ;
    skos:inScheme ER-1110-2-1156: ;
    skos:prefLabel "Length of dam" .

ER-1110-2-1156:Levee a wov:GlossaryTerm,
        skos:Concept ;
    rdfs:label "Levee" ;
    dcterms:bibliographicCitation "https://www.publications.usace.army.mil/Portals/76/Users/182/86/2486/er_1110-2-1156.pdf#page=512" ;
    pav:wasDerivedFrom "glossaries/CivilWorks/ER-1110-2-1156.yaml#term[Levee]" ;
    skos:definition "An embankment whose primary purpose is to furnish flood protection from seasonal high water. Embankments that are subject to water loading for prolonged periods or permanently should be designed in accordance with earth dam criteria." ;
    skos:inScheme ER-1110-2-1156: ;
    skos:prefLabel "Levee" .

ER-1110-2-1156:Life_Loss_Consequences a wov:GlossaryTerm,
        skos:Concept ;
    rdfs:label "Life Loss Consequences" ;
    dcterms:bibliographicCitation "https://www.publications.usace.army.mil/Portals/76/Users/182/86/2486/er_1110-2-1156.pdf#page=512" ;
    pav:wasDerivedFrom "glossaries/CivilWorks/ER-1110-2-1156.yaml#term[Life Loss Consequences]" ;
    skos:definition "This includes the determination of the population at risk, threaten population, and the estimated potential loss of life." ;
    skos:inScheme ER-1110-2-1156: ;
    skos:prefLabel "Life Loss Consequences" .

ER-1110-2-1156:Life_Loss_Estimates a wov:GlossaryTerm,
        skos:Concept ;
    rdfs:label "Life Loss Estimates" ;
    dcterms:bibliographicCitation "https://www.publications.usace.army.mil/Portals/76/Users/182/86/2486/er_1110-2-1156.pdf#page=512" ;
    pav:wasDerivedFrom "glossaries/CivilWorks/ER-1110-2-1156.yaml#term[Life Loss Estimates]" ;
    skos:definition "Estimate of potential life loss using approved life loss estimating methodology. May be for individual failure modes, or combined for a set of potential failure modes for specified loading scenario(s)." ;
    skos:inScheme ER-1110-2-1156: ;
    skos:prefLabel "Life Loss Estimates" .

ER-1110-2-1156:Life_Safety_Tolerable_Risk_Guidelines a wov:GlossaryTerm,
        skos:Concept ;
    rdfs:label "Life Safety Tolerable Risk Guidelines" ;
    dcterms:bibliographicCitation "https://www.publications.usace.army.mil/Portals/76/Users/182/86/2486/er_1110-2-1156.pdf#page=512" ;
    pav:wasDerivedFrom "glossaries/CivilWorks/ER-1110-2-1156.yaml#term[Life Safety Tolerable Risk Guidelines]" ;
    skos:definition "Three types of life safety tolerable risk guidelines will be used under the USACE tolerable risk guidelines. Individual incremental life safety risk using probability of life loss and Societal incremental life safety risk express in two different ways - Probability distribution of potential life loss (F- Nchart);andthef-NÌ… withaverageannualLifeLoss(AALL)." ;
    skos:inScheme ER-1110-2-1156: ;
    skos:prefLabel "Life Safety Tolerable Risk Guidelines" .

ER-1110-2-1156:Lifeline_Systems a wov:GlossaryTerm,
        skos:Concept ;
    rdfs:label "Lifeline Systems" ;
    dcterms:bibliographicCitation "https://www.publications.usace.army.mil/Portals/76/Users/182/86/2486/er_1110-2-1156.pdf#page=513" ;
    pav:wasDerivedFrom "glossaries/CivilWorks/ER-1110-2-1156.yaml#term[Lifeline Systems]" ;
    skos:definition "Public works and utilities such as electrical power, gas and liquid fuels, telecommunications, transportation, and water and sewer systems." ;
    skos:inScheme ER-1110-2-1156: ;
    skos:prefLabel "Lifeline Systems" .

ER-1110-2-1156:Lifelines a wov:GlossaryTerm,
        skos:Concept ;
    rdfs:label "Lifelines" ;
    dcterms:bibliographicCitation "https://www.publications.usace.army.mil/Portals/76/Users/182/86/2486/er_1110-2-1156.pdf#page=513" ;
    pav:wasDerivedFrom "glossaries/CivilWorks/ER-1110-2-1156.yaml#term[Lifelines]" ;
    skos:definition "The public facilities and systems that provide basic life support services such as water, energy, sanitation, communications and transportation." ;
    skos:inScheme ER-1110-2-1156: ;
    skos:prefLabel "Lifelines" .

ER-1110-2-1156:Likelihood a wov:GlossaryTerm,
        skos:Concept ;
    rdfs:label "Likelihood" ;
    dcterms:bibliographicCitation "https://www.publications.usace.army.mil/Portals/76/Users/182/86/2486/er_1110-2-1156.pdf#page=513" ;
    pav:wasDerivedFrom "glossaries/CivilWorks/ER-1110-2-1156.yaml#term[Likelihood]" ;
    skos:definition "Used as a qualitative description of probability and frequency. (ICOLD) A description of the occurrence chance of a particular event." ;
    skos:inScheme ER-1110-2-1156: ;
    skos:prefLabel "Likelihood" .

ER-1110-2-1156:Limit_Line_for_Life_Safety a wov:GlossaryTerm,
        skos:Concept ;
    rdfs:label "Limit Line for Life Safety" ;
    dcterms:bibliographicCitation "https://www.publications.usace.army.mil/Portals/76/Users/182/86/2486/er_1110-2-1156.pdf#page=513" ;
    pav:wasDerivedFrom "glossaries/CivilWorks/ER-1110-2-1156.yaml#term[Limit Line for Life Safety]" ;
    skos:definition "Tolerable Risk Limit Line is depicted in Figures 5.4 and 5.5 of Chapter 5, Tolerable Risk Guidelines. It defines the limit line separating unacceptable riskfromtolerableriskonf-NÌ… andF-Ndiagram." ;
    skos:inScheme ER-1110-2-1156: ;
    skos:prefLabel "Limit Line for Life Safety" .

ER-1110-2-1156:Limit_of_Tolerability a wov:GlossaryTerm,
        skos:Concept ;
    rdfs:label "Limit of Tolerability" ;
    dcterms:bibliographicCitation "https://www.publications.usace.army.mil/Portals/76/Users/182/86/2486/er_1110-2-1156.pdf#page=513" ;
    pav:wasDerivedFrom "glossaries/CivilWorks/ER-1110-2-1156.yaml#term[Limit of Tolerability]" ;
    skos:definition "Limit of Tolerability as depicted on Figure 5.1 of Chapter 5. It defines the limit line separating Intolerable Residual Risk from Tolerable Residual Risk within the range of tolerability conceptually depicting the ALARP principle." ;
    skos:inScheme ER-1110-2-1156: ;
    skos:prefLabel "Limit of Tolerability" .

ER-1110-2-1156:Liquefaction a wov:GlossaryTerm,
        skos:Concept ;
    rdfs:label "Liquefaction" ;
    dcterms:bibliographicCitation "https://www.publications.usace.army.mil/Portals/76/Users/182/86/2486/er_1110-2-1156.pdf#page=513" ;
    pav:wasDerivedFrom "glossaries/CivilWorks/ER-1110-2-1156.yaml#term[Liquefaction]" ;
    skos:definition "A condition whereby soil undergoes continued deformation at a constant low residual stress or with low residual resistance, due to the buildup and maintenance of high pore water pressures, which reduces the effective confining pressure to a very low value. Pore pressure buildup leading to liquefaction may be due either to static or cyclic stress applications and the possibility of its occurrence will depend on the void ratio or relative density of a cohesionless or slightly cohesive soil and the confining pressure." ;
    skos:inScheme ER-1110-2-1156: ;
    skos:prefLabel "Liquefaction" .

ER-1110-2-1156:Live_storage a wov:GlossaryTerm,
        skos:Concept ;
    rdfs:label "Live storage" ;
    dcterms:bibliographicCitation "https://www.publications.usace.army.mil/Portals/76/Users/182/86/2486/er_1110-2-1156.pdf#page=523" ;
    pav:wasDerivedFrom "glossaries/CivilWorks/ER-1110-2-1156.yaml#term[Live storage]" ;
    skos:definition "The sum of the active and the inactive storage." ;
    skos:inScheme ER-1110-2-1156: ;
    skos:prefLabel "Live storage" .

ER-1110-2-1156:Locally_Controlled_System a wov:GlossaryTerm,
        skos:Concept ;
    rdfs:label "Locally Controlled System" ;
    dcterms:bibliographicCitation "https://www.publications.usace.army.mil/Portals/76/Users/182/86/2486/er_1110-2-1156.pdf#page=513" ;
    pav:wasDerivedFrom "glossaries/CivilWorks/ER-1110-2-1156.yaml#term[Locally Controlled System]" ;
    skos:definition "A locally controlled system is a system where operation is made by personnel physically located at the project site using controls that are physically located at the structure being operated." ;
    skos:inScheme ER-1110-2-1156: ;
    skos:prefLabel "Locally Controlled System" .

ER-1110-2-1156:Logboom a wov:GlossaryTerm,
        skos:Concept ;
    rdfs:label "Logboom" ;
    dcterms:bibliographicCitation "https://www.publications.usace.army.mil/Portals/76/Users/182/86/2486/er_1110-2-1156.pdf#page=513" ;
    pav:wasDerivedFrom "glossaries/CivilWorks/ER-1110-2-1156.yaml#term[Logboom]" ;
    skos:definition "A chain of logs, drums, or pontoons secured end-to-end and floating on the surface of a reservoir so as to divert floating debris, trash, and logs." ;
    skos:inScheme ER-1110-2-1156: ;
    skos:prefLabel "Logboom" .

ER-1110-2-1156:Maximum_flood_control_level a wov:GlossaryTerm,
        skos:Concept ;
    rdfs:label "Maximum flood control level" ;
    dcterms:bibliographicCitation "https://www.publications.usace.army.mil/Portals/76/Users/182/86/2486/er_1110-2-1156.pdf#page=513" ;
    pav:wasDerivedFrom "glossaries/CivilWorks/ER-1110-2-1156.yaml#term[Maximum flood control level]" ;
    skos:definition "The highest elevation of the flood control storage." ;
    skos:inScheme ER-1110-2-1156: ;
    skos:prefLabel "Maximum flood control level" .

ER-1110-2-1156:Maximum_pool a wov:GlossaryTerm,
        skos:Concept ;
    rdfs:label "Maximum pool" ;
    dcterms:bibliographicCitation "https://www.publications.usace.army.mil/Portals/76/Users/182/86/2486/er_1110-2-1156.pdf#page=513" ;
    pav:wasDerivedFrom "glossaries/CivilWorks/ER-1110-2-1156.yaml#term[Maximum pool]" ;
    skos:definition "The highest pool elevation resulting from the inflow design flood." ;
    skos:inScheme ER-1110-2-1156: ;
    skos:prefLabel "Maximum pool" .

ER-1110-2-1156:Maximum_wave a wov:GlossaryTerm,
        skos:Concept ;
    rdfs:label "Maximum wave" ;
    dcterms:bibliographicCitation "https://www.publications.usace.army.mil/Portals/76/Users/182/86/2486/er_1110-2-1156.pdf#page=513" ;
    pav:wasDerivedFrom "glossaries/CivilWorks/ER-1110-2-1156.yaml#term[Maximum wave]" ;
    skos:definition "The highest wave in a wave group." ;
    skos:inScheme ER-1110-2-1156: ;
    skos:prefLabel "Maximum wave" .

ER-1110-2-1156:Minimum_operating_level a wov:GlossaryTerm,
        skos:Concept ;
    rdfs:label "Minimum operating level" ;
    dcterms:bibliographicCitation "https://www.publications.usace.army.mil/Portals/76/Users/182/86/2486/er_1110-2-1156.pdf#page=513" ;
    pav:wasDerivedFrom "glossaries/CivilWorks/ER-1110-2-1156.yaml#term[Minimum operating level]" ;
    skos:definition "The lowest level to which the reservoir is drawn down under normal operating conditions." ;
    skos:inScheme ER-1110-2-1156: ;
    skos:prefLabel "Minimum operating level" .

ER-1110-2-1156:National_Dam_Safety_Review_Board a wov:GlossaryTerm,
        skos:Concept ;
    rdfs:label "National Dam Safety Review Board" ;
    dcterms:bibliographicCitation "https://www.publications.usace.army.mil/Portals/76/Users/182/86/2486/er_1110-2-1156.pdf#page=513" ;
    pav:wasDerivedFrom "glossaries/CivilWorks/ER-1110-2-1156.yaml#term[National Dam Safety Review Board]" ;
    skos:definition "The National Dam Safety Review Board provides the Director of FEMA with advice in setting national dam safety priorities and considers the effects of national policy issues affecting dam safety. Review Board members include FEMA, the Chair of the Board; representatives from four federal agencies that serve on the Interagency Committee on Dam Safety (ICODS); five state dam safety officials; and one member from the private sector." ;
    skos:inScheme ER-1110-2-1156: ;
    skos:prefLabel "National Dam Safety Review Board" .

ER-1110-2-1156:National_Environmental_Policy_Act_%28NEPA%29 a wov:GlossaryTerm,
        skos:Concept ;
    rdfs:label "National Environmental Policy Act (NEPA)" ;
    dcterms:bibliographicCitation "https://www.publications.usace.army.mil/Portals/76/Users/182/86/2486/er_1110-2-1156.pdf#page=514" ;
    pav:wasDerivedFrom "glossaries/CivilWorks/ER-1110-2-1156.yaml#term[National Environmental Policy Act (NEPA)]" ;
    skos:altLabel "NEPA" ;
    skos:definition "The National Environmental Policy Act (NEPA) (reference A.6) requires federal agencies to integrate environmental values into their decision making processes by considering the environmental impacts of their proposed actions and reasonable alternatives to those actions. To meet NEPA requirements federal agencies prepare a detailed statement known as an Environmental Impact Statement (EIS). EPA reviews and comments on EIS's prepared by other federal agencies, maintains a national filing system for all EIS's, and assures that its own actions comply with NEPA." ;
    skos:inScheme ER-1110-2-1156: ;
    skos:prefLabel "National Environmental Policy Act (NEPA)" .

ER-1110-2-1156:National_Inventory_of_Dams a wov:GlossaryTerm,
        skos:Concept ;
    rdfs:label "National Inventory of Dams" ;
    dcterms:bibliographicCitation "https://www.publications.usace.army.mil/Portals/76/Users/182/86/2486/er_1110-2-1156.pdf#page=514" ;
    pav:wasDerivedFrom "glossaries/CivilWorks/ER-1110-2-1156.yaml#term[National Inventory of Dams]" ;
    skos:definition "The National Inventory of Dams (NID) contains information on approximately 84,000 dams throughout the U.S. that are more than 25 feet high, hold more than 50 acre-feet of water, or are considered a significant hazard if they fail. The NID is maintained and published by USACE with information from all 50 states, Puerto Rico, and 16 Federal agencies. The NID is available on the web athttp://geo.usace.army.mil/pgis/f?p=397:12:0" ;
    skos:inScheme ER-1110-2-1156: ;
    skos:prefLabel "National Inventory of Dams" .

ER-1110-2-1156:Non-Structural_Risk_Reduction a wov:GlossaryTerm,
        skos:Concept ;
    rdfs:label "Non-Structural Risk Reduction" ;
    dcterms:bibliographicCitation "https://www.publications.usace.army.mil/Portals/76/Users/182/86/2486/er_1110-2-1156.pdf#page=514" ;
    pav:wasDerivedFrom "glossaries/CivilWorks/ER-1110-2-1156.yaml#term[Non-Structural Risk Reduction]" ;
    skos:definition "Risk reduction by measures that do not require structural modification or construction related to the dam and its appurtenant works." ;
    skos:inScheme ER-1110-2-1156: ;
    skos:prefLabel "Non-Structural Risk Reduction" .

ER-1110-2-1156:Normal_Operations a wov:GlossaryTerm,
        skos:Concept ;
    rdfs:label "Normal Operations" ;
    dcterms:bibliographicCitation "https://www.publications.usace.army.mil/Portals/76/Users/182/86/2486/er_1110-2-1156.pdf#page=514" ;
    pav:wasDerivedFrom "glossaries/CivilWorks/ER-1110-2-1156.yaml#term[Normal Operations]" ;
    skos:definition "Loading on the dam resulting from day-to-day pool operations to achieve authorized purposes. (For the purposes of a screening analysis for dry dams, or where pool elevations fluctuate widely and no historical normal pool elevation has been established, the normal loading is usually correlated to a 1 to 10 year return period.)" ;
    skos:inScheme ER-1110-2-1156: ;
    skos:prefLabel "Normal Operations" .

ER-1110-2-1156:Observation_well a wov:GlossaryTerm,
        skos:Concept ;
    rdfs:label "Observation well" ;
    dcterms:bibliographicCitation "https://www.publications.usace.army.mil/Portals/76/Users/182/86/2486/er_1110-2-1156.pdf#page=514" ;
    pav:wasDerivedFrom "glossaries/CivilWorks/ER-1110-2-1156.yaml#term[Observation well]" ;
    skos:definition "A hole used to observe the groundwater surface at atmospheric pressure within soil or rock." ;
    skos:inScheme ER-1110-2-1156: ;
    skos:prefLabel "Observation well" .

ER-1110-2-1156:Operation_restrictions a wov:GlossaryTerm,
        skos:Concept ;
    rdfs:label "Operation restrictions" ;
    dcterms:bibliographicCitation "https://www.publications.usace.army.mil/Portals/76/Users/182/86/2486/er_1110-2-1156.pdf#page=514" ;
    pav:wasDerivedFrom "glossaries/CivilWorks/ER-1110-2-1156.yaml#term[Operation restrictions]" ;
    skos:definition "Changes to operating pool levels and durations, or reduced lockages, power generation, water supply, or conservation operations." ;
    skos:inScheme ER-1110-2-1156: ;
    skos:prefLabel "Operation restrictions" .

ER-1110-2-1156:Outlet a wov:GlossaryTerm,
        skos:Concept ;
    rdfs:label "Outlet" ;
    dcterms:bibliographicCitation "https://www.publications.usace.army.mil/Portals/76/Users/182/86/2486/er_1110-2-1156.pdf#page=514" ;
    pav:wasDerivedFrom "glossaries/CivilWorks/ER-1110-2-1156.yaml#term[Outlet]" ;
    skos:definition "An opening through which water can be freely discharged from a reservoir to the river for a particular purpose." ;
    skos:inScheme ER-1110-2-1156: ;
    skos:prefLabel "Outlet" .

ER-1110-2-1156:Outlet_gate a wov:GlossaryTerm,
        skos:Concept ;
    rdfs:label "Outlet gate" ;
    dcterms:bibliographicCitation "https://www.publications.usace.army.mil/Portals/76/Users/182/86/2486/er_1110-2-1156.pdf#page=506" ;
    pav:wasDerivedFrom "glossaries/CivilWorks/ER-1110-2-1156.yaml#term[Outlet gate]" ;
    skos:definition "A gate controlling the flow of water through a reservoir outlet." ;
    skos:inScheme ER-1110-2-1156: ;
    skos:prefLabel "Outlet gate" .

ER-1110-2-1156:Outlet_works a wov:GlossaryTerm,
        skos:Concept ;
    rdfs:label "Outlet works" ;
    dcterms:bibliographicCitation "https://www.publications.usace.army.mil/Portals/76/Users/182/86/2486/er_1110-2-1156.pdf#page=514" ;
    pav:wasDerivedFrom "glossaries/CivilWorks/ER-1110-2-1156.yaml#term[Outlet works]" ;
    skos:definition "A dam appurtenance that provides release of water (generally controlled) from a reservoir." ;
    skos:inScheme ER-1110-2-1156: ;
    skos:prefLabel "Outlet works" .

ER-1110-2-1156:Parametric_Studies a wov:GlossaryTerm,
        skos:Concept ;
    rdfs:label "Parametric Studies" ;
    dcterms:bibliographicCitation "https://www.publications.usace.army.mil/Portals/76/Users/182/86/2486/er_1110-2-1156.pdf#page=514" ;
    pav:wasDerivedFrom "glossaries/CivilWorks/ER-1110-2-1156.yaml#term[Parametric Studies]" ;
    skos:definition "Parametric studies execute one application many times with different sets of input parameters. Such studies are in-effect, systematic, carefully controlled sensitivity studies." ;
    skos:inScheme ER-1110-2-1156: ;
    skos:prefLabel "Parametric Studies" .

ER-1110-2-1156:Parapet_wall a wov:GlossaryTerm,
        skos:Concept ;
    rdfs:label "Parapet wall" ;
    dcterms:bibliographicCitation "https://www.publications.usace.army.mil/Portals/76/Users/182/86/2486/er_1110-2-1156.pdf#page=514" ;
    pav:wasDerivedFrom "glossaries/CivilWorks/ER-1110-2-1156.yaml#term[Parapet wall]" ;
    skos:definition "A solid wall built along the top of a dam (upstream or downstream edge) used for ornamentation, for safety of vehicles and pedestrians, or to prevent overtopping caused by wave run-up." ;
    skos:inScheme ER-1110-2-1156: ;
    skos:prefLabel "Parapet wall" .

ER-1110-2-1156:Peer_Review a wov:GlossaryTerm,
        skos:Concept ;
    rdfs:label "Peer Review" ;
    dcterms:bibliographicCitation "https://www.publications.usace.army.mil/Portals/76/Users/182/86/2486/er_1110-2-1156.pdf#page=515" ;
    pav:wasDerivedFrom "glossaries/CivilWorks/ER-1110-2-1156.yaml#term[Peer Review]" ;
    skos:definition "Peer review is a form of deliberation involving an exchange of judgments about the appropriateness of methods and the strength of the author's inferences. Peer review involves the review of a draft product for quality by specialists in the field who were not involved in producing the draft." ;
    skos:inScheme ER-1110-2-1156: ;
    skos:prefLabel "Peer Review" .

ER-1110-2-1156:Peer_Review_Panel a wov:GlossaryTerm,
        skos:Concept ;
    rdfs:label "Peer Review Panel" ;
    dcterms:bibliographicCitation "https://www.publications.usace.army.mil/Portals/76/Users/182/86/2486/er_1110-2-1156.pdf#page=515" ;
    pav:wasDerivedFrom "glossaries/CivilWorks/ER-1110-2-1156.yaml#term[Peer Review Panel]" ;
    skos:definition "A panel of peer experts, usually formed by a district, to review and to advise on particular difficult or controversial technical issues related to a dam safety study. The peer group may be from inside or outside USACE, or whatever combination of experts is judged to best fit the need." ;
    skos:inScheme ER-1110-2-1156: ;
    skos:prefLabel "Peer Review Panel" .

ER-1110-2-1156:Penstock a wov:GlossaryTerm,
        skos:Concept ;
    rdfs:label "Penstock" ;
    dcterms:bibliographicCitation "https://www.publications.usace.army.mil/Portals/76/Users/182/86/2486/er_1110-2-1156.pdf#page=515" ;
    pav:wasDerivedFrom "glossaries/CivilWorks/ER-1110-2-1156.yaml#term[Penstock]" ;
    skos:definition "A pressurized pipeline or shaft between the reservoir and hydraulic machinery." ;
    skos:inScheme ER-1110-2-1156: ;
    skos:prefLabel "Penstock" .

ER-1110-2-1156:Performance_Evaluation a wov:GlossaryTerm,
        skos:Concept ;
    rdfs:label "Performance Evaluation" ;
    dcterms:bibliographicCitation "https://www.publications.usace.army.mil/Portals/76/Users/182/86/2486/er_1110-2-1156.pdf#page=515" ;
    pav:wasDerivedFrom "glossaries/CivilWorks/ER-1110-2-1156.yaml#term[Performance Evaluation]" ;
    skos:definition "Description of how the dam and appurtenant structures have performed over the years since construction." ;
    skos:inScheme ER-1110-2-1156: ;
    skos:prefLabel "Performance Evaluation" .

ER-1110-2-1156:Performance_Uncertainty a wov:GlossaryTerm,
        skos:Concept ;
    rdfs:label "Performance Uncertainty" ;
    dcterms:bibliographicCitation "https://www.publications.usace.army.mil/Portals/76/Users/182/86/2486/er_1110-2-1156.pdf#page=515" ;
    pav:wasDerivedFrom "glossaries/CivilWorks/ER-1110-2-1156.yaml#term[Performance Uncertainty]" ;
    skos:definition "Performance uncertainty refers to the situation in which more rigorous and detailed studies are needed to more accurately predict the system response probabilities within each applicable failure mode." ;
    skos:inScheme ER-1110-2-1156: ;
    skos:prefLabel "Performance Uncertainty" .

ER-1110-2-1156:Periodic_Assessments_%28PA%29 a wov:GlossaryTerm,
        skos:Concept ;
    rdfs:label "Periodic Assessments (PA)" ;
    dcterms:bibliographicCitation "https://www.publications.usace.army.mil/Portals/76/Users/182/86/2486/er_1110-2-1156.pdf#page=515" ;
    pav:wasDerivedFrom "glossaries/CivilWorks/ER-1110-2-1156.yaml#term[Periodic Assessments (PA)]" ;
    skos:altLabel "PA" ;
    skos:definition "The periodic assessment will consist of a site visit, typically associated with a periodic inspection, a potential failure modes analysis, and a semi- quantitative risk assessment based on existing data and limited development of estimated consequence data developed by the Modeling, Mapping, and Consequence Production Center. The primary purposes of the Periodic Assessment are as follows:  Evaluate the project vulnerabilities and associated risks, including non-breach risks; Reevaluate the DSAC of a project and recommend a change, if necessary; Review and if necessary revise the IRRMP; Identify the need for issue evaluation studies and provide data to prioritize issue evaluation studies; Identify and prioritize any data collection, analyses, and study needs; Identify operations and maintenance, monitoring, emergency action plan, training and other recurrent needs ; and Provide a better understanding of vulnerabilities and a basis for future dam safety inspections and activities." ;
    skos:inScheme ER-1110-2-1156: ;
    skos:prefLabel "Periodic Assessments (PA)" .

ER-1110-2-1156:Periodic_Inspections_%28PI%29 a wov:GlossaryTerm,
        skos:Concept ;
    rdfs:label "Periodic Inspections (PI)" ;
    dcterms:bibliographicCitation "https://www.publications.usace.army.mil/Portals/76/Users/182/86/2486/er_1110-2-1156.pdf#page=515" ;
    pav:wasDerivedFrom "glossaries/CivilWorks/ER-1110-2-1156.yaml#term[Periodic Inspections (PI)]" ;
    skos:altLabel "PI" ;
    skos:definition "The recurrent engineering inspections conducted at dams and other civil works structures whose failure or partial failure could jeopardize the operational integrity of the project, endanger the lives and safety of the public or cause substantial property damage must be periodically inspected and evaluated to ensure their structural stability, safety, and operational adequacy." ;
    skos:inScheme ER-1110-2-1156: ;
    skos:prefLabel "Periodic Inspections (PI)" .

ER-1110-2-1156:Phreatic_surface a wov:GlossaryTerm,
        skos:Concept ;
    rdfs:label "Phreatic surface" ;
    dcterms:bibliographicCitation "https://www.publications.usace.army.mil/Portals/76/Users/182/86/2486/er_1110-2-1156.pdf#page=515" ;
    pav:wasDerivedFrom "glossaries/CivilWorks/ER-1110-2-1156.yaml#term[Phreatic surface]" ;
    skos:definition "The free surface of water seeping at atmospheric pressure through soil or rock." ;
    skos:inScheme ER-1110-2-1156: ;
    skos:prefLabel "Phreatic surface" .

ER-1110-2-1156:Piezometer a wov:GlossaryTerm,
        skos:Concept ;
    rdfs:label "Piezometer" ;
    dcterms:bibliographicCitation "https://www.publications.usace.army.mil/Portals/76/Users/182/86/2486/er_1110-2-1156.pdf#page=515" ;
    pav:wasDerivedFrom "glossaries/CivilWorks/ER-1110-2-1156.yaml#term[Piezometer]" ;
    skos:definition "An instrument used for measuring fluid pressure (air or water) within soil, rock, or concrete." ;
    skos:inScheme ER-1110-2-1156: ;
    skos:prefLabel "Piezometer" .

ER-1110-2-1156:Piping a wov:GlossaryTerm,
        skos:Concept ;
    rdfs:label "Piping" ;
    dcterms:bibliographicCitation "https://www.publications.usace.army.mil/Portals/76/Users/182/86/2486/er_1110-2-1156.pdf#page=516" ;
    pav:wasDerivedFrom "glossaries/CivilWorks/ER-1110-2-1156.yaml#term[Piping]" ;
    skos:definition "A mechanism of internal erosion which progresses backward in the opposite direction of seepage flow." ;
    skos:inScheme ER-1110-2-1156: ;
    skos:prefLabel "Piping" .

ER-1110-2-1156:Plunge_pool a wov:GlossaryTerm,
        skos:Concept ;
    rdfs:label "Plunge pool" ;
    dcterms:bibliographicCitation "https://www.publications.usace.army.mil/Portals/76/Users/182/86/2486/er_1110-2-1156.pdf#page=516" ;
    pav:wasDerivedFrom "glossaries/CivilWorks/ER-1110-2-1156.yaml#term[Plunge pool]" ;
    skos:definition "A natural or artificially created pool that dissipates the energy of free falling water." ;
    skos:inScheme ER-1110-2-1156: ;
    skos:prefLabel "Plunge pool" .

ER-1110-2-1156:Population_at_Risk a wov:GlossaryTerm,
        skos:Concept ;
    rdfs:label "Population at Risk" ;
    dcterms:bibliographicCitation "https://www.publications.usace.army.mil/Portals/76/Users/182/86/2486/er_1110-2-1156.pdf#page=516" ;
    pav:wasDerivedFrom "glossaries/CivilWorks/ER-1110-2-1156.yaml#term[Population at Risk]" ;
    skos:definition "The population downstream of a dam that would be subject to risk from flooding in the instance of a potential dam failure; usually documented in numbers of persons at risk." ;
    skos:inScheme ER-1110-2-1156: ;
    skos:prefLabel "Population at Risk" .

ER-1110-2-1156:Pore_water_pressure a wov:GlossaryTerm,
        skos:Concept ;
    rdfs:label "Pore water pressure" ;
    dcterms:bibliographicCitation "https://www.publications.usace.army.mil/Portals/76/Users/182/86/2486/er_1110-2-1156.pdf#page=516" ;
    pav:wasDerivedFrom "glossaries/CivilWorks/ER-1110-2-1156.yaml#term[Pore water pressure]" ;
    skos:definition "The interstitial water pressure within a mass of soil, rock, or concrete." ;
    skos:inScheme ER-1110-2-1156: ;
    skos:prefLabel "Pore water pressure" .

ER-1110-2-1156:Portfolio_Risk_Management_Process a wov:GlossaryTerm,
        skos:Concept ;
    rdfs:label "Portfolio Risk Management Process" ;
    dcterms:bibliographicCitation "https://www.publications.usace.army.mil/Portals/76/Users/182/86/2486/er_1110-2-1156.pdf#page=516" ;
    pav:wasDerivedFrom "glossaries/CivilWorks/ER-1110-2-1156.yaml#term[Portfolio Risk Management Process]" ;
    skos:definition "The management process shown generally on Figure 2.3 and in detail for USACE Figure 3.1. It is a risk-informed USACE-wide portfolio perspective process applied to all features of all dams on a continuing basis. Same definition as 'Dam Safety Portfolio Risk Management Process\" above." ;
    skos:inScheme ER-1110-2-1156: ;
    skos:prefLabel "Portfolio Risk Management Process" .

ER-1110-2-1156:Potential_Failure_Mode_%28PFM%29 a wov:GlossaryTerm,
        skos:Concept ;
    rdfs:label "Potential Failure Mode (PFM)" ;
    dcterms:bibliographicCitation "https://www.publications.usace.army.mil/Portals/76/Users/182/86/2486/er_1110-2-1156.pdf#page=516" ;
    pav:wasDerivedFrom "glossaries/CivilWorks/ER-1110-2-1156.yaml#term[Potential Failure Mode (PFM)]" ;
    skos:altLabel "PFM" ;
    skos:definition "The chain of events leading to dam failure or a portion there of that could lead to dam failure. The dam does not have to completely fail in the sense of a complete release of the impounded water." ;
    skos:inScheme ER-1110-2-1156: ;
    skos:prefLabel "Potential Failure Mode (PFM)" .

ER-1110-2-1156:Potential_Failure_Mode_Analysis_%28PFMA%29 a wov:GlossaryTerm,
        skos:Concept ;
    rdfs:label "Potential Failure Mode Analysis (PFMA)" ;
    dcterms:bibliographicCitation "https://www.publications.usace.army.mil/Portals/76/Users/182/86/2486/er_1110-2-1156.pdf#page=516" ;
    pav:wasDerivedFrom "glossaries/CivilWorks/ER-1110-2-1156.yaml#term[Potential Failure Mode Analysis (PFMA)]" ;
    skos:altLabel "PFMA" ;
    skos:definition "A PFMA is an examination of potential failure modes for an existing dam by a team of persons who are qualified either by experience and\\or education to evaluate dams. It is based on a review of existing data and information, first hand input from field and operational personnel, site inspection, completed engineering analyses, discussion of dam characteristics, failure causes and an understanding of the consequences of failure. The PFMA is intended to provide enhanced understanding and insight on the risk exposure associated with the dam or levee." ;
    skos:inScheme ER-1110-2-1156: ;
    skos:prefLabel "Potential Failure Mode Analysis (PFMA)" .

ER-1110-2-1156:Probability a wov:GlossaryTerm,
        skos:Concept ;
    rdfs:label "Probability" ;
    dcterms:bibliographicCitation "https://www.publications.usace.army.mil/Portals/76/Users/182/86/2486/er_1110-2-1156.pdf#page=516" ;
    pav:wasDerivedFrom "glossaries/CivilWorks/ER-1110-2-1156.yaml#term[Probability]" ;
    skos:definition "A measure, of the likelihood, chance, or degree of belief that a particular outcome or consequence will occur. A probability provides a quantitative description of the likelihood of occurrence of a particular event. This is expressed as a value between 0 and 1. (USACE)" ;
    skos:inScheme ER-1110-2-1156: ;
    skos:prefLabel "Probability" .

ER-1110-2-1156:Probability_of_Failure a wov:GlossaryTerm,
        skos:Concept ;
    rdfs:label "Probability of Failure" ;
    dcterms:bibliographicCitation "https://www.publications.usace.army.mil/Portals/76/Users/182/86/2486/er_1110-2-1156.pdf#page=516" ;
    pav:wasDerivedFrom "glossaries/CivilWorks/ER-1110-2-1156.yaml#term[Probability of Failure]" ;
    skos:definition "The probability that a component of a dam or the dam will fail, given a specified load, leading to sudden, rapid, and uncontrolled release of impounded water." ;
    skos:inScheme ER-1110-2-1156: ;
    skos:prefLabel "Probability of Failure" .

ER-1110-2-1156:Probability_of_Individual_Life_Loss a wov:GlossaryTerm,
        skos:Concept ;
    rdfs:label "Probability of Individual Life Loss" ;
    dcterms:bibliographicCitation "https://www.publications.usace.army.mil/Portals/76/Users/182/86/2486/er_1110-2-1156.pdf#page=516" ;
    pav:wasDerivedFrom "glossaries/CivilWorks/ER-1110-2-1156.yaml#term[Probability of Individual Life Loss]" ;
    skos:definition "The probability of individual life loss, which is used in the evaluation of Individual incremental life safety risk, is not necessarily the same as the probability of failure that is used in the evaluation of Reclamation's APF guideline. The probability of life loss is based on the probability of failure and a consideration of exposure factors such as day-night differences in PAR and evaluation and the seasonal presence of people in campgrounds. The level of detail that is appropriate for characterizing exposure factors should be decision driven, although it is noted that FEMA's HAZUS data base provides opportunity for some level of automation in capturing information on exposure factors. The distinction between probability of failure and probability of life loss is particularly important for navigation dams, but can also have a significant effect on the evaluation of life safety for other types of dams. It applies to societal risk as well as to individual risk." ;
    skos:inScheme ER-1110-2-1156: ;
    skos:prefLabel "Probability of Individual Life Loss" .

ER-1110-2-1156:Probable_Maximum_Precipitation_%28PMP%29 a wov:GlossaryTerm,
        skos:Concept ;
    rdfs:label "Probable Maximum Precipitation (PMP)" ;
    dcterms:bibliographicCitation "https://www.publications.usace.army.mil/Portals/76/Users/182/86/2486/er_1110-2-1156.pdf#page=517" ;
    pav:wasDerivedFrom "glossaries/CivilWorks/ER-1110-2-1156.yaml#term[Probable Maximum Precipitation (PMP)]" ;
    skos:altLabel "PMP" ;
    skos:definition "Theoretically, the greatest depth of precipitation for a given duration that is physically possible over a given size storm area at a particular geographical location." ;
    skos:inScheme ER-1110-2-1156: ;
    skos:prefLabel "Probable Maximum Precipitation (PMP)" .

ER-1110-2-1156:Pumped_storage_reservoir a wov:GlossaryTerm,
        skos:Concept ;
    rdfs:label "Pumped storage reservoir" ;
    dcterms:bibliographicCitation "https://www.publications.usace.army.mil/Portals/76/Users/182/86/2486/er_1110-2-1156.pdf#page=517" ;
    pav:wasDerivedFrom "glossaries/CivilWorks/ER-1110-2-1156.yaml#term[Pumped storage reservoir]" ;
    skos:definition "A reservoir filled entirely or mainly with water pumped from outside its natural drainage area." ;
    skos:inScheme ER-1110-2-1156: ;
    skos:prefLabel "Pumped storage reservoir" .

ER-1110-2-1156:Quality_%28as_related_to_construction%29 a wov:GlossaryTerm,
        skos:Concept ;
    rdfs:label "Quality (as related to construction)" ;
    dcterms:bibliographicCitation "https://www.publications.usace.army.mil/Portals/76/Users/182/86/2486/er_1110-2-1156.pdf#page=517" ;
    pav:wasDerivedFrom "glossaries/CivilWorks/ER-1110-2-1156.yaml#term[Quality (as related to construction)]" ;
    skos:definition "Conformance to properly developed requirements." ;
    skos:inScheme ER-1110-2-1156: ;
    skos:prefLabel "Quality (as related to construction)" .

ER-1110-2-1156:Quality_Assurance_%28QA%29 a wov:GlossaryTerm,
        skos:Concept ;
    rdfs:label "Quality Assurance (QA)" ;
    dcterms:bibliographicCitation "https://www.publications.usace.army.mil/Portals/76/Users/182/86/2486/er_1110-2-1156.pdf#page=517" ;
    pav:wasDerivedFrom "glossaries/CivilWorks/ER-1110-2-1156.yaml#term[Quality Assurance (QA)]" ;
    skos:altLabel "QA" ;
    skos:definition "The procedure by which the Government fulfills its responsibility to be certain the contractors' quality control is functioning and the specified end product is realized." ;
    skos:inScheme ER-1110-2-1156: ;
    skos:prefLabel "Quality Assurance (QA)" .

ER-1110-2-1156:Quality_Management a wov:GlossaryTerm,
        skos:Concept ;
    rdfs:label "Quality Management" ;
    dcterms:bibliographicCitation "https://www.publications.usace.army.mil/Portals/76/Users/182/86/2486/er_1110-2-1156.pdf#page=517" ;
    pav:wasDerivedFrom "glossaries/CivilWorks/ER-1110-2-1156.yaml#term[Quality Management]" ;
    skos:definition "All control and assurance activities instituted to achieve the product quality established by the contract requirements" ;
    skos:inScheme ER-1110-2-1156: ;
    skos:prefLabel "Quality Management" .

ER-1110-2-1156:Radial_gate a wov:GlossaryTerm,
        skos:Concept ;
    rdfs:label "Radial gate" ;
    dcterms:bibliographicCitation "https://www.publications.usace.army.mil/Portals/76/Users/182/86/2486/er_1110-2-1156.pdf#page=506" ;
    pav:wasDerivedFrom "glossaries/CivilWorks/ER-1110-2-1156.yaml#term[Radial gate]" ;
    skos:altLabel "tainter gate" ;
    skos:definition "A gate with a curved upstream plate and radial arms hinged to piers or other supporting structure." ;
    skos:inScheme ER-1110-2-1156: ;
    skos:prefLabel "Radial gate" .

ER-1110-2-1156:Rapid_Consequence_Analysis%2FEstimate a wov:GlossaryTerm,
        skos:Concept ;
    rdfs:label "Rapid Consequence Analysis/Estimate" ;
    dcterms:bibliographicCitation "https://www.publications.usace.army.mil/Portals/76/Users/182/86/2486/er_1110-2-1156.pdf#page=517" ;
    pav:wasDerivedFrom "glossaries/CivilWorks/ER-1110-2-1156.yaml#term[Rapid Consequence Analysis/Estimate]" ;
    skos:definition "The rapid consequence estimate requires a very limited detail, unsteady-flow hydraulic model to reproduce various, with and without, dam failure scenarios. These failure scenarios would include sunny day, Probably Maximum Flood (PMF) and several intermediate load cases between these extremes for both the with and without dam failure condition." ;
    skos:inScheme ER-1110-2-1156: ;
    skos:prefLabel "Rapid Consequence Analysis/Estimate" .

ER-1110-2-1156:Redundancy a wov:GlossaryTerm,
        skos:Concept ;
    rdfs:label "Redundancy" ;
    dcterms:bibliographicCitation "https://www.publications.usace.army.mil/Portals/76/Users/182/86/2486/er_1110-2-1156.pdf#page=517" ;
    pav:wasDerivedFrom "glossaries/CivilWorks/ER-1110-2-1156.yaml#term[Redundancy]" ;
    skos:definition "The duplication of critical components of a system with the intention of increasing reliability of the system, usually in the case of a backup or fail-safe." ;
    skos:inScheme ER-1110-2-1156: ;
    skos:prefLabel "Redundancy" .

ER-1110-2-1156:Regional_Cadres a wov:GlossaryTerm,
        skos:Concept ;
    rdfs:label "Regional Cadres" ;
    dcterms:bibliographicCitation "https://www.publications.usace.army.mil/Portals/76/Users/182/86/2486/er_1110-2-1156.pdf#page=517" ;
    pav:wasDerivedFrom "glossaries/CivilWorks/ER-1110-2-1156.yaml#term[Regional Cadres]" ;
    skos:definition "Teams of technical specialists and analysts (cadre) assembled to conduct project specific risk evaluations, such as PFMAs, based on expert knowledge of the geology, hydrology, structural integrity, soils, consequences, and other relevant factors." ;
    skos:inScheme ER-1110-2-1156: ;
    skos:prefLabel "Regional Cadres" .

ER-1110-2-1156:Regulating_gate a wov:GlossaryTerm,
        skos:Concept ;
    rdfs:label "Regulating gate" ;
    dcterms:bibliographicCitation "https://www.publications.usace.army.mil/Portals/76/Users/182/86/2486/er_1110-2-1156.pdf#page=506" ;
    pav:wasDerivedFrom "glossaries/CivilWorks/ER-1110-2-1156.yaml#term[Regulating gate]" ;
    skos:altLabel "regulating valve" ;
    skos:definition "A gate or valve that operates under full pressure flow conditions to regulate the rate of discharge." ;
    skos:inScheme ER-1110-2-1156: ;
    skos:prefLabel "Regulating gate" .

ER-1110-2-1156:Regulating_sleeve_valve a wov:GlossaryTerm,
        skos:Concept ;
    rdfs:label "Regulating sleeve valve" ;
    dcterms:bibliographicCitation "https://www.publications.usace.army.mil/Portals/76/Users/182/86/2486/er_1110-2-1156.pdf#page=525" ;
    pav:wasDerivedFrom "glossaries/CivilWorks/ER-1110-2-1156.yaml#term[Regulating sleeve valve]" ;
    skos:definition "A valve for regulating high-pressure outlets and ensuring energy dissipation. Inside the valve there is a fixed-cone, pointed upstream, which ensures dispersion of the jet. Outside the valve a cylindrical sleeve moves downstream to shut off flow by sealing on the periphery of the cone." ;
    skos:inScheme ER-1110-2-1156: ;
    skos:prefLabel "Regulating sleeve valve" .

ER-1110-2-1156:Regulation_Design_Capacity a wov:GlossaryTerm,
        skos:Concept ;
    rdfs:label "Regulation Design Capacity" ;
    dcterms:bibliographicCitation "https://www.publications.usace.army.mil/Portals/76/Users/182/86/2486/er_1110-2-1156.pdf#page=517" ;
    pav:wasDerivedFrom "glossaries/CivilWorks/ER-1110-2-1156.yaml#term[Regulation Design Capacity]" ;
    skos:definition "The maximum hydrologic loading condition (flood hydrograph) above which the project no longer has storage capacity to reduce flow that would provide flood damage reduction benefits. The regulation design capacity is typically the reservoir storage capacity (and attendant operation rules and policies) that are authorized for a flood damage reduction reservoir project. This will always be a hydrologic loading level less than the loading levels used as the structural design capacity." ;
    skos:inScheme ER-1110-2-1156: ;
    skos:prefLabel "Regulation Design Capacity" .

ER-1110-2-1156:Reliability a wov:GlossaryTerm,
        skos:Concept ;
    rdfs:label "Reliability" ;
    dcterms:bibliographicCitation "https://www.publications.usace.army.mil/Portals/76/Users/182/86/2486/er_1110-2-1156.pdf#page=518" ;
    pav:wasDerivedFrom "glossaries/CivilWorks/ER-1110-2-1156.yaml#term[Reliability]" ;
    skos:definition "For gate and mechanical systems reliability is defined as the likelihood of successful performance of a given project element. It may be measured on an annual basis or for some specified time period of interest or, for example, in the case of spillway gates, on a per demand basis. Mathematically, Reliability = 1 - Probability of unsatisfactory operation." ;
    skos:inScheme ER-1110-2-1156: ;
    skos:prefLabel "Reliability" .

ER-1110-2-1156:Remediation a wov:GlossaryTerm,
        skos:Concept ;
    rdfs:label "Remediation" ;
    dcterms:bibliographicCitation "https://www.publications.usace.army.mil/Portals/76/Users/182/86/2486/er_1110-2-1156.pdf#page=518" ;
    pav:wasDerivedFrom "glossaries/CivilWorks/ER-1110-2-1156.yaml#term[Remediation]" ;
    skos:definition "Implementation of long-term structural and non-structural risk reduction measures to resolve Dam Safety issues." ;
    skos:inScheme ER-1110-2-1156: ;
    skos:prefLabel "Remediation" .

ER-1110-2-1156:Remotely_Controlled_System a wov:GlossaryTerm,
        skos:Concept ;
    rdfs:label "Remotely Controlled System" ;
    dcterms:bibliographicCitation "https://www.publications.usace.army.mil/Portals/76/Users/182/86/2486/er_1110-2-1156.pdf#page=518" ;
    pav:wasDerivedFrom "glossaries/CivilWorks/ER-1110-2-1156.yaml#term[Remotely Controlled System]" ;
    skos:definition "A remotely controlled system is a system where operation is made by personnel who are physically located at the project site using remote controls that are not physically at the structure being operated." ;
    skos:inScheme ER-1110-2-1156: ;
    skos:prefLabel "Remotely Controlled System" .

ER-1110-2-1156:Remotely_Operated_System a wov:GlossaryTerm,
        skos:Concept ;
    rdfs:label "Remotely Operated System" ;
    dcterms:bibliographicCitation "https://www.publications.usace.army.mil/Portals/76/Users/182/86/2486/er_1110-2-1156.pdf#page=518" ;
    pav:wasDerivedFrom "glossaries/CivilWorks/ER-1110-2-1156.yaml#term[Remotely Operated System]" ;
    skos:definition "A remotely operated system is a system where operation is made by personnel who are not physically located at the project site using remote controls that are not physically located at the structure being operated." ;
    skos:inScheme ER-1110-2-1156: ;
    skos:prefLabel "Remotely Operated System" .

ER-1110-2-1156:Reservoir a wov:GlossaryTerm,
        skos:Concept ;
    rdfs:label "Reservoir" ;
    dcterms:bibliographicCitation "https://www.publications.usace.army.mil/Portals/76/Users/182/86/2486/er_1110-2-1156.pdf#page=518" ;
    pav:wasDerivedFrom "glossaries/CivilWorks/ER-1110-2-1156.yaml#term[Reservoir]" ;
    skos:definition "A body of water impounded by a dam and in which water can be stored." ;
    skos:inScheme ER-1110-2-1156: ;
    skos:prefLabel "Reservoir" .

ER-1110-2-1156:Reservoir_capacity a wov:GlossaryTerm,
        skos:Concept ;
    rdfs:label "Reservoir capacity" ;
    dcterms:bibliographicCitation "https://www.publications.usace.army.mil/Portals/76/Users/182/86/2486/er_1110-2-1156.pdf#page=523" ;
    pav:wasDerivedFrom "glossaries/CivilWorks/ER-1110-2-1156.yaml#term[Reservoir capacity]" ;
    skos:definition "The sum of the dead and live storage of the reservoir." ;
    skos:inScheme ER-1110-2-1156: ;
    skos:prefLabel "Reservoir capacity" .

ER-1110-2-1156:Reservoir_regulation_%28or_operating%29_procedure a wov:GlossaryTerm,
        skos:Concept ;
    rdfs:label "Reservoir regulation (or operating) procedure" ;
    dcterms:bibliographicCitation "https://www.publications.usace.army.mil/Portals/76/Users/182/86/2486/er_1110-2-1156.pdf#page=518" ;
    pav:wasDerivedFrom "glossaries/CivilWorks/ER-1110-2-1156.yaml#term[Reservoir regulation (or operating) procedure]" ;
    skos:definition "Operating procedures that govern reservoir storage and releases." ;
    skos:inScheme ER-1110-2-1156: ;
    skos:prefLabel "Reservoir regulation (or operating) procedure" .

ER-1110-2-1156:Reservoir_surface_area a wov:GlossaryTerm,
        skos:Concept ;
    rdfs:label "Reservoir surface area" ;
    dcterms:bibliographicCitation "https://www.publications.usace.army.mil/Portals/76/Users/182/86/2486/er_1110-2-1156.pdf#page=518" ;
    pav:wasDerivedFrom "glossaries/CivilWorks/ER-1110-2-1156.yaml#term[Reservoir surface area]" ;
    skos:definition "The area covered by a reservoir when filled to a specified level." ;
    skos:inScheme ER-1110-2-1156: ;
    skos:prefLabel "Reservoir surface area" .

ER-1110-2-1156:Residual_Risk a wov:GlossaryTerm,
        skos:Concept ;
    rdfs:label "Residual Risk" ;
    dcterms:bibliographicCitation "https://www.publications.usace.army.mil/Portals/76/Users/182/86/2486/er_1110-2-1156.pdf#page=518" ;
    pav:wasDerivedFrom "glossaries/CivilWorks/ER-1110-2-1156.yaml#term[Residual Risk]" ;
    skos:definition "The remaining level of risk at any time before, during and after a program of risk mitigation measures has been taken." ;
    skos:inScheme ER-1110-2-1156: ;
    skos:prefLabel "Residual Risk" .

ER-1110-2-1156:Resilience a wov:GlossaryTerm,
        skos:Concept ;
    rdfs:label "Resilience" ;
    dcterms:bibliographicCitation "https://www.publications.usace.army.mil/Portals/76/Users/182/86/2486/er_1110-2-1156.pdf#page=518" ;
    pav:wasDerivedFrom "glossaries/CivilWorks/ER-1110-2-1156.yaml#term[Resilience]" ;
    skos:definition "The ability to avoid, minimize, withstand, and recover from the effects of adversity, whether natural or manmade, under all circumstances of use." ;
    skos:inScheme ER-1110-2-1156: ;
    skos:prefLabel "Resilience" .

ER-1110-2-1156:Riprap a wov:GlossaryTerm,
        skos:Concept ;
    rdfs:label "Riprap" ;
    dcterms:bibliographicCitation "https://www.publications.usace.army.mil/Portals/76/Users/182/86/2486/er_1110-2-1156.pdf#page=518" ;
    pav:wasDerivedFrom "glossaries/CivilWorks/ER-1110-2-1156.yaml#term[Riprap]" ;
    skos:definition "A layer of large uncoursed stone, precast blocks, bags of cement, or other suitable material, generally placed on the upstream slopes of an embankment or along a watercourse as protection against wave action, erosion, or scour. Riprap is usually placed by dumping or other mechanical methods and in some cases is hand placed. It consists of pieces of relatively large size as distinguished from a gravel blanket. Also known as stone slope protection." ;
    skos:inScheme ER-1110-2-1156: ;
    skos:prefLabel "Riprap" .

ER-1110-2-1156:Risk a wov:GlossaryTerm,
        skos:Concept ;
    rdfs:label "Risk" ;
    dcterms:bibliographicCitation "https://www.publications.usace.army.mil/Portals/76/Users/182/86/2486/er_1110-2-1156.pdf#page=518" ;
    pav:wasDerivedFrom "glossaries/CivilWorks/ER-1110-2-1156.yaml#term[Risk]" ;
    skos:definition "A measure of the probability and severity of undesirable consequences or outcome." ;
    skos:inScheme ER-1110-2-1156: ;
    skos:prefLabel "Risk" .

ER-1110-2-1156:Risk-informed a wov:GlossaryTerm,
        skos:Concept ;
    rdfs:label "Risk-informed" ;
    dcterms:bibliographicCitation "https://www.publications.usace.army.mil/Portals/76/Users/182/86/2486/er_1110-2-1156.pdf#page=519" ;
    pav:wasDerivedFrom "glossaries/CivilWorks/ER-1110-2-1156.yaml#term[Risk-informed]" ;
    skos:definition "Risk information will play a key role in decisions related to dam safety but will not be the only information to influence the final decisions." ;
    skos:inScheme ER-1110-2-1156: ;
    skos:prefLabel "Risk-informed" .

ER-1110-2-1156:Risk_Characterization a wov:GlossaryTerm,
        skos:Concept ;
    rdfs:label "Risk Characterization" ;
    dcterms:bibliographicCitation "https://www.publications.usace.army.mil/Portals/76/Users/182/86/2486/er_1110-2-1156.pdf#page=519" ;
    pav:wasDerivedFrom "glossaries/CivilWorks/ER-1110-2-1156.yaml#term[Risk Characterization]" ;
    skos:definition "Risk characterization is the qualitative or quantitative description of the nature, magnitude and likelihood of the adverse effects associated with a hazard with and without a risk management action. A risk characterization often includes: one or more estimates of risk; risk descriptions; evaluations of risk management options; economic and other evaluations; estimates of changes in risk attributable to the management options." ;
    skos:inScheme ER-1110-2-1156: ;
    skos:prefLabel "Risk Characterization" .

ER-1110-2-1156:Risk_Communication a wov:GlossaryTerm,
        skos:Concept ;
    rdfs:label "Risk Communication" ;
    dcterms:bibliographicCitation "https://www.publications.usace.army.mil/Portals/76/Users/182/86/2486/er_1110-2-1156.pdf#page=519" ;
    pav:wasDerivedFrom "glossaries/CivilWorks/ER-1110-2-1156.yaml#term[Risk Communication]" ;
    skos:definition "Risk communication is the open, two-way exchange of information and opinion about hazards and risks leading to a better understanding of the risks and better risk management decisions." ;
    skos:inScheme ER-1110-2-1156: ;
    skos:prefLabel "Risk Communication" .

ER-1110-2-1156:Risk_Engine a wov:GlossaryTerm,
        skos:Concept ;
    rdfs:label "Risk Engine" ;
    dcterms:bibliographicCitation "https://www.publications.usace.army.mil/Portals/76/Users/182/86/2486/er_1110-2-1156.pdf#page=519" ;
    pav:wasDerivedFrom "glossaries/CivilWorks/ER-1110-2-1156.yaml#term[Risk Engine]" ;
    skos:definition "Software and computational algorithms either commercially available or under development by USACE that is used to construct an event tree for a plausible failure mode and automatically calculate the estimated risk." ;
    skos:inScheme ER-1110-2-1156: ;
    skos:prefLabel "Risk Engine" .

ER-1110-2-1156:Risk_Estimate a wov:GlossaryTerm,
        skos:Concept ;
    rdfs:label "Risk Estimate" ;
    dcterms:bibliographicCitation "https://www.publications.usace.army.mil/Portals/76/Users/182/86/2486/er_1110-2-1156.pdf#page=519" ;
    pav:wasDerivedFrom "glossaries/CivilWorks/ER-1110-2-1156.yaml#term[Risk Estimate]" ;
    skos:definition "The end result risk evaluation generated by application of a risk engine to the credible failure mode under study." ;
    skos:inScheme ER-1110-2-1156: ;
    skos:prefLabel "Risk Estimate" .

ER-1110-2-1156:Risk_Exposure a wov:GlossaryTerm,
        skos:Concept ;
    rdfs:label "Risk Exposure" ;
    dcterms:bibliographicCitation "https://www.publications.usace.army.mil/Portals/76/Users/182/86/2486/er_1110-2-1156.pdf#page=519" ;
    pav:wasDerivedFrom "glossaries/CivilWorks/ER-1110-2-1156.yaml#term[Risk Exposure]" ;
    skos:definition "The population, infrastructure, and other assets and valued resources that would be adversely impact from a dam failure." ;
    skos:inScheme ER-1110-2-1156: ;
    skos:prefLabel "Risk Exposure" .

ER-1110-2-1156:Risk_Management_Center_%28RMC%29 a wov:GlossaryTerm,
        skos:Concept ;
    rdfs:label "Risk Management Center (RMC)" ;
    dcterms:bibliographicCitation "https://www.publications.usace.army.mil/Portals/76/Users/182/86/2486/er_1110-2-1156.pdf#page=519" ;
    pav:wasDerivedFrom "glossaries/CivilWorks/ER-1110-2-1156.yaml#term[Risk Management Center (RMC)]" ;
    skos:altLabel "RMC" ;
    skos:definition "An independent USACE Center assigned to the Institute for Water Resources, which is responsible for development and implementation of dam and levee safety policy, prioritization of national dam and levee safety projects and technical consistency of dam and levee safety products. The Center utilizes a combination of in-situ and virtual resources (district, contract, the Modeling, Mapping, and Consequence Production Center, and Policy and Procedures workgroups) to manage the program." ;
    skos:inScheme ER-1110-2-1156: ;
    skos:prefLabel "Risk Management Center (RMC)" .

ER-1110-2-1156:Risk_Reduction_Measure a wov:GlossaryTerm,
        skos:Concept ;
    rdfs:label "Risk Reduction Measure" ;
    dcterms:bibliographicCitation "https://www.publications.usace.army.mil/Portals/76/Users/182/86/2486/er_1110-2-1156.pdf#page=519" ;
    pav:wasDerivedFrom "glossaries/CivilWorks/ER-1110-2-1156.yaml#term[Risk Reduction Measure]" ;
    skos:definition "Actions formulated and undertaken to reduce risk." ;
    skos:inScheme ER-1110-2-1156: ;
    skos:prefLabel "Risk Reduction Measure" .

ER-1110-2-1156:Risk_assessment a wov:GlossaryTerm,
        skos:Concept ;
    rdfs:label "Risk assessment" ;
    dcterms:bibliographicCitation "https://www.publications.usace.army.mil/Portals/76/Users/182/86/2486/er_1110-2-1156.pdf#page=518" ;
    pav:wasDerivedFrom "glossaries/CivilWorks/ER-1110-2-1156.yaml#term[Risk assessment]" ;
    skos:definition "Risk assessment is a broad term that encompasses a variety of analytic techniques that are used in different situations, depending upon the nature of the risk, the available data, and needs of decision makers. A risk assessment is a systematic, evidence based approach for quantifying and describing the nature, likelihood, and magnitude of risk associated with the current condition and the same values resulting from a changed condition due to some action. Risk assessment includes explicit acknowledgment of the uncertainties in the risk. As applied to dam safety, the process of identifying the likelihood and consequences of dam failure to provide the basis for informed decisions on a course of action." ;
    skos:inScheme ER-1110-2-1156: ;
    skos:prefLabel "Risk assessment" .

ER-1110-2-1156:Risk_management a wov:GlossaryTerm,
        skos:Concept ;
    rdfs:label "Risk management" ;
    dcterms:bibliographicCitation "https://www.publications.usace.army.mil/Portals/76/Users/182/86/2486/er_1110-2-1156.pdf#page=519" ;
    pav:wasDerivedFrom "glossaries/CivilWorks/ER-1110-2-1156.yaml#term[Risk management]" ;
    skos:definition "Risk management is the process of problem finding and initiating action to identify, evaluate, select, implement, monitor and modify actions taken to alter levels of risk, as compared to taking no action. The purpose of risk management is to choose and prioritize work required to reduce risk." ;
    skos:inScheme ER-1110-2-1156: ;
    skos:prefLabel "Risk management" .

ER-1110-2-1156:Risk_to_Tolerable_Levels a wov:GlossaryTerm,
        skos:Concept ;
    rdfs:label "Risk to Tolerable Levels" ;
    dcterms:bibliographicCitation "https://www.publications.usace.army.mil/Portals/76/Users/182/86/2486/er_1110-2-1156.pdf#page=519" ;
    pav:wasDerivedFrom "glossaries/CivilWorks/ER-1110-2-1156.yaml#term[Risk to Tolerable Levels]" ;
    skos:definition "In context, this refers to implementing dam safety risk reduction measures such that the resulting risk is 'tolerable' as shown graphically in figure 5.1. Generally is the outcome of application of the ALARP (As Low As Reasonably Possible) considerations." ;
    skos:inScheme ER-1110-2-1156: ;
    skos:prefLabel "Risk to Tolerable Levels" .

ER-1110-2-1156:Robustness a wov:GlossaryTerm,
        skos:Concept ;
    rdfs:label "Robustness" ;
    dcterms:bibliographicCitation "https://www.publications.usace.army.mil/Portals/76/Users/182/86/2486/er_1110-2-1156.pdf#page=520" ;
    pav:wasDerivedFrom "glossaries/CivilWorks/ER-1110-2-1156.yaml#term[Robustness]" ;
    skos:definition "Robustness is the ability of a system to continue to operate correctly across a wide range of operational conditions, with minimal damage, alteration or loss of functionality, and to fail gracefully outside of that range. The wider the range of conditions included, the more robust the system." ;
    skos:inScheme ER-1110-2-1156: ;
    skos:prefLabel "Robustness" .

ER-1110-2-1156:Rock_anchor a wov:GlossaryTerm,
        skos:Concept ;
    rdfs:label "Rock anchor" ;
    dcterms:bibliographicCitation "https://www.publications.usace.army.mil/Portals/76/Users/182/86/2486/er_1110-2-1156.pdf#page=520" ;
    pav:wasDerivedFrom "glossaries/CivilWorks/ER-1110-2-1156.yaml#term[Rock anchor]" ;
    skos:definition "A steel rod or cable placed in a hole drilled in rock, held in position by grout, mechanical means, or both. In principle, the same as a rock bolt, but usually the rock anchor is more than 4 meters long." ;
    skos:inScheme ER-1110-2-1156: ;
    skos:prefLabel "Rock anchor" .

ER-1110-2-1156:Rock_bolt a wov:GlossaryTerm,
        skos:Concept ;
    rdfs:label "Rock bolt" ;
    dcterms:bibliographicCitation "https://www.publications.usace.army.mil/Portals/76/Users/182/86/2486/er_1110-2-1156.pdf#page=520" ;
    pav:wasDerivedFrom "glossaries/CivilWorks/ER-1110-2-1156.yaml#term[Rock bolt]" ;
    skos:definition "A steel rod placed in a hole drilled in rock, held in position by grout, mechanical means, or both. A rock bolt can be tensioned." ;
    skos:inScheme ER-1110-2-1156: ;
    skos:prefLabel "Rock bolt" .

ER-1110-2-1156:Roller_drum_gate a wov:GlossaryTerm,
        skos:Concept ;
    rdfs:label "Roller drum gate" ;
    dcterms:bibliographicCitation "https://www.publications.usace.army.mil/Portals/76/Users/182/86/2486/er_1110-2-1156.pdf#page=506" ;
    pav:wasDerivedFrom "glossaries/CivilWorks/ER-1110-2-1156.yaml#term[Roller drum gate]" ;
    skos:definition "See drum gate." ;
    skos:inScheme ER-1110-2-1156: ;
    skos:prefLabel "Roller drum gate" .

ER-1110-2-1156:Roller_gate a wov:GlossaryTerm,
        skos:Concept ;
    rdfs:label "Roller gate" ;
    dcterms:bibliographicCitation "https://www.publications.usace.army.mil/Portals/76/Users/182/86/2486/er_1110-2-1156.pdf#page=506" ;
    pav:wasDerivedFrom "glossaries/CivilWorks/ER-1110-2-1156.yaml#term[Roller gate]" ;
    skos:altLabel "stoney gate" ;
    skos:definition "A gate for large openings that bears on a train of rollers in each gate guide." ;
    skos:inScheme ER-1110-2-1156: ;
    skos:prefLabel "Roller gate" .

ER-1110-2-1156:Run-up a wov:GlossaryTerm,
        skos:Concept ;
    rdfs:label "Run-up" ;
    dcterms:bibliographicCitation "https://www.publications.usace.army.mil/Portals/76/Users/182/86/2486/er_1110-2-1156.pdf#page=520" ;
    pav:wasDerivedFrom "glossaries/CivilWorks/ER-1110-2-1156.yaml#term[Run-up]" ;
    skos:definition "The vertical distance above the setup that the rush of water reaches when a wave breaks on the dam embankment." ;
    skos:inScheme ER-1110-2-1156: ;
    skos:prefLabel "Run-up" .

ER-1110-2-1156:Safe_%28Unsafe%29 a wov:GlossaryTerm,
        skos:Concept ;
    rdfs:label "Safe (Unsafe)" ;
    dcterms:bibliographicCitation "https://www.publications.usace.army.mil/Portals/76/Users/182/86/2486/er_1110-2-1156.pdf#page=520" ;
    pav:wasDerivedFrom "glossaries/CivilWorks/ER-1110-2-1156.yaml#term[Safe (Unsafe)]" ;
    skos:definition "Involving little or no chance of dam failure. Meets all required USACE guidelines and criteria." ;
    skos:inScheme ER-1110-2-1156: ;
    skos:prefLabel "Safe (Unsafe)" .

ER-1110-2-1156:Safety a wov:GlossaryTerm,
        skos:Concept ;
    rdfs:label "Safety" ;
    dcterms:bibliographicCitation "https://www.publications.usace.army.mil/Portals/76/Users/182/86/2486/er_1110-2-1156.pdf#page=520" ;
    pav:wasDerivedFrom "glossaries/CivilWorks/ER-1110-2-1156.yaml#term[Safety]" ;
    skos:definition "Safety is thought of as the condition of being free from danger, risk, or injury. However, safety is not something that can be absolutely achieved or guaranteed. Instead safety is the condition to which risks are managed to acceptable levels. Therefore, safety is a subjective concept based on individual perceptions of risks and their tolerability" ;
    skos:inScheme ER-1110-2-1156: ;
    skos:prefLabel "Safety" .

ER-1110-2-1156:Safety_Assurance_Review_Team a wov:GlossaryTerm,
        skos:Concept ;
    rdfs:label "Safety Assurance Review Team" ;
    dcterms:bibliographicCitation "https://www.publications.usace.army.mil/Portals/76/Users/182/86/2486/er_1110-2-1156.pdf#page=520" ;
    pav:wasDerivedFrom "glossaries/CivilWorks/ER-1110-2-1156.yaml#term[Safety Assurance Review Team]" ;
    skos:definition "Section 2035, Safety assurance review team, Public Law 110-114, the Water Resource Development Act of 2007, requires a safety assurance review of the design and construction of work effecting public safety. This review team is formed at the time pre-construction engineering and design starts and stays with the project until the completion of construction." ;
    skos:inScheme ER-1110-2-1156: ;
    skos:prefLabel "Safety Assurance Review Team" .

ER-1110-2-1156:Screening_for_Portfolio_Risk_Analysis_%28SPRA%29 a wov:GlossaryTerm,
        skos:Concept ;
    rdfs:label "Screening for Portfolio Risk Analysis (SPRA)" ;
    dcterms:bibliographicCitation "https://www.publications.usace.army.mil/Portals/76/Users/182/86/2486/er_1110-2-1156.pdf#page=520" ;
    pav:wasDerivedFrom "glossaries/CivilWorks/ER-1110-2-1156.yaml#term[Screening for Portfolio Risk Analysis (SPRA)]" ;
    skos:altLabel "SPRA" ;
    skos:definition "This analysis screened projects based on available information, to expeditiously identify the highest risk dams requiring urgent and compelling action (Dam Safety Action Classification 1 and 2 Dams) with low chance of missing any such dams Also, the SPRA is to provide information for preliminary classification of the remainder of the USACE dams into Dam Safety Action Classes 3 - 4. SPRA does not provide sufficient information to confirm whether a dam can be placed in Dam Safety Action Classification Class 5. SPRA will be performed only once for every dam in the USACE inventory. Risk estimates that are computed from SPRA are a relative measure only to compare dams across the USACE portfolio. Decisions and actions relative to tolerable risk cannot be made solely from SPRA results." ;
    skos:inScheme ER-1110-2-1156: ;
    skos:prefLabel "Screening for Portfolio Risk Analysis (SPRA)" .

ER-1110-2-1156:Section_1203_-_Dam_Safety_Assurance_Cost_Sharing a wov:GlossaryTerm,
        skos:Concept ;
    rdfs:label "Section 1203 - Dam Safety Assurance Cost Sharing" ;
    dcterms:bibliographicCitation "https://www.publications.usace.army.mil/Portals/76/Users/182/86/2486/er_1110-2-1156.pdf#page=520" ;
    pav:wasDerivedFrom "glossaries/CivilWorks/ER-1110-2-1156.yaml#term[Section 1203 - Dam Safety Assurance Cost Sharing]" ;
    skos:definition "Section 1203, WRDA, 1986 (reference A.12) provides for special cost-sharing for modification of completed USACE dam projects that are potential safety hazards in light of current engineering standards and criteria. The problems that meet the criteria of Section 1203 fall into three main categories: hydrologic, seismic, and change in state-of-the-art. (Modifications required on a project due to state-of-the-art changes, but not related to hydrologic or seismic deficiencies, must be decided on a case-by-case basis by the ASA(CW). Costs incurred in modifications for dam safety assurance must be recovered in accordance with provisions of the statute." ;
    skos:inScheme ER-1110-2-1156: ;
    skos:prefLabel "Section 1203 - Dam Safety Assurance Cost Sharing" .

ER-1110-2-1156:Seepage a wov:GlossaryTerm,
        skos:Concept ;
    rdfs:label "Seepage" ;
    dcterms:bibliographicCitation "https://www.publications.usace.army.mil/Portals/76/Users/182/86/2486/er_1110-2-1156.pdf#page=521" ;
    pav:wasDerivedFrom "glossaries/CivilWorks/ER-1110-2-1156.yaml#term[Seepage]" ;
    skos:definition "Flow through porous media." ;
    skos:inScheme ER-1110-2-1156: ;
    skos:prefLabel "Seepage" .

ER-1110-2-1156:Significant_Failure_Modes a wov:GlossaryTerm,
        skos:Concept ;
    rdfs:label "Significant Failure Modes" ;
    dcterms:bibliographicCitation "https://www.publications.usace.army.mil/Portals/76/Users/182/86/2486/er_1110-2-1156.pdf#page=521" ;
    pav:wasDerivedFrom "glossaries/CivilWorks/ER-1110-2-1156.yaml#term[Significant Failure Modes]" ;
    skos:definition "Significant failure modes are a subset of credible failure modes (i.e. physically possible). The term significant should be judged in the context of the purpose of the risk assessment and the decisions that it will inform. Factors to consider include Dam Safety Action Classification, comparisons with tolerable risk guidelines, scoping the next level of study, portfolio roll-up of the risk estimates, the level of confidence in risk estimates, representation of uncertainty in estimates, and prioritization for next phase of work. For example credible failure mode should be considered significant if the probability of failure and associated consequences approach closely or exceed a tolerable risk limit guideline." ;
    skos:inScheme ER-1110-2-1156: ;
    skos:prefLabel "Significant Failure Modes" .

ER-1110-2-1156:Significant_wave_height a wov:GlossaryTerm,
        skos:Concept ;
    rdfs:label "Significant wave height" ;
    dcterms:bibliographicCitation "https://www.publications.usace.army.mil/Portals/76/Users/182/86/2486/er_1110-2-1156.pdf#page=521" ;
    pav:wasDerivedFrom "glossaries/CivilWorks/ER-1110-2-1156.yaml#term[Significant wave height]" ;
    skos:definition "The average height of the one-third highest waves of a given wave group." ;
    skos:inScheme ER-1110-2-1156: ;
    skos:prefLabel "Significant wave height" .

ER-1110-2-1156:Sill a wov:GlossaryTerm,
        skos:Concept ;
    rdfs:label "Sill" ;
    dcterms:bibliographicCitation "https://www.publications.usace.army.mil/Portals/76/Users/182/86/2486/er_1110-2-1156.pdf#page=521" ;
    pav:wasDerivedFrom "glossaries/CivilWorks/ER-1110-2-1156.yaml#term[Sill]" ;
    skos:definition "A submerged structure across a river to control the water level upstream. The crest of a spillway. A horizontal gate seating, made of wood, stone, concrete, or metal at the invert of any opening or gap in a structure; hence, the expressions gate sill and stoplog sill." ;
    skos:inScheme ER-1110-2-1156: ;
    skos:prefLabel "Sill" .

ER-1110-2-1156:Skimmer_gate a wov:GlossaryTerm,
        skos:Concept ;
    rdfs:label "Skimmer gate" ;
    dcterms:bibliographicCitation "https://www.publications.usace.army.mil/Portals/76/Users/182/86/2486/er_1110-2-1156.pdf#page=506" ;
    pav:wasDerivedFrom "glossaries/CivilWorks/ER-1110-2-1156.yaml#term[Skimmer gate]" ;
    skos:definition "A gate at the spillway crest whose prime purpose is to control the release of debris and logs with a limited amount of water. It is usually a bottom hinged flap or Bascule gate." ;
    skos:inScheme ER-1110-2-1156: ;
    skos:prefLabel "Skimmer gate" .

ER-1110-2-1156:Slide_gate a wov:GlossaryTerm,
        skos:Concept ;
    rdfs:label "Slide gate" ;
    dcterms:bibliographicCitation "https://www.publications.usace.army.mil/Portals/76/Users/182/86/2486/er_1110-2-1156.pdf#page=506" ;
    pav:wasDerivedFrom "glossaries/CivilWorks/ER-1110-2-1156.yaml#term[Slide gate]" ;
    skos:altLabel "sluice gate" ;
    skos:definition "A gate that can be opened or closed by sliding in supporting guides." ;
    skos:inScheme ER-1110-2-1156: ;
    skos:prefLabel "Slide gate" .

ER-1110-2-1156:Slope a wov:GlossaryTerm,
        skos:Concept ;
    rdfs:label "Slope" ;
    dcterms:bibliographicCitation "https://www.publications.usace.army.mil/Portals/76/Users/182/86/2486/er_1110-2-1156.pdf#page=521" ;
    pav:wasDerivedFrom "glossaries/CivilWorks/ER-1110-2-1156.yaml#term[Slope]" ;
    skos:definition "Inclination from the horizontal. Sometimes referred to as batter when measured from vertical." ;
    skos:inScheme ER-1110-2-1156: ;
    skos:prefLabel "Slope" .

ER-1110-2-1156:Sluice a wov:GlossaryTerm,
        skos:Concept ;
    rdfs:label "Sluice" ;
    dcterms:bibliographicCitation "https://www.publications.usace.army.mil/Portals/76/Users/182/86/2486/er_1110-2-1156.pdf#page=521" ;
    pav:wasDerivedFrom "glossaries/CivilWorks/ER-1110-2-1156.yaml#term[Sluice]" ;
    skos:definition "An opening for releasing water from below the static head elevation." ;
    skos:inScheme ER-1110-2-1156: ;
    skos:prefLabel "Sluice" .

ER-1110-2-1156:Societal_Risk a wov:GlossaryTerm,
        skos:Concept ;
    rdfs:label "Societal Risk" ;
    dcterms:bibliographicCitation "https://www.publications.usace.army.mil/Portals/76/Users/182/86/2486/er_1110-2-1156.pdf#page=521" ;
    pav:wasDerivedFrom "glossaries/CivilWorks/ER-1110-2-1156.yaml#term[Societal Risk]" ;
    skos:definition "The risk of widespread or large scale detriment from the realization of a defined risk, the implication being that the consequence would be on such a scale as to provoke a socio/political response, and/or that the risk (that is, the likelihood combined with the consequence) provokes public discussion and is effectively regulated by society as a whole through its political processes and regulatory mechanisms. Such large risks are typically unevenly distributed, as are their attendant benefits. Thus the construction of a dam represents a risk to those close by and a benefit to those further off, or a process may harm some future generation more than the present one. The distribution and balancing of such major costs and benefits is a classic function of Government, subject to public discussion and discussion (HSE, 1995 reference A.144) and (ANCOLD October 2003) (reference A.130)." ;
    skos:inScheme ER-1110-2-1156: ;
    skos:prefLabel "Societal Risk" .

ER-1110-2-1156:Societal_incremental_life_safety_tolerable_risk_guideline a wov:GlossaryTerm,
        skos:Concept ;
    rdfs:label "Societal incremental life safety tolerable risk guideline" ;
    dcterms:bibliographicCitation "https://www.publications.usace.army.mil/Portals/76/Users/182/86/2486/er_1110-2-1156.pdf#page=521" ;
    pav:wasDerivedFrom "glossaries/CivilWorks/ER-1110-2-1156.yaml#term[Societal incremental life safety tolerable risk guideline]" ;
    skos:definition "For existing dams, the societal risk should be less than the limit line shown in the chart of societal risk guideline for existing dams, except in extraordinary circumstances, following an adaptation of the ANCOLD (2003) (reference A.130) and NSW(2006) (reference A.147) societal life safety risk guideline. For new dams or Section 216 major modifications (reference A.7), the societal risk should be less than the limit line shown in the chart for societal risk guideline for new dams and Section 216 major modifications (reference A.7), except in extraordinary circumstances, following an adaptation of the ANCOLD (2003) (reference A.130) and NSW (2006) (reference A.147) societal life safety risk guideline. Societal risks are to be lower than the limit lines to an extent determined in accordance with the ALARP principle." ;
    skos:inScheme ER-1110-2-1156: ;
    skos:prefLabel "Societal incremental life safety tolerable risk guideline" .

ER-1110-2-1156:Special_Assistant_for_Dam_and_Levee_Safety a wov:GlossaryTerm,
        skos:Concept ;
    rdfs:label "Special Assistant for Dam and Levee Safety" ;
    dcterms:bibliographicCitation "https://www.publications.usace.army.mil/Portals/76/Users/182/86/2486/er_1110-2-1156.pdf#page=522" ;
    pav:wasDerivedFrom "glossaries/CivilWorks/ER-1110-2-1156.yaml#term[Special Assistant for Dam and Levee Safety]" ;
    skos:definition "Acts for the USACE DSO in the execution of daily program activities and serves as Chairman of the DSSC and the DSOG. The Special Assistant must be a registered professional civil engineer with management abilities, be competent in the areas related to the design, construction, or evaluation of dams and understand adverse dam incidents and the potential causes and consequences of dam failure. The Special Assistant works for and reports directly to the USACE DSO and represents the USACE DSO in the development of the budget submission, working with the appropriate Business Line Managers and the RMC to ensure that dam safety priorities are addressed. The Special Assistant serves as the Department of Defense and/or USACE representative on various national teams as directed by the USACE DSO." ;
    skos:inScheme ER-1110-2-1156: ;
    skos:prefLabel "Special Assistant for Dam and Levee Safety" .

ER-1110-2-1156:Spillway a wov:GlossaryTerm,
        skos:Concept ;
    rdfs:label "Spillway" ;
    dcterms:bibliographicCitation "https://www.publications.usace.army.mil/Portals/76/Users/182/86/2486/er_1110-2-1156.pdf#page=522" ;
    pav:wasDerivedFrom "glossaries/CivilWorks/ER-1110-2-1156.yaml#term[Spillway]" ;
    skos:definition "A structure over or through which flow is discharged from a reservoir. If the rate of flow is controlled by mechanical means such as gates, it is considered a controlled spillway. If the geometry of the spillway is the only control, it is considered an uncontrolled spillway." ;
    skos:inScheme ER-1110-2-1156: ;
    skos:prefLabel "Spillway" .

<https://usace-data.com/civil-works/glossary/ER-1110-2-1156#Spillway,_auxiliary> a wov:GlossaryTerm,
        skos:Concept ;
    rdfs:label "Spillway, auxiliary" ;
    dcterms:bibliographicCitation "https://www.publications.usace.army.mil/Portals/76/Users/182/86/2486/er_1110-2-1156.pdf#page=522" ;
    pav:wasDerivedFrom "glossaries/CivilWorks/ER-1110-2-1156.yaml#term[Spillway, auxiliary]" ;
    skos:definition "Any secondary spillway, which is designed to be operated very infrequently and possibly in anticipation of some degree of structural damage or erosion to the spillway during operation." ;
    skos:inScheme ER-1110-2-1156: ;
    skos:prefLabel "Spillway, auxiliary" .

<https://usace-data.com/civil-works/glossary/ER-1110-2-1156#Spillway,_fuse_plug> a wov:GlossaryTerm,
        skos:Concept ;
    rdfs:label "Spillway, fuse plug" ;
    dcterms:bibliographicCitation "https://www.publications.usace.army.mil/Portals/76/Users/182/86/2486/er_1110-2-1156.pdf#page=522" ;
    pav:wasDerivedFrom "glossaries/CivilWorks/ER-1110-2-1156.yaml#term[Spillway, fuse plug]" ;
    skos:definition "A form of auxiliary spillway consisting of a low embankment designed to be overtopped and washed away during an exceptionally large flood." ;
    skos:inScheme ER-1110-2-1156: ;
    skos:prefLabel "Spillway, fuse plug" .

<https://usace-data.com/civil-works/glossary/ER-1110-2-1156#Spillway,_primary_%28or_service%29> a wov:GlossaryTerm,
        skos:Concept ;
    rdfs:label "Spillway, primary (or service)" ;
    dcterms:bibliographicCitation "https://www.publications.usace.army.mil/Portals/76/Users/182/86/2486/er_1110-2-1156.pdf#page=522" ;
    pav:wasDerivedFrom "glossaries/CivilWorks/ER-1110-2-1156.yaml#term[Spillway, primary (or service)]" ;
    skos:definition "A spillway designed to provide continuous or frequent releases from a reservoir without significant damage to either the dam or its appurtenant structures." ;
    skos:inScheme ER-1110-2-1156: ;
    skos:prefLabel "Spillway, primary (or service)" .

<https://usace-data.com/civil-works/glossary/ER-1110-2-1156#Spillway,_shaft> a wov:GlossaryTerm,
        skos:Concept ;
    rdfs:label "Spillway, shaft" ;
    dcterms:bibliographicCitation "https://www.publications.usace.army.mil/Portals/76/Users/182/86/2486/er_1110-2-1156.pdf#page=523" ;
    pav:wasDerivedFrom "glossaries/CivilWorks/ER-1110-2-1156.yaml#term[Spillway, shaft]" ;
    skos:definition "A vertical or inclined shaft into which water spills and then is conveyed through, under, or around a dam by means of a conduit or tunnel. If the upper part of the shaft is splayed cut and terminates in a circular horizontal weir, it is termed a bellmouth or morning glory spillway." ;
    skos:inScheme ER-1110-2-1156: ;
    skos:prefLabel "Spillway, shaft" .

ER-1110-2-1156:Spillway_Design_Flood_%28SDF%29 a wov:GlossaryTerm,
        skos:Concept ;
    rdfs:label "Spillway Design Flood (SDF)" ;
    dcterms:bibliographicCitation "https://www.publications.usace.army.mil/Portals/76/Users/182/86/2486/er_1110-2-1156.pdf#page=522" ;
    pav:wasDerivedFrom "glossaries/CivilWorks/ER-1110-2-1156.yaml#term[Spillway Design Flood (SDF)]" ;
    skos:altLabel "SDF" ;
    skos:definition "See Flood, Inflow Design." ;
    skos:inScheme ER-1110-2-1156: ;
    skos:prefLabel "Spillway Design Flood (SDF)" .

ER-1110-2-1156:Spillway_channel a wov:GlossaryTerm,
        skos:Concept ;
    rdfs:label "Spillway channel" ;
    dcterms:bibliographicCitation "https://www.publications.usace.army.mil/Portals/76/Users/182/86/2486/er_1110-2-1156.pdf#page=522" ;
    pav:wasDerivedFrom "glossaries/CivilWorks/ER-1110-2-1156.yaml#term[Spillway channel]" ;
    skos:definition "An open channel or closed conduit conveying water from the spillway inlet downstream." ;
    skos:inScheme ER-1110-2-1156: ;
    skos:prefLabel "Spillway channel" .

ER-1110-2-1156:Spillway_chute a wov:GlossaryTerm,
        skos:Concept ;
    rdfs:label "Spillway chute" ;
    dcterms:bibliographicCitation "https://www.publications.usace.army.mil/Portals/76/Users/182/86/2486/er_1110-2-1156.pdf#page=522" ;
    pav:wasDerivedFrom "glossaries/CivilWorks/ER-1110-2-1156.yaml#term[Spillway chute]" ;
    skos:definition "A steeply sloping spillway channel that conveys discharges at supercritical velocities." ;
    skos:inScheme ER-1110-2-1156: ;
    skos:prefLabel "Spillway chute" .

ER-1110-2-1156:Spillway_crest a wov:GlossaryTerm,
        skos:Concept ;
    rdfs:label "Spillway crest" ;
    dcterms:bibliographicCitation "https://www.publications.usace.army.mil/Portals/76/Users/182/86/2486/er_1110-2-1156.pdf#page=522" ;
    pav:wasDerivedFrom "glossaries/CivilWorks/ER-1110-2-1156.yaml#term[Spillway crest]" ;
    skos:definition "The lowest level at which water can flow over or through the spillway." ;
    skos:inScheme ER-1110-2-1156: ;
    skos:prefLabel "Spillway crest" .

ER-1110-2-1156:Stakeholders a wov:GlossaryTerm,
        skos:Concept ;
    rdfs:label "Stakeholders" ;
    dcterms:bibliographicCitation "https://www.publications.usace.army.mil/Portals/76/Users/182/86/2486/er_1110-2-1156.pdf#page=523" ;
    pav:wasDerivedFrom "glossaries/CivilWorks/ER-1110-2-1156.yaml#term[Stakeholders]" ;
    skos:definition "Elected, and agency officials, public and private individuals and groups that have a direct stake in the subject matter under consideration." ;
    skos:inScheme ER-1110-2-1156: ;
    skos:prefLabel "Stakeholders" .

ER-1110-2-1156:Stilling_basin a wov:GlossaryTerm,
        skos:Concept ;
    rdfs:label "Stilling basin" ;
    dcterms:bibliographicCitation "https://www.publications.usace.army.mil/Portals/76/Users/182/86/2486/er_1110-2-1156.pdf#page=523" ;
    pav:wasDerivedFrom "glossaries/CivilWorks/ER-1110-2-1156.yaml#term[Stilling basin]" ;
    skos:definition "A basin constructed to dissipate the energy of rapidly flowing water, e.g., from a spillway or outlet, and to protect the riverbed from erosion." ;
    skos:inScheme ER-1110-2-1156: ;
    skos:prefLabel "Stilling basin" .

ER-1110-2-1156:Stoplogs a wov:GlossaryTerm,
        skos:Concept ;
    rdfs:label "Stoplogs" ;
    dcterms:bibliographicCitation "https://www.publications.usace.army.mil/Portals/76/Users/182/86/2486/er_1110-2-1156.pdf#page=523" ;
    pav:wasDerivedFrom "glossaries/CivilWorks/ER-1110-2-1156.yaml#term[Stoplogs]" ;
    skos:definition "Large logs, timbers, metal beams, or metal frames placed on top of each other with their ends held in guides on each side of a channel or conduit so as to provide a cheaper or more easily handled means of temporary closure than a bulkhead gate." ;
    skos:inScheme ER-1110-2-1156: ;
    skos:prefLabel "Stoplogs" .

ER-1110-2-1156:Storage a wov:GlossaryTerm,
        skos:Concept ;
    rdfs:label "Storage" ;
    dcterms:bibliographicCitation "https://www.publications.usace.army.mil/Portals/76/Users/182/86/2486/er_1110-2-1156.pdf#page=523" ;
    pav:wasDerivedFrom "glossaries/CivilWorks/ER-1110-2-1156.yaml#term[Storage]" ;
    skos:definition "The retention of water or delay of runoff either by planned operation, as in a reservoir, or by temporary filling of overflow areas, as in the progression of a flood wave through a natural stream channel. Definitions of specific types of storage in reservoirs are:" ;
    skos:inScheme ER-1110-2-1156: ;
    skos:prefLabel "Storage" .

ER-1110-2-1156:Surcharge a wov:GlossaryTerm,
        skos:Concept ;
    rdfs:label "Surcharge" ;
    dcterms:bibliographicCitation "https://www.publications.usace.army.mil/Portals/76/Users/182/86/2486/er_1110-2-1156.pdf#page=523" ;
    pav:wasDerivedFrom "glossaries/CivilWorks/ER-1110-2-1156.yaml#term[Surcharge]" ;
    skos:definition "Any storage above the full pool." ;
    skos:inScheme ER-1110-2-1156: ;
    skos:prefLabel "Surcharge" .

ER-1110-2-1156:Tailrace a wov:GlossaryTerm,
        skos:Concept ;
    rdfs:label "Tailrace" ;
    dcterms:bibliographicCitation "https://www.publications.usace.army.mil/Portals/76/Users/182/86/2486/er_1110-2-1156.pdf#page=523" ;
    pav:wasDerivedFrom "glossaries/CivilWorks/ER-1110-2-1156.yaml#term[Tailrace]" ;
    skos:definition "The tunnel, channel, or conduit that conveys the discharge from the turbine to the river; hence, the terms tailrace tunnel and tailrace canal." ;
    skos:inScheme ER-1110-2-1156: ;
    skos:prefLabel "Tailrace" .

ER-1110-2-1156:Tailwater_level a wov:GlossaryTerm,
        skos:Concept ;
    rdfs:label "Tailwater level" ;
    dcterms:bibliographicCitation "https://www.publications.usace.army.mil/Portals/76/Users/182/86/2486/er_1110-2-1156.pdf#page=523" ;
    pav:wasDerivedFrom "glossaries/CivilWorks/ER-1110-2-1156.yaml#term[Tailwater level]" ;
    skos:definition "The level of water in the tailrace at the nearest free surface to the turbine or in the discharge channel immediately downstream of the dam." ;
    skos:inScheme ER-1110-2-1156: ;
    skos:prefLabel "Tailwater level" .

ER-1110-2-1156:Threshold_Flood a wov:GlossaryTerm,
        skos:Concept ;
    rdfs:label "Threshold Flood" ;
    dcterms:bibliographicCitation "https://www.publications.usace.army.mil/Portals/76/Users/182/86/2486/er_1110-2-1156.pdf#page=524" ;
    pav:wasDerivedFrom "glossaries/CivilWorks/ER-1110-2-1156.yaml#term[Threshold Flood]" ;
    skos:definition "The flood that fully utilizes the existing dam, i.e., the flood that just exceeds the design maximum water surface elevation at the dam." ;
    skos:inScheme ER-1110-2-1156: ;
    skos:prefLabel "Threshold Flood" .

ER-1110-2-1156:Thrust_block a wov:GlossaryTerm,
        skos:Concept ;
    rdfs:label "Thrust block" ;
    dcterms:bibliographicCitation "https://www.publications.usace.army.mil/Portals/76/Users/182/86/2486/er_1110-2-1156.pdf#page=524" ;
    pav:wasDerivedFrom "glossaries/CivilWorks/ER-1110-2-1156.yaml#term[Thrust block]" ;
    skos:definition "A massive block of concrete built to withstand a thrust or pull." ;
    skos:inScheme ER-1110-2-1156: ;
    skos:prefLabel "Thrust block" .

ER-1110-2-1156:Toe_of_dam a wov:GlossaryTerm,
        skos:Concept ;
    rdfs:label "Toe of dam" ;
    dcterms:bibliographicCitation "https://www.publications.usace.army.mil/Portals/76/Users/182/86/2486/er_1110-2-1156.pdf#page=524" ;
    pav:wasDerivedFrom "glossaries/CivilWorks/ER-1110-2-1156.yaml#term[Toe of dam]" ;
    skos:definition "The junction of the face of a dam with the ground surface. For concrete dams, see heel." ;
    skos:inScheme ER-1110-2-1156: ;
    skos:prefLabel "Toe of dam" .

ER-1110-2-1156:Tolerable_Risk a wov:GlossaryTerm,
        skos:Concept ;
    rdfs:label "Tolerable Risk" ;
    dcterms:bibliographicCitation "https://www.publications.usace.army.mil/Portals/76/Users/182/86/2486/er_1110-2-1156.pdf#page=524" ;
    pav:wasDerivedFrom "glossaries/CivilWorks/ER-1110-2-1156.yaml#term[Tolerable Risk]" ;
    skos:definition "A risk within a range that society can live with so as to secure the benefits provided by the dam. It is a range of risk that we do not regard as negligible or as something we might ignore, but rather as something we need to keep under review and reduce it still further if and as we can (HSE, 1999 reference A.145). In addition to the tolerable risk limit the ALARP considerations will be applied to determine tolerable risk." ;
    skos:inScheme ER-1110-2-1156: ;
    skos:prefLabel "Tolerable Risk" .

ER-1110-2-1156:Tolerable_Risk_Guidelines a wov:GlossaryTerm,
        skos:Concept ;
    rdfs:label "Tolerable Risk Guidelines" ;
    dcterms:bibliographicCitation "https://www.publications.usace.army.mil/Portals/76/Users/182/86/2486/er_1110-2-1156.pdf#page=524" ;
    pav:wasDerivedFrom "glossaries/CivilWorks/ER-1110-2-1156.yaml#term[Tolerable Risk Guidelines]" ;
    skos:definition "Tolerable risk guidelines are used in risk management to guide the process of examining and judging the significance of estimated risks obtained using risk assessment. The outcomes of risk assessment are inputs to the risk management decision process along with other considerations. Meeting or achieving the tolerable risk guidelines is the goal for all risk reduction measures including permanent and interim measures." ;
    skos:inScheme ER-1110-2-1156: ;
    skos:prefLabel "Tolerable Risk Guidelines" .

ER-1110-2-1156:Tolerable_Risk_Limit a wov:GlossaryTerm,
        skos:Concept ;
    rdfs:label "Tolerable Risk Limit" ;
    dcterms:bibliographicCitation "https://www.publications.usace.army.mil/Portals/76/Users/182/86/2486/er_1110-2-1156.pdf#page=524" ;
    pav:wasDerivedFrom "glossaries/CivilWorks/ER-1110-2-1156.yaml#term[Tolerable Risk Limit]" ;
    skos:definition "Tolerable risk limit, as depicted on Figure 5.1, defines the limit separating the unacceptable risk region from the range of tolerability." ;
    skos:inScheme ER-1110-2-1156: ;
    skos:prefLabel "Tolerable Risk Limit" .

ER-1110-2-1156:Top_of_dam a wov:GlossaryTerm,
        skos:Concept ;
    rdfs:label "Top of dam" ;
    dcterms:bibliographicCitation "https://www.publications.usace.army.mil/Portals/76/Users/182/86/2486/er_1110-2-1156.pdf#page=524" ;
    pav:wasDerivedFrom "glossaries/CivilWorks/ER-1110-2-1156.yaml#term[Top of dam]" ;
    skos:definition "The elevation of the uppermost surface of a dam, usually a road or walkway excluding any parapet wall, railing, etc." ;
    skos:inScheme ER-1110-2-1156: ;
    skos:prefLabel "Top of dam" .

ER-1110-2-1156:Trashrack a wov:GlossaryTerm,
        skos:Concept ;
    rdfs:label "Trashrack" ;
    dcterms:bibliographicCitation "https://www.publications.usace.army.mil/Portals/76/Users/182/86/2486/er_1110-2-1156.pdf#page=524" ;
    pav:wasDerivedFrom "glossaries/CivilWorks/ER-1110-2-1156.yaml#term[Trashrack]" ;
    skos:definition "A device located at an intake to prevent floating or submerged debris from entering the intake." ;
    skos:inScheme ER-1110-2-1156: ;
    skos:prefLabel "Trashrack" .

ER-1110-2-1156:Tunnel a wov:GlossaryTerm,
        skos:Concept ;
    rdfs:label "Tunnel" ;
    dcterms:bibliographicCitation "https://www.publications.usace.army.mil/Portals/76/Users/182/86/2486/er_1110-2-1156.pdf#page=524" ;
    pav:wasDerivedFrom "glossaries/CivilWorks/ER-1110-2-1156.yaml#term[Tunnel]" ;
    skos:definition "A long underground excavation with two or more openings to the surface, usually having a uniform cross section used for access, conveying flows, etc." ;
    skos:inScheme ER-1110-2-1156: ;
    skos:prefLabel "Tunnel" .

ER-1110-2-1156:Type_II_IEPR a wov:GlossaryTerm,
        skos:Concept ;
    rdfs:label "Type II IEPR" ;
    dcterms:bibliographicCitation "https://www.publications.usace.army.mil/Portals/76/Users/182/86/2486/er_1110-2-1156.pdf#page=525" ;
    pav:wasDerivedFrom "glossaries/CivilWorks/ER-1110-2-1156.yaml#term[Type II IEPR]" ;
    skos:definition "A Safety Assurance Review (SAR) of design and construction activities for flood damage reduction or coastal storm damage reduction projects or for other activities that affect public safety, and will also be conducted for reviewing the relevancy and effectiveness of USACE inspection of completed works and safety programs in promoting safety and competent performance. They are not required to be managed by OEO's and may be managed by USACE, MSC, or by an outside organization. While all aspects of the project may be included in the review, it will focus on the public safety aspects." ;
    skos:inScheme ER-1110-2-1156: ;
    skos:prefLabel "Type II IEPR" .

ER-1110-2-1156:Type_I_IEPR a wov:GlossaryTerm,
        skos:Concept ;
    rdfs:label "Type I IEPR" ;
    dcterms:bibliographicCitation "https://www.publications.usace.army.mil/Portals/76/Users/182/86/2486/er_1110-2-1156.pdf#page=524" ;
    pav:wasDerivedFrom "glossaries/CivilWorks/ER-1110-2-1156.yaml#term[Type I IEPR]" ;
    skos:definition "An Independent External Peer Review conducted for feasibility, reevaluation, modification, and assessment reports with an EIS and managed by an outside eligible organization (OEO) that is described in Internal Revenue Code Section 501(c) (3); as exempt from Federal tax under section 501(a), of the Internal Revenue Code of 1986; as independent; as free from conflicts of interest; does not carry out or advocate for or against Federal water resources projects; and has experience in establishing and administering IEPR panels. These reviews are exempt from the Federal Advisory Committees Act (FACA). The scope of review will address all the underlying planning, engineering, including safety assurance, economics, and environmental analyses performed, not just one aspect of the project." ;
    skos:inScheme ER-1110-2-1156: ;
    skos:prefLabel "Type I IEPR" .

ER-1110-2-1156:Unacceptable_Level_of_Risk a wov:GlossaryTerm,
        skos:Concept ;
    rdfs:label "Unacceptable Level of Risk" ;
    dcterms:bibliographicCitation "https://www.publications.usace.army.mil/Portals/76/Users/182/86/2486/er_1110-2-1156.pdf#page=525" ;
    pav:wasDerivedFrom "glossaries/CivilWorks/ER-1110-2-1156.yaml#term[Unacceptable Level of Risk]" ;
    skos:definition "The risk cannot be justified except under extraordinary circumstances." ;
    skos:inScheme ER-1110-2-1156: ;
    skos:prefLabel "Unacceptable Level of Risk" .

ER-1110-2-1156:Unacceptable_Risk_Region a wov:GlossaryTerm,
        skos:Concept ;
    rdfs:label "Unacceptable Risk Region" ;
    dcterms:bibliographicCitation "https://www.publications.usace.army.mil/Portals/76/Users/182/86/2486/er_1110-2-1156.pdf#page=525" ;
    pav:wasDerivedFrom "glossaries/CivilWorks/ER-1110-2-1156.yaml#term[Unacceptable Risk Region]" ;
    skos:definition "The region within the risk range shown in figure 5.1 that is above the zone referred to as the 'Range of Tolerability'. In the 'Unacceptable Region' the risk is considered unacceptable and cannot be justified except in extraordinary circumstance HSE (2001) (reference A.146)" ;
    skos:inScheme ER-1110-2-1156: ;
    skos:prefLabel "Unacceptable Risk Region" .

ER-1110-2-1156:Uncertainty a wov:GlossaryTerm,
        skos:Concept ;
    rdfs:label "Uncertainty" ;
    dcterms:bibliographicCitation "https://www.publications.usace.army.mil/Portals/76/Users/182/86/2486/er_1110-2-1156.pdf#page=525" ;
    pav:wasDerivedFrom "glossaries/CivilWorks/ER-1110-2-1156.yaml#term[Uncertainty]" ;
    skos:definition "Uncertainty is the result of imperfect knowledge concerning the present or future state of a system, event, situation, or (sub) population under consideration. The level of uncertainty governs the confidence in predictions, inferences, or conclusions." ;
    skos:inScheme ER-1110-2-1156: ;
    skos:prefLabel "Uncertainty" .

ER-1110-2-1156:United_States_Society_on_Dams a wov:GlossaryTerm,
        skos:Concept ;
    rdfs:label "United States Society on Dams" ;
    dcterms:bibliographicCitation "https://www.publications.usace.army.mil/Portals/76/Users/182/86/2486/er_1110-2-1156.pdf#page=486" ;
    pav:wasDerivedFrom "glossaries/CivilWorks/ER-1110-2-1156.yaml#term[United States Society on Dams]" ;
    skos:altLabel "USCOLD",
        "USSD" ;
    skos:definition "United States Committee on Large Dams" ;
    skos:inScheme ER-1110-2-1156: ;
    skos:prefLabel "United States Society on Dams" .

ER-1110-2-1156:Unsafe a wov:GlossaryTerm,
        skos:Concept ;
    rdfs:label "Unsafe" ;
    dcterms:bibliographicCitation "https://www.publications.usace.army.mil/Portals/76/Users/182/86/2486/er_1110-2-1156.pdf#page=525" ;
    pav:wasDerivedFrom "glossaries/CivilWorks/ER-1110-2-1156.yaml#term[Unsafe]" ;
    skos:definition "Unacceptable chance of a dam failure." ;
    skos:inScheme ER-1110-2-1156: ;
    skos:prefLabel "Unsafe" .

ER-1110-2-1156:Uplift a wov:GlossaryTerm,
        skos:Concept ;
    rdfs:label "Uplift" ;
    dcterms:bibliographicCitation "https://www.publications.usace.army.mil/Portals/76/Users/182/86/2486/er_1110-2-1156.pdf#page=525" ;
    pav:wasDerivedFrom "glossaries/CivilWorks/ER-1110-2-1156.yaml#term[Uplift]" ;
    skos:definition "The uplift pressure in the pores of a material (interstitial pressure) or on the base of a structure." ;
    skos:inScheme ER-1110-2-1156: ;
    skos:prefLabel "Uplift" .

ER-1110-2-1156:Upstream_blanket a wov:GlossaryTerm,
        skos:Concept ;
    rdfs:label "Upstream blanket" ;
    dcterms:bibliographicCitation "https://www.publications.usace.army.mil/Portals/76/Users/182/86/2486/er_1110-2-1156.pdf#page=525" ;
    pav:wasDerivedFrom "glossaries/CivilWorks/ER-1110-2-1156.yaml#term[Upstream blanket]" ;
    skos:definition "An impervious blanket placed on the reservoir floor and abutments upstream of a dam. For an embankment dam, the blanket may be connected to the core." ;
    skos:inScheme ER-1110-2-1156: ;
    skos:prefLabel "Upstream blanket" .

ER-1110-2-1156:Valve a wov:GlossaryTerm,
        skos:Concept ;
    rdfs:label "Valve" ;
    dcterms:bibliographicCitation "https://www.publications.usace.army.mil/Portals/76/Users/182/86/2486/er_1110-2-1156.pdf#page=525" ;
    pav:wasDerivedFrom "glossaries/CivilWorks/ER-1110-2-1156.yaml#term[Valve]" ;
    skos:definition "A device fitted to a pipeline or orifice in which the closure member is either rotated or moved transversely or longitudinally in the waterway so as to control or stop the flow." ;
    skos:inScheme ER-1110-2-1156: ;
    skos:prefLabel "Valve" .

ER-1110-2-1156:Variability a wov:GlossaryTerm,
        skos:Concept ;
    rdfs:label "Variability" ;
    dcterms:bibliographicCitation "https://www.publications.usace.army.mil/Portals/76/Users/182/86/2486/er_1110-2-1156.pdf#page=526" ;
    pav:wasDerivedFrom "glossaries/CivilWorks/ER-1110-2-1156.yaml#term[Variability]" ;
    skos:definition "One of two components often thought of as comprising 'uncertainty'. Epistemic or 'knowledge uncertainty' that is possible to reduce with additional data and study; and aleatory or 'natural variability' that reflects a process that is random but uncertainty in its magnitude and values may not be reduced with additional data and study. Annual stream flow is an example of 'natural variability." ;
    skos:inScheme ER-1110-2-1156: ;
    skos:prefLabel "Variability" .

ER-1110-2-1156:Volume_of_dam a wov:GlossaryTerm,
        skos:Concept ;
    rdfs:label "Volume of dam" ;
    dcterms:bibliographicCitation "https://www.publications.usace.army.mil/Portals/76/Users/182/86/2486/er_1110-2-1156.pdf#page=526" ;
    pav:wasDerivedFrom "glossaries/CivilWorks/ER-1110-2-1156.yaml#term[Volume of dam]" ;
    skos:definition "The total space occupied by the materials forming the dam structure computed between abutments and from top to bottom of dam. No deduction is made for small openings such as galleries, adits, tunnels, and operating chambers within the dam structure. Portions of powerplants, locks, spillway, etc., should be included only if they are necessary for the structural stability of the dam." ;
    skos:inScheme ER-1110-2-1156: ;
    skos:prefLabel "Volume of dam" .

ER-1110-2-1156:WEDGE_Fund a wov:GlossaryTerm,
        skos:Concept ;
    rdfs:label "WEDGE Fund" ;
    dcterms:bibliographicCitation "https://www.publications.usace.army.mil/Portals/76/Users/182/86/2486/er_1110-2-1156.pdf#page=526" ;
    pav:wasDerivedFrom "glossaries/CivilWorks/ER-1110-2-1156.yaml#term[WEDGE Fund]" ;
    skos:definition "A special line item in the Construction Remaining items entitled Dam Safety Assurance and Seepage Stability Correction Program. Funding is provided to a project for investigation (study and report) and the start of construction for a dam safety modification while waiting for the current budget cycle project funding to become available." ;
    skos:inScheme ER-1110-2-1156: ;
    skos:prefLabel "WEDGE Fund" .

ER-1110-2-1156:Water_Control_System a wov:GlossaryTerm,
        skos:Concept ;
    rdfs:label "Water Control System" ;
    dcterms:bibliographicCitation "https://www.publications.usace.army.mil/Portals/76/Users/182/86/2486/er_1110-2-1156.pdf#page=526" ;
    pav:wasDerivedFrom "glossaries/CivilWorks/ER-1110-2-1156.yaml#term[Water Control System]" ;
    skos:definition "Any structure or group of structures and its appurtenant components that is used as part of a system to control or modify the conveyance of water such as gates, pumps, valves, motors, controls, power supply, etc." ;
    skos:inScheme ER-1110-2-1156: ;
    skos:prefLabel "Water Control System" .

ER-1110-2-1156:Watershed_divide a wov:GlossaryTerm,
        skos:Concept ;
    rdfs:label "Watershed divide" ;
    dcterms:bibliographicCitation "https://www.publications.usace.army.mil/Portals/76/Users/182/86/2486/er_1110-2-1156.pdf#page=526" ;
    pav:wasDerivedFrom "glossaries/CivilWorks/ER-1110-2-1156.yaml#term[Watershed divide]" ;
    skos:definition "The divide or boundary between catchment areas (or drainage areas)." ;
    skos:inScheme ER-1110-2-1156: ;
    skos:prefLabel "Watershed divide" .

ER-1110-2-1156:Waterstop a wov:GlossaryTerm,
        skos:Concept ;
    rdfs:label "Waterstop" ;
    dcterms:bibliographicCitation "https://www.publications.usace.army.mil/Portals/76/Users/182/86/2486/er_1110-2-1156.pdf#page=526" ;
    pav:wasDerivedFrom "glossaries/CivilWorks/ER-1110-2-1156.yaml#term[Waterstop]" ;
    skos:definition "A strip of metal, rubber, or other material used to prevent leakage through joints between adjacent sections of concrete." ;
    skos:inScheme ER-1110-2-1156: ;
    skos:prefLabel "Waterstop" .

ER-1110-2-1156:Wave_run-up a wov:GlossaryTerm,
        skos:Concept ;
    rdfs:label "Wave run-up" ;
    dcterms:bibliographicCitation "https://www.publications.usace.army.mil/Portals/76/Users/182/86/2486/er_1110-2-1156.pdf#page=526" ;
    pav:wasDerivedFrom "glossaries/CivilWorks/ER-1110-2-1156.yaml#term[Wave run-up]" ;
    skos:definition "Vertical height above the stillwater level to which water from a specific wave will run up the face of a structure or embankment." ;
    skos:inScheme ER-1110-2-1156: ;
    skos:prefLabel "Wave run-up" .

ER-1110-2-1156:Weir a wov:GlossaryTerm,
        skos:Concept ;
    rdfs:label "Weir" ;
    dcterms:bibliographicCitation "https://www.publications.usace.army.mil/Portals/76/Users/182/86/2486/er_1110-2-1156.pdf#page=526" ;
    pav:wasDerivedFrom "glossaries/CivilWorks/ER-1110-2-1156.yaml#term[Weir]" ;
    skos:definition "A notch of regular form through which water flows." ;
    skos:inScheme ER-1110-2-1156: ;
    skos:prefLabel "Weir" .

<https://usace-data.com/civil-works/glossary/ER-1110-2-1156#Weir,_broad-crested> a wov:GlossaryTerm,
        skos:Concept ;
    rdfs:label "Weir, broad-crested" ;
    dcterms:bibliographicCitation "https://www.publications.usace.army.mil/Portals/76/Users/182/86/2486/er_1110-2-1156.pdf#page=526" ;
    pav:wasDerivedFrom "glossaries/CivilWorks/ER-1110-2-1156.yaml#term[Weir, broad-crested]" ;
    skos:definition "An overflow structure on which the nape is supported for an appreciable length in the direction of flow." ;
    skos:inScheme ER-1110-2-1156: ;
    skos:prefLabel "Weir, broad-crested" .

<https://usace-data.com/civil-works/glossary/ER-1110-2-1156#Weir,_measuring> a wov:GlossaryTerm,
        skos:Concept ;
    rdfs:label "Weir, measuring" ;
    dcterms:bibliographicCitation "https://www.publications.usace.army.mil/Portals/76/Users/182/86/2486/er_1110-2-1156.pdf#page=526" ;
    pav:wasDerivedFrom "glossaries/CivilWorks/ER-1110-2-1156.yaml#term[Weir, measuring]" ;
    skos:definition "A device for measuring the rate of flow of water. It generally consists of a rectangular, trapezoidal, triangular, or other shaped notch, located in a vertical, thin plate over which water flows. The height of water above the weir crest is used to determine the rate of flow." ;
    skos:inScheme ER-1110-2-1156: ;
    skos:prefLabel "Weir, measuring" .

<https://usace-data.com/civil-works/glossary/ER-1110-2-1156#Weir,_ogee> a wov:GlossaryTerm,
        skos:Concept ;
    rdfs:label "Weir, ogee" ;
    dcterms:bibliographicCitation "https://www.publications.usace.army.mil/Portals/76/Users/182/86/2486/er_1110-2-1156.pdf#page=526" ;
    pav:wasDerivedFrom "glossaries/CivilWorks/ER-1110-2-1156.yaml#term[Weir, ogee]" ;
    skos:definition "A reverse curve, shaped like an elongated letter S. The downstream faces of overflow spillways are often made to this shape." ;
    skos:inScheme ER-1110-2-1156: ;
    skos:prefLabel "Weir, ogee" .

ER-1110-2-1156:Willingness-to-Pay-to-Prevent-a-Statistical-Fatality a wov:GlossaryTerm,
        skos:Concept ;
    rdfs:label "Willingness-to-Pay-to-Prevent-a-Statistical-Fatality" ;
    dcterms:bibliographicCitation "https://www.publications.usace.army.mil/Portals/76/Users/182/86/2486/er_1110-2-1156.pdf#page=526" ;
    pav:wasDerivedFrom "glossaries/CivilWorks/ER-1110-2-1156.yaml#term[Willingness-to-Pay-to-Prevent-a-Statistical-Fatality]" ;
    skos:definition "This is defined as the economic principle that attempts to place a value on a potential life lost by determining the willingness of society to pay to prevent a statistical fatality. Such values are determined from studies of court cases involving involuntary death, from Federal and other agency studies of establishing regulatory standards for public safety." ;
    skos:inScheme ER-1110-2-1156: ;
    skos:prefLabel "Willingness-to-Pay-to-Prevent-a-Statistical-Fatality" .

ER-1110-2-1156:Wind_setup a wov:GlossaryTerm,
        skos:Concept ;
    rdfs:label "Wind setup" ;
    dcterms:bibliographicCitation "https://www.publications.usace.army.mil/Portals/76/Users/182/86/2486/er_1110-2-1156.pdf#page=527" ;
    pav:wasDerivedFrom "glossaries/CivilWorks/ER-1110-2-1156.yaml#term[Wind setup]" ;
    skos:definition "The vertical rise in the stillwater level at the face of a structure or embankment caused by wind stresses on the surface of the water." ;
    skos:inScheme ER-1110-2-1156: ;
    skos:prefLabel "Wind setup" .

ER-1110-2-1156: a wov:Glossary,
        owl:Ontology,
        skos:ConceptScheme,
        voaf:Vocabulary ;
    rdfs:label "ER 1110-2-1156  - Safety of Dams - Policy and Procedures" ;
    dcterms:created "2024-07-16T13:37:41.522106+00:00"^^xsd:dateTime ;
    dcterms:description "The USACE Safety of Dams Policies and Procedures (Engineeering Report 1110-2-1156) defines various acronyms and terms commonly used in this regulation to describe phases, types, and parts of cost products. These terms are defined in the glossary section of the regulation." ;
    dcterms:publisher "None" ;
    dcterms:rights "MIT" ;
    dcterms:title "ER 1110-2-1156  - Safety of Dams - Policy and Procedures" ;
    pav:ImportedFrom "glossaries/CivilWorks/ER-1110-2-1156.yaml" ;
    pav:createdOn "2024-07-16T13:37:41.522106+00:00"^^xsd:dateTime ;
    pav:createdWith "gloss" ;
    pav:wasInfluencedBy "ER 1110-2-1156  - Safety of Dams - Policy and Procedures" ;
    vann:preferredNamespaceUri "https://usace-data.com/civil-works/glossary/ER-1110-2-1156#" ;
    skos:hasTopConcept ER-1110-2-1156:ATR_Team,
        ER-1110-2-1156:Abutment,
        ER-1110-2-1156:Acceptable_Risk,
        ER-1110-2-1156:Acre-foot,
        ER-1110-2-1156:Active_storage,
        ER-1110-2-1156:Adit,
        ER-1110-2-1156:Adverse_Consequences,
        ER-1110-2-1156:Agency_Technical_Review_%28ATR%29,
        ER-1110-2-1156:Annual_Inspections,
        ER-1110-2-1156:Annual_Probability_of_Failure_%28APF%29,
        ER-1110-2-1156:Appurtenant_structure,
        ER-1110-2-1156:As-Low-As-Reasonably-Practicable_%28ALARP%29,
        ER-1110-2-1156:Automatically_Operated_System,
        ER-1110-2-1156:Average_Annual_Life_Lost_%28AALL%29,
        ER-1110-2-1156:Axis_of_dam,
        ER-1110-2-1156:Baffle_block,
        ER-1110-2-1156:Bascule_gate,
        ER-1110-2-1156:Base_thickness,
        ER-1110-2-1156:Batter,
        ER-1110-2-1156:Bedrock,
        ER-1110-2-1156:Berm,
        ER-1110-2-1156:Borrow_Area,
        ER-1110-2-1156:Breach,
        ER-1110-2-1156:Broadly_Acceptable_Risk,
        ER-1110-2-1156:Bulkhead_gate,
        ER-1110-2-1156:Caretaker_Status,
        ER-1110-2-1156:Catastrophe,
        ER-1110-2-1156:Channel,
        ER-1110-2-1156:Cofferdam,
        ER-1110-2-1156:Combined_Annual_Probability_of_all_Failure_Modes,
        ER-1110-2-1156:Compaction,
        ER-1110-2-1156:Component_Risks,
        ER-1110-2-1156:Conditional_Load_Response_Probabilities,
        ER-1110-2-1156:Conditional_System_Response_Probability_Estimates,
        ER-1110-2-1156:Conduit,
        ER-1110-2-1156:Confirmed_%28Unconfirmed%29,
        ER-1110-2-1156:Confirmed_Dam_Safety_Issues,
        ER-1110-2-1156:Conservation_Pool,
        ER-1110-2-1156:Constructability_evaluation_%28CE%29,
        ER-1110-2-1156:Construction_Joint,
        ER-1110-2-1156:Contact_Grouting,
        ER-1110-2-1156:Contractor_Quality_Control_%28CQC%29,
        ER-1110-2-1156:Core,
        ER-1110-2-1156:Core_Wall,
        ER-1110-2-1156:Cost-to-Save-a-Statistical-Life_%28CSSL%29,
        ER-1110-2-1156:Credible_Existing_and_Future_Without_Federal_Action_Risk_Estimate,
        ER-1110-2-1156:Crest_gate,
        ER-1110-2-1156:Crest_of_dam,
        ER-1110-2-1156:Critical_feature,
        ER-1110-2-1156:Critically_near_failure,
        ER-1110-2-1156:Cross_section,
        ER-1110-2-1156:Cutoff_trench,
        ER-1110-2-1156:Cutoff_wall,
        ER-1110-2-1156:DSAC_1_%28Very_High_Urgency%29,
        ER-1110-2-1156:DSAC_2_%28High_Urgency%29,
        ER-1110-2-1156:DSAC_3_%28Moderate_Urgency%29,
        ER-1110-2-1156:DSAC_4_%28Low_Urgency%29,
        ER-1110-2-1156:DSAC_5_%28Normal%29,
        ER-1110-2-1156:Dam,
        ER-1110-2-1156:Dam_Safety,
        ER-1110-2-1156:Dam_Safety_Action_Classification_%28DSAC%29_System,
        ER-1110-2-1156:Dam_Safety_Committee,
        ER-1110-2-1156:Dam_Safety_Deficiency,
        ER-1110-2-1156:Dam_Safety_Issue,
        ER-1110-2-1156:Dam_Safety_Modification,
        ER-1110-2-1156:Dam_Safety_Modification_%28DSM%29_Lead_Engineer,
        ER-1110-2-1156:Dam_Safety_Modification_Risk_Assessment,
        ER-1110-2-1156:Dam_Safety_Modification_Study,
        ER-1110-2-1156:Dam_Safety_Officer,
        ER-1110-2-1156:Dam_Safety_Portfolio_Risk_Management,
        ER-1110-2-1156:Dam_Safety_Program_Management_Tools,
        ER-1110-2-1156:Dam_Safety_Program_Manager_%28DSPM%29,
        ER-1110-2-1156:Dam_Safety_Steering_Committee_%28DSSC%29,
        ER-1110-2-1156:Dam_Senior_Oversight_Group_%28DSOG%29,
        ER-1110-2-1156:Dam_failure,
        ER-1110-2-1156:Dam_safety_preparedness,
        ER-1110-2-1156:Damming_Surface,
        ER-1110-2-1156:Dead_storage,
        ER-1110-2-1156:Design_Structural_Capacity,
        ER-1110-2-1156:Design_water_level,
        ER-1110-2-1156:Design_wind,
        ER-1110-2-1156:Diaphragm_wall,
        ER-1110-2-1156:Dike,
        ER-1110-2-1156:Direct_Economic_Losses,
        <https://usace-data.com/civil-works/glossary/ER-1110-2-1156#Diversion_channel,_canal,_or_tunnel>,
        <https://usace-data.com/civil-works/glossary/ER-1110-2-1156#Drain,_blanket>,
        <https://usace-data.com/civil-works/glossary/ER-1110-2-1156#Drain,_chimney>,
        <https://usace-data.com/civil-works/glossary/ER-1110-2-1156#Drain,_toe>,
        ER-1110-2-1156:Drainage_area,
        ER-1110-2-1156:Drainage_curtain,
        ER-1110-2-1156:Drawdown,
        ER-1110-2-1156:Drum_gate,
        ER-1110-2-1156:Earthquake,
        <https://usace-data.com/civil-works/glossary/ER-1110-2-1156#Earthquake,_Maximum_Credible_%28MCE%29>,
        <https://usace-data.com/civil-works/glossary/ER-1110-2-1156#Earthquake,_Maximum_Design_%28MDE%29>,
        <https://usace-data.com/civil-works/glossary/ER-1110-2-1156#Earthquake,_Operating_Basis_%28OBE%29>,
        <https://usace-data.com/civil-works/glossary/ER-1110-2-1156#Earthquake,_Safety_Evaluation_%28SEE%29>,
        <https://usace-data.com/civil-works/glossary/ER-1110-2-1156#Earthquake,_synthetic>,
        ER-1110-2-1156:Economic_Consequences,
        ER-1110-2-1156:Economic_Damages,
        ER-1110-2-1156:Economic_Regret,
        ER-1110-2-1156:Efficiency,
        ER-1110-2-1156:Embankment,
        ER-1110-2-1156:Emergency,
        ER-1110-2-1156:Emergency_Action_Plan_%28EAP%29,
        ER-1110-2-1156:Emergency_Exercise,
        ER-1110-2-1156:Emergency_gate,
        ER-1110-2-1156:Endangered_Species_Act_%28ESA%29,
        ER-1110-2-1156:Energy_dissipater,
        ER-1110-2-1156:Environmental_Impact_Statement_%28EIS%29,
        ER-1110-2-1156:Environmental_and_other_Non-monetary_Consequences,
        ER-1110-2-1156:Epicenter,
        ER-1110-2-1156:Equity_in_Risk_Management,
        ER-1110-2-1156:Essential_Agency_Guidelines,
        ER-1110-2-1156:Event_Tree%28s%29,
        ER-1110-2-1156:Existing_Condition_Component_Risk_Estimates,
        ER-1110-2-1156:Existing_Condition_Risk_Estimate,
        ER-1110-2-1156:Existing_and_Future_Condition_Without_Federal_Action_Consequence_Analysis,
        ER-1110-2-1156:Exposure_Assessment,
        ER-1110-2-1156:F-N_chart,
        ER-1110-2-1156:Failure_Mode,
        ER-1110-2-1156:Failure_of_a_Water_Control_System,
        ER-1110-2-1156:Fault,
        <https://usace-data.com/civil-works/glossary/ER-1110-2-1156#Fault,_active>,
        <https://usace-data.com/civil-works/glossary/ER-1110-2-1156#Fault,_capable>,
        ER-1110-2-1156:Fetch,
        ER-1110-2-1156:Filter_%28filter_zone%29,
        ER-1110-2-1156:Fixed_wheel_gate,
        ER-1110-2-1156:Flap_gate,
        ER-1110-2-1156:Flashboards,
        ER-1110-2-1156:Flip_bucket,
        ER-1110-2-1156:Flood,
        <https://usace-data.com/civil-works/glossary/ER-1110-2-1156#Flood,_Inflow_Design_%28IDF%29>,
        <https://usace-data.com/civil-works/glossary/ER-1110-2-1156#Flood,_Probable_Maximum_%28PMF%29>,
        <https://usace-data.com/civil-works/glossary/ER-1110-2-1156#Flood,_Safety_Evaluation_%28SEF%29>,
        <https://usace-data.com/civil-works/glossary/ER-1110-2-1156#Flood,_antecedent>,
        <https://usace-data.com/civil-works/glossary/ER-1110-2-1156#Flood,_base_safety_standard_%28BSS%29>,
        ER-1110-2-1156:Flood_Control,
        ER-1110-2-1156:Flood_Damage_Reduction,
        ER-1110-2-1156:Flood_Level,
        ER-1110-2-1156:Flood_Risk_Management,
        ER-1110-2-1156:Flood_gate,
        ER-1110-2-1156:Flood_routing,
        ER-1110-2-1156:Flood_surcharge,
        ER-1110-2-1156:Floodplain,
        ER-1110-2-1156:Freeboard,
        ER-1110-2-1156:Full_pool,
        ER-1110-2-1156:Future_Without_Federal_Action_Condition,
        ER-1110-2-1156:Gallery,
        ER-1110-2-1156:Gantry_crane,
        ER-1110-2-1156:Gate,
        ER-1110-2-1156:Gate_chamber,
        ER-1110-2-1156:Geotextiles,
        ER-1110-2-1156:Groin,
        ER-1110-2-1156:Grout,
        ER-1110-2-1156:Grout_blanket,
        ER-1110-2-1156:Grout_cap,
        ER-1110-2-1156:Grout_curtain,
        ER-1110-2-1156:HAZUS,
        ER-1110-2-1156:Hazard,
        ER-1110-2-1156:Hazard_Characterization,
        ER-1110-2-1156:Hazard_Identification,
        ER-1110-2-1156:Hazard_potential_classification,
        <https://usace-data.com/civil-works/glossary/ER-1110-2-1156#Head,_static>,
        <https://usace-data.com/civil-works/glossary/ER-1110-2-1156#Head,_velocity>,
        ER-1110-2-1156:Headrace,
        ER-1110-2-1156:Heel,
        <https://usace-data.com/civil-works/glossary/ER-1110-2-1156#Height,_above_ground>,
        <https://usace-data.com/civil-works/glossary/ER-1110-2-1156#Height,_dam>,
        <https://usace-data.com/civil-works/glossary/ER-1110-2-1156#Height,_hydraulic>,
        <https://usace-data.com/civil-works/glossary/ER-1110-2-1156#Height,_structural>,
        ER-1110-2-1156:Hollow_jet_valve,
        ER-1110-2-1156:Inactive_storage,
        ER-1110-2-1156:Incident,
        ER-1110-2-1156:Inclinometer,
        ER-1110-2-1156:Incremental_consequences,
        ER-1110-2-1156:Independent_External_Peer_Review_Team,
        ER-1110-2-1156:Independent_Technical_Review_%28ITR%29,
        ER-1110-2-1156:Indirect_Economic_Impacts,
        ER-1110-2-1156:Individual_Risk,
        ER-1110-2-1156:Individual_incremental_life_safety_tolerable_risk_guideline_%28ANCOLD%29,
        ER-1110-2-1156:Initial_reservoir_filling,
        ER-1110-2-1156:Institute_for_Water_Resources,
        ER-1110-2-1156:Instrumentation,
        ER-1110-2-1156:Intake,
        ER-1110-2-1156:Intangible_Consequences,
        ER-1110-2-1156:Interagency_Committee_on_Dam_Safety,
        ER-1110-2-1156:Interim_Risk_Reduction_Measure_%28IRRM%29,
        ER-1110-2-1156:Interim_Risk_Reduction_Measures_Plans_%28IRRMP%29,
        ER-1110-2-1156:Interlock,
        ER-1110-2-1156:Internal_Erosion,
        ER-1110-2-1156:Intervention,
        ER-1110-2-1156:Inundation_map,
        ER-1110-2-1156:Issue_Evaluation_Studies,
        ER-1110-2-1156:Lead_Engineer,
        ER-1110-2-1156:Leakage,
        ER-1110-2-1156:Length_of_dam,
        ER-1110-2-1156:Levee,
        ER-1110-2-1156:Life_Loss_Consequences,
        ER-1110-2-1156:Life_Loss_Estimates,
        ER-1110-2-1156:Life_Safety_Tolerable_Risk_Guidelines,
        ER-1110-2-1156:Lifeline_Systems,
        ER-1110-2-1156:Lifelines,
        ER-1110-2-1156:Likelihood,
        ER-1110-2-1156:Limit_Line_for_Life_Safety,
        ER-1110-2-1156:Limit_of_Tolerability,
        ER-1110-2-1156:Liquefaction,
        ER-1110-2-1156:Live_storage,
        ER-1110-2-1156:Locally_Controlled_System,
        ER-1110-2-1156:Logboom,
        ER-1110-2-1156:Maximum_flood_control_level,
        ER-1110-2-1156:Maximum_pool,
        ER-1110-2-1156:Maximum_wave,
        ER-1110-2-1156:Minimum_operating_level,
        ER-1110-2-1156:National_Dam_Safety_Review_Board,
        ER-1110-2-1156:National_Environmental_Policy_Act_%28NEPA%29,
        ER-1110-2-1156:National_Inventory_of_Dams,
        ER-1110-2-1156:Non-Structural_Risk_Reduction,
        ER-1110-2-1156:Normal_Operations,
        ER-1110-2-1156:Observation_well,
        ER-1110-2-1156:Operation_restrictions,
        ER-1110-2-1156:Outlet,
        ER-1110-2-1156:Outlet_gate,
        ER-1110-2-1156:Outlet_works,
        ER-1110-2-1156:Parametric_Studies,
        ER-1110-2-1156:Parapet_wall,
        ER-1110-2-1156:Peer_Review,
        ER-1110-2-1156:Peer_Review_Panel,
        ER-1110-2-1156:Penstock,
        ER-1110-2-1156:Performance_Evaluation,
        ER-1110-2-1156:Performance_Uncertainty,
        ER-1110-2-1156:Periodic_Assessments_%28PA%29,
        ER-1110-2-1156:Periodic_Inspections_%28PI%29,
        ER-1110-2-1156:Phreatic_surface,
        ER-1110-2-1156:Piezometer,
        ER-1110-2-1156:Piping,
        ER-1110-2-1156:Plunge_pool,
        ER-1110-2-1156:Population_at_Risk,
        ER-1110-2-1156:Pore_water_pressure,
        ER-1110-2-1156:Portfolio_Risk_Management_Process,
        ER-1110-2-1156:Potential_Failure_Mode_%28PFM%29,
        ER-1110-2-1156:Potential_Failure_Mode_Analysis_%28PFMA%29,
        ER-1110-2-1156:Probability,
        ER-1110-2-1156:Probability_of_Failure,
        ER-1110-2-1156:Probability_of_Individual_Life_Loss,
        ER-1110-2-1156:Probable_Maximum_Precipitation_%28PMP%29,
        ER-1110-2-1156:Pumped_storage_reservoir,
        ER-1110-2-1156:Quality_%28as_related_to_construction%29,
        ER-1110-2-1156:Quality_Assurance_%28QA%29,
        ER-1110-2-1156:Quality_Management,
        ER-1110-2-1156:Radial_gate,
        ER-1110-2-1156:Rapid_Consequence_Analysis%2FEstimate,
        ER-1110-2-1156:Redundancy,
        ER-1110-2-1156:Regional_Cadres,
        ER-1110-2-1156:Regulating_gate,
        ER-1110-2-1156:Regulating_sleeve_valve,
        ER-1110-2-1156:Regulation_Design_Capacity,
        ER-1110-2-1156:Reliability,
        ER-1110-2-1156:Remediation,
        ER-1110-2-1156:Remotely_Controlled_System,
        ER-1110-2-1156:Remotely_Operated_System,
        ER-1110-2-1156:Reservoir,
        ER-1110-2-1156:Reservoir_capacity,
        ER-1110-2-1156:Reservoir_regulation_%28or_operating%29_procedure,
        ER-1110-2-1156:Reservoir_surface_area,
        ER-1110-2-1156:Residual_Risk,
        ER-1110-2-1156:Resilience,
        ER-1110-2-1156:Riprap,
        ER-1110-2-1156:Risk,
        ER-1110-2-1156:Risk-informed,
        ER-1110-2-1156:Risk_Characterization,
        ER-1110-2-1156:Risk_Communication,
        ER-1110-2-1156:Risk_Engine,
        ER-1110-2-1156:Risk_Estimate,
        ER-1110-2-1156:Risk_Exposure,
        ER-1110-2-1156:Risk_Management_Center_%28RMC%29,
        ER-1110-2-1156:Risk_Reduction_Measure,
        ER-1110-2-1156:Risk_assessment,
        ER-1110-2-1156:Risk_management,
        ER-1110-2-1156:Risk_to_Tolerable_Levels,
        ER-1110-2-1156:Robustness,
        ER-1110-2-1156:Rock_anchor,
        ER-1110-2-1156:Rock_bolt,
        ER-1110-2-1156:Roller_drum_gate,
        ER-1110-2-1156:Roller_gate,
        ER-1110-2-1156:Run-up,
        ER-1110-2-1156:Safe_%28Unsafe%29,
        ER-1110-2-1156:Safety,
        ER-1110-2-1156:Safety_Assurance_Review_Team,
        ER-1110-2-1156:Screening_for_Portfolio_Risk_Analysis_%28SPRA%29,
        ER-1110-2-1156:Section_1203_-_Dam_Safety_Assurance_Cost_Sharing,
        ER-1110-2-1156:Seepage,
        ER-1110-2-1156:Significant_Failure_Modes,
        ER-1110-2-1156:Significant_wave_height,
        ER-1110-2-1156:Sill,
        ER-1110-2-1156:Skimmer_gate,
        ER-1110-2-1156:Slide_gate,
        ER-1110-2-1156:Slope,
        ER-1110-2-1156:Sluice,
        ER-1110-2-1156:Societal_Risk,
        ER-1110-2-1156:Societal_incremental_life_safety_tolerable_risk_guideline,
        ER-1110-2-1156:Special_Assistant_for_Dam_and_Levee_Safety,
        ER-1110-2-1156:Spillway,
        <https://usace-data.com/civil-works/glossary/ER-1110-2-1156#Spillway,_auxiliary>,
        <https://usace-data.com/civil-works/glossary/ER-1110-2-1156#Spillway,_fuse_plug>,
        <https://usace-data.com/civil-works/glossary/ER-1110-2-1156#Spillway,_primary_%28or_service%29>,
        <https://usace-data.com/civil-works/glossary/ER-1110-2-1156#Spillway,_shaft>,
        ER-1110-2-1156:Spillway_Design_Flood_%28SDF%29,
        ER-1110-2-1156:Spillway_channel,
        ER-1110-2-1156:Spillway_chute,
        ER-1110-2-1156:Spillway_crest,
        ER-1110-2-1156:Stakeholders,
        ER-1110-2-1156:Stilling_basin,
        ER-1110-2-1156:Stoplogs,
        ER-1110-2-1156:Storage,
        ER-1110-2-1156:Surcharge,
        ER-1110-2-1156:Tailrace,
        ER-1110-2-1156:Tailwater_level,
        ER-1110-2-1156:Threshold_Flood,
        ER-1110-2-1156:Thrust_block,
        ER-1110-2-1156:Toe_of_dam,
        ER-1110-2-1156:Tolerable_Risk,
        ER-1110-2-1156:Tolerable_Risk_Guidelines,
        ER-1110-2-1156:Tolerable_Risk_Limit,
        ER-1110-2-1156:Top_of_dam,
        ER-1110-2-1156:Trashrack,
        ER-1110-2-1156:Tunnel,
        ER-1110-2-1156:Type_II_IEPR,
        ER-1110-2-1156:Type_I_IEPR,
        ER-1110-2-1156:Unacceptable_Level_of_Risk,
        ER-1110-2-1156:Unacceptable_Risk_Region,
        ER-1110-2-1156:Uncertainty,
        ER-1110-2-1156:United_States_Society_on_Dams,
        ER-1110-2-1156:Unsafe,
        ER-1110-2-1156:Uplift,
        ER-1110-2-1156:Upstream_blanket,
        ER-1110-2-1156:Valve,
        ER-1110-2-1156:Variability,
        ER-1110-2-1156:Volume_of_dam,
        ER-1110-2-1156:WEDGE_Fund,
        ER-1110-2-1156:Water_Control_System,
        ER-1110-2-1156:Watershed_divide,
        ER-1110-2-1156:Waterstop,
        ER-1110-2-1156:Wave_run-up,
        ER-1110-2-1156:Weir,
        <https://usace-data.com/civil-works/glossary/ER-1110-2-1156#Weir,_broad-crested>,
        <https://usace-data.com/civil-works/glossary/ER-1110-2-1156#Weir,_measuring>,
        <https://usace-data.com/civil-works/glossary/ER-1110-2-1156#Weir,_ogee>,
        ER-1110-2-1156:Willingness-to-Pay-to-Prevent-a-Statistical-Fatality,
        ER-1110-2-1156:Wind_setup .

