@prefix ER-37-1-30-P12: <https://usace-data.com/civil-works/glossary/ER-37-1-30-P12#> .
@prefix dcterms: <http://purl.org/dc/terms/> .
@prefix owl: <http://www.w3.org/2002/07/owl#> .
@prefix pav: <http://purl.org/pav#> .
@prefix rdfs: <http://www.w3.org/2000/01/rdf-schema#> .
@prefix skos: <http://www.w3.org/2004/02/skos/core#> .
@prefix vann: <http://purl.org/vocab/vann/> .
@prefix voaf: <https://lov.linkeddata.es/vocommons/voaf/v2.0/voaf_v2.0.rdf#> .
@prefix wov: <http://www.knowledgesmarts.com/ontologies/wov#> .
@prefix xsd: <http://www.w3.org/2001/XMLSchema#> .

ER-37-1-30-P12:ADA_Reporting_Procedures a wov:GlossaryTerm,
        skos:Concept ;
    rdfs:label "ADA Reporting Procedures" ;
    dcterms:bibliographicCitation "https://www.publications.usace.army.mil/Portals/76/Users/182/86/2486/ER%2037-1-30.pdf#page=36" ;
    pav:wasDerivedFrom "glossaries/CivilWorks/ER-37-1-30-P12.yaml#term[ADA Reporting Procedures]" ;
    skos:definition "The purpose of a potential ADA violation investigation is to determine if a violation has occurred. An ADA investigation is initiated by the applicable assigned individual or team and must be reported to the Army as required. One of the most important outcomes of an ADA investigation is preparing necessary reports." ;
    skos:inScheme ER-37-1-30-P12: ;
    skos:prefLabel "ADA Reporting Procedures" .

ER-37-1-30-P12:ADA_Violations a wov:GlossaryTerm,
        skos:Concept ;
    rdfs:label "ADA Violations" ;
    dcterms:bibliographicCitation "https://www.publications.usace.army.mil/Portals/76/Users/182/86/2486/ER%2037-1-30.pdf#page=35" ;
    pav:wasDerivedFrom "glossaries/CivilWorks/ER-37-1-30-P12.yaml#term[ADA Violations]" ;
    skos:definition """The three ADA statutes most frequently cited are title 31 USC sections 1341, 1342, and 1517. Section 1341 prohibits a federal employee from making or authorizing an expenditure or obligation exceeding an amount available in an appropriation or fund. Section 1342 prohibits a federal employee from accepting voluntary services except for emergencies involving the safety of human life or the protection of property. Similar to section 1341, section 1517 prohibits federal employees from making or authorizing an expenditure or obligation exceeding an apportionment or formal administrative subdivision of funds. Not all alleged violations unfold as actual violations of the ADA statutes; the alleged violations however represent trouble areas or pitfalls to be avoided.
Any officer or employee of the United States is prohibited from:
a. Making or authorizing an expenditure from, or creating or authorizing an obligation under, any appropriation or fund in excess of the amount available in the appropriation or fund unless authorized by law. Involving the government in any obligation to pay money before funds have been appropriated for that purpose, unless otherwise allowed by law.
c. Accepting voluntary services for the U.S., or employing personal services not authorized by law except in cases of emergency involving the safety of human life or the protection of property.
d. Making obligations or expenditures in excess of an apportionment or reapportionment or in excess of the amount permitted by agency regulations. A violation will also result from the over-expenditure of an appropriation, allotment, statutory limitation or earmark, or an obligation in advance of an appropriation.
e. A violation of the ADA will occur from any of the actions above. Congress enacted the ADA to prevent the obligation of Government funds that are not available.""" ;
    skos:inScheme ER-37-1-30-P12: ;
    skos:prefLabel "ADA Violations" .

ER-37-1-30-P12:Accounting_Procedures a wov:GlossaryTerm,
        skos:Concept ;
    rdfs:label "Accounting Procedures" ;
    dcterms:bibliographicCitation "https://www.publications.usace.army.mil/Portals/76/Users/182/86/2486/ER%2037-1-30.pdf#page=37" ;
    pav:wasDerivedFrom "glossaries/CivilWorks/ER-37-1-30-P12.yaml#term[Accounting Procedures]" ;
    skos:definition "Proper procedures for recording financial transactions and conducting JRP reviews are available in the CEFMS II User Manual." ;
    skos:inScheme ER-37-1-30-P12: ;
    skos:prefLabel "Accounting Procedures" .

ER-37-1-30-P12:Accounting_Support_for_Fund_Control_Systems a wov:GlossaryTerm,
        skos:Concept ;
    rdfs:label "Accounting Support for Fund Control Systems" ;
    dcterms:bibliographicCitation "https://www.publications.usace.army.mil/Portals/76/Users/182/86/2486/ER%2037-1-30.pdf#page=35" ;
    pav:wasDerivedFrom "glossaries/CivilWorks/ER-37-1-30-P12.yaml#term[Accounting Support for Fund Control Systems]" ;
    skos:definition """CEFMS II is a fully operational, integrated financial management system supporting agency fund control. This field-level financial management tool integrates USACE work management functions with accounting requirements prescribed under U.S. Government Standard General Ledger policies. All transactions which affect dollars (commitments, obligations, expenditures, disbursements) for all USACE missions and programs are entered into CEFMS II. CEFMS II records all transactions, stores records electronically for easy access and retrieval, and updates United States Standard General Ledgers based on each transaction. CEFMS II provides for:
a. Recording all financial transactions affecting apportionments, reapportionments, allotments, agency restrictions, financial plans, program operating plans, obligations and expenditures as well as anticipated, earned, and collected reimbursements.
b. Preparing and reconciling financial reports that display cumulative obligations and the remaining unobligated balance by appropriation and allotment and cumulative obligations by budget activity and object class.""" ;
    skos:inScheme ER-37-1-30-P12: ;
    skos:prefLabel "Accounting Support for Fund Control Systems" .

ER-37-1-30-P12:Administrative_Penalties a wov:GlossaryTerm,
        skos:Concept ;
    rdfs:label "Administrative Penalties" ;
    dcterms:bibliographicCitation "https://www.publications.usace.army.mil/Portals/76/Users/182/86/2486/ER%2037-1-30.pdf#page=37" ;
    pav:wasDerivedFrom "glossaries/CivilWorks/ER-37-1-30-P12.yaml#term[Administrative Penalties]" ;
    skos:definition "The law provides that any officer or employee of the United States who violates the prohibitions of Title 31 USC 1341(a), 1342, 1349-1351, 1511-1516, 1517(a)-1519 will be subject to administrative discipline. The DoD FMR contains additional guidance regarding recommended disciplinary actions. Administrative discipline for a civilian employee may include written admonishment or reprimand, reduction in grade, suspension from duty without pay, or removal from office. Military personnel may be subject to appropriate administrative discipline or may be subject to action under the Uniform Code of Military Justice (UCMJ). If a violation is determined to have been knowingly and willfully committed, there are statutory provisions applying criminal penalties. An officer or employee found responsible for committing a violation knowingly and willfully may be subject to criminal penalties. The investigating officer should consult with legal counsel to determine if the investigation should be referred to the appropriate criminal investigation organization for action." ;
    skos:inScheme ER-37-1-30-P12: ;
    skos:prefLabel "Administrative Penalties" .

ER-37-1-30-P12:Allotment a wov:GlossaryTerm,
        skos:Concept ;
    rdfs:label "Allotment" ;
    dcterms:bibliographicCitation "https://www.publications.usace.army.mil/Portals/76/Users/182/86/2486/ER%2037-1-30.pdf#page=30" ;
    pav:wasDerivedFrom "glossaries/CivilWorks/ER-37-1-30-P12.yaml#term[Allotment]" ;
    skos:definition "Subdivisions of apportionments that are made by the head of an agency. An allotment is an authority delegated by the head of the agency or other authorized employee to incur obligations within the specified amount consistent with the requirements in OMB Circular A-11. The amount allotted by an agency cannot exceed the amount apportioned by OMB. In USACE, the Director of Resource Management (DRM) or authorized designee is responsible for issuing, reducing, or changing the structure of allotments for Civil Works appropriations. The sum of a sub-allotment, a subdivision of an allotment, or amount issued cannot exceed the allotment amount. The amount of an allotment is fixed and cannot be changed except as otherwise authorized by the head of the agency or the DRM." ;
    skos:inScheme ER-37-1-30-P12: ;
    skos:prefLabel "Allotment" .

ER-37-1-30-P12:Allowances_and_Allocations a wov:GlossaryTerm,
        skos:Concept ;
    rdfs:label "Allowances and Allocations" ;
    dcterms:bibliographicCitation "https://www.publications.usace.army.mil/Portals/76/Users/182/86/2486/ER%2037-1-30.pdf#page=31" ;
    pav:wasDerivedFrom "glossaries/CivilWorks/ER-37-1-30-P12.yaml#term[Allowances and Allocations]" ;
    skos:definition "Subdivisions of sub-allotments." ;
    skos:inScheme ER-37-1-30-P12: ;
    skos:prefLabel "Allowances and Allocations" .

ER-37-1-30-P12:Apportionment a wov:GlossaryTerm,
        skos:Concept ;
    rdfs:label "Apportionment" ;
    dcterms:bibliographicCitation "https://www.publications.usace.army.mil/Portals/76/Users/182/86/2486/ER%2037-1-30.pdf#page=30" ;
    pav:wasDerivedFrom "glossaries/CivilWorks/ER-37-1-30-P12.yaml#term[Apportionment]" ;
    skos:definition "Distribution of amounts made by OMB of amounts available for obligation in an appropriation or fund account into amounts available for specified time periods, programs, activities, projects, objects, or any combinations of these. The apportioned amount limits the obligations that may be incurred. An apportionment may be further subdivided by an agency into allotments, sub-allotments, and allocations. The OMB apportions funds from the Energy and Water Development and related agencies Appropriations Act to USACE making appropriated funds available for obligation and expenditure. The process of apportionment of funds for military appropriations, such as Operation and Maintenance, Army, can be found in Volume 14, Chapter 1 of the DoD Financial Management Regulation (FMR). Apportionment restricts, by appropriation, the quarterly amounts available for obligation to ensure an orderly distribution of funds throughout the fiscal year. Included in the apportionment are newly appropriated funds, anticipated reimbursable activity, and unobligated balances carried over from prior year appropriations. The OMB may use apportionment to restrict the use of funds when the work intended by Congress is contrary to Administration policy or not legislatively authorized. The apportioned amount limits the obligations that may be incurred. An apportionment may be further subdivided into allotments, sub-allotments, and allocations all of which are subject to the provisions of the ADA. OMB may use apportionment to restrict the use of funds when the work intended by Congress is contrary to Administration policy or not legislatively authorized. Apportionments are subject to adjustment in the event of substantially increased allotments or major revocations, a Supplemental Appropriations Act, or if appropriations are deferred or rescinded according to the Congressional Budget and Impoundment Control Act of 1974 (PL 93-344). The head of an executive agency may request an apportionment under title 31 USC section 1512. This chapter serves as the governing directive on apportionments. Appendix F details the procedures for requesting the apportionment of funds in USACE. Congressional Budget and Impoundment Control Act of 1974 (PL 93-344)." ;
    skos:inScheme ER-37-1-30-P12: ;
    skos:prefLabel "Apportionment" .

ER-37-1-30-P12:Appropriations a wov:GlossaryTerm,
        skos:Concept ;
    rdfs:label "Appropriations" ;
    dcterms:bibliographicCitation "https://www.publications.usace.army.mil/Portals/76/Users/182/86/2486/ER%2037-1-30.pdf#page=29" ;
    pav:wasDerivedFrom "glossaries/CivilWorks/ER-37-1-30-P12.yaml#term[Appropriations]" ;
    skos:definition "Acts of Congress signed into law by the President that provide budget authority and permit an Agency to incur obligations and to spend public funds. Congressional restrictions contained in appropriations acts will be enforced unless otherwise specified by Congress. Appendix C provides the common military appropriations used in USACE. Common Civil Works appropriations are in Chapter 7 of this regulation. Appendix D is an example of the obligation life of current, expired and cancelled appropriations. The annual Appropriations Acts provide budget authority on the following basis: (1) Annual Authority or authority that is available for new obligations for only one specific fiscal year or less; (2) Multi- Year Authority or authority that is available for new obligations for two or more fiscal years; or (3) No-Year Authority or authority that is available for new obligations for an indefinite period of time, usually until the objectives for which the authority was made available are attained." ;
    skos:inScheme ER-37-1-30-P12: ;
    skos:prefLabel "Appropriations" .

ER-37-1-30-P12:Cancelled_Accounts a wov:GlossaryTerm,
        skos:Concept ;
    rdfs:label "Cancelled Accounts" ;
    dcterms:bibliographicCitation "https://www.publications.usace.army.mil/Portals/76/Users/182/86/2486/ER%2037-1-30.pdf#page=30" ;
    pav:wasDerivedFrom "glossaries/CivilWorks/ER-37-1-30-P12.yaml#term[Cancelled Accounts]" ;
    skos:definition "Appropriation or fund accounts at the end of the fifth year for valid upward adjustment period, any unobligated budget authority remaining in that year's account reverts to the General Fund in the Treasury." ;
    skos:inScheme ER-37-1-30-P12: ;
    skos:prefLabel "Cancelled Accounts" .

<https://usace-data.com/civil-works/glossary/ER-37-1-30-P12#Category,_Class,_Sub-class> a wov:GlossaryTerm,
        skos:Concept ;
    rdfs:label "Category, Class, Sub-class" ;
    dcterms:bibliographicCitation "https://www.publications.usace.army.mil/Portals/76/Users/182/86/2486/ER%2037-1-30.pdf#page=84" ;
    pav:wasDerivedFrom "glossaries/CivilWorks/ER-37-1-30-P12.yaml#term[Category, Class, Sub-class]" ;
    skos:altLabel "CCS" ;
    skos:definition "A three-digit code used to identify specific activities, purposes, and descriptions of work to be performed, as defined by CECW policy/National Account Manager. This code is used for civil appropriations only. See CEFMS II screen 10.22 for current listing." ;
    skos:inScheme ER-37-1-30-P12: ;
    skos:prefLabel "Category, Class, Sub-class" .

ER-37-1-30-P12:Commitment a wov:GlossaryTerm,
        skos:Concept ;
    rdfs:label "Commitment" ;
    dcterms:bibliographicCitation "https://www.publications.usace.army.mil/Portals/76/Users/182/86/2486/ER%2037-1-30.pdf#page=31" ;
    pav:wasDerivedFrom "glossaries/CivilWorks/ER-37-1-30-P12.yaml#term[Commitment]" ;
    skos:definition "Administrative reservation of funds based upon firm procurement requests, orders, directives, and equivalent instruments. Commitments reduce the uncommitted and available balance. A commitment document will be signed by a person authorized to reserve funds; that is, the official responsible for administrative control of funds for the affected subdivision of the appropriation. This ensures that the subsequent entry of an undelivered order or accrued expenditure will not exceed available funds. The amount of the obligation will not exceed the amount of the commitment." ;
    skos:inScheme ER-37-1-30-P12: ;
    skos:prefLabel "Commitment" .

<https://usace-data.com/civil-works/glossary/ER-37-1-30-P12#Construction,_Corps_of_Engineers,_Civil_096X3122> a wov:GlossaryTerm,
        skos:Concept ;
    rdfs:label "Construction, Corps of Engineers, Civil 096X3122" ;
    dcterms:bibliographicCitation "https://www.publications.usace.army.mil/Portals/76/Users/182/86/2486/ER%2037-1-30.pdf#page=82" ;
    pav:wasDerivedFrom "glossaries/CivilWorks/ER-37-1-30-P12.yaml#term[Construction, Corps of Engineers, Civil 096X3122]" ;
    skos:definition "For expenses necessary for the construction of river and harbor, flood and storm damage reduction shore protection, aquatic ecosystem restoration, and related projects, authorized by law; for conducting detailed studies, and plans and specifications, of such projects (including those involving participation by States, local governments, or private groups) authorized or made eligible for selection by law (but such detailed studies, and plans and specifications will not constitute a commitment of the Government to construction)." ;
    skos:inScheme ER-37-1-30-P12: ;
    skos:prefLabel "Construction, Corps of Engineers, Civil 096X3122" .

ER-37-1-30-P12:Cost_Account_Requirements a wov:GlossaryTerm,
        skos:Concept ;
    rdfs:label "Cost Account Requirements" ;
    dcterms:bibliographicCitation "https://www.publications.usace.army.mil/Portals/76/Users/182/86/2486/ER%2037-1-30.pdf#page=84" ;
    pav:wasDerivedFrom "glossaries/CivilWorks/ER-37-1-30-P12.yaml#term[Cost Account Requirements]" ;
    skos:definition "Cost accounts will be maintained by project, class, or category of work under each appropriation according to the uniform code of accounts. Cost accounts will be established within this structure on the basis of programming documents and/or approved Work Orders, ENG Forms 3013." ;
    skos:inScheme ER-37-1-30-P12: ;
    skos:prefLabel "Cost Account Requirements" .

ER-37-1-30-P12:Cost_Accounting_Procedures a wov:GlossaryTerm,
        skos:Concept ;
    rdfs:label "Cost Accounting Procedures" ;
    dcterms:bibliographicCitation "https://www.publications.usace.army.mil/Portals/76/Users/182/86/2486/ER%2037-1-30.pdf#page=85" ;
    pav:wasDerivedFrom "glossaries/CivilWorks/ER-37-1-30-P12.yaml#term[Cost Accounting Procedures]" ;
    skos:definition "A listing of valid cost accounting codes for each appropriation is available in CEFMS II on the screens identified above. For ease, dated listings of the codes referenced above will be included in an Excel file on the Finance and Accounting Policy Division webpage, but these listings are subject to change without notice." ;
    skos:inScheme ER-37-1-30-P12: ;
    skos:prefLabel "Cost Accounting Procedures" .

ER-37-1-30-P12:Criminal_Penalties a wov:GlossaryTerm,
        skos:Concept ;
    rdfs:label "Criminal Penalties" ;
    dcterms:bibliographicCitation "https://www.publications.usace.army.mil/Portals/76/Users/182/86/2486/ER%2037-1-30.pdf#page=38" ;
    pav:wasDerivedFrom "glossaries/CivilWorks/ER-37-1-30-P12.yaml#term[Criminal Penalties]" ;
    skos:definition """(a) An employee who knowingly and willfully violates the statute will be fined not more than $5,000, imprisoned for not more than 2 years, or both.
(b) Criminal penalties for military personnel may include punishment under Article 15 of the UCMJ or trial by Court Martial.""" ;
    skos:inScheme ER-37-1-30-P12: ;
    skos:prefLabel "Criminal Penalties" .

ER-37-1-30-P12:Department_Accountable_Official a wov:GlossaryTerm,
        skos:Concept ;
    rdfs:label "Department Accountable Official" ;
    dcterms:bibliographicCitation "https://www.publications.usace.army.mil/Portals/76/Users/182/86/2486/ER%2037-1-30.pdf#page=34" ;
    pav:wasDerivedFrom "glossaries/CivilWorks/ER-37-1-30-P12.yaml#term[Department Accountable Official]" ;
    skos:altLabel "DAO" ;
    skos:definition "DAOs provide information, data, or service to a Certifying Officer or DO to support the payment process. The DAO carries out many approving official roles in CEFMS II, such as ensuring that required funds are available before obligating funds and that obligating documents reflect the applicable appropriation account and CEFMS II budget fund code. This official has financial liability in the certifying process and works with Government Purchase Cards, RMs, fund holders, Contracting Officers, Administrative Contracting Officers, Contracting Officer Technical Representatives and others who have distinct roles essential to funds control. These appointments will be signed electronically and maintained in CEFMS II in addition to the DD Form 577." ;
    skos:inScheme ER-37-1-30-P12: ;
    skos:prefLabel "Department Accountable Official" .

ER-37-1-30-P12:Directorate%2FOffice_Chiefs a wov:GlossaryTerm,
        skos:Concept ;
    rdfs:label "Directorate/Office Chiefs" ;
    dcterms:bibliographicCitation "https://www.publications.usace.army.mil/Portals/76/Users/182/86/2486/ER%2037-1-30.pdf#page=34" ;
    pav:wasDerivedFrom "glossaries/CivilWorks/ER-37-1-30-P12.yaml#term[Directorate/Office Chiefs]" ;
    skos:definition "ensure that mandatory fiscal law training requirements are fulfilled according to USACE guidance described in appointment letters for all its employees. The DoD FMR requires annual refresher fiscal law training. Directorate/Office Chiefs are also responsible for establishing and maintaining internal controls necessary to meet statutory requirements for time, purpose and amount." ;
    skos:inScheme ER-37-1-30-P12: ;
    skos:prefLabel "Directorate/Office Chiefs" .

ER-37-1-30-P12:Disbursement a wov:GlossaryTerm,
        skos:Concept ;
    rdfs:label "Disbursement" ;
    dcterms:bibliographicCitation "https://www.publications.usace.army.mil/Portals/76/Users/182/86/2486/ER%2037-1-30.pdf#page=32" ;
    pav:wasDerivedFrom "glossaries/CivilWorks/ER-37-1-30-P12.yaml#term[Disbursement]" ;
    skos:definition "Actual payment by the U.S. Treasury by cash, check, or electronic funds transfer based on certification by a department, agency, or certifying officer." ;
    skos:inScheme ER-37-1-30-P12: ;
    skos:prefLabel "Disbursement" .

ER-37-1-30-P12:Disbursing_Officer a wov:GlossaryTerm,
        skos:Concept ;
    rdfs:label "Disbursing Officer" ;
    dcterms:bibliographicCitation "https://www.publications.usace.army.mil/Portals/76/Users/182/86/2486/ER%2037-1-30.pdf#page=33" ;
    pav:wasDerivedFrom "glossaries/CivilWorks/ER-37-1-30-P12.yaml#term[Disbursing Officer]" ;
    skos:definition """The USACE Disbursing Officer is located in the UFC in Millington, Tennessee. District and Division offices do not have the disbursing role. DO responsibilities include:
(1) Ensuring that accounts are in agreement with laws and regulations that govern disbursement of public funds.
(2) Having physical possession or control of the funds. All payments are made centrally by USACE UFC.""" ;
    skos:inScheme ER-37-1-30-P12: ;
    skos:prefLabel "Disbursing Officer" .

ER-37-1-30-P12:Element_of_Resource_%28EOR%29_Codes a wov:GlossaryTerm,
        skos:Concept ;
    rdfs:label "Element of Resource (EOR) Codes" ;
    dcterms:bibliographicCitation "https://www.publications.usace.army.mil/Portals/76/Users/182/86/2486/ER%2037-1-30.pdf#page=84" ;
    pav:wasDerivedFrom "glossaries/CivilWorks/ER-37-1-30-P12.yaml#term[Element of Resource (EOR) Codes]" ;
    skos:altLabel "EOR Codes" ;
    skos:definition """A four-digit code which identifies the type of resource being employed or consumed (such as military personnel, civilian personnel, travel of personnel, utilities and rents, and communication). The EOR classifies the resource according to the nature of the usage rather than the purpose, as defined by DFAS-IN Manual 37-100-17, Chapter 2b. The first and second digits identify the object class as defined by OMB (above). The third digit identifies category or type of pay or benefit. The fourth digit identifies the type of employee for pay-related EORs, or the purpose of the payment or benefit for non-pay EORs.
See CEFMS II screen 10.49 for current listing.""" ;
    skos:inScheme ER-37-1-30-P12: ;
    skos:prefLabel "Element of Resource (EOR) Codes" .

<https://usace-data.com/civil-works/glossary/ER-37-1-30-P12#Expenses,_Corps_of_Engineers,_Civil_096Y3124> a wov:GlossaryTerm,
        skos:Concept ;
    rdfs:label "Expenses, Corps of Engineers, Civil 096Y3124" ;
    dcterms:bibliographicCitation "https://www.publications.usace.army.mil/Portals/76/Users/182/86/2486/ER%2037-1-30.pdf#page=83" ;
    pav:wasDerivedFrom "glossaries/CivilWorks/ER-37-1-30-P12.yaml#term[Expenses, Corps of Engineers, Civil 096Y3124]" ;
    skos:definition "For expenses necessary for the supervision and general administration of the civil works program in USACE headquarters, and the offices of the Division Engineers, and for the costs allocable to the civil works program for management and operation of the Humphreys Engineer Center Support Activity, the Institute for Water Resources, the United States Army Engineer Research and Development Center, and the United States Army Corps of Engineers Finance Center." ;
    skos:inScheme ER-37-1-30-P12: ;
    skos:prefLabel "Expenses, Corps of Engineers, Civil 096Y3124" .

ER-37-1-30-P12:Expired_Accounts a wov:GlossaryTerm,
        skos:Concept ;
    rdfs:label "Expired Accounts" ;
    dcterms:bibliographicCitation "https://www.publications.usace.army.mil/Portals/76/Users/182/86/2486/ER%2037-1-30.pdf#page=30" ;
    pav:wasDerivedFrom "glossaries/CivilWorks/ER-37-1-30-P12.yaml#term[Expired Accounts]" ;
    skos:definition "Appropriations or fund accounts in which the balances are no longer available for incurring new obligations. In certain circumstances, these accounts are available for recording, adjusting and liquidating obligations. Obligated balances for these expired appropriations are retained by the activity and remain available for an additional five years only for valid upward adjustments; that is, to liquidate obligations properly incurred during the period of obligation availability as outlined in title 31 USC section 1502." ;
    skos:inScheme ER-37-1-30-P12: ;
    skos:prefLabel "Expired Accounts" .

ER-37-1-30-P12:FOA_Commanders%2FDirectors a wov:GlossaryTerm,
        skos:Concept ;
    rdfs:label "FOA Commanders/Directors" ;
    dcterms:bibliographicCitation "https://www.publications.usace.army.mil/Portals/76/Users/182/86/2486/ER%2037-1-30.pdf#page=34" ;
    pav:wasDerivedFrom "glossaries/CivilWorks/ER-37-1-30-P12.yaml#term[FOA Commanders/Directors]" ;
    skos:definition "Commanders/Directors are designated with primary responsibility for the administrative control of funds. Commanders/Directors may re-delegate responsibility for execution of funds to Departmental Accountable Official (DAO) and certifying officials through appointment letters." ;
    skos:inScheme ER-37-1-30-P12: ;
    skos:prefLabel "FOA Commanders/Directors" .

ER-37-1-30-P12:Finance_and_Accounting_Officers a wov:GlossaryTerm,
        skos:Concept ;
    rdfs:label "Finance and Accounting Officers" ;
    dcterms:bibliographicCitation "https://www.publications.usace.army.mil/Portals/76/Users/182/86/2486/ER%2037-1-30.pdf#page=34" ;
    pav:wasDerivedFrom "glossaries/CivilWorks/ER-37-1-30-P12.yaml#term[Finance and Accounting Officers]" ;
    skos:altLabel "FAOs" ;
    skos:definition "FAOs will provide fund holders with a listing(s) of ULO Reports, which identifies outstanding commitments, unliquidated obligations, open accounts payable and open customer orders, recorded for the fund holder. Reviews are conducted a minimum of three times per year in compliance with JRP. Accounting offices will coordinate tri-annual reviews of commitments and obligations to ensure timely compliance with the DoD FMR." ;
    skos:inScheme ER-37-1-30-P12: ;
    skos:prefLabel "Finance and Accounting Officers" .

ER-37-1-30-P12:Fiscal_law_and_ADA_violation_management a wov:GlossaryTerm,
        skos:Concept ;
    rdfs:label "Fiscal law and ADA violation management" ;
    dcterms:bibliographicCitation "https://www.publications.usace.army.mil/Portals/76/Users/182/86/2486/ER%2037-1-30.pdf#page=33" ;
    pav:wasDerivedFrom "glossaries/CivilWorks/ER-37-1-30-P12.yaml#term[Fiscal law and ADA violation management]" ;
    skos:definition "The Finance and Accounting Policy Division advises USACE activities on the procedures for reporting potential violations to Assistant Secretary of the Army (Financial Management and Comptroller), including the coordination, submission and management of flash, preliminary, and final investigation reports." ;
    skos:inScheme ER-37-1-30-P12: ;
    skos:prefLabel "Fiscal law and ADA violation management" .

<https://usace-data.com/civil-works/glossary/ER-37-1-30-P12#Flood_Control_%26_Coastal_Emergencies,_Corps_of_Engineers,_Civil_096X3125> a wov:GlossaryTerm,
        skos:Concept ;
    rdfs:label "Flood Control & Coastal Emergencies, Corps of Engineers, Civil 096X3125" ;
    dcterms:bibliographicCitation "https://www.publications.usace.army.mil/Portals/76/Users/182/86/2486/ER%2037-1-30.pdf#page=83" ;
    pav:wasDerivedFrom "glossaries/CivilWorks/ER-37-1-30-P12.yaml#term[Flood Control & Coastal Emergencies, Corps of Engineers, Civil 096X3125]" ;
    skos:definition "For expenses necessary to prepare for flood, hurricane, and other natural disasters and support emergency operations, repairs, and other activities in response to such disasters as authorized by law." ;
    skos:inScheme ER-37-1-30-P12: ;
    skos:prefLabel "Flood Control & Coastal Emergencies, Corps of Engineers, Civil 096X3125" .

ER-37-1-30-P12:Formal_Reviews a wov:GlossaryTerm,
        skos:Concept ;
    rdfs:label "Formal Reviews" ;
    dcterms:bibliographicCitation "https://www.publications.usace.army.mil/Portals/76/Users/182/86/2486/ER%2037-1-30.pdf#page=37" ;
    pav:wasDerivedFrom "glossaries/CivilWorks/ER-37-1-30-P12.yaml#term[Formal Reviews]" ;
    skos:definition "Generally, the existence of a potential violation will be established during the preliminary review and before a formal investigation begins. If Army determines that there is a need for formal investigation then it directs USACE to initiate a formal review within two weeks from the notification from Army." ;
    skos:inScheme ER-37-1-30-P12: ;
    skos:prefLabel "Formal Reviews" .

<https://usace-data.com/civil-works/glossary/ER-37-1-30-P12#Formerly_Utilized_Sites_Remedial_Action_Program_%28FUSRAP%29,_Corps_of_Engineers,_096X3130> a wov:GlossaryTerm,
        skos:Concept ;
    rdfs:label "Formerly Utilized Sites Remedial Action Program (FUSRAP), Corps of Engineers, 096X3130" ;
    dcterms:bibliographicCitation "https://www.publications.usace.army.mil/Portals/76/Users/182/86/2486/ER%2037-1-30.pdf#page=83" ;
    pav:wasDerivedFrom "glossaries/CivilWorks/ER-37-1-30-P12.yaml#term[Formerly Utilized Sites Remedial Action Program (FUSRAP), Corps of Engineers, 096X3130]" ;
    skos:definition "For expenses necessary to clean up contamination from sites in the United States resulting from work performed as part of the Nation's early atomic energy program." ;
    skos:inScheme ER-37-1-30-P12: ;
    skos:prefLabel "Formerly Utilized Sites Remedial Action Program (FUSRAP), Corps of Engineers, 096X3130" .

ER-37-1-30-P12:Fund_Holders a wov:GlossaryTerm,
        skos:Concept ;
    rdfs:label "Fund Holders" ;
    dcterms:bibliographicCitation "https://www.publications.usace.army.mil/Portals/76/Users/182/86/2486/ER%2037-1-30.pdf#page=34" ;
    pav:wasDerivedFrom "glossaries/CivilWorks/ER-37-1-30-P12.yaml#term[Fund Holders]" ;
    skos:definition "(Responsible Employee in CEFMS II) are responsible for conducting reviews of items identified on the ULO report to confirm that all open commitments and obligations are valid, accurate and complete. Unliquidated balances that are nominal in amount and dormant are usually a red flag that deobligation action is needed. Special attention is required for items citing expiring funds. It is imperative that funds holders return unused funds to customers as soon as possible for re-use prior to expiration. The return of funds should take place well before 30 September of each fiscal year." ;
    skos:inScheme ER-37-1-30-P12: ;
    skos:prefLabel "Fund Holders" .

ER-37-1-30-P12:Funding_Authorization_Documents a wov:GlossaryTerm,
        skos:Concept ;
    rdfs:label "Funding Authorization Documents" ;
    dcterms:bibliographicCitation "https://www.publications.usace.army.mil/Portals/76/Users/182/86/2486/ER%2037-1-30.pdf#page=31" ;
    pav:wasDerivedFrom "glossaries/CivilWorks/ER-37-1-30-P12.yaml#term[Funding Authorization Documents]" ;
    skos:altLabel "FAD" ;
    skos:definition "HQUSACE allots budget authority via FAD at the appropriation level to each USACE Field Operating Activity (FOA). For Civil Works appropriations, work allowances are issued by HQUSACE program managers for individual programs, projects, and activities in that FOA. For Military appropriations, draft directives are issued by HQUSACE program managers, in the Military Programs Directorate, for individual programs, projects and activities in a FOA. Historically, the appropriations acts for the eight Civil Works accounts have provided that the budget authority is to be available until expended. Accordingly, all funds remaining unobligated at the end of one fiscal year have automatically resulted in carryover of budget authority to the next fiscal year without issuance of fund advice. This carry over budget authority does not apply to the regulatory program and expense Civil Works appropriations; Congress has limited these appropriations to only two years of availability. FADs must include information on the amount available, funding source, the period of availability, the position and title of the responsible official, as well as any justifications for changes in allotments as applicable." ;
    skos:inScheme ER-37-1-30-P12: ;
    skos:prefLabel "Funding Authorization Documents" .

<https://usace-data.com/civil-works/glossary/ER-37-1-30-P12#HQUSACE,_Resource_Management_Office> a wov:GlossaryTerm,
        skos:Concept ;
    rdfs:label "HQUSACE, Resource Management Office" ;
    dcterms:bibliographicCitation "https://www.publications.usace.army.mil/Portals/76/Users/182/86/2486/ER%2037-1-30.pdf#page=32" ;
    pav:wasDerivedFrom "glossaries/CivilWorks/ER-37-1-30-P12.yaml#term[HQUSACE, Resource Management Office]" ;
    skos:definition """This office, through the DRM, CFO for USACE, is responsible for:
(1) Establishing and maintaining a system of administrative control of funds according to Title 31 USC sections 3511 and 3512, Federal law and OMB guidance.
(2) Developing and prescribing an accounting system that provides prompt and accurate recording in the official accounts of all financial transactions that have an effect on apportionment or other subdivision of funds.
(3) Oversight of investigations and reporting of any alleged statutory and/or administrative control of funds violation. Depending on the results of necessary investigations, the Resource Manager (RM) may be required to recommend disciplinary actions against the cited individuals, modify procedures, or take other actions as warranted.""" ;
    skos:inScheme ER-37-1-30-P12: ;
    skos:prefLabel "HQUSACE, Resource Management Office" .

<https://usace-data.com/civil-works/glossary/ER-37-1-30-P12#HQUSACE_Chief,_Budget_%26_Programs_Division> a wov:GlossaryTerm,
        skos:Concept ;
    rdfs:label "HQUSACE Chief, Budget & Programs Division" ;
    dcterms:bibliographicCitation "https://www.publications.usace.army.mil/Portals/76/Users/182/86/2486/ER%2037-1-30.pdf#page=32" ;
    pav:wasDerivedFrom "glossaries/CivilWorks/ER-37-1-30-P12.yaml#term[HQUSACE Chief, Budget & Programs Division]" ;
    skos:altLabel "CERM-B" ;
    skos:definition """The HQUSACE Chief, Budget & Programs Division is responsible for: (1) Establishing USACE budgetary policies and procedures and providing implementing guidance to staff and operating officials.
(2) Consolidating and submitting Civil Works and military budgets to OMB and HQDA in congruence with Title 31 USC sections 1101, 1104-1108 and 3324.
(3) Obtaining civil and military funds from OMB/Headquarter, Department of Army, and issuing funds to Divisions, Districts and separate FOAs.  Monitoring proper execution of USACE's budget.
(5) Reporting to OMB on the use of apportionments.""" ;
    skos:inScheme ER-37-1-30-P12: ;
    skos:prefLabel "HQUSACE Chief, Budget & Programs Division" .

<https://usace-data.com/civil-works/glossary/ER-37-1-30-P12#HQUSACE_Chief,_Finance_and_Accounting_Policy_Division> a wov:GlossaryTerm,
        skos:Concept ;
    rdfs:label "HQUSACE Chief, Finance and Accounting Policy Division" ;
    dcterms:bibliographicCitation "https://www.publications.usace.army.mil/Portals/76/Users/182/86/2486/ER%2037-1-30.pdf#page=33" ;
    pav:wasDerivedFrom "glossaries/CivilWorks/ER-37-1-30-P12.yaml#term[HQUSACE Chief, Finance and Accounting Policy Division]" ;
    skos:altLabel "CERM-F" ;
    skos:definition "is responsible for: (1) Establishing USACE finance and accounting policy." ;
    skos:inScheme ER-37-1-30-P12: ;
    skos:prefLabel "HQUSACE Chief, Finance and Accounting Policy Division" .

<https://usace-data.com/civil-works/glossary/ER-37-1-30-P12#Hydraulic_Mining_in_California,_Debris,_096X5066> a wov:GlossaryTerm,
        skos:Concept ;
    rdfs:label "Hydraulic Mining in California, Debris, 096X5066" ;
    dcterms:bibliographicCitation "https://www.publications.usace.army.mil/Portals/76/Users/182/86/2486/ER%2037-1-30.pdf#page=83" ;
    pav:wasDerivedFrom "glossaries/CivilWorks/ER-37-1-30-P12.yaml#term[Hydraulic Mining in California, Debris, 096X5066]" ;
    skos:definition "The Hydraulic Mining in California, Debris Removal account receives money paid to the United States as a tax on the operation of hydraulic mines. All sums of money paid into the Treasury under this section are credited to the 'debris fund', and expended under the supervision of the Chief of Engineers and direction of the Secretary of the Army, for repayment of any funds advanced by the Federal Government or other agency for the construction of restraining works and settling reservoirs and for maintenance. Currently, USACE use of amounts from this fund include fees collected from Pacific Gas and Electric Company to help maintain the Englebright Dam, Yuba River, California, mine debris restraining works and associated hydropower generation facilities. (33 U.S.C. 683)" ;
    skos:inScheme ER-37-1-30-P12: ;
    skos:prefLabel "Hydraulic Mining in California, Debris, 096X5066" .

ER-37-1-30-P12:Identifying_Circumstances_and_Responsibility a wov:GlossaryTerm,
        skos:Concept ;
    rdfs:label "Identifying Circumstances and Responsibility" ;
    dcterms:bibliographicCitation "https://www.publications.usace.army.mil/Portals/76/Users/182/86/2486/ER%2037-1-30.pdf#page=37" ;
    pav:wasDerivedFrom "glossaries/CivilWorks/ER-37-1-30-P12.yaml#term[Identifying Circumstances and Responsibility]" ;
    skos:definition "The investigating officer in a formal investigation will carefully consider the facts and circumstances surrounding the violation before affixing responsibility for the violation. Commanding officers, budget officers, or fiscal officers may be named because of their overall responsibility or position, or because they are designated as the holder of a subdivision of funds, if they failed to properly exercise their responsibilities. The investigating officer will attempt to discover the specific act or the failure to take action that resulted in the violation and the individual(s) responsible." ;
    skos:inScheme ER-37-1-30-P12: ;
    skos:prefLabel "Identifying Circumstances and Responsibility" .

ER-37-1-30-P12:Implementing_CFO_Act_requirements a wov:GlossaryTerm,
        skos:Concept ;
    rdfs:label "Implementing CFO Act requirements" ;
    dcterms:bibliographicCitation "https://www.publications.usace.army.mil/Portals/76/Users/182/86/2486/ER%2037-1-30.pdf#page=33" ;
    pav:wasDerivedFrom "glossaries/CivilWorks/ER-37-1-30-P12.yaml#term[Implementing CFO Act requirements]" ;
    skos:definition "CERM-F develops strategies and recommendations to management on the implementation of the CFO Act, preparation of financial statements, and the associated annual financial audits." ;
    skos:inScheme ER-37-1-30-P12: ;
    skos:prefLabel "Implementing CFO Act requirements" .

ER-37-1-30-P12:Initial_Discovery a wov:GlossaryTerm,
        skos:Concept ;
    rdfs:label "Initial Discovery" ;
    dcterms:bibliographicCitation "https://www.publications.usace.army.mil/Portals/76/Users/182/86/2486/ER%2037-1-30.pdf#page=36" ;
    pav:wasDerivedFrom "glossaries/CivilWorks/ER-37-1-30-P12.yaml#term[Initial Discovery]" ;
    skos:altLabel "Flash Report" ;
    skos:definition "When an alleged ADA violation is discovered, the local Resource Management Office and or Finance and Accounting Officer will immediately contact CERM-F. The local Resource Management Office will coordinate the issue with the local Office of Counsel and submit a flash report to CERM-F. The local activity must submit the Flash Report to CERM-F within 10 days of discovering the potential violation. The Flash Report will be duly signed by the Commander where the potential violation occurred. Upon receipt of the Flash Report, CERM-F coordinates with HQ Legal for a legal sufficiency letter and prepares a CERM transmittal letter. CERM submits these letters along with the Flash Report, to the Deputy Assistant Secretary of the Army for Financial Operations (DASA-FO) within two weeks of discovery of the potential violation. The format of the flash report is at Appendix E." ;
    skos:inScheme ER-37-1-30-P12: ;
    skos:prefLabel "Initial Discovery" .

ER-37-1-30-P12:Interpretation_and_Legal_Issues a wov:GlossaryTerm,
        skos:Concept ;
    rdfs:label "Interpretation and Legal Issues" ;
    dcterms:bibliographicCitation "https://www.publications.usace.army.mil/Portals/76/Users/182/86/2486/ER%2037-1-30.pdf#page=37" ;
    pav:wasDerivedFrom "glossaries/CivilWorks/ER-37-1-30-P12.yaml#term[Interpretation and Legal Issues]" ;
    skos:definition "The existence of a violation may depend on an interpretation of statutory or regulatory constraints imposed on the use of a particular appropriation or account, the proper fiscal year to be charged, or similar issues. HQUSACE Office of the Chief Counsel will assign an attorney to advise the investigating officer." ;
    skos:inScheme ER-37-1-30-P12: ;
    skos:prefLabel "Interpretation and Legal Issues" .

<https://usace-data.com/civil-works/glossary/ER-37-1-30-P12#Investigations,_Corps_of_Engineers,_Civil_096X3121> a wov:GlossaryTerm,
        skos:Concept ;
    rdfs:label "Investigations, Corps of Engineers, Civil 096X3121" ;
    dcterms:bibliographicCitation "https://www.publications.usace.army.mil/Portals/76/Users/182/86/2486/ER%2037-1-30.pdf#page=82" ;
    pav:wasDerivedFrom "glossaries/CivilWorks/ER-37-1-30-P12.yaml#term[Investigations, Corps of Engineers, Civil 096X3121]" ;
    skos:definition "For expenses necessary where authorized by law for the collection and study of basic information pertaining to river and harbor, flood and storm damage reduction, shore protection, aquatic ecosystem restoration and related needs, for surveys and detailed studies, plans and specifications of proposed river and harbor, flood and storm damage reduction, shore protection, and aquatic ecosystem restoration projects, and related efforts prior to construction; for restudy of authorized projects; for miscellaneous investigations; and, when authorized by law, surveys and detailed studies, and plans and specifications of projects prior to construction." ;
    skos:inScheme ER-37-1-30-P12: ;
    skos:prefLabel "Investigations, Corps of Engineers, Civil 096X3121" .

<https://usace-data.com/civil-works/glossary/ER-37-1-30-P12#Maintenance_%26_Operation_of_Dams_and_Other_Improvements_of_Navigable_Water,_096X5125> a wov:GlossaryTerm,
        skos:Concept ;
    rdfs:label "Maintenance & Operation of Dams and Other Improvements of Navigable Water, 096X5125" ;
    dcterms:bibliographicCitation "https://www.publications.usace.army.mil/Portals/76/Users/182/86/2486/ER%2037-1-30.pdf#page=83" ;
    pav:wasDerivedFrom "glossaries/CivilWorks/ER-37-1-30-P12.yaml#term[Maintenance & Operation of Dams and Other Improvements of Navigable Water, 096X5125]" ;
    skos:definition "USACE uses its share of certain fees levied by the Federal Energy Regulatory Commission (on the private use of Federal property, including facilities and land; private construction and operation of water management and appurtenant facilities; and private benefit from headwater improvement by others) for maintenance and operation of dams and other navigation structures owned by the United States or in the construction, maintenance or operation of headwater or other improvements of navigable waters of the United States. (16 U.S.C. 810(a))" ;
    skos:inScheme ER-37-1-30-P12: ;
    skos:prefLabel "Maintenance & Operation of Dams and Other Improvements of Navigable Water, 096X5125" .

<https://usace-data.com/civil-works/glossary/ER-37-1-30-P12#Mississippi_River_and_Tributaries,_Civil_096X3112> a wov:GlossaryTerm,
        skos:Concept ;
    rdfs:label "Mississippi River and Tributaries, Civil 096X3112" ;
    dcterms:bibliographicCitation "https://www.publications.usace.army.mil/Portals/76/Users/182/86/2486/ER%2037-1-30.pdf#page=83" ;
    pav:wasDerivedFrom "glossaries/CivilWorks/ER-37-1-30-P12.yaml#term[Mississippi River and Tributaries, Civil 096X3112]" ;
    skos:definition "For expenses necessary for flood damage reduction projects and related efforts in the Mississippi River alluvial valley below Cape Girardeau, Missouri, as authorized by law." ;
    skos:inScheme ER-37-1-30-P12: ;
    skos:prefLabel "Mississippi River and Tributaries, Civil 096X3112" .

ER-37-1-30-P12:Object_Classes a wov:GlossaryTerm,
        skos:Concept ;
    rdfs:label "Object Classes" ;
    dcterms:bibliographicCitation "https://www.publications.usace.army.mil/Portals/76/Users/182/86/2486/ER%2037-1-30.pdf#page=84" ;
    pav:wasDerivedFrom "glossaries/CivilWorks/ER-37-1-30-P12.yaml#term[Object Classes]" ;
    skos:definition "The object class codes are categories assigned for the purposes of the President's annual budget to present obligations by the items or services purchased by the Federal Government, as defined by OMB Circular A-11, section 83 (MAX Schedule O), and required by law (31 U.S.C. 1104(b)). See CEFMS II screen 10.49 for current listing." ;
    skos:inScheme ER-37-1-30-P12: ;
    skos:prefLabel "Object Classes" .

ER-37-1-30-P12:Obligation a wov:GlossaryTerm,
        skos:Concept ;
    rdfs:label "Obligation" ;
    dcterms:bibliographicCitation "https://www.publications.usace.army.mil/Portals/76/Users/182/86/2486/ER%2037-1-30.pdf#page=31" ;
    pav:wasDerivedFrom "glossaries/CivilWorks/ER-37-1-30-P12.yaml#term[Obligation]" ;
    skos:definition "Amounts of orders placed, contracts awarded, services received, and similar transactions during an accounting period that will require payment during the same or future period. Title 31 section 1501 of the United States Code (USC) defines what constitutes an obligation." ;
    skos:inScheme ER-37-1-30-P12: ;
    skos:prefLabel "Obligation" .

<https://usace-data.com/civil-works/glossary/ER-37-1-30-P12#Office_of_Assistant_Secretary_of_the_Army_%28Civil_Works%29,_096Y3132> a wov:GlossaryTerm,
        skos:Concept ;
    rdfs:label "Office of Assistant Secretary of the Army (Civil Works), 096Y3132" ;
    dcterms:bibliographicCitation "https://www.publications.usace.army.mil/Portals/76/Users/182/86/2486/ER%2037-1-30.pdf#page=84" ;
    pav:wasDerivedFrom "glossaries/CivilWorks/ER-37-1-30-P12.yaml#term[Office of Assistant Secretary of the Army (Civil Works), 096Y3132]" ;
    skos:definition "For the Office of the Assistant Secretary of the Army for Civil Works as authorized by 10 U.S.C. 3016(b)(3)." ;
    skos:inScheme ER-37-1-30-P12: ;
    skos:prefLabel "Office of Assistant Secretary of the Army (Civil Works), 096Y3132" .

<https://usace-data.com/civil-works/glossary/ER-37-1-30-P12#Operation_%26_Maintenance,_Corps_of_Engineers,_Civil_096X3123> a wov:GlossaryTerm,
        skos:Concept ;
    rdfs:label "Operation & Maintenance, Corps of Engineers, Civil 096X3123" ;
    dcterms:bibliographicCitation "https://www.publications.usace.army.mil/Portals/76/Users/182/86/2486/ER%2037-1-30.pdf#page=82" ;
    pav:wasDerivedFrom "glossaries/CivilWorks/ER-37-1-30-P12.yaml#term[Operation & Maintenance, Corps of Engineers, Civil 096X3123]" ;
    skos:definition "For expenses necessary for the operation, maintenance, and care of existing river and harbor, flood and storm damage reduction, aquatic ecosystem restoration, and related projects authorized by law; for providing security for infrastructure owned and operated by the United States Army Corps of Engineers (USACE), including administrative buildings and laboratories; maintaining harbor channels provided by a State municipality, or other public agency that serve essential navigation needs of general commerce, where authorized by law; surveying and charting of northern and northwestern lakes and connecting waters, clearing and straightening channels, and removing obstructions to navigation." ;
    skos:inScheme ER-37-1-30-P12: ;
    skos:prefLabel "Operation & Maintenance, Corps of Engineers, Civil 096X3123" .

<https://usace-data.com/civil-works/glossary/ER-37-1-30-P12#Payment_to_the_South_Dakota_Terrestrial_Wildlife_Habitat_Restoration_Trust_Fund,_096X3129> a wov:GlossaryTerm,
        skos:Concept ;
    rdfs:label "Payment to the South Dakota Terrestrial Wildlife Habitat Restoration Trust Fund, 096X3129" ;
    dcterms:bibliographicCitation "https://www.publications.usace.army.mil/Portals/76/Users/182/86/2486/ER%2037-1-30.pdf#page=84" ;
    pav:wasDerivedFrom "glossaries/CivilWorks/ER-37-1-30-P12.yaml#term[Payment to the South Dakota Terrestrial Wildlife Habitat Restoration Trust Fund, 096X3129]" ;
    skos:definition "Funds expended from the South Dakota Terrestrial Wildlife Habitat Restoration Trust Fund are derived from the interest paid on the underlying fully funded principal of the trust account. The Secretary of the Treasury warrants USACE $10M annually which is transferred to the state of South Dakota to fund wildlife habitat restoration." ;
    skos:inScheme ER-37-1-30-P12: ;
    skos:prefLabel "Payment to the South Dakota Terrestrial Wildlife Habitat Restoration Trust Fund, 096X3129" .

<https://usace-data.com/civil-works/glossary/ER-37-1-30-P12#Payments_to_States,_Flood_Control_Act_of_1954,_096X5090> a wov:GlossaryTerm,
        skos:Concept ;
    rdfs:label "Payments to States, Flood Control Act of 1954, 096X5090" ;
    dcterms:bibliographicCitation "https://www.publications.usace.army.mil/Portals/76/Users/182/86/2486/ER%2037-1-30.pdf#page=83" ;
    pav:wasDerivedFrom "glossaries/CivilWorks/ER-37-1-30-P12.yaml#term[Payments to States, Flood Control Act of 1954, 096X5090]" ;
    skos:definition "The Payment to States account receives money paid to the United States under certain leases. The statute mandates that 75 percent of all moneys received and deposited in the Treasury of the United States during any fiscal year on account of the leasing of lands acquired by the United States for flood control, navigation, and allied purposes, including the development of hydroelectric power, will be paid\" to the appropriate states. (33 U.S.C. 701c-3)" ;
    skos:inScheme ER-37-1-30-P12: ;
    skos:prefLabel "Payments to States, Flood Control Act of 1954, 096X5090" .

ER-37-1-30-P12:Preliminary_Review a wov:GlossaryTerm,
        skos:Concept ;
    rdfs:label "Preliminary Review" ;
    dcterms:bibliographicCitation "https://www.publications.usace.army.mil/Portals/76/Users/182/86/2486/ER%2037-1-30.pdf#page=36" ;
    pav:wasDerivedFrom "glossaries/CivilWorks/ER-37-1-30-P12.yaml#term[Preliminary Review]" ;
    skos:definition "Army reviews the potential ADA flash report and determines whether a preliminary investigation is warranted after coordinating with Army General Counsel. If warranted, DASA-FO will direct CERM-F to initiate a preliminary investigation and a case number is assigned. To help assure independence and impartiality during the review, CERM-F selects an investigator from an organization external to the USACE activity being reviewed. Investigating Officer is appointed by the USACE Deputy Commanding General. DASA- FO memorandum will assign a date to complete preliminary review. Per DoD FMR, preliminary review should be completed within 14 weeks from the date of initial discovery. The USACE activity that reported the alleged violation is responsible for all the costs for the investigating officer. CERM-F coordinates with HQ Legal Counsel to obtain a Legal Sufficiency letter that is submitted to DASA-FO along with the preliminary report. The preliminary review must focus on the potential violation not the corrective actions. Applicable corrective actions will be developed during the formal investigation, if formal investigation is warranted. The preliminary investigator or the review team lead must be capable of conducting a complete, impartial, and unbiased review." ;
    skos:inScheme ER-37-1-30-P12: ;
    skos:prefLabel "Preliminary Review" .

<https://usace-data.com/civil-works/glossary/ER-37-1-30-P12#Regulatory_Program,_Corps_of_Engineers,_Civil_096Y3126> a wov:GlossaryTerm,
        skos:Concept ;
    rdfs:label "Regulatory Program, Corps of Engineers, Civil 096Y3126" ;
    dcterms:bibliographicCitation "https://www.publications.usace.army.mil/Portals/76/Users/182/86/2486/ER%2037-1-30.pdf#page=83" ;
    pav:wasDerivedFrom "glossaries/CivilWorks/ER-37-1-30-P12.yaml#term[Regulatory Program, Corps of Engineers, Civil 096Y3126]" ;
    skos:definition "For expenses necessary for administration of laws pertaining to regulation of navigable waters and wetlands." ;
    skos:inScheme ER-37-1-30-P12: ;
    skos:prefLabel "Regulatory Program, Corps of Engineers, Civil 096Y3126" .

ER-37-1-30-P12:Research_Effort a wov:GlossaryTerm,
        skos:Concept ;
    rdfs:label "Research Effort" ;
    dcterms:bibliographicCitation "https://www.publications.usace.army.mil/Portals/76/Users/182/86/2486/ER%2037-1-30.pdf#page=37" ;
    pav:wasDerivedFrom "glossaries/CivilWorks/ER-37-1-30-P12.yaml#term[Research Effort]" ;
    skos:definition "An investigating officer may be required to perform extensive research. This effort may include researching accounting directives and regulations, directives and regulations related to the functional area involved, legal directives, public law, and legal opinions. An investigating officer will review all specific documentation in the functional area involved that relates to the violation such as purchase requests, contracts, work orders, vouchers, and supporting materials, etc. All appointing officials will stipulate in the investigating office appointment memorandum a due date for the ADA Report. Such due date must conform to the timeframes stipulated in DoD FMR, regardless of the scope of the event or amount of the potential violation." ;
    skos:inScheme ER-37-1-30-P12: ;
    skos:prefLabel "Research Effort" .

ER-37-1-30-P12:Resource_Codes a wov:GlossaryTerm,
        skos:Concept ;
    rdfs:label "Resource Codes" ;
    dcterms:bibliographicCitation "https://www.publications.usace.army.mil/Portals/76/Users/182/86/2486/ER%2037-1-30.pdf#page=85" ;
    pav:wasDerivedFrom "glossaries/CivilWorks/ER-37-1-30-P12.yaml#term[Resource Codes]" ;
    skos:definition "Resource codes are used to classify categories of obligations and expenditures. They are classified according to the initial purpose rather than the end product or service provided. The resource codes are rolled up at object class level for financial reporting purposes. From the CEFMS II data dictionary: The specific resources within manpower, equipment, service, material, facility and real property used to accomplish the Corps mission. The code may identify a standard resource type or any component in a breakdown thereof. Resource codes are also tied to object classes. Resource codes may only belong to one object class, with the exception of OTHCONSVC, which maybe in 25% or 32%, due to the nature of this resource code and by HQ policy. EOR and resource code combinations must be of the same object class. See CEFMS II screen 10.90 for current listing." ;
    skos:inScheme ER-37-1-30-P12: ;
    skos:prefLabel "Resource Codes" .

ER-37-1-30-P12:Resource_Management_Office a wov:GlossaryTerm,
        skos:Concept ;
    rdfs:label "Resource Management Office" ;
    dcterms:bibliographicCitation "https://www.publications.usace.army.mil/Portals/76/Users/182/86/2486/ER%2037-1-30.pdf#page=34" ;
    pav:wasDerivedFrom "glossaries/CivilWorks/ER-37-1-30-P12.yaml#term[Resource Management Office]" ;
    skos:definition "grants CEFMS II roles upon receipt of the standard appointment letters. An automated appointment letter with electronic signature capability is generated in CEFMS II based on the appointment roles granted and maintained electronically. CEFMS II will automatically generate a DD Form 577 based on the appointment letter." ;
    skos:inScheme ER-37-1-30-P12: ;
    skos:prefLabel "Resource Management Office" .

ER-37-1-30-P12:Resource_Management_Officers a wov:GlossaryTerm,
        skos:Concept ;
    rdfs:label "Resource Management Officers" ;
    dcterms:bibliographicCitation "https://www.publications.usace.army.mil/Portals/76/Users/182/86/2486/ER%2037-1-30.pdf#page=34" ;
    pav:wasDerivedFrom "glossaries/CivilWorks/ER-37-1-30-P12.yaml#term[Resource Management Officers]" ;
    skos:altLabel "RMOs" ;
    skos:definition "ensure adequate internal controls for funds management. The RMO participates in the quarterly Directorate Management Review (DMR)/Command Management Review (CMR) and is responsible for all aspects of the JRP. The RM is responsible for certifying completion of tri-annual reviews of commitments and unliquidated obligations (ULOs) and attesting to the accuracy and completeness of the review. The ULOs are monitored closely and RMOs are required to explain the status during quarterly DMR reviews." ;
    skos:inScheme ER-37-1-30-P12: ;
    skos:prefLabel "Resource Management Officers" .

ER-37-1-30-P12:Review_Results a wov:GlossaryTerm,
        skos:Concept ;
    rdfs:label "Review Results" ;
    dcterms:bibliographicCitation "https://www.publications.usace.army.mil/Portals/76/Users/182/86/2486/ER%2037-1-30.pdf#page=37" ;
    pav:wasDerivedFrom "glossaries/CivilWorks/ER-37-1-30-P12.yaml#term[Review Results]" ;
    skos:definition "The results of the preliminary review will be documented in a preliminary review report and forwarded to CERM-F for approval and coordination with the HQUSACE Office of the Chief Counsel. If the Army determines that there is no ADA violation, then the preliminary report completes the action upon Army's closure of the case." ;
    skos:inScheme ER-37-1-30-P12: ;
    skos:prefLabel "Review Results" .

ER-37-1-30-P12:Revolving_Fund a wov:GlossaryTerm,
        skos:Concept ;
    rdfs:label "Revolving Fund" ;
    dcterms:bibliographicCitation "https://www.publications.usace.army.mil/Portals/76/Users/182/86/2486/ER%2037-1-30.pdf#page=32" ;
    pav:wasDerivedFrom "glossaries/CivilWorks/ER-37-1-30-P12.yaml#term[Revolving Fund]" ;
    skos:altLabel "RF" ;
    skos:definition "The USACE RF is operated entirely within its own resources rather than from annual appropriations, which requires that prompt reimbursement be obtained from the benefiting appropriations or projects for services rendered in order that sufficient funds are available for continued operation. This self-sustaining nature requires that RF accounts and operations be frequently reviewed to ensure that costs are equitably distributed to customers in the current fiscal year and that a sufficient cash balance is maintained in each USACE command to permit prompt liquidation of obligations as they mature." ;
    skos:inScheme ER-37-1-30-P12: ;
    skos:prefLabel "Revolving Fund" .

<https://usace-data.com/civil-works/glossary/ER-37-1-30-P12#Rivers_%26_Harbors_Contributed_and_Advance_Funds,_Corps_of_Engineers,_Civil_096X8862> a wov:GlossaryTerm,
        skos:Concept ;
    rdfs:label "Rivers & Harbors Contributed and Advance Funds, Corps of Engineers, Civil 096X8862" ;
    dcterms:bibliographicCitation "https://www.publications.usace.army.mil/Portals/76/Users/182/86/2486/ER%2037-1-30.pdf#page=84" ;
    pav:wasDerivedFrom "glossaries/CivilWorks/ER-37-1-30-P12.yaml#term[Rivers & Harbors Contributed and Advance Funds, Corps of Engineers, Civil 096X8862]" ;
    skos:definition "Funds contributed by local interests for expenditure in connection with funds appropriated by Congress for any authorized work of public improvements of rivers and harbors. This includes cash contributions required by terms prescribed in the agreement with non-federal interests for study" ;
    skos:inScheme ER-37-1-30-P12: ;
    skos:prefLabel "Rivers & Harbors Contributed and Advance Funds, Corps of Engineers, Civil 096X8862" .

ER-37-1-30-P12:Sub-allotments a wov:GlossaryTerm,
        skos:Concept ;
    rdfs:label "Sub-allotments" ;
    dcterms:bibliographicCitation "https://www.publications.usace.army.mil/Portals/76/Users/182/86/2486/ER%2037-1-30.pdf#page=31" ;
    pav:wasDerivedFrom "glossaries/CivilWorks/ER-37-1-30-P12.yaml#term[Sub-allotments]" ;
    skos:definition "Subdivisions of allotments." ;
    skos:inScheme ER-37-1-30-P12: ;
    skos:prefLabel "Sub-allotments" .

ER-37-1-30-P12:Undelivered_Order a wov:GlossaryTerm,
        skos:Concept ;
    rdfs:label "Undelivered Order" ;
    dcterms:bibliographicCitation "https://www.publications.usace.army.mil/Portals/76/Users/182/86/2486/ER%2037-1-30.pdf#page=32" ;
    pav:wasDerivedFrom "glossaries/CivilWorks/ER-37-1-30-P12.yaml#term[Undelivered Order]" ;
    skos:definition "Contract or order issued for goods and services for which the liability has not yet accrued. The orders may be for any goods or services that are required to meet a bona fide need of the issuing entity." ;
    skos:inScheme ER-37-1-30-P12: ;
    skos:prefLabel "Undelivered Order" .

<https://usace-data.com/civil-works/glossary/ER-37-1-30-P12#Washington_Aqueduct_Capital_Improvements,_Corps_of_Engineers,_096X3128> a wov:GlossaryTerm,
        skos:Concept ;
    rdfs:label "Washington Aqueduct Capital Improvements, Corps of Engineers, 096X3128" ;
    dcterms:bibliographicCitation "https://www.publications.usace.army.mil/Portals/76/Users/182/86/2486/ER%2037-1-30.pdf#page=83" ;
    pav:wasDerivedFrom "glossaries/CivilWorks/ER-37-1-30-P12.yaml#term[Washington Aqueduct Capital Improvements, Corps of Engineers, 096X3128]" ;
    skos:definition "This appropriation provides funding authority for capital improvements and repairs to the Washington Aqueduct." ;
    skos:inScheme ER-37-1-30-P12: ;
    skos:prefLabel "Washington Aqueduct Capital Improvements, Corps of Engineers, 096X3128" .

ER-37-1-30-P12:Work_Allowances a wov:GlossaryTerm,
        skos:Concept ;
    rdfs:label "Work Allowances" ;
    dcterms:bibliographicCitation "https://www.publications.usace.army.mil/Portals/76/Users/182/86/2486/ER%2037-1-30.pdf#page=31" ;
    pav:wasDerivedFrom "glossaries/CivilWorks/ER-37-1-30-P12.yaml#term[Work Allowances]" ;
    skos:definition "Provide instructions for the distribution among programs, projects and activities of the budget authority provided to a USACE activity on a Funding Authorization Document (FAD) for Civil Works appropriations only. For military appropriations, the instruction document is referred to as a draft directive. Draft Directives serve the same function for military appropriations." ;
    skos:inScheme ER-37-1-30-P12: ;
    skos:prefLabel "Work Allowances" .

ER-37-1-30-P12:Work_Category_Code a wov:GlossaryTerm,
        skos:Concept ;
    rdfs:label "Work Category Code" ;
    dcterms:bibliographicCitation "https://www.publications.usace.army.mil/Portals/76/Users/182/86/2486/ER%2037-1-30.pdf#page=84" ;
    pav:wasDerivedFrom "glossaries/CivilWorks/ER-37-1-30-P12.yaml#term[Work Category Code]" ;
    skos:altLabel "WCC" ;
    skos:definition "These codes are used to accumulate cost data to meet requirements for budgeting, programming, execution, and reporting, as defined by CECW policy/National Account Manager or CEMP policy/National Account Manager. See CEFMS II screen 10.116 for current listing." ;
    skos:inScheme ER-37-1-30-P12: ;
    skos:prefLabel "Work Category Code" .

ER-37-1-30-P12:Work_Category_Elements a wov:GlossaryTerm,
        skos:Concept ;
    rdfs:label "Work Category Elements" ;
    dcterms:bibliographicCitation "https://www.publications.usace.army.mil/Portals/76/Users/182/86/2486/ER%2037-1-30.pdf#page=84" ;
    pav:wasDerivedFrom "glossaries/CivilWorks/ER-37-1-30-P12.yaml#term[Work Category Elements]" ;
    skos:altLabel "WCE" ;
    skos:definition "The WCE is an extension of the WCC and provides a further breakdown for capturing costs, as defined by CECW policy/National Account Manager or CEMP policy/National Account Manager. See CEFMS II screen 10.120 for current listing." ;
    skos:inScheme ER-37-1-30-P12: ;
    skos:prefLabel "Work Category Elements" .

ER-37-1-30-P12: a wov:Glossary,
        owl:Ontology,
        skos:ConceptScheme,
        voaf:Vocabulary ;
    rdfs:label "Financial Administration Accounting and Reporting ER 37-1-30 pub. 12 December 2019" ;
    dcterms:created "2024-07-16T04:27:12.630845+00:00"^^xsd:dateTime ;
    dcterms:description "Financial Administration Accounting and Reporting ER 37-1-30, published 12 December 2019 defines acronyms and terms commonly used in this report, which describes  principles and standards for governing the design and operation of the financial/cost accounting and reporting systems for U.S. Army Corps of Engineers (USACE). These terms are defined in the glossary section of the regulation." ;
    dcterms:publisher "None" ;
    dcterms:rights "MIT" ;
    dcterms:title "Financial Administration Accounting and Reporting ER 37-1-30 pub. 12 December 2019" ;
    pav:ImportedFrom "glossaries/CivilWorks/ER-37-1-30-P12.yaml" ;
    pav:createdOn "2024-07-16T04:27:12.630845+00:00"^^xsd:dateTime ;
    pav:createdWith "gloss" ;
    pav:wasInfluencedBy "Financial Administration Accounting and Reporting ER 37-1-30 pub. 12 December 2019" ;
    vann:preferredNamespaceUri "https://usace-data.com/civil-works/glossary/ER-37-1-30-P12#" ;
    skos:hasTopConcept ER-37-1-30-P12:ADA_Reporting_Procedures,
        ER-37-1-30-P12:ADA_Violations,
        ER-37-1-30-P12:Accounting_Procedures,
        ER-37-1-30-P12:Accounting_Support_for_Fund_Control_Systems,
        ER-37-1-30-P12:Administrative_Penalties,
        ER-37-1-30-P12:Allotment,
        ER-37-1-30-P12:Allowances_and_Allocations,
        ER-37-1-30-P12:Apportionment,
        ER-37-1-30-P12:Appropriations,
        ER-37-1-30-P12:Cancelled_Accounts,
        <https://usace-data.com/civil-works/glossary/ER-37-1-30-P12#Category,_Class,_Sub-class>,
        ER-37-1-30-P12:Commitment,
        <https://usace-data.com/civil-works/glossary/ER-37-1-30-P12#Construction,_Corps_of_Engineers,_Civil_096X3122>,
        ER-37-1-30-P12:Cost_Account_Requirements,
        ER-37-1-30-P12:Cost_Accounting_Procedures,
        ER-37-1-30-P12:Criminal_Penalties,
        ER-37-1-30-P12:Department_Accountable_Official,
        ER-37-1-30-P12:Directorate%2FOffice_Chiefs,
        ER-37-1-30-P12:Disbursement,
        ER-37-1-30-P12:Disbursing_Officer,
        ER-37-1-30-P12:Element_of_Resource_%28EOR%29_Codes,
        <https://usace-data.com/civil-works/glossary/ER-37-1-30-P12#Expenses,_Corps_of_Engineers,_Civil_096Y3124>,
        ER-37-1-30-P12:Expired_Accounts,
        ER-37-1-30-P12:FOA_Commanders%2FDirectors,
        ER-37-1-30-P12:Finance_and_Accounting_Officers,
        ER-37-1-30-P12:Fiscal_law_and_ADA_violation_management,
        <https://usace-data.com/civil-works/glossary/ER-37-1-30-P12#Flood_Control_%26_Coastal_Emergencies,_Corps_of_Engineers,_Civil_096X3125>,
        ER-37-1-30-P12:Formal_Reviews,
        <https://usace-data.com/civil-works/glossary/ER-37-1-30-P12#Formerly_Utilized_Sites_Remedial_Action_Program_%28FUSRAP%29,_Corps_of_Engineers,_096X3130>,
        ER-37-1-30-P12:Fund_Holders,
        ER-37-1-30-P12:Funding_Authorization_Documents,
        <https://usace-data.com/civil-works/glossary/ER-37-1-30-P12#HQUSACE,_Resource_Management_Office>,
        <https://usace-data.com/civil-works/glossary/ER-37-1-30-P12#HQUSACE_Chief,_Budget_%26_Programs_Division>,
        <https://usace-data.com/civil-works/glossary/ER-37-1-30-P12#HQUSACE_Chief,_Finance_and_Accounting_Policy_Division>,
        <https://usace-data.com/civil-works/glossary/ER-37-1-30-P12#Hydraulic_Mining_in_California,_Debris,_096X5066>,
        ER-37-1-30-P12:Identifying_Circumstances_and_Responsibility,
        ER-37-1-30-P12:Implementing_CFO_Act_requirements,
        ER-37-1-30-P12:Initial_Discovery,
        ER-37-1-30-P12:Interpretation_and_Legal_Issues,
        <https://usace-data.com/civil-works/glossary/ER-37-1-30-P12#Investigations,_Corps_of_Engineers,_Civil_096X3121>,
        <https://usace-data.com/civil-works/glossary/ER-37-1-30-P12#Maintenance_%26_Operation_of_Dams_and_Other_Improvements_of_Navigable_Water,_096X5125>,
        <https://usace-data.com/civil-works/glossary/ER-37-1-30-P12#Mississippi_River_and_Tributaries,_Civil_096X3112>,
        ER-37-1-30-P12:Object_Classes,
        ER-37-1-30-P12:Obligation,
        <https://usace-data.com/civil-works/glossary/ER-37-1-30-P12#Office_of_Assistant_Secretary_of_the_Army_%28Civil_Works%29,_096Y3132>,
        <https://usace-data.com/civil-works/glossary/ER-37-1-30-P12#Operation_%26_Maintenance,_Corps_of_Engineers,_Civil_096X3123>,
        <https://usace-data.com/civil-works/glossary/ER-37-1-30-P12#Payment_to_the_South_Dakota_Terrestrial_Wildlife_Habitat_Restoration_Trust_Fund,_096X3129>,
        <https://usace-data.com/civil-works/glossary/ER-37-1-30-P12#Payments_to_States,_Flood_Control_Act_of_1954,_096X5090>,
        ER-37-1-30-P12:Preliminary_Review,
        <https://usace-data.com/civil-works/glossary/ER-37-1-30-P12#Regulatory_Program,_Corps_of_Engineers,_Civil_096Y3126>,
        ER-37-1-30-P12:Research_Effort,
        ER-37-1-30-P12:Resource_Codes,
        ER-37-1-30-P12:Resource_Management_Office,
        ER-37-1-30-P12:Resource_Management_Officers,
        ER-37-1-30-P12:Review_Results,
        ER-37-1-30-P12:Revolving_Fund,
        <https://usace-data.com/civil-works/glossary/ER-37-1-30-P12#Rivers_%26_Harbors_Contributed_and_Advance_Funds,_Corps_of_Engineers,_Civil_096X8862>,
        ER-37-1-30-P12:Sub-allotments,
        ER-37-1-30-P12:Undelivered_Order,
        <https://usace-data.com/civil-works/glossary/ER-37-1-30-P12#Washington_Aqueduct_Capital_Improvements,_Corps_of_Engineers,_096X3128>,
        ER-37-1-30-P12:Work_Allowances,
        ER-37-1-30-P12:Work_Category_Code,
        ER-37-1-30-P12:Work_Category_Elements .

